Of course. Here is a detailed, step-by-step solution to the problem. We will present two proofs: a direct proof using calculus and an alternative, more conceptual proof using a probabilistic interpretation.

### Method 1: Direct Proof using Calculus

Our goal is to prove that the function $f(t)$ is non-increasing on $[0,1]$. A differentiable function is non-increasing on an interval if its derivative is less than or equal to zero on that interval.

The function is given by:
$$
f(t) = \sum_{A\in\mathcal{F}} t^{|A|}(1-t)^{|S\setminus A|}
$$
Since $|S|=n$, we have $|S\setminus A| = n - |A|$. So we can write:
$$
f(t) = \sum_{A\in\mathcal{F}} t^{|A|}(1-t)^{n-|A|}
$$
As $f(t)$ is a polynomial in $t$, it is differentiable for all $t \in \mathbb{R}$. We will compute its derivative for $t \in (0,1)$.

**Step 1: Differentiate the function**
Using the sum rule and the product rule for differentiation, we get:
$$
\begin{aligned}
f'(t) &= \frac{d}{dt} \sum_{A\in\mathcal{F}} t^{|A|}(1-t)^{n-|A|} \\
&= \sum_{A\in\mathcal{F}} \frac{d}{dt} \left( t^{|A|}(1-t)^{n-|A|} \right) \\
&= \sum_{A\in\mathcal{F}} \left[ |A|t^{|A|-1}(1-t)^{n-|A|} + t^{|A|} \cdot (n-|A|)(1-t)^{n-|A|-1}(-1) \right] \\
&= \sum_{A\in\mathcal{F}} |A|t^{|A|-1}(1-t)^{n-|A|} - \sum_{A\in\mathcal{F}} (n-|A|)t^{|A|}(1-t)^{n-|A|-1}
\end{aligned}
$$

**Step 2: Rewrite the sums by partitioning over elements of S**
Let's analyze the two sums separately.
For the first sum, $S_1 = \sum_{A\in\mathcal{F}} |A|t^{|A|-1}(1-t)^{n-|A|}$:
We can express $|A|$ as $\sum_{i \in A} 1$.
$$
S_1 = \sum_{A\in\mathcal{F}} \left(\sum_{i \in A} 1\right) t^{|A|-1}(1-t)^{n-|A|}
$$
By swapping the order of summation:
$$
S_1 = \sum_{i \in S} \sum_{\substack{A \in \mathcal{F} \\ i \in A}} t^{|A|-1}(1-t)^{n-|A|}
$$
Let's perform a change of variable in the inner sum. Let $B = A \setminus \{i\}$. Then $|B| = |A|-1$, and $A = B \cup \{i\}$. The condition $A \in \mathcal{F}$ becomes $B \cup \{i\} \in \mathcal{F}$, and the condition $i \in A$ implies $i \notin B$. The summation over $A$ becomes a summation over subsets $B$ of $S \setminus \{i\}$.
$$
S_1 = \sum_{i \in S} \sum_{\substack{B \subset S\setminus\{i\} \\ B\cup\{i\} \in \mathcal{F}}} t^{|B|}(1-t)^{n-(|B|+1)} = \sum_{i \in S} \sum_{\substack{B \subset S\setminus\{i\} \\ B\cup\{i\} \in \mathcal{F}}} t^{|B|}(1-t)^{n-|B|-1}
$$

For the second sum, $S_2 = \sum_{A\in\mathcal{F}} (n-|A|)t^{|A|}(1-t)^{n-|A|-1}$:
We can express $(n-|A|)$ as $|S \setminus A| = \sum_{i \in S \setminus A} 1$.
$$
S_2 = \sum_{A\in\mathcal{F}} \left(\sum_{i \in S\setminus A} 1\right) t^{|A|}(1-t)^{n-|A|-1}
$$
By swapping the order of summation:
$$
S_2 = \sum_{i \in S} \sum_{\substack{A \in \mathcal{F} \\ i \notin A}} t^{|A|}(1-t)^{n-|A|-1}
$$
The inner sum is over sets $A \in \mathcal{F}$ that are subsets of $S \setminus \{i\}$. To align this with the expression for $S_1$, let's rename the summation variable $A$ to $B$.
$$
S_2 = \sum_{i \in S} \sum_{\substack{B \subset S\setminus\{i\} \\ B \in \mathcal{F}}} t^{|B|}(1-t)^{n-|B|-1}
$$

**Step 3: Combine the expressions and use the property of $\mathcal{F}$**
Now we can write $f'(t) = S_1 - S_2$:
$$
f'(t) = \sum_{i \in S} \left( \sum_{\substack{B \subset S\setminus\{i\} \\ B\cup\{i\} \in \mathcal{F}}} t^{|B|}(1-t)^{n-|B|-1} - \sum_{\substack{B \subset S\setminus\{i\} \\ B \in \mathcal{F}}} t^{|B|}(1-t)^{n-|B|-1} \right)
$$
We can combine the inner sums, which are over the same domain of subsets $B \subset S\setminus\{i\}$:
$$
f'(t) = \sum_{i \in S} \sum_{B \subset S\setminus\{i\}} \left( \mathbf{1}_{B\cup\{i\} \in \mathcal{F}} - \mathbf{1}_{B \in \mathcal{F}} \right) t^{|B|}(1-t)^{n-|B|-1}
$$
where $\mathbf{1}_{\text{condition}}$ is the indicator function which is 1 if the condition is true, and 0 otherwise.

Now we use the given property of the family $\mathcal{F}$:
$$
A\in\mathcal{F}, C\subset A \Rightarrow C\in\mathcal{F}.
$$
Let's apply this property to the sets $B$ and $B\cup\{i\}$. We know that $B \subset B\cup\{i\}$.
If $B\cup\{i\} \in \mathcal{F}$, then by the property (with $A = B\cup\{i\}$ and $C=B$), it must be that $B \in \mathcal{F}$.
This means that if $\mathbf{1}_{B\cup\{i\} \in \mathcal{F}} = 1$, then $\mathbf{1}_{B \in \mathcal{F}}$ must also be $1$.
Therefore, the term $(\mathbf{1}_{B\cup\{i\} \in \mathcal{F}} - \mathbf{1}_{B \in \mathcal{F}})$ can take only two possible values:
*   If $B\cup\{i\} \in \mathcal{F}$, then $B \in \mathcal{F}$, so the term is $1 - 1 = 0$.
*   If $B\cup\{i\} \notin \mathcal{F}$, the term is $0 - \mathbf{1}_{B \in \mathcal{F}}$. This is either $0-0=0$ or $0-1=-1$.
In all cases, $(\mathbf{1}_{B\cup\{i\} \in \mathcal{F}} - \mathbf{1}_{B \in \mathcal{F}}) \le 0$.

**Step 4: Conclude that $f'(t) \le 0$**
For $t \in (0,1)$, the term $t^{|B|}(1-t)^{n-|B|-1}$ is always positive.
Thus, each term in the sum over $B \subset S\setminus\{i\}$ is a non-positive value multiplied by a positive value, which results in a non-positive value.
$$
\sum_{B \subset S\setminus\{i\}} \underbrace{\left( \mathbf{1}_{B\cup\{i\} \in \mathcal{F}} - \mathbf{1}_{B \in \mathcal{F}} \right)}_{\le 0} \underbrace{t^{|B|}(1-t)^{n-|B|-1}}_{>0} \le 0
$$
Since this holds for every $i \in S$, the full sum for $f'(t)$ is a sum of non-positive terms, and therefore must be non-positive.
$$
f'(t) = \sum_{i \in S} (\text{a non-positive term}) \le 0.
$$
Since $f(t)$ is continuous on $[0,1]$ and $f'(t) \le 0$ for all $t \in (0,1)$, we can conclude that $f(t)$ is a non-increasing function on the closed interval $[0,1]$.

---

### Method 2: Probabilistic Interpretation

This method provides a more intuitive understanding of why the property of $\mathcal{F}$ leads to the desired conclusion.

**Step 1: Reinterpret the function f(t) as a probability**
Let us define a random subset $X$ of $S=\{1,2,\ldots,n\}$. For each element $i \in S$, we decide whether $i \in X$ by flipping a biased coin. Let the probability that $i \in X$ be $t$, independently for each $i$.
The outcome of these $n$ independent Bernoulli trials defines the random set $X$. For any specific subset $A \subset S$, the probability of obtaining exactly that set is:
$$
P(X=A) = \left(\prod_{i\in A} P(i\in X)\right) \left(\prod_{j\in S\setminus A} P(j\notin X)\right) = t^{|A|} (1-t)^{|S\setminus A|}
$$
The function $f(t)$ can now be interpreted as the total probability of the random set $X$ being a member of the family $\mathcal{F}$:
$$
f(t) = \sum_{A\in\mathcal{F}} P(X=A) = P(X \in \mathcal{F})
$$
To show that $f(t)$ is non-increasing, we need to show that if $t_1 < t_2$, then $f(t_1) \ge f(t_2)$. In our probabilistic framework, this means $P_{t_1}(X \in \mathcal{F}) \ge P_{t_2}(X \in \mathcal{F})$, where $P_t$ denotes the probability measure with parameter $t$.

**Step 2: Couple the random experiments**
Let $0 \le t_1 < t_2 \le 1$. We can construct two random sets, $X_1$ and $X_2$, on the same probability space in a way that allows for a direct comparison.
For each element $k \in S$, let $U_k$ be an independent random variable uniformly distributed on $[0,1]$.
Define the sets $X_1$ and $X_2$ as follows:
*   $X_1 = \{k \in S \mid U_k \le t_1\}$
*   $X_2 = \{k \in S \mid U_k \le t_2\}$

For any $k \in S$, $P(k \in X_1) = P(U_k \le t_1) = t_1$ and $P(k \in X_2) = P(U_k \le t_2) = t_2$. Since the $U_k$ are independent, the choices for including elements in the sets are independent. Thus, $X_1$ has the same distribution as a random set with parameter $t_1$, and $X_2$ has the same distribution as a random set with parameter $t_2$.
Therefore, $f(t_1) = P(X_1 \in \mathcal{F})$ and $f(t_2) = P(X_2 \in \mathcal{F})$.

**Step 3: Relate the outcomes and use the property of $\mathcal{F}$**
Because $t_1 < t_2$, the condition $U_k \le t_1$ implies $U_k \le t_2$.
This means that for any outcome of the random variables $U_1, \ldots, U_n$, if an element $k$ is in $X_1$, it must also be in $X_2$. This establishes a relationship between the sets:
$$
X_1 \subset X_2
$$
This inclusion holds for every possible outcome, i.e., with probability 1.

Now, consider the event that $X_2 \in \mathcal{F}$. If this event occurs, it means the generated set $X_2$ is in the family $\mathcal{F}$.
We are given the property that if $A \in \mathcal{F}$ and $B \subset A$, then $B \in \mathcal{F}$.
Applying this to our random sets, since $X_1 \subset X_2$, if $X_2 \in \mathcal{F}$, it must follow that $X_1 \in \mathcal{F}$.

**Step 4: Conclude that f(t) is non-increasing**
The reasoning in Step 3 shows that the event $\{X_2 \in \mathcal{F}\}$ is a subset of the event $\{X_1 \in \mathcal{F}\}$.
In formal notation: $\{\omega \mid X_2(\omega) \in \mathcal{F}\} \subset \{\omega \mid X_1(\omega) \in \mathcal{F}\}$.
From basic probability theory, if an event $E_A$ is a subset of an event $E_B$, then $P(E_A) \le P(E_B)$.
Applying this to our events, we get:
$$
P(X_2 \in \mathcal{F}) \le P(X_1 \in \mathcal{F})
$$
Substituting back the definition of $f(t)$:
$$
f(t_2) \le f(t_1)
$$
This holds for any $t_1, t_2 \in [0,1]$ with $t_1 < t_2$. This is the definition of a non-increasing function.

Both proofs rigorously establish that $f(t)$ is non-increasing.