Notice that:
$$\frac{x^{10}+1}{x^6+x^4}=\frac{\frac{x^{10}+1}{x^5}}{x+\frac{1}{x}}=\frac{x^5+\frac{1}{x^5}}{x+\frac{1}{x}}.$$ 

It is clear that $x$ is a real number since $x^2-\sqrt{7}x+1=0$ has real solutions. Squaring we have:
$$\left(x+\frac{1}{x}\right)^2=x^2+\frac{1}{x^2}+2=7$$ so $x^2+1/x^2=5$. Squaring again we have that $x^4+1/x^4+2=25$ so $x^4+1/x^4=23$. Notice that $(x^4+1/x^4)(x+1/x)=x^5+1/x^5+x^3+1/x^3$ and:
$$\left(x^2+\frac{1}{x^2}\right)\left(x+\frac{1}{x}\right)=x^3+\frac{1}{x^3}+x+\frac{1}{x}$$
\noindent so:
\begin{eqnarray*}
x^5+\frac{1}{x^5}=\left(x^4+\frac{1}{x^4}\right)\left(x+\frac{1}{x}\right)-\left(x^2+\frac{1}{x^2}\right)\left(x+\frac{1}{x}\right)+x+\frac{1}{x}\\ =23 \sqrt{7}-5 \sqrt{7}+\sqrt{7}=19 \sqrt{7}.\end{eqnarray*} 

Hence the expression is given by $\frac{19 \sqrt{7}}{\sqrt{7}}=19$ and we are done.