# Solution

In this problem, we need to find the value of $\sum_{n=1}^\infty nb_n$ where $b_n=a_n-3a_{n+1}+3a_{n+2}-a_{n+3}$.

Let's expand $\sum_{n=1}^\infty nb_n$ by substituting the expression for $b_n$:

$$\sum_{n=1}^\infty nb_n = \sum_{n=1}^\infty n(a_n-3a_{n+1}+3a_{n+2}-a_{n+3})$$

This can be rewritten as:

$$\sum_{n=1}^\infty nb_n = \sum_{n=1}^\infty na_n - 3\sum_{n=1}^\infty na_{n+1} + 3\sum_{n=1}^\infty na_{n+2} - \sum_{n=1}^\infty na_{n+3}$$

Now we'll reindex each sum to make the comparison easier. For the second sum, let $m = n+1$, so $n = m-1$:

$$\sum_{n=1}^\infty na_{n+1} = \sum_{m=2}^\infty (m-1)a_m = \sum_{m=2}^\infty ma_m - \sum_{m=2}^\infty a_m$$

For the third sum, let $p = n+2$, so $n = p-2$:

$$\sum_{n=1}^\infty na_{n+2} = \sum_{p=3}^\infty (p-2)a_p = \sum_{p=3}^\infty pa_p - 2\sum_{p=3}^\infty a_p$$

For the fourth sum, let $q = n+3$, so $n = q-3$:

$$\sum_{n=1}^\infty na_{n+3} = \sum_{q=4}^\infty (q-3)a_q = \sum_{q=4}^\infty qa_q - 3\sum_{q=4}^\infty a_q$$

To compare these sums directly, we'll rewrite each in terms of sums starting from index 1:

$$\sum_{m=2}^\infty ma_m = \sum_{k=1}^\infty ka_k - a_1$$
$$\sum_{m=2}^\infty a_m = \sum_{k=1}^\infty a_k - a_1$$

$$\sum_{p=3}^\infty pa_p = \sum_{k=1}^\infty ka_k - a_1 - 2a_2$$
$$\sum_{p=3}^\infty a_p = \sum_{k=1}^\infty a_k - a_1 - a_2$$

$$\sum_{q=4}^\infty qa_q = \sum_{k=1}^\infty ka_k - a_1 - 2a_2 - 3a_3$$
$$\sum_{q=4}^\infty a_q = \sum_{k=1}^\infty a_k - a_1 - a_2 - a_3$$

Substituting these expressions into our original equation:

$$\begin{align*}
\sum_{n=1}^\infty nb_n &= \sum_{k=1}^\infty ka_k - 3\left(\sum_{k=1}^\infty ka_k - a_1 - \sum_{k=1}^\infty a_k + a_1\right) \\
&+ 3\left(\sum_{k=1}^\infty ka_k - a_1 - 2a_2 - 2\sum_{k=1}^\infty a_k + 2a_1 + 2a_2\right) \\
&- \left(\sum_{k=1}^\infty ka_k - a_1 - 2a_2 - 3a_3 - 3\sum_{k=1}^\infty a_k + 3a_1 + 3a_2 + 3a_3\right)
\end{align*}$$

Let's simplify and group like terms:

$$\begin{align*}
\sum_{n=1}^\infty nb_n &= \sum_{k=1}^\infty ka_k - 3\sum_{k=1}^\infty ka_k + 3\sum_{k=1}^\infty a_k + 3\sum_{k=1}^\infty ka_k - 6\sum_{k=1}^\infty a_k + 3a_1 \\
&- \sum_{k=1}^\infty ka_k + 3\sum_{k=1}^\infty a_k - 2a_1 - a_2 \\
&= (1-3+3-1)\sum_{k=1}^\infty ka_k + (0+3-6+3)\sum_{k=1}^\infty a_k + (0+0+3-2)a_1 + (0+0+0-1)a_2 \\
&= 0 \cdot \sum_{k=1}^\infty ka_k + 0 \cdot \sum_{k=1}^\infty a_k + a_1 - a_2 \\
&= a_1 - a_2
\end{align*}$$

Therefore, $\sum_{n=1}^\infty nb_n = a_1 - a_2$.

Note: The condition $a_{n+1} \leq \frac{1}{2}a_n$ ensures that the sequence $(a_n)$ approaches zero quickly enough for all the infinite sums involved to converge.