Of course. Here is a detailed, step-by-step solution to the problem.

### Problem Statement
Find the limit
$$ L = \lim_{n\to\infty} \int_0^1 \frac{(1-\ln(1-x))^n}{n!} \, dx. $$

### Method
The integrand is complicated, but the presence of the `n!` and a term raised to the power of `n` suggests a connection to the Taylor series for the exponential function. A direct application of limit interchange theorems like the Dominated Convergence Theorem is difficult because the integrand's value grows infinitely large as `x` approaches 1.

A more effective strategy is to simplify the integral using a substitution. This will transform the integral into a more recognizable form, which we can then analyze as `n` approaches infinity.

### Step 1: Perform a substitution to simplify the integral
Let the integral be denoted by $I_n$:
$$ I_n = \int_0^1 \frac{(1-\ln(1-x))^n}{n!} \, dx $$
Let's make the substitution $u = 1 - \ln(1-x)$. This choice simplifies the term being raised to the power of `n`.

First, we find the relationship between $dx$ and $du$:
$$ u = 1 - \ln(1-x) \implies \ln(1-x) = 1-u $$
Exponentiating both sides gives:
$$ 1-x = e^{1-u} $$
$$ x = 1 - e^{1-u} $$
Now, we differentiate with respect to $u$ to find $dx$:
$$ \frac{dx}{du} = -e^{1-u}(-1) = e^{1-u} $$
So, $dx = e^{1-u} \, du$.

Next, we change the limits of integration from $x$ to $u$:
*   When $x=0$, $u = 1 - \ln(1-0) = 1 - \ln(1) = 1 - 0 = 1$.
*   When $x \to 1^-$, $1-x \to 0^+$, so $\ln(1-x) \to -\infty$. Therefore, $u = 1 - \ln(1-x) \to \infty$.

Substituting $u$, $dx$, and the new limits into the integral $I_n$:
$$ I_n = \int_1^\infty \frac{u^n}{n!} \cdot e^{1-u} \, du $$

### Step 2: Relate the integral to the Gamma function
We can rewrite the expression for $I_n$:
$$ I_n = \frac{1}{n!} \int_1^\infty u^n e^1 e^{-u} \, du = \frac{e}{n!} \int_1^\infty u^n e^{-u} \, du $$
This integral is related to the Gamma function, $\Gamma(z)$, which is defined as:
$$ \Gamma(z) = \int_0^\infty t^{z-1} e^{-t} \, dt $$
A key property of the Gamma function is that for any non-negative integer $n$, $\Gamma(n+1) = n!$.
Therefore, we can write $n!$ as an integral:
$$ n! = \Gamma(n+1) = \int_0^\infty u^n e^{-u} \, du $$
We can split this integral into two parts:
$$ n! = \int_0^1 u^n e^{-u} \, du + \int_1^\infty u^n e^{-u} \, du $$
The integral in our expression for $I_n$ is the second part of this sum. We can express it as:
$$ \int_1^\infty u^n e^{-u} \, du = n! - \int_0^1 u^n e^{-u} \, du $$

### Step 3: Substitute the expression back into $I_n$
Now, substitute this back into our formula for $I_n$:
$$ I_n = \frac{e}{n!} \left( n! - \int_0^1 u^n e^{-u} \, du \right) $$
$$ I_n = e \left( 1 - \frac{1}{n!} \int_0^1 u^n e^{-u} \, du \right) $$
The problem is now reduced to finding the limit of the second term as $n \to \infty$.
$$ L = \lim_{n\to\infty} I_n = \lim_{n\to\infty} e \left( 1 - \frac{1}{n!} \int_0^1 u^n e^{-u} \, du \right) = e \left( 1 - \lim_{n\to\infty} \frac{1}{n!} \int_0^1 u^n e^{-u} \, du \right) $$

### Step 4: Evaluate the limit of the remaining integral term
Let's evaluate the limit of the term $J_n = \frac{1}{n!} \int_0^1 u^n e^{-u} \, du$. We can bound the integral using the Squeeze Theorem.

For $u \in [0, 1]$, the function $e^{-u}$ is decreasing.
*   The maximum value is $e^{-0} = 1$.
*   The minimum value is $e^{-1} = 1/e$.

So, for $u \in [0, 1]$, we have the inequality:
$$ \frac{1}{e} \le e^{-u} \le 1 $$
Since $u^n \ge 0$ on this interval, we can multiply the inequality by $u^n$ and integrate from 0 to 1:
$$ \int_0^1 u^n \cdot \frac{1}{e} \, du \le \int_0^1 u^n e^{-u} \, du \le \int_0^1 u^n \cdot 1 \, du $$
Let's evaluate the bounding integrals:
$$ \int_0^1 u^n \, du = \left[ \frac{u^{n+1}}{n+1} \right]_0^1 = \frac{1^{n+1}}{n+1} - \frac{0^{n+1}}{n+1} = \frac{1}{n+1} $$
Applying this result to our inequality:
$$ \frac{1}{e} \cdot \frac{1}{n+1} \le \int_0^1 u^n e^{-u} \, du \le \frac{1}{n+1} $$
Now, we divide the entire inequality by $n!$ (which is positive):
$$ \frac{1}{e \cdot (n+1) \cdot n!} \le \frac{1}{n!} \int_0^1 u^n e^{-u} \, du \le \frac{1}{(n+1) \cdot n!} $$
This simplifies to:
$$ \frac{1}{e \cdot (n+1)!} \le J_n \le \frac{1}{(n+1)!} $$
Now we take the limit as $n \to \infty$:
$$ \lim_{n\to\infty} \frac{1}{e \cdot (n+1)!} = 0 $$
$$ \lim_{n\to\infty} \frac{1}{(n+1)!} = 0 $$
By the Squeeze Theorem, since $J_n$ is squeezed between two terms that both approach 0, its limit must also be 0:
$$ \lim_{n\to\infty} J_n = \lim_{n\to\infty} \frac{1}{n!} \int_0^1 u^n e^{-u} \, du = 0 $$

### Step 5: Final Calculation
We can now substitute this result back into our expression for the overall limit $L$:
$$ L = e \left( 1 - \lim_{n\to\infty} J_n \right) $$
$$ L = e (1 - 0) $$
$$ L = e $$

### Final Answer
The limit is **e**.