Of course. Here is a detailed, step-by-step solution to the problem.

### Problem Statement

Compute the sum
$$ S = \sum_{k=0}^{\left\lfloor \frac{n}{2} \right\rfloor} \sum_{\ell = \max\{1, 2k\}}^n \frac{1}{4^k} {\ell \choose 2k}. $$

### Solution

The given expression is a double summation. A common and powerful technique for such problems is to change the order of summation.

#### Step 1: Analyze the summation bounds

Let's analyze the region of summation in the $(k, \ell)$ plane. The indices $k$ and $\ell$ are integers satisfying the following inequalities:
1.  $0 \le k \le \left\lfloor \frac{n}{2} \right\rfloor$
2.  $\max\{1, 2k\} \le \ell \le n$

Let's break down the second inequality based on the value of $k$:
-   If $k=0$, the condition becomes $\max\{1, 0\} \le \ell \le n$, which simplifies to $1 \le \ell \le n$.
-   If $k \ge 1$, the condition becomes $\max\{1, 2k\} \le \ell \le n$, which simplifies to $2k \le \ell \le n$.

These conditions define the set of pairs $(k, \ell)$ over which we are summing.

#### Step 2: Change the order of summation

To change the order of summation, we first sum over $\ell$ and then over $k$. We need to find the new bounds for $k$ and $\ell$.

From the original bounds, we can see that $\ell$ ranges from a minimum value up to $n$. The lowest possible value for $\ell$ is 1 (when $k=0$). Thus, the new outer sum will be over $\ell$ from $1$ to $n$.

Now, for a fixed value of $\ell$ (where $1 \le \ell \le n$), we need to determine the range of possible values for $k$. Let's combine the original inequalities to find the constraints on $k$ for a fixed $\ell$:
1.  $k \ge 0$
2.  $k \le \left\lfloor \frac{n}{2} \right\rfloor$
3.  $\ell \ge \max\{1, 2k\}$

The third inequality implies $\ell \ge 2k$, which gives $k \le \frac{\ell}{2}$. Since $k$ must be an integer, this means $k \le \left\lfloor \frac{\ell}{2} \right\rfloor$.

Let's check if the condition $k \le \left\lfloor \frac{n}{2} \right\rfloor$ is redundant. Since we are considering a fixed $\ell$ such that $1 \le \ell \le n$, we have $\ell \le n$, which implies $\frac{\ell}{2} \le \frac{n}{2}$. Therefore, $\left\lfloor \frac{\ell}{2} \right\rfloor \le \left\lfloor \frac{n}{2} \right\rfloor$. So, the condition $k \le \left\lfloor \frac{\ell}{2} \right\rfloor$ is stricter than or equal to $k \le \left\lfloor \frac{n}{2} \right\rfloor$.

Thus, for a fixed $\ell \in \{1, 2, \dots, n\}$, the bounds for $k$ are $0 \le k \le \left\lfloor \frac{\ell}{2} \right\rfloor$.

With the order of summation swapped, the sum becomes:
$$ S = \sum_{\ell=1}^{n} \sum_{k=0}^{\left\lfloor \frac{\ell}{2} \right\rfloor} \frac{1}{4^k} {\ell \choose 2k}. $$

#### Step 3: Evaluate the inner sum

Let's focus on the inner sum, which we will call $T_\ell$:
$$ T_\ell = \sum_{k=0}^{\left\lfloor \frac{\ell}{2} \right\rfloor} \frac{1}{4^k} {\ell \choose 2k} = \sum_{k=0}^{\left\lfloor \frac{\ell}{2} \right\rfloor} {\ell \choose 2k} \left(\frac{1}{2}\right)^{2k}. $$
This sum involves binomial coefficients with even lower indices. It can be evaluated using a standard identity derived from the binomial theorem.

Consider the binomial expansions of $(1+x)^\ell$ and $(1-x)^\ell$:
$$ (1+x)^\ell = \sum_{j=0}^{\ell} {\ell \choose j} x^j = {\ell \choose 0} + {\ell \choose 1}x + {\ell \choose 2}x^2 + \dots $$
$$ (1-x)^\ell = \sum_{j=0}^{\ell} {\ell \choose j} (-x)^j = {\ell \choose 0} - {\ell \choose 1}x + {\ell \choose 2}x^2 - \dots $$
Adding these two equations cancels the terms with odd powers of $x$:
$$ (1+x)^\ell + (1-x)^\ell = 2{\ell \choose 0} + 2{\ell \choose 2}x^2 + 2{\ell \choose 4}x^4 + \dots = 2 \sum_{k=0}^{\left\lfloor \frac{\ell}{2} \right\rfloor} {\ell \choose 2k} x^{2k}. $$
Dividing by 2, we get the identity:
$$ \frac{(1+x)^\ell + (1-x)^\ell}{2} = \sum_{k=0}^{\left\lfloor \frac{\ell}{2} \right\rfloor} {\ell \choose 2k} x^{2k}. $$
Our inner sum $T_\ell$ matches this form with $x = \frac{1}{2}$. Substituting $x = \frac{1}{2}$ into the identity:
$$ T_\ell = \frac{\left(1+\frac{1}{2}\right)^\ell + \left(1-\frac{1}{2}\right)^\ell}{2} = \frac{\left(\frac{3}{2}\right)^\ell + \left(\frac{1}{2}\right)^\ell}{2} = \frac{\frac{3^\ell}{2^\ell} + \frac{1^\ell}{2^\ell}}{2} = \frac{3^\ell+1}{2^\ell \cdot 2} = \frac{3^\ell+1}{2^{\ell+1}}. $$

#### Step 4: Evaluate the outer sum

Now we substitute the closed form of the inner sum $T_\ell$ back into the expression for $S$:
$$ S = \sum_{\ell=1}^n T_\ell = \sum_{\ell=1}^n \frac{3^\ell+1}{2^{\ell+1}}. $$
We can split this into two separate sums:
$$ S = \sum_{\ell=1}^n \left( \frac{3^\ell}{2^{\ell+1}} + \frac{1}{2^{\ell+1}} \right) = \frac{1}{2} \sum_{\ell=1}^n \frac{3^\ell}{2^\ell} + \frac{1}{2} \sum_{\ell=1}^n \frac{1}{2^\ell} = \frac{1}{2} \sum_{\ell=1}^n \left(\frac{3}{2}\right)^\ell + \frac{1}{2} \sum_{\ell=1}^n \left(\frac{1}{2}\right)^\ell. $$
Both of these are finite geometric series. The sum of a finite geometric series is given by the formula $\sum_{k=1}^m ar^{k-1} = a \frac{r^m-1}{r-1}$, or for a series starting at $k=1$, $\sum_{k=1}^m r^k = r \frac{r^m-1}{r-1}$.

For the first sum, the common ratio is $r_1 = \frac{3}{2}$:
$$ \sum_{\ell=1}^n \left(\frac{3}{2}\right)^\ell = \frac{3}{2} \cdot \frac{\left(\frac{3}{2}\right)^n - 1}{\frac{3}{2} - 1} = \frac{3}{2} \cdot \frac{\frac{3^n}{2^n} - 1}{\frac{1}{2}} = 3 \left(\frac{3^n - 2^n}{2^n}\right) = \frac{3^{n+1} - 3 \cdot 2^n}{2^n}. $$
Alternatively, we can use $a(r^n-1)/(r-1)$ with $a=r=3/2$.
$\frac{3}{2}\frac{(3/2)^n-1}{3/2-1} = \frac{3}{2}\frac{(3/2)^n-1}{1/2} = 3((3/2)^n-1) = 3 \cdot \frac{3^n}{2^n} - 3 = \frac{3^{n+1}}{2^n} - 3$.

For the second sum, the common ratio is $r_2 = \frac{1}{2}$:
$$ \sum_{\ell=1}^n \left(\frac{1}{2}\right)^\ell = \frac{1}{2} \cdot \frac{1 - \left(\frac{1}{2}\right)^n}{1 - \frac{1}{2}} = \frac{1}{2} \cdot \frac{1 - \frac{1}{2^n}}{\frac{1}{2}} = 1 - \frac{1}{2^n} = \frac{2^n-1}{2^n}. $$

#### Step 5: Combine the results

Now, we substitute these results back into the expression for $S$:
$$ S = \frac{1}{2} \left[ \left(\frac{3^{n+1}}{2^n} - 3\right) + \left(1 - \frac{1}{2^n}\right) \right]. $$
Let's simplify the expression inside the brackets:
$$ \frac{3^{n+1}}{2^n} - 3 + 1 - \frac{1}{2^n} = \frac{3^{n+1} - 1}{2^n} - 2. $$
Now, multiply by $\frac{1}{2}$:
$$ S = \frac{1}{2} \left( \frac{3^{n+1} - 1}{2^n} - 2 \right) = \frac{3^{n+1} - 1}{2 \cdot 2^n} - \frac{2}{2} = \frac{3^{n+1} - 1}{2^{n+1}} - 1. $$

### Final Answer

The computed sum is:
$$ \sum_{k=0}^{\left\lfloor \frac{n}{2} \right\rfloor} \sum_{\ell = \max\{1, 2k\}}^n \frac{1}{4^k} {\ell \choose 2k} = \frac{3^{n+1} - 1}{2^{n+1}} - 1. $$