# Solution

I'll prove that if we start with the sequence $(1, 2, \ldots, n)$, after $(n-1)$ actions, the resulting number is less than $\frac{n+1}{2}$.

## Finding a formula for the result

Let me first establish what happens after each action. Let's denote the sequence after $k$ actions as $s_k$, where $s_0 = (1, 2, \ldots, n)$ is our initial sequence.

After the first action:
$s_1 = (\sqrt{1 \cdot 2}, \sqrt{2 \cdot 3}, \ldots, \sqrt{(n-1) \cdot n})$

After the second action:
$s_2 = (\sqrt{\sqrt{1 \cdot 2} \cdot \sqrt{2 \cdot 3}}, \ldots)$

This can be simplified to:
$s_2 = ((1 \cdot 2^2 \cdot 3)^{1/4}, \ldots)$

Continuing this pattern and tracking the exponents of each original number, after $(n-1)$ actions, the final result can be expressed as:

$$\text{result} = \left(\prod_{i=1}^{n} i^{C(n-1, i-1)}\right)^{1/2^{n-1}}$$

where $C(n-1, i-1)$ represents the binomial coefficient $\binom{n-1}{i-1}$.

## Verifying the formula

Let's verify this formula for a simple case, $n = 3$:
- Initial sequence: $(1, 2, 3)$
- After first action: $(\sqrt{1 \cdot 2}, \sqrt{2 \cdot 3}) = (\sqrt{2}, \sqrt{6})$
- After second action: $\sqrt{\sqrt{2} \cdot \sqrt{6}} = (2 \cdot 6)^{1/4} = 12^{1/4}$

Using our formula: $\left(1^{C(2,0)} \cdot 2^{C(2,1)} \cdot 3^{C(2,2)}\right)^{1/2^2} = \left(1^1 \cdot 2^2 \cdot 3^1\right)^{1/4} = 12^{1/4}$

The formula matches our calculation.

## Proving the inequality

The expression $\left(\prod_{i=1}^{n} i^{C(n-1, i-1)}\right)^{1/2^{n-1}}$ can be interpreted as a weighted geometric mean of the numbers $1, 2, \ldots, n$ with weights $\frac{C(n-1, i-1)}{2^{n-1}}$.

The corresponding weighted arithmetic mean is:
$$\sum_{i=1}^{n} \frac{C(n-1, i-1)}{2^{n-1}} \cdot i$$

Through a change of index $j = i-1$, this becomes:
$$\sum_{j=0}^{n-1} \frac{C(n-1, j)}{2^{n-1}} \cdot (j+1) = \sum_{j=0}^{n-1} \frac{C(n-1, j)}{2^{n-1}} \cdot j + \sum_{j=0}^{n-1} \frac{C(n-1, j)}{2^{n-1}}$$

Since $\sum_{j=0}^{n-1} C(n-1, j) = 2^{n-1}$, the second sum equals 1.

The first sum represents the expected value of a binomial random variable $X \sim \text{Bin}(n-1, 0.5)$, which is $E[X] = (n-1) \cdot 0.5 = \frac{n-1}{2}$.

Therefore, the weighted arithmetic mean equals $\frac{n-1}{2} + 1 = \frac{n+1}{2}$.

By the AM-GM inequality, the weighted geometric mean is less than or equal to the weighted arithmetic mean, with equality if and only if all numbers are the same. Since the numbers $1, 2, \ldots, n$ are not all the same for $n > 1$, we have:

$$\text{result} = \left(\prod_{i=1}^{n} i^{C(n-1, i-1)}\right)^{1/2^{n-1}} < \frac{n+1}{2}$$

This proves that the result is smaller than $\frac{n+1}{2}$ as required.