First, we determine the coordinates of the centers and the original radii of the circles from the provided image.
Let the circles be denoted by their centers A, B, C, D, and E.
From the grid, we can read the coordinates of the centers:
A = (2, 2)
B = (5, 2)
C = (5, 0)
D = (4, -2)
E = (2, -1)

The circles are tangent to each other in a chain: A-B-C-D-E-A.
Let the original radii be $r_A, r_B, r_C, r_D, r_E$.
From the image, the radius of circle A is $r_A = 2$.
The distance between the centers of two tangent circles is the sum of their radii.
1.  Distance $d_{AB} = \sqrt{(5-2)^2 + (2-2)^2} = 3$. So, $r_A + r_B = 3$. Since $r_A = 2$, we get $r_B = 1$.
2.  Distance $d_{BC} = \sqrt{(5-5)^2 + (0-2)^2} = 2$. So, $r_B + r_C = 2$. Since $r_B = 1$, we get $r_C = 1$.
3.  Distance $d_{CD} = \sqrt{(4-5)^2 + (-2-0)^2} = \sqrt{1+4} = \sqrt{5}$. So, $r_C + r_D = \sqrt{5}$. Since $r_C = 1$, we get $r_D = \sqrt{5} - 1$.
4.  Distance $d_{DE} = \sqrt{(2-4)^2 + (-1-(-2))^2} = \sqrt{4+1} = \sqrt{5}$. So, $r_D + r_E = \sqrt{5}$. Since $r_D = \sqrt{5}-1$, we get $r_E = 1$.
5.  Distance $d_{EA} = \sqrt{(2-2)^2 + (2-(-1))^2} = 3$. So, $r_E + r_A = 3$. As a check, $1 + 2 = 3$, which is correct.

The problem states we can adjust the radii such that the tangency relationships are preserved. Let the new radii be $r'_A, r'_B, r'_C, r'_D, r'_E$. The condition implies that the sum of radii for tangent pairs must equal the fixed distance between their centers.
1.  $r'_A + r'_B = 3$
2.  $r'_B + r'_C = 2$
3.  $r'_C + r'_D = \sqrt{5}$
4.  $r'_D + r'_E = \sqrt{5}$
5.  $r'_E + r'_A = 3$

Let's see if we can change the radii. Suppose we change $r'_A$ by a small amount $\delta$, so $r'_A = r_A + \delta = 2 + \delta$.
From (1), $r'_B = 3 - r'_A = 3 - (2+\delta) = 1 - \delta = r_B - \delta$.
From (2), $r'_C = 2 - r'_B = 2 - (1-\delta) = 1 + \delta = r_C + \delta$.
From (3), $r'_D = \sqrt{5} - r'_C = \sqrt{5} - (1+\delta) = (\sqrt{5}-1) - \delta = r_D - \delta$.
From (4), $r'_E = \sqrt{5} - r'_D = \sqrt{5} - (\sqrt{5}-1-\delta) = 1 + \delta = r_E + \delta$.
Now we substitute these back into the last constraint (5):
$r'_E + r'_A = (r_E + \delta) + (r_A + \delta) = (r_E + r_A) + 2\delta$.
Since we must have $r'_E + r'_A = d_{EA} = r_E + r_A$, this gives:
$(r_E + r_A) + 2\delta = r_E + r_A$
$2\delta = 0 \implies \delta = 0$.
This shows that the radii cannot be changed at all. The only possible adjustment is no adjustment.

Therefore, the maximum possible sum of areas is simply the sum of the areas of the original circles.
The total area $S$ is the sum of the areas of the five circles, $S = \sum \pi r_i^2$.
$$S = \pi (r_A^2 + r_B^2 + r_C^2 + r_D^2 + r_E^2)$$
$$S = \pi (2^2 + 1^2 + 1^2 + (\sqrt{5} - 1)^2 + 1^2)$$
$$S = \pi (4 + 1 + 1 + (5 - 2\sqrt{5} + 1) + 1)$$
$$S = \pi (7 + 6 - 2\sqrt{5})$$
$$S = \pi (13 - 2\sqrt{5})$$
Now, we calculate the numerical value:
$S \approx 3.14159265 \times (13 - 2 \times 2.23606798) \approx 3.14159265 \times (13 - 4.47213596)$
$S \approx 3.14159265 \times 8.52786404 \approx 26.791075$

The problem asks to round the answer to the nearest integer. Rounding 26.791075 to the nearest integer gives 27.