Solution:
Let $B(0,1)$ denote the unit ball in $\mathbb{R}^n$. We want to show that
$$ I = \int_{B(0,1)} |x_1|^{2k} \, dx \geq \frac{\omega_n}{n^{k} (2k+n)} $$
for any integer $k \geq 1$, where $\omega_n$ denotes the surface area of the unit sphere $S^{n-1} = \partial B(0,1)$ in $\mathbb{R}^n$.

We use spherical coordinates in $\mathbb{R}^n$. Let $x = (x_1, \dots, x_n)$. The spherical coordinates $(r, \phi_1, \dots, \phi_{n-1})$ are defined by:
$x_1 = r \cos\phi_1$
$x_2 = r \sin\phi_1 \cos\phi_2$
...
$x_{n-1} = r \sin\phi_1 \dots \sin\phi_{n-2} \cos\phi_{n-1}$
$x_n = r \sin\phi_1 \dots \sin\phi_{n-2} \sin\phi_{n-1}$
where $r \in [0, \infty)$, $\phi_1, \dots, \phi_{n-2} \in [0, \pi]$, and $\phi_{n-1} \in [0, 2\pi)$.
The volume element is $dx = r^{n-1} \sin^{n-2}\phi_1 \sin^{n-3}\phi_2 \dots \sin\phi_{n-2} dr d\phi_1 \dots d\phi_{n-1}$.
The integral is over the unit ball $B(0,1)$, so $r \in [0, 1]$. The integrand is $|x_1|^{2k} = (x_1^2)^k = (r \cos\phi_1)^{2k} = r^{2k} \cos^{2k}\phi_1$.

The integral becomes:
$$ I = \int_0^1 \int_0^\pi \dots \int_0^{2\pi} (r^{2k} \cos^{2k}\phi_1) (r^{n-1} \sin^{n-2}\phi_1 \dots \sin\phi_{n-2}) dr d\phi_1 \dots d\phi_{n-1} $$
We can separate the radial part and the angular parts:
$$ I = \left( \int_0^1 r^{2k+n-1} dr \right) \left( \int_0^\pi \dots \int_0^{2\pi} \cos^{2k}\phi_1 \sin^{n-2}\phi_1 \dots \sin\phi_{n-2} d\phi_1 \dots d\phi_{n-1} \right) $$
The radial integral is:
$$ \int_0^1 r^{2k+n-1} dr = \left[ \frac{r^{2k+n}}{2k+n} \right]_0^1 = \frac{1}{2k+n} $$
The angular integral can be split:
$$ \int_0^\pi \dots \int_0^{2\pi} \cos^{2k}\phi_1 \sin^{n-2}\phi_1 \dots \sin\phi_{n-2} d\phi_1 \dots d\phi_{n-1} = \left( \int_0^\pi \cos^{2k}\phi_1 \sin^{n-2}\phi_1 d\phi_1 \right) \left( \int_0^\pi \sin^{n-3}\phi_2 d\phi_2 \dots \int_0^{2\pi} d\phi_{n-1} \right) $$
Let $A = \int_0^\pi \cos^{2k}\phi_1 \sin^{n-2}\phi_1 d\phi_1$.
Let $C = \int_0^\pi \sin^{n-3}\phi_2 d\phi_2 \dots \int_0^{2\pi} d\phi_{n-1}$.
So $I = \frac{1}{2k+n} A C$.

The surface area of the unit sphere $S^{n-1}$ is given by $\omega_n$. In spherical coordinates, the surface element $d\sigma = \sin^{n-2}\phi_1 \dots \sin\phi_{n-2} d\phi_1 \dots d\phi_{n-1}$.
$$ \omega_n = \int_{S^{n-1}} d\sigma = \int_0^\pi \dots \int_0^{2\pi} \sin^{n-2}\phi_1 \dots \sin\phi_{n-2} d\phi_1 \dots d\phi_{n-1} $$
$$ \omega_n = \left( \int_0^\pi \sin^{n-2}\phi_1 d\phi_1 \right) \left( \int_0^\pi \sin^{n-3}\phi_2 d\phi_2 \dots \int_0^{2\pi} d\phi_{n-1} \right) $$
Let $B = \int_0^\pi \sin^{n-2}\phi_1 d\phi_1$. Then $\omega_n = B C$.
Substituting $C = \omega_n / B$ into the expression for $I$:
$$ I = \frac{1}{2k+n} A \frac{\omega_n}{B} = \frac{\omega_n}{2k+n} \frac{A}{B} $$

Now we need to evaluate the ratio $A/B$. We use the Beta function definition $B(x,y) = 2 \int_0^{\pi/2} (\sin\theta)^{2x-1} (\cos\theta)^{2y-1} d\theta = \frac{\Gamma(x)\Gamma(y)}{\Gamma(x+y)}$.
Since $\cos^{2k}\phi$ and $\sin^{n-2}\phi$ are symmetric about $\phi=\pi/2$, we have:
$A = 2 \int_0^{\pi/2} \cos^{2k}\phi \sin^{n-2}\phi d\phi$.
We set $2x-1 = n-2 \implies x = (n-1)/2$ and $2y-1 = 2k \implies y = (2k+1)/2$.
$A = B(\frac{n-1}{2}, \frac{2k+1}{2}) = \frac{\Gamma(\frac{n-1}{2}) \Gamma(k+\frac{1}{2})}{\Gamma(\frac{n-1}{2}+k+\frac{1}{2})} = \frac{\Gamma(\frac{n-1}{2}) \Gamma(k+\frac{1}{2})}{\Gamma(k+\frac{n}{2})}$.

$B = \int_0^\pi \sin^{n-2}\phi d\phi = 2 \int_0^{\pi/2} \sin^{n-2}\phi \cos^0\phi d\phi$.
We set $2x-1 = n-2 \implies x = (n-1)/2$ and $2y-1 = 0 \implies y = 1/2$.
$B = B(\frac{n-1}{2}, \frac{1}{2}) = \frac{\Gamma(\frac{n-1}{2}) \Gamma(\frac{1}{2})}{\Gamma(\frac{n-1}{2}+\frac{1}{2})} = \frac{\Gamma(\frac{n-1}{2}) \Gamma(\frac{1}{2})}{\Gamma(\frac{n}{2})}$.

The ratio is:
$$ \frac{A}{B} = \frac{\Gamma(\frac{n-1}{2}) \Gamma(k+\frac{1}{2})}{\Gamma(k+\frac{n}{2})} \frac{\Gamma(\frac{n}{2})}{\Gamma(\frac{n-1}{2}) \Gamma(\frac{1}{2})} = \frac{\Gamma(k+\frac{1}{2}) \Gamma(\frac{n}{2})}{\Gamma(k+\frac{n}{2}) \Gamma(\frac{1}{2})} $$
Using the property $\Gamma(z+m) = (z+m-1)(z+m-2)\dots z \Gamma(z)$:
$\Gamma(k+\frac{1}{2}) = (k-\frac{1}{2})(k-\frac{3}{2})\dots(\frac{1}{2}) \Gamma(\frac{1}{2})$.
$\Gamma(k+\frac{n}{2}) = (k+\frac{n}{2}-1)(k+\frac{n}{2}-2)\dots(\frac{n}{2}) \Gamma(\frac{n}{2})$.
So,
$$ \frac{A}{B} = \frac{[(k-1/2)(k-3/2)\dots(1/2)] \Gamma(1/2) \Gamma(n/2)}{[(k+n/2-1)(k+n/2-2)\dots(n/2)] \Gamma(n/2) \Gamma(1/2)} = \frac{(k-1/2)(k-3/2)\dots(1/2)}{(k+n/2-1)(k+n/2-2)\dots(n/2)} $$
Multiply numerator and denominator by $2^k$:
$$ \frac{A}{B} = \frac{(2k-1)(2k-3)\dots(1)}{(2k+n-2)(2k+n-4)\dots(n)} = \frac{(2k-1)!!}{n(n+2)\dots(n+2k-2)} $$
Here $(2k-1)!! = (2k-1)(2k-3)\dots 3 \cdot 1$ is the double factorial.

We want to show $I \geq \frac{\omega_n}{n^{k} (2k+n)}$. Substituting $I = \frac{\omega_n}{2k+n} \frac{A}{B}$:
$$ \frac{\omega_n}{2k+n} \frac{A}{B} \geq \frac{\omega_n}{n^{k} (2k+n)} $$
This is equivalent to showing:
$$ \frac{A}{B} \geq \frac{1}{n^k} $$
Substituting the expression for $A/B$:
$$ \frac{(2k-1)!!}{n(n+2)\dots(n+2k-2)} \geq \frac{1}{n^k} $$
Multiply both sides by $n^k$ and the denominator:
$$ n^k (2k-1)!! \geq n(n+2)(n+4)\dots(n+2k-2) $$
The right hand side is a product of $k$ terms: $\prod_{j=0}^{k-1} (n+2j)$.
The left hand side is $n^k (2k-1)!! = n^k \prod_{j=1}^{k} (2j-1) = \prod_{j=1}^{k} [n(2j-1)]$.

We prove the inequality by comparing the $j$-th terms of the products. We claim that for each $j=1, 2, \dots, k$:
$$ n(2j-1) \geq n+2j-2 $$
Let's verify this inequality.
$$ 2nj - n \geq n + 2j - 2 $$
$$ 2nj - 2j \geq 2n - 2 $$
$$ 2j(n-1) \geq 2(n-1) $$
If $n=1$, the inequality becomes $0 \geq 0$, which is true.
If $n > 1$, then $n-1 > 0$. We can divide by $2(n-1)$:
$$ j \geq 1 $$
This is true for all $j=1, 2, \dots, k$, since $k \geq 1$.
So the inequality $n(2j-1) \geq n+2j-2$ holds for all $j \in \{1, \dots, k\}$ and $n \geq 1$.

Now, we multiply these inequalities for $j=1, \dots, k$:
$$ \prod_{j=1}^{k} [n(2j-1)] \geq \prod_{j=1}^{k} (n+2j-2) $$
$$ n^k \prod_{j=1}^{k} (2j-1) \geq n(n+2)(n+4)\dots(n+2k-2) $$
$$ n^k (2k-1)!! \geq n(n+2)\dots(n+2k-2) $$
This confirms the inequality $\frac{A}{B} \geq \frac{1}{n^k}$.

Since $I = \frac{\omega_n}{2k+n} \frac{A}{B}$ and $\frac{A}{B} \geq \frac{1}{n^k}$, we have:
$$ I \geq \frac{\omega_n}{2k+n} \frac{1}{n^k} = \frac{\omega_n}{n^k (2k+n)} $$
This completes the proof.

Final Answer: The final answer is $\boxed{\int_{B(0,1)} |x_1|^{2k} \, dx \geq \frac{\omega_n}{n^{k} (2k+n)}}$