Let $S$ denote the sum we want to prove is non-positive:
$$
S = \sum_{k=1}^n \sum_{1 \leq i_1 < \ldots < i_k \leq n} (-1)^{k} \frac{m_{i_1, \ldots, i_k}^{2N+i_1+\ldots+i_k-1}}{i_1 + \ldots + i_k + N}.
$$
Let $I = \{i_1, \ldots, i_k\}$ be a non-empty subset of $\{1, \ldots, n\}$. Let $s(I) = \sum_{j \in I} j$ denote the sum of elements in $I$, and $|I| = k$ denote the cardinality of $I$. Let $m_I = \min \{ r_i : i \in I \}$.
The sum can be rewritten as:
$$
S = \sum_{\emptyset \neq I \subseteq \{1, \ldots, n\}} (-1)^{|I|} \frac{m_I^{2N+s(I)-1}}{s(I) + N}.
$$
We can express the term $\frac{m_I^{s(I)+N}}{s(I)+N}$ as an integral:
$$
\frac{m_I^{s(I)+N}}{s(I)+N} = \int_0^{m_I} x^{s(I)+N-1} dx.
$$
The term in the sum $S$ is $\frac{m_I^{2N+s(I)-1}}{s(I)+N} = m_I^{N-1} \frac{m_I^{s(I)+N}}{s(I)+N}$. Since $N \in \mathbb{N}$, $N-1 \ge 0$. $m_I \in (0,1)$, so $m_I^{N-1}$ is well-defined and positive.
$$
S = \sum_{\emptyset \neq I \subseteq \{1, \ldots, n\}} (-1)^{|I|} m_I^{N-1} \int_0^{m_I} x^{s(I)+N-1} dx.
$$
Since $m_I^{N-1}$ is a constant with respect to the integration variable $x$, we can bring it inside the integral:
$$
S = \sum_{\emptyset \neq I \subseteq \{1, \ldots, n\}} (-1)^{|I|} \int_0^{m_I} m_I^{N-1} x^{s(I)+N-1} dx.
$$
Now we can swap the summation and the integration. The integral is over $(0, m_I]$. We can extend the integration range to $(0, 1)$ by using an indicator function $\mathbf{1}_{x \leq m_I}$.
$$
S = \sum_{\emptyset \neq I \subseteq \{1, \ldots, n\}} (-1)^{|I|} \int_0^1 \mathbf{1}_{x \leq m_I} m_I^{N-1} x^{s(I)+N-1} dx.
$$
$$
S = \int_0^1 \sum_{\emptyset \neq I \subseteq \{1, \ldots, n\}} (-1)^{|I|} \mathbf{1}_{x \leq m_I} m_I^{N-1} x^{s(I)+N-1} dx.
$$
For a fixed $x \in (0,1)$, the condition $x \leq m_I = \min_{i \in I} r_i$ is equivalent to $x \leq r_i$ for all $i \in I$. Let $K_x = \{i \in \{1, \ldots, n\} : r_i \geq x\}$. Then $x \leq m_I$ if and only if $I \subseteq K_x$.
The sum inside the integral becomes:
$$
\sum_{\emptyset \neq I \subseteq K_x} (-1)^{|I|} m_I^{N-1} x^{s(I)+N-1}.
$$
Factor out $x^{N-1}$:
$$
x^{N-1} \sum_{\emptyset \neq I \subseteq K_x} (-1)^{|I|} m_I^{N-1} x^{s(I)}.
$$
Let $F(x) = \sum_{\emptyset \neq I \subseteq K_x} (-1)^{|I|} m_I^{N-1} x^{s(I)}$. Then the integral is $S = \int_0^1 x^{N-1} F(x) dx$.
We need to show that $F(x) \leq 0$ for all $x \in (0,1)$.
Let $K_x = K = \{k_1, k_2, \ldots, k_p\}$ where $p = |K_x|$. If $K_x$ is empty, then $F(x) = 0$. Assume $K_x$ is not empty. Let the elements of $K$ be indexed such that the corresponding $r_i$ values are sorted: $r_{k_1} \leq r_{k_2} \leq \ldots \leq r_{k_p}$. Note that $r_{k_j} \geq x$ for all $j=1, \ldots, p$.
We can group the terms in the sum $F(x)$ based on the value of $m_I = \min_{i \in I} r_i$. The value $m_I$ must be one of the $r_{k_j}$.
$m_I = r_{k_j}$ if and only if $k_j \in I$ and $I \subseteq \{k_j, k_{j+1}, \ldots, k_p\}$. Let $K_{\ge j} = \{k_j, k_{j+1}, \ldots, k_p\}$.
$$
F(x) = \sum_{j=1}^p \sum_{I \subseteq K_{\ge j}, k_j \in I} (-1)^{|I|} r_{k_j}^{N-1} x^{s(I)}.
$$
Let $I = I' \cup \{k_j\}$, where $I' \subseteq K_{\ge j+1} = \{k_{j+1}, \ldots, k_p\}$. Then $|I| = |I'|+1$ and $s(I) = s(I') + k_j$.
The inner sum for a fixed $j$ is:
$$
\sum_{I' \subseteq K_{\ge j+1}} (-1)^{|I'|+1} r_{k_j}^{N-1} x^{s(I')+k_j}.
$$
$$
= (-1) r_{k_j}^{N-1} x^{k_j} \sum_{I' \subseteq K_{\ge j+1}} (-1)^{|I'|} x^{s(I')}.
$$
The sum $\sum_{I' \subseteq K_{\ge j+1}} (-1)^{|I'|} x^{s(I')}$ is the expansion of the product $\prod_{l=j+1}^p (1 - x^{k_l})$. Note that the empty product (for $j=p$) is 1.
So the inner sum is:
$$
(-1) r_{k_j}^{N-1} x^{k_j} \prod_{l=j+1}^p (1 - x^{k_l}).
$$
Therefore,
$$
F(x) = \sum_{j=1}^p (-1) r_{k_j}^{N-1} x^{k_j} \prod_{l=j+1}^p (1 - x^{k_l}).
$$
Now we analyze the sign of each term in this sum.
Since $r_i \in (0,1)$ and $N \in \mathbb{N}$, $N-1 \ge 0$, so $r_{k_j}^{N-1} > 0$.
Since $x \in (0,1)$ and $k_j \in \{1, \ldots, n\}$, $x^{k_j} > 0$.
Since $x \in (0,1)$ and $k_l \in \{1, \ldots, n\}$, $x^{k_l} \in (0,1)$, so $1 - x^{k_l} \in (0,1)$.
The product $\prod_{l=j+1}^p (1 - x^{k_l})$ is positive (or 1 if $j=p$).
Thus, each term $(-1) r_{k_j}^{N-1} x^{k_j} \prod_{l=j+1}^p (1 - x^{k_l})$ is negative.
So $F(x)$ is a sum of negative terms. Hence $F(x) \leq 0$. If $K_x$ is empty, $F(x)=0$.

Now we return to the integral $S = \int_0^1 x^{N-1} F(x) dx$.
Since $N \in \mathbb{N}$, $N-1 \ge 0$. For $x \in (0,1)$, $x^{N-1} \geq 0$.
The integrand $x^{N-1} F(x)$ is the product of a non-negative function $x^{N-1}$ and a non-positive function $F(x)$.
Therefore, the integrand $x^{N-1} F(x) \leq 0$ for all $x \in (0,1)$.
The integral of a non-positive function over $(0,1)$ must be non-positive.
$$
S = \int_0^1 x^{N-1} F(x) dx \leq 0.
$$
This completes the proof.

Final check of the steps:
1. Rewrite sum definition.
2. Express term as $m_I^{N-1}$ times an integral $\int_0^{m_I} x^{s(I)+N-1} dx$.
3. Swap sum and integral, using indicator function $\mathbf{1}_{x \le m_I}$.
4. Identify the condition $I \subseteq K_x$.
5. Factor out $x^{N-1}$ from the inner sum $F(x)$.
6. Analyze the sign of $F(x)$ by grouping terms according to $m_I$.
7. Show $F(x) \leq 0$ using the product formula $\sum_{I' \subseteq K'} (-1)^{|I'|} x^{s(I')} = \prod_{k \in K'} (1-x^k)$.
8. Conclude the integral $S$ is non-positive because the integrand is non-positive.

All steps seem correct.

Final expression for $F(x)$:
$F(x) = \sum_{j=1}^p (-1) r_{k_j}^{N-1} x^{k_j} \prod_{l=j+1}^p (1 - x^{k_l})$.
This shows $F(x) \leq 0$.


```markdown
Let $S$ denote the sum we want to prove is non-positive:
$$
S = \sum_{k=1}^n \sum_{1 \leq i_1 < \ldots < i_k \leq n} (-1)^{k} \frac{m_{i_1, \ldots, i_k}^{2N+i_1+\ldots+i_k-1}}{i_1 + \ldots + i_k + N}.
$$
Let $I = \{i_1, \ldots, i_k\}$ be a non-empty subset of $\{1, \ldots, n\}$. Let $s(I) = \sum_{j \in I} j$ denote the sum of elements in $I$, and $|I| = k$ denote the cardinality of $I$. Let $m_I = \min \{ r_i : i \in I \}$.
The sum can be rewritten using this notation as:
$$
S = \sum_{\emptyset \neq I \subseteq \{1, \ldots, n\}} (-1)^{|I|} \frac{m_I^{2N+s(I)-1}}{s(I) + N}.
$$
We can express the term $\frac{a^P}{P}$ using the integral representation $\frac{a^P}{P} = \int_0^a x^{P-1} dx$. Let $P = s(I)+N$. We have the term $\frac{m_I^{2N+s(I)-1}}{s(I) + N}$.
We can rewrite the term as:
$$
\frac{m_I^{2N+s(I)-1}}{s(I) + N} = m_I^{N-1} \frac{m_I^{s(I)+N}}{s(I)+N}.
$$
Since $N \in \mathbb{N}$, $N-1 \ge 0$. Since $r_i \in (0,1)$, $m_I \in (0,1)$, so $m_I^{N-1}$ is well-defined and positive.
Using the integral representation for the second part:
$$
\frac{m_I^{s(I)+N}}{s(I)+N} = \int_0^{m_I} x^{s(I)+N-1} dx.
$$
Substituting this into the sum $S$:
$$
S = \sum_{\emptyset \neq I \subseteq \{1, \ldots, n\}} (-1)^{|I|} m_I^{N-1} \int_0^{m_I} x^{s(I)+N-1} dx.
$$
Since $m_I^{N-1}$ is a constant with respect to the integration variable $x$, we can move it inside the integral:
$$
S = \sum_{\emptyset \neq I \subseteq \{1, \ldots, n\}} (-1)^{|I|} \int_0^{m_I} m_I^{N-1} x^{s(I)+N-1} dx.
$$
We can swap the summation and integration. To do this, we extend the integration range to $(0, 1)$ by introducing an indicator function $\mathbf{1}_{x \leq m_I}$. The condition $x \leq m_I$ means $x \leq r_i$ for all $i \in I$.
$$
S = \sum_{\emptyset \neq I \subseteq \{1, \ldots, n\}} (-1)^{|I|} \int_0^1 \mathbf{1}_{x \leq m_I} m_I^{N-1} x^{s(I)+N-1} dx.
$$
$$
S = \int_0^1 \sum_{\emptyset \neq I \subseteq \{1, \ldots, n\}} (-1)^{|I|} \mathbf{1}_{x \leq m_I} m_I^{N-1} x^{s(I)+N-1} dx.
$$
For a fixed $x \in (0,1)$, let $K_x = \{i \in \{1, \ldots, n\} : r_i \geq x\}$. The condition $x \leq m_I = \min_{i \in I} r_i$ is equivalent to $x \leq r_i$ for all $i \in I$, which means $I \subseteq K_x$.
The sum inside the integral becomes:
$$
\sum_{\emptyset \neq I \subseteq K_x} (-1)^{|I|} m_I^{N-1} x^{s(I)+N-1}.
$$
We can factor out $x^{N-1}$ from the sum:
$$
x^{N-1} \sum_{\emptyset \neq I \subseteq K_x} (-1)^{|I|} m_I^{N-1} x^{s(I)}.
$$
Let $F(x) = \sum_{\emptyset \neq I \subseteq K_x} (-1)^{|I|} m_I^{N-1} x^{s(I)}$. Then the integral is $S = \int_0^1 x^{N-1} F(x) dx$.
We now show that $F(x) \leq 0$ for all $x \in (0,1)$.
If $K_x$ is empty, then $F(x) = 0$. Assume $K_x$ is not empty. Let $K_x = K = \{k_1, k_2, \ldots, k_p\}$ where $p = |K_x|$. Let the elements of $K$ be indexed such that the corresponding $r_i$ values are sorted in non-decreasing order: $r_{k_1} \leq r_{k_2} \leq \ldots \leq r_{k_p}$. Note that $r_{k_j} \geq x$ for all $j=1, \ldots, p$.
We group the terms in the sum $F(x)$ based on the value of $m_I = \min_{i \in I} r_i$. The value $m_I$ must be one of the $r_{k_j}$ for some $j \in \{1, \dots, p\}$.
$m_I = r_{k_j}$ if and only if $k_j \in I$ and $I \subseteq \{k_j, k_{j+1}, \ldots, k_p\}$. Let $K_{\ge j} = \{k_j, k_{j+1}, \ldots, k_p\}$.
$$
F(x) = \sum_{j=1}^p \sum_{I \subseteq K_{\ge j}, k_j \in I} (-1)^{|I|} m_I^{N-1} x^{s(I)} = \sum_{j=1}^p \sum_{I \subseteq K_{\ge j}, k_j \in I} (-1)^{|I|} r_{k_j}^{N-1} x^{s(I)}.
$$
Let $I = I' \cup \{k_j\}$, where $I' \subseteq K_{\ge j+1} = \{k_{j+1}, \ldots, k_p\}$. Then $|I| = |I'|+1$ and $s(I) = s(I') + k_j$.
The inner sum for a fixed $j$ is:
$$
\sum_{I' \subseteq K_{\ge j+1}} (-1)^{|I'|+1} r_{k_j}^{N-1} x^{s(I')+k_j}.
$$
$$
= (-1) r_{k_j}^{N-1} x^{k_j} \sum_{I' \subseteq K_{\ge j+1}} (-1)^{|I'|} x^{s(I')}.
$$
The sum $\sum_{I' \subseteq K_{\ge j+1}} (-1)^{|I'|} x^{s(I')}$ is the expansion of the product $\prod_{l=j+1}^p (1 - x^{k_l})$. The empty product (for $j=p$) is defined as 1.
So the inner sum is:
$$
(-1) r_{k_j}^{N-1} x^{k_j} \prod_{l=j+1}^p (1 - x^{k_l}).
$$
Substituting this back into the expression for $F(x)$:
$$
F(x) = \sum_{j=1}^p (-1) r_{k_j}^{N-1} x^{k_j} \prod_{l=j+1}^p (1 - x^{k_l}).
$$
Now we analyze the sign of each term in this sum for $x \in (0,1)$.
Since $r_i \in (0,1)$ and $N \in \mathbb{N}$, $N-1 \ge 0$. Thus $r_{k_j}^{N-1} > 0$.
Since $x \in (0,1)$ and $k_j \in \{1, \ldots, n\}$, $k_j \ge 1$, so $x^{k_j} > 0$.
Since $x \in (0,1)$ and $k_l \in \{1, \ldots, n\}$, $k_l \ge 1$, so $x^{k_l} \in (0,1)$. This implies $1 - x^{k_l} \in (0,1)$.
The product $\prod_{l=j+1}^p (1 - x^{k_l})$ is a product of positive numbers in $(0,1)$, hence it is positive (or 1 if $j=p$).
Therefore, each term $(-1) r_{k_j}^{N-1} x^{k_j} \prod_{l=j+1}^p (1 - x^{k_l})$ is negative.
Since $F(x)$ is a sum of negative terms, $F(x) \leq 0$. If $K_x$ is empty, $F(x)=0$.

Now we return to the integral expression for $S$:
$$
S = \int_0^1 x^{N-1} F(x) dx.
$$
Since $N \in \mathbb{N}$, $N-1 \ge 0$. For $x \in (0,1)$, $x^{N-1} \geq 0$.
The integrand $x^{N-1} F(x)$ is the product of a non-negative function $x^{N-1}$ and a non-positive function $F(x)$.
Therefore, the integrand $x^{N-1} F(x) \leq 0$ for all $x \in (0,1)$.
The integral of a non-positive function over a positive interval $(0,1)$ must be non-positive.
$$
S = \int_0^1 x^{N-1} F(x) dx \leq 0.
$$
This completes the proof.
```