Notice that:
$$a_2=a_4-a_2+1-8+4$$
\noindent so:
$$a_2=\frac{1}{2} \left(a_4-3\right)=\frac{1}{2}(11-3)=4.$$
Hence we have $$a_1=a_2-a_1+1-2+1$$
\noindent so:
$$a_1=\frac{1}{2} a_2=\frac{1}{2} \cdot 4=2.$$
\noindent so:
$$a_{n-1}=a_n-a_1+1-n \cdot 1+1^2$$
\noindent and we have:
$$a_n-a_{n-1}=n$$

\noindent and since:
\begin{eqnarray*}
a_n=(a_n-a_{n-1})+(a_{n-1}-a_{n-2})+\cdots+(a_{2}-a_1)+a_1 =\\ n + (n-1)+(n-2)+\cdots+3+2+2=\frac{n(n+1)}{2}+1.
\end{eqnarray*}
\noindent so:
$$a_{2024}=\frac{2024 \cdot 2025}{2}+1=2049301.$$