**Solution:**

Let \(G\) be the group defined by the presentation
\[
G = \langle x, y : x^n=e, y^2=e, xyxy=e \rangle
\]
where \( n \in \mathbb{N} \) and \( n \geq 3 \). We want to prove that \(G\) is a non-abelian group of order \(2n\).

**1. Simplifying the Relations**

The relations are:
(1) \(x^n = e\)
(2) \(y^2 = e\)
(3) \(xyxy = e\)

From relation (2), we have \(y = y^{-1}\).
We can manipulate relation (3):
\(xyxy = e\)
Multiply by \(y^{-1}\) on the right:
\(xyx y y^{-1} = e y^{-1}\)
\(xyx = y^{-1}\)
Using \(y^{-1}=y\), we get:
(4) \(xyx = y\)

Alternatively, multiply \(xyx=y\) by \(x^{-1}\) on the left:
\(x^{-1}xyx = x^{-1}y\)
\(yx = x^{-1}y\)

This relation \(yx = x^{-1}y\) is crucial. It allows us to express any product of \(x\)'s and \(y\)'s in a standard form.

Let's verify that \(yx=x^{-1}y\) is consistent with the original relation \(xyxy=e\).
If \(yx=x^{-1}y\), then \(xy = x(x^{-1}y)y = ey^2 = e\). This seems wrong. Let's re-derive.
Start from \(xyxy=e\).
Multiply by \(x^{-1}\) on the left: \(yxy = x^{-1}\).
Multiply by \(y^{-1}\) on the right: \(yx = x^{-1}y^{-1}\).
Since \(y^2=e\), \(y^{-1}=y\). So, \(yx = x^{-1}y\). This derivation is correct.

Let's check the consistency again. If \(yx = x^{-1}y\):
\(xyxy = x(yx)y = x(x^{-1}y)y = (xx^{-1})y^2 = e \cdot e = e\).
This confirms that the relation \(xyxy=e\) is equivalent to \(yx=x^{-1}y\) (given \(y^2=e\)).

The set of relations defining \(G\) is equivalent to:
\[
\langle x, y : x^n=e, y^2=e, yx=x^{-1}y \rangle
\]
or equivalently
\[
\langle x, y : x^n=e, y^2=e, yxy=x^{-1} \rangle
\]

**2. Showing \(|G| \le 2n\)**

Since \(G\) is generated by \(x\) and \(y\), any element of \(G\) can be written as a word in \(x, y, x^{-1}, y^{-1}\). Using \(y^{-1}=y\) and \(x^{-1}=x^{n-1}\) (from \(x^n=e\)), any element can be written as a product of \(x\)'s and \(y\)'s.
The relation \(yx = x^{-1}y\) allows us to move all occurrences of \(y\) to the right. For example:
\(x^a y x^b = x^a (y x) x^{b-1} = x^a (x^{-1} y) x^{b-1} = x^{a-1} y x^{b-1}\).
By repeatedly applying this, any word can be transformed into the form \(x^i y^j\) for some integers \(i, j\).

Using \(x^n=e\), we can assume \(0 \le i \le n-1\).
Using \(y^2=e\), we can assume \(j \in \{0, 1\}\).

Therefore, any element of \(G\) can be written in the form \(x^i y^j\) where \(0 \le i < n\) and \(j \in \{0, 1\}\).
The set of these elements is \(S = \{x^i y^j : 0 \le i < n, j \in \{0, 1\}\}\).
The number of elements in this set is \(n \times 2 = 2n\).
This shows that \(|G| \le 2n\).

**3. Showing \(|G| \ge 2n\)**

The presentation \( \langle x, y : x^n=e, y^2=e, yxy=x^{-1} \rangle \) is the standard presentation for the dihedral group \(D_{2n}\) (sometimes denoted \(D_n\)). Let \(D_{2n}\) be generated by elements \(r\) (rotation) and \(s\) (reflection) satisfying \(r^n=e, s^2=e, srs=r^{-1}\).

Consider the map \(\phi: G \to D_{2n}\) defined by \(\phi(x) = r\) and \(\phi(y) = s\). We need to check if this map respects the relations of \(G\).
\begin{itemize}
    \item \(\phi(x^n) = \phi(x)^n = r^n = e_{D_{2n}}\). This holds.
    \item \(\phi(y^2) = \phi(y)^2 = s^2 = e_{D_{2n}}\). This holds.
    \item \(\phi(xyxy) = \phi(x)\phi(y)\phi(x)\phi(y) = rsrs\). In \(D_{2n}\), we know \(srs = r^{-1}\). So, \(rsrs = r(srs) = r(r^{-1}) = e_{D_{2n}}\). This holds.
\end{itemize}
Since the relations are satisfied, \(\phi\) is a well-defined group homomorphism (by the universal property of group presentations, or von Dyck's theorem).

The image of \(\phi\) contains \(\phi(x)=r\) and \(\phi(y)=s\). Since \(r\) and \(s\) generate \(D_{2n}\), the homomorphism \(\phi\) is surjective.
A surjective homomorphism implies that \(|G| \ge |D_{2n}|\).
We know that the order of the dihedral group \(D_{2n}\) is \(2n\).
Therefore, \(|G| \ge 2n\).

**4. Determining the Order of \(G\)**

Combining the results from steps 2 and 3:
\(|G| \le 2n\) and \(|G| \ge 2n\).
Therefore, \(|G| = 2n\).

Furthermore, since \(\phi: G \to D_{2n}\) is a surjective homomorphism between groups of the same finite order, \(\phi\) must be an isomorphism. Thus, \(G \cong D_{2n}\).

**5. Proving \(G\) is Non-Abelian**

A group \(G\) is abelian if and only if \(ab=ba\) for all \(a, b \in G\). It suffices to check this for the generators. \(G\) is abelian iff \(xy=yx\).
We derived the relation \(yx = x^{-1}y\).
So, \(G\) is abelian iff \(xy = x^{-1}y\).
Multiply by \(y^{-1}\) on the right. Since \(y^2=e\), \(y^{-1}=y\).
\(xyy^{-1} = x^{-1}yy^{-1}\)
\(x = x^{-1}\)
This is equivalent to \(x^2 = e\).

So, \(G\) is abelian if and only if \(x^2=e\).
We need to determine if \(x^2=e\) holds in \(G\).
Since \(G \cong D_{2n}\) via the isomorphism \(\phi(x)=r\), we have \(x^2=e\) in \(G\) if and only if \(r^2=e\) in \(D_{2n}\).
In \(D_{2n}\), the element \(r\) represents a rotation by \(2\pi/n\). The order of \(r\) is \(n\).
So, \(r^2=e\) if and only if the order of \(r\), which is \(n\), divides 2.
This means \(n=1\) or \(n=2\).

However, the problem statement specifies that \(n \ge 3\).
For \(n \ge 3\), the order \(n\) does not divide 2.
Therefore, \(r^2 \neq e\) in \(D_{2n}\).
This implies \(x^2 \neq e\) in \(G\).
Since \(x^2 \neq e\), we have \(x \neq x^{-1}\), which means \(xy \neq yx\).
Thus, \(G\) is non-abelian for \(n \ge 3\).

**Conclusion**

We have shown that the group \(G\) defined by the presentation \( \langle x, y : x^n=e, y^2=e, xyxy=e \rangle \) is isomorphic to the dihedral group \(D_{2n}\). The order of \(D_{2n}\) is \(2n\). The dihedral group \(D_{2n}\) is non-abelian for \(n \ge 3\).
Therefore, for \(n \ge 3\), \(G\) is a non-abelian group of order \(2n\).

```markdown
**Solution:**

Let \(G\) be the group defined by the presentation
\[
G = \langle x, y : x^n=e, y^2=e, xyxy=e \rangle
\]
where \( n \in \mathbb{N} \) and \( n \geq 3 \). We want to prove that \(G\) is a non-abelian group of order \(2n\).

**1. Simplifying the Relations**

The relations defining \(G\) are:
(1) \(x^n = e\)
(2) \(y^2 = e\)
(3) \(xyxy = e\)

From relation (2), we have \(y^{-1} = y\).
We can manipulate relation (3) by multiplying by \(y^{-1}\) on the right:
\[ xyx y y^{-1} = e y^{-1} \]
\[ xyx = y^{-1} \]
Using \(y^{-1} = y\), we obtain:
\[ xyx = y \]
Now, multiply this by \(x^{-1}\) on the left:
\[ x^{-1}xyx = x^{-1}y \]
\[ yx = x^{-1}y \]
This relation shows how \(y\) interacts with \(x\). Let's check consistency with the original relation \(xyxy=e\). Using \(yx=x^{-1}y\) and \(y^2=e\):
\[ xyxy = x(yx)y = x(x^{-1}y)y = (xx^{-1})y^2 = e \cdot e = e \]
So the relation \(xyxy=e\) is equivalent to \(yx = x^{-1}y\) (given \(y^2=e\)).
Thus, the presentation for \(G\) is equivalent to:
\[ G = \langle x, y : x^n=e, y^2=e, yx=x^{-1}y \rangle \]

**2. Bounding the Order of \(G\)**

Since \(G\) is generated by \(x\) and \(y\), any element of \(G\) can be expressed as a word in \(x, y, x^{-1}, y^{-1}\). Using \(y^{-1}=y\) and the relation \(yx = x^{-1}y\), we can systematically move all \(y\)'s to the right of \(x\)'s in any word. For example, \(x^k y x^m = x^k (yx) x^{m-1} = x^k (x^{-1}y) x^{m-1} = x^{k-1} y x^{m-1}\). Repeated application allows any word to be written in the form \(x^i y^j\) for some integers \(i, j\).
Using the relation \(x^n=e\), we can reduce the exponent \(i\) modulo \(n\), so we only need to consider \(i \in \{0, 1, \dots, n-1\}\).
Using the relation \(y^2=e\), we can reduce the exponent \(j\) modulo 2, so we only need to consider \(j \in \{0, 1\}\).
Therefore, every element of \(G\) can be written in the form \(x^i y^j\) where \(0 \le i < n\) and \(j \in \{0, 1\}\). The set of such elements is \(S = \{x^i y^j : 0 \le i < n, j \in \{0, 1\}\}\).
The size of this set is \(n \times 2 = 2n\). This shows that the order of \(G\) is at most \(2n\), i.e., \(|G| \le 2n\).

**3. Identifying the Group \(G\)**

The relations \(x^n=e, y^2=e, yx=x^{-1}y\) (or equivalently \(yxy=x^{-1}\)) are the standard defining relations for the dihedral group \(D_{2n}\), the group of symmetries of a regular \(n\)-gon. Let \(D_{2n} = \langle r, s : r^n=e, s^2=e, srs=r^{-1} \rangle\).
Consider the map \(\phi: G \to D_{2n}\) defined by \(\phi(x)=r\) and \(\phi(y)=s\). We verify that this map respects the relations of \(G\):
\begin{itemize}
    \item \(\phi(x^n) = \phi(x)^n = r^n = e_{D_{2n}}\).
    \item \(\phi(y^2) = \phi(y)^2 = s^2 = e_{D_{2n}}\).
    \item \(\phi(xyxy) = \phi(x)\phi(y)\phi(x)\phi(y) = rsrs\). Using the relation \(srs=r^{-1}\) in \(D_{2n}\), we have \(rsrs = r(srs) = r(r^{-1}) = e_{D_{2n}}\).
\end{itemize}
Since the relations defining \(G\) are satisfied by the images of \(x\) and \(y\) in \(D_{2n}\), the map \(\phi\) extends to a well-defined group homomorphism from \(G\) to \(D_{2n}\) (by the von Dyck's theorem).
The image of \(\phi\) contains \(r=\phi(x)\) and \(s=\phi(y)\). Since \(r\) and \(s\) generate \(D_{2n}\), the homomorphism \(\phi\) is surjective.
A surjective homomorphism implies that \(|G| \ge |D_{2n}|\). The order of the dihedral group \(D_{2n}\) is known to be \(2n\). Thus, \(|G| \ge 2n\).

**4. Determining the Order of \(G\)**

Combining the inequalities from steps 2 and 3, we have \(|G| \le 2n\) and \(|G| \ge 2n\). Therefore, \(|G| = 2n\).
Since \(\phi: G \to D_{2n}\) is a surjective homomorphism between groups of the same finite order \(2n\), \(\phi\) must be an isomorphism. Hence, \(G \cong D_{2n}\).

**5. Proving \(G\) is Non-Abelian**

A group \(G\) is abelian if and only if \(ab=ba\) for all \(a, b \in G\). It suffices to check commutativity for the generators \(x\) and \(y\). \(G\) is abelian if and only if \(xy=yx\).
From step 1, we derived the relation \(yx = x^{-1}y\).
So, \(G\) is abelian iff \(xy = x^{-1}y\).
Multiplying by \(y^{-1}=y\) on the right gives:
\[ xy y^{-1} = x^{-1}y y^{-1} \]
\[ x = x^{-1} \]
\[ x^2 = e \]
Thus, \(G\) is abelian if and only if \(x^2 = e\).

We need to show that \(x^2 \neq e\) for \(n \ge 3\).
Since \(G \cong D_{2n}\) and \(\phi(x)=r\), \(x^2 = e\) in \(G\) if and only if \(r^2 = e\) in \(D_{2n}\).
In \(D_{2n}\), the element \(r\) corresponds to a rotation of order \(n\). Therefore, \(r^k=e\) if and only if \(n\) divides \(k\).
So, \(r^2 = e\) if and only if \(n\) divides 2. This happens only when \(n=1\) or \(n=2\).
The problem states that \(n \ge 3\). For \(n \ge 3\), \(n\) does not divide 2, so \(r^2 \neq e\).
Consequently, \(x^2 \neq e\) in \(G\) for \(n \ge 3\).
Since \(x^2 \neq e\), it follows that \(xy \neq yx\), and therefore \(G\) is non-abelian.

**Conclusion**

The group \(G\) defined by the presentation \( \langle x, y : x^n=e, y^2=e, xyxy=e \rangle \) is isomorphic to the dihedral group \(D_{2n}\). Its order is \(|G| = 2n\). For \(n \ge 3\), the group \(D_{2n}\) (and hence \(G\)) is non-abelian.
```