```latex
\textbf{Solution:}

Let \( p \) be an odd prime divisor of 
\[
a^{2^k} + b^{2^k},
\]
where \( a \), \( b \), and \( k \) are positive integers with \(\gcd(a,b) = 1\).

Since \( p \mid a^{2^k} + b^{2^k} \), we have
\[
a^{2^k} \equiv -b^{2^k} \pmod{p}.
\]
Because \(\gcd(a,b)=1\), neither \(a\) nor \(b\) is divisible by \(p\); hence, \(b\) is invertible modulo \(p\). Multiplying the congruence by the inverse \(b^{-2^k}\) modulo \(p\) gives
\[
\left(a\,b^{-1}\right)^{2^k} \equiv -1 \pmod{p}.
\]
Squaring both sides, we obtain
\[
\left(a\,b^{-1}\right)^{2^{k+1}} \equiv 1 \pmod{p}.
\]

Let \( r \) be the order of \( a\,b^{-1} \) modulo \( p \). Then \( r \) divides \( 2^{k+1} \). Moreover, since
\[
\left(a\,b^{-1}\right)^{2^k} \equiv -1 \not\equiv 1 \pmod{p},
\]
the order \( r \) cannot be a divisor of \( 2^k \). Hence, we must have
\[
r = 2^{k+1}.
\]

By Fermat's Little Theorem, the order of any element modulo \( p \) divides \( p - 1 \). Thus,
\[
2^{k+1} \mid (p - 1).
\]
This means there exists an integer \( d \ge k+1 \) and an odd integer \( m \) such that
\[
p - 1 = 2^d m.
\]
Rewriting this, we have
\[
p = 2^d m + 1,
\]
with \( d \ge k+1 \) and \( m \) odd.

This completes the proof.
```