Here is a detailed, step-by-step solution to the problem.

### Step 1: Understanding the Sequence $(a_n)$

The sequence $(a_n)$ is defined by the initial values $a_0=1$, $a_1=1$ and the recurrence relations for $n \ge 1$:
1.  $a_{2n-1} = a_n + a_{n-1}$
2.  $a_{2n} = a_n$

Let's compute the first few terms of the sequence to gain some intuition.
*   $a_0 = 1$
*   $a_1 = 1$
*   For $n=1$: $a_2 = a_{2(1)} = a_1 = 1$. (The relation $a_{2(1)-1} = a_1 = a_1+a_0$ would give $1=1+1$, which is false. This implies the recurrence relations are for defining $a_k$ for $k \ge 2$.)
*   For $n=2$:
    *   $a_3 = a_{2(2)-1} = a_2 + a_{2-1} = a_2 + a_1 = 1 + 1 = 2$.
    *   $a_4 = a_{2(2)} = a_2 = 1$.
*   For $n=3$:
    *   $a_5 = a_{2(3)-1} = a_3 + a_2 = 2 + 1 = 3$.
    *   $a_6 = a_{2(3)} = a_3 = 2$.
*   For $n=4$:
    *   $a_7 = a_{2(4)-1} = a_4 + a_3 = 1 + 2 = 3$.
    *   $a_8 = a_{2(4)} = a_4 = 1$.

The sequence begins: $a_0=1, a_1=1, a_2=1, a_3=2, a_4=1, a_5=3, a_6=2, a_7=3, a_8=1, \dots$.
All terms are positive integers.

### Step 2: A Key Property of the Sequence

Let's investigate the relationship between consecutive terms. We hypothesize that $\gcd(a_n, a_{n+1}) = 1$ for all $n \ge 0$. We can prove this by induction.

**Base Cases:**
*   $\gcd(a_0, a_1) = \gcd(1, 1) = 1$.
*   $\gcd(a_1, a_2) = \gcd(1, 1) = 1$.
*   $\gcd(a_2, a_3) = \gcd(1, 2) = 1$.

**Inductive Step:** Assume $\gcd(a_k, a_{k+1}) = 1$ for all $k < N$. We want to prove it for $N$.

*   **Case 1: $N$ is even.** Let $N=2m$ for some $m \ge 1$. We want to find $\gcd(a_{2m}, a_{2m+1})$.
    *   $a_{2m} = a_m$.
    *   The index $2m+1$ is odd. We can write $2m+1 = 2(m+1)-1$. So, using the first recurrence with $n=m+1$:
        $a_{2m+1} = a_{m+1} + a_m$.
    *   Now, we compute the gcd:
        $\gcd(a_{2m}, a_{2m+1}) = \gcd(a_m, a_{m+1} + a_m)$.
    *   Using the property $\gcd(x, y+x) = \gcd(x, y)$, we have:
        $\gcd(a_m, a_{m+1} + a_m) = \gcd(a_m, a_{m+1})$.
    *   Since $m < 2m = N$, the inductive hypothesis applies to $\gcd(a_m, a_{m+1})$, so it is 1.

*   **Case 2: $N$ is odd.** Let $N=2m-1$ for some $m \ge 2$. We want to find $\gcd(a_{2m-1}, a_{2m})$.
    *   $a_{2m-1} = a_m + a_{m-1}$.
    *   $a_{2m} = a_m$.
    *   Now, we compute the gcd:
        $\gcd(a_{2m-1}, a_{2m}) = \gcd(a_m + a_{m-1}, a_m)$.
    *   Using the property $\gcd(x+y, x) = \gcd(y, x)$, we have:
        $\gcd(a_m + a_{m-1}, a_m) = \gcd(a_{m-1}, a_m)$.
    *   Since $m-1 < 2m-1 = N$, the inductive hypothesis applies to $\gcd(a_{m-1}, a_m)$, so it is 1.

By induction, $\gcd(a_n, a_{n+1})=1$ for all $n \ge 0$. This means that any fraction $\frac{a_{n+1}}{a_n}$ is already in its simplest form.

### Step 3: Deriving Recurrence Relations for the Ratios

The problem asks to describe the set $S = \left\{ r \in \mathbb{Q}^+ \mid r = \frac{a_{n+1}}{a_n} \text{ for some } n \in \mathbb{N} \right\}$. Let's define the sequence of ratios $r_n = \frac{a_{n+1}}{a_n}$ for $n \ge 1$ (as $\mathbb{N}=\{1, 2, 3, \dots\}$).

Let's find recurrence relations for $r_n$. We consider two cases for the index $n$.

*   **Case 1: The index is even.** Let $n = 2m$ for some $m \in \mathbb{N}$.
    $r_{2m} = \frac{a_{2m+1}}{a_{2m}}$.
    Using the formulas for $a_k$:
    *   $a_{2m} = a_m$.
    *   $a_{2m+1} = a_{2(m+1)-1} = a_{m+1} + a_m$.
    So, $r_{2m} = \frac{a_{m+1} + a_m}{a_m} = \frac{a_{m+1}}{a_m} + 1 = r_m + 1$.
    Thus, for $m \ge 1$, we have $r_{2m} = r_m + 1$.

*   **Case 2: The index is odd.** Let $n = 2m-1$ for some $m \in \mathbb{N}, m \ge 1$. (Note: for $n=1, m=1$. for $n=3, m=2$, etc.) Let's instead use $n=2m+1$ to keep indices positive. Let $n=2m+1$ for $m \ge 0$. But $n \in \mathbb{N}$ so $m$ cannot be 0. Let's use $n=2m-1$ for $m \ge 1$.
    Ah, it is simpler to relate $r_{2n+1}$ to $r_n$. Let's try that.
    Let $n=2m+1$ for $m \ge 1$.
    $r_{2m+1} = \frac{a_{2m+2}}{a_{2m+1}}$.
    *   $a_{2m+2} = a_{2(m+1)} = a_{m+1}$.
    *   $a_{2m+1} = a_{2(m+1)-1} = a_{m+1} + a_m$.
    So, $r_{2m+1} = \frac{a_{m+1}}{a_{m+1} + a_m}$.
    We can divide the numerator and denominator by $a_m$:
    $r_{2m+1} = \frac{a_{m+1}/a_m}{a_{m+1}/a_m + 1} = \frac{r_m}{r_m+1}$.
    Thus, for $m \ge 1$, we have $r_{2m+1} = \frac{r_m}{r_m+1}$.

We have found two recurrence relations for the sequence of ratios $(r_n)_{n \in \mathbb{N}}$:
1.  $r_{2n} = r_n + 1$
2.  $r_{2n+1} = \frac{r_n}{r_n+1}$

The sequence starts with $r_1 = \frac{a_2}{a_1} = \frac{1}{1} = 1$.

### Step 4: Connecting to the Calkin-Wilf Tree

Let's analyze the operations that generate the sequence of ratios. Starting with $r_1=1$:
*   $r_2 = r_{2(1)} = r_1 + 1 = 1+1 = 2$.
*   $r_3 = r_{2(1)+1} = \frac{r_1}{r_1+1} = \frac{1}{1+1} = \frac{1}{2}$.
*   $r_4 = r_{2(2)} = r_2 + 1 = 2+1 = 3$.
*   $r_5 = r_{2(2)+1} = \frac{r_2}{r_2+1} = \frac{2}{2+1} = \frac{2}{3}$.
*   $r_6 = r_{2(3)} = r_3 + 1 = \frac{1}{2}+1 = \frac{3}{2}$.
*   $r_7 = r_{2(3)+1} = \frac{r_3}{r_3+1} = \frac{1/2}{1/2+1} = \frac{1/2}{3/2} = \frac{1}{3}$.

The sequence of ratios is $1, 2, \frac{1}{2}, 3, \frac{2}{3}, \frac{3}{2}, \frac{1}{3}, \dots$.

These generation rules are precisely those of the **Calkin-Wilf tree**. The Calkin-Wilf tree is a binary tree containing every positive rational number exactly once.
*   The root of the tree is the fraction $\frac{1}{1}$.
*   For any node $\frac{p}{q}$ in the tree, its two children are:
    *   The "left" child: $\frac{p}{p+q}$
    *   The "right" child: $\frac{p+q}{q}$

Let's define two functions corresponding to these operations: $f(x) = \frac{x}{x+1}$ and $g(x) = x+1$.
If we have a rational number $x = p/q$, then:
*   $f(x) = \frac{p/q}{p/q+1} = \frac{p}{p+q}$ (left child).
*   $g(x) = \frac{p}{q}+1 = \frac{p+q}{q}$ (right child).

Our recurrence relations for $r_n$ are:
*   $r_{2n+1} = \frac{r_n}{r_n+1} = f(r_n)$.
*   $r_{2n} = r_n+1 = g(r_n)$.

The sequence $(r_n)$ is constructed as follows:
*   $r_1 = 1/1$.
*   $r_2 = g(r_1)$ and $r_3 = f(r_1)$.
*   $r_4 = g(r_2)$ and $r_5 = f(r_2)$.
*   $r_6 = g(r_3)$ and $r_7 = f(r_3)$.
... and so on.

This shows that the sequence $r_1, r_2, r_3, \dots$ is a breadth-first traversal of the Calkin-Wilf tree, starting from the root $r_1=1$.

### Step 5: The Set S is the Set of All Positive Rational Numbers

A fundamental theorem about the Calkin-Wilf tree states that the set of all its nodes is precisely the set of all positive rational numbers, $\mathbb{Q}^+$. Each positive rational number appears exactly once in the tree.

Our set $S$ is the set of all values in the sequence $(r_n)_{n \in \mathbb{N}}$. Since this sequence is a breadth-first enumeration of the nodes of the Calkin-Wilf tree, the set of values in the sequence is the set of all nodes of the tree.

Therefore, the set $S$ is the set of all positive rational numbers.

To be fully rigorous, we can argue this in two steps:
1.  **$S \subseteq \mathbb{Q}^+$**: The initial terms $a_0, a_1$ are positive integers. The recurrence relations $a_{2n-1}=a_n+a_{n-1}$ and $a_{2n}=a_n$ only involve additions of positive integers, so all $a_n$ are positive integers. Thus, $r_n = a_{n+1}/a_n$ is a ratio of two positive integers, which is a positive rational number.

2.  **$\mathbb{Q}^+ \subseteq S$**: We need to show that any positive rational number $q$ is equal to $r_n$ for some $n \in \mathbb{N}$. Any rational number $q \in \mathbb{Q}^+$ has a unique position in the Calkin-Wilf tree. We can find this position by tracing a path from $q$ back to the root $1/1$ using the inverse functions $f^{-1}(y) = \frac{y}{1-y}$ (for $0<y<1$) and $g^{-1}(y) = y-1$ (for $y>1$). This shows that $q$ can be generated from $1/1$ by a finite sequence of the forward functions $f$ and $g$.
    Our construction $r_{2n}=g(r_n)$ and $r_{2n+1}=f(r_n)$ ensures that every node that can be reached from the root $r_1=1$ will appear in the sequence $(r_n)$. For any node $q$ in the tree, there is a unique path from the root to $q$. This path corresponds to a unique sequence of indices, mapping back to an index $n$ such that $r_n=q$. For example, the node $g(f(g(r_1)))$ would correspond to the index $n=2(2(1)+1) = 6$. No, let's trace this carefully: $r_1 \xrightarrow{g} r_2 \xrightarrow{f} r_5 \xrightarrow{g} r_{10}$. The index is constructed by applying the rules $k \to 2k$ for $g$ and $k \to 2k+1$ for $f$.
    Since every positive rational number is in the Calkin-Wilf tree, and our sequence $(r_n)$ enumerates all nodes of this tree, every positive rational number will appear as some $r_n$. Thus, $\mathbb{Q}^+ \subseteq S$.

Combining both inclusions, we have $S = \mathbb{Q}^+$.

### Conclusion

The set $S$ is the set of all positive rational numbers.

$$ S = \mathbb{Q}^+ $$