# Solution

I need to find the probability of getting an even number of heads when tossing $n$ biased coins, where the $m$-th coin has probability $\frac{1}{2m+1}$ of landing heads.

I'll use the property that for independent events, the expectation of a product is the product of the expectations. Specifically, I'll calculate the expectation of $(-1)^X$ where $X$ is the total number of heads.

## Step 1: Calculate the expectation for each coin

For a single coin with probability $p$ of heads:
$$E[(-1)^X] = (-1)^0 \cdot P(X=0) + (-1)^1 \cdot P(X=1) = (1)(1-p) + (-1)(p) = 1-2p$$

For the $m$-th coin with $p_m = \frac{1}{2m+1}$:
$$E[(-1)^{X_m}] = 1-2\left(\frac{1}{2m+1}\right) = \frac{2m+1-2}{2m+1} = \frac{2m-1}{2m+1}$$

## Step 2: Find the expectation for all coins combined

For independent random variables, we have:
$$E[(-1)^{X_1+X_2+...+X_n}] = E[(-1)^{X_1}]E[(-1)^{X_2}]...E[(-1)^{X_n}]$$

Therefore:
$$E[(-1)^X] = \prod_{m=1}^{n}\frac{2m-1}{2m+1} = \frac{1}{3} \cdot \frac{3}{5} \cdot \frac{5}{7} \cdot ... \cdot \frac{2n-1}{2n+1}$$

This product telescopes (most terms cancel) to give:
$$E[(-1)^X] = \frac{1}{2n+1}$$

## Step 3: Compute the probability

The probability of getting an even number of heads is:
$$P(X \text{ is even}) = P((-1)^X = 1) = \frac{1 + E[(-1)^X]}{2}$$

Substituting our result:
$$P(X \text{ is even}) = \frac{1 + \frac{1}{2n+1}}{2} = \frac{2n+1+1}{2(2n+1)} = \frac{n+1}{2n+1}$$

Therefore, the probability of getting an even number of heads when tossing these $n$ biased coins is $\boxed{\frac{n+1}{2n+1}}$.