Of course. Here is a detailed, step-by-step solution to the problem.

### The Problem

We are looking for all real polynomials $P(x)$ that satisfy the functional equation:
$$x P(x-2) = (x-2024)P(x) \quad (*)$$
for all $x \in \mathbb{R}$.

### Step 1: Analyze the equation for specific values of x

A common strategy for functional equations is to substitute specific values of $x$ that simplify the equation, particularly values that make coefficients zero.

*   **Let $x = 0$:**
    Substituting $x=0$ into equation $(*)$, we get:
    $0 \cdot P(0-2) = (0-2024)P(0)$
    $0 = -2024 \cdot P(0)$
    This implies that $P(0) = 0$.
    Since $P(0)=0$, we know that $x=0$ is a root of the polynomial $P(x)$.

*   **Let $x = 2024$:**
    Substituting $x=2024$ into equation $(*)$, we get:
    $2024 \cdot P(2024-2) = (2024-2024)P(2024)$
    $2024 \cdot P(2022) = 0 \cdot P(2024)$
    $2024 \cdot P(2022) = 0$
    This implies that $P(2022) = 0$.
    So, $x=2022$ is another root of the polynomial $P(x)$.

### Step 2: Search for a pattern of roots

The equation relates $P(x)$ with $P(x-2)$. This suggests that if we know a root, we might be able to find others by shifting by 2.

We know $P(0)=0$. Let's use this to find more roots.

*   **Let $x=2$:**
    $2 \cdot P(2-2) = (2-2024)P(2)$
    $2 \cdot P(0) = -2022 \cdot P(2)$
    Since $P(0)=0$, we have $2 \cdot 0 = -2022 \cdot P(2)$, which means $P(2)=0$.
    So, $x=2$ is a root.

*   **Let $x=4$:**
    $4 \cdot P(4-2) = (4-2024)P(4)$
    $4 \cdot P(2) = -2020 \cdot P(4)$
    Since $P(2)=0$, we have $4 \cdot 0 = -2020 \cdot P(4)$, which means $P(4)=0$.
    So, $x=4$ is a root.

This suggests a pattern. Let's prove by induction that $P(2k)=0$ for a range of non-negative integers $k$.

**Claim:** $P(2k) = 0$ for all integers $k$ such that $0 \le k \le 1011$.

**Proof by Induction:**

*   **Base Case:** For $k=0$, we have $P(2 \cdot 0) = P(0)$. We have already shown that $P(0)=0$. The base case holds.

*   **Inductive Step:** Assume that $P(2k)=0$ for some integer $k$ where $0 \le k < 1011$. We want to show that $P(2(k+1))=P(2k+2)=0$.
    Let's substitute $x=2k+2$ into the original equation $(*)$:
    $(2k+2) P((2k+2)-2) = ((2k+2)-2024) P(2k+2)$
    $(2k+2) P(2k) = (2k-2022) P(2k+2)$

    By our inductive hypothesis, $P(2k)=0$. So the left side of the equation is 0:
    $(2k+2) \cdot 0 = (2k-2022) P(2k+2)$
    $0 = (2k-2022) P(2k+2)$

    This equation implies that either $2k-2022=0$ or $P(2k+2)=0$.
    The condition $2k-2022=0$ means $2k=2022$, so $k=1011$.
    However, our inductive assumption is for $k < 1011$. For this range, the term $(2k-2022)$ is non-zero.
    Therefore, for $0 \le k < 1011$, we must have $P(2k+2)=0$.

By the principle of mathematical induction, $P(2k)=0$ for all integers $k$ from $0$ to $1011$. This means the polynomial $P(x)$ has the following roots:
$0, 2, 4, 6, \dots, 2 \cdot 1011 = 2022$.
These are $1012$ distinct roots.

### Step 3: Determine the general form of the polynomial

Since $P(x)$ is a polynomial with roots $0, 2, 4, \dots, 2022$, it must be divisible by the product of the corresponding linear factors. We can write $P(x)$ in the form:
$$P(x) = x(x-2)(x-4)\cdots(x-2022) \cdot Q(x)$$
where $Q(x)$ is also a polynomial.
Let's define $P_0(x) = x(x-2)(x-4)\cdots(x-2022) = \prod_{k=0}^{1011} (x-2k)$.
So, $P(x) = P_0(x) Q(x)$.

Now, we substitute this form of $P(x)$ back into the original equation $(*)$:
$$x P(x-2) = (x-2024)P(x)$$
$$x \cdot [P_0(x-2) Q(x-2)] = (x-2024) \cdot [P_0(x) Q(x)]$$

Let's analyze the term $P_0(x-2)$:
$P_0(x-2) = (x-2)(x-2-2)(x-2-4)\cdots(x-2-2022)$
$P_0(x-2) = (x-2)(x-4)(x-6)\cdots(x-2024)$

We can relate $P_0(x-2)$ to $P_0(x)$:
$P_0(x) = x \cdot (x-2)(x-4)\cdots(x-2022)$
$P_0(x-2) = (x-2)(x-4)\cdots(x-2022) \cdot (x-2024)$
So, $P_0(x-2) = \frac{P_0(x)}{x} \cdot (x-2024)$, for $x\neq 0$.

Substituting this into our equation:
$$x \left[ \frac{P_0(x)}{x} (x-2024) \right] Q(x-2) = (x-2024) P_0(x) Q(x)$$
$$(x-2024) P_0(x) Q(x-2) = (x-2024) P_0(x) Q(x)$$

This equation must hold for all $x \in \mathbb{R}$. The polynomial $(x-2024)P_0(x)$ is not the zero polynomial. Therefore, we can divide both sides by it for all values of $x$ where it is not zero. This gives:
$$Q(x-2) = Q(x)$$
This equality holds for infinitely many values of $x$. Since $Q(x)$ and $Q(x-2)$ are polynomials, if they agree on infinitely many points, they must be the same polynomial. Thus, the identity $Q(x-2) = Q(x)$ holds for all $x \in \mathbb{R}$.

### Step 4: Find all polynomials Q(x) such that Q(x-2) = Q(x)

Let $Q(x)$ be a polynomial such that $Q(x) = Q(x-2)$ for all $x$. This means $Q(x)$ is a periodic function with period $-2$ (and also period 2).
Let's consider the polynomial $H(x) = Q(x) - Q(0)$.
We know $H(0) = Q(0) - Q(0) = 0$.
Also, $H(-2) = Q(-2) - Q(0) = Q(0) - Q(0) = 0$.
$H(-4) = Q(-4) - Q(0) = Q(-2) - Q(0) = Q(0) - Q(0) = 0$.
In general, for any positive integer $n$, $H(-2n) = Q(-2n) - Q(0) = 0$.
So, the polynomial $H(x)$ has infinitely many roots: $0, -2, -4, -6, \dots$.
A non-zero polynomial can only have a finite number of roots. Therefore, $H(x)$ must be the zero polynomial, i.e., $H(x) = 0$ for all $x$.
This means $Q(x) - Q(0) = 0$, so $Q(x) = Q(0)$.
This shows that $Q(x)$ must be a constant polynomial. Let's call this constant $C$.
So, $Q(x) = C$ for some real constant $C$.

### Step 5: State the final solution and verify

From our work, the polynomial $P(x)$ must be of the form:
$$P(x) = C \cdot x(x-2)(x-4)\cdots(x-2022)$$
$$P(x) = C \prod_{k=0}^{1011} (x-2k)$$
where $C$ is any real constant.

This family of polynomials includes the zero polynomial (when $C=0$), which we can quickly check is a solution: $x \cdot 0 = (x-2024) \cdot 0$, which is true.

Let's verify the general solution for any constant $C$.
Let $P(x) = C \prod_{k=0}^{1011} (x-2k)$.

**Left-Hand Side (LHS) of $(*)$:**
$x P(x-2) = x \cdot C \prod_{k=0}^{1011} (x-2-2k) = C x \prod_{k=0}^{1011} (x-(2k+2))$
$x P(x-2) = C x (x-2)(x-4)\cdots(x-2022)(x-2024)$

**Right-Hand Side (RHS) of $(*)$:**
$(x-2024) P(x) = (x-2024) \cdot C \prod_{k=0}^{1011} (x-2k)$
$(x-2024) P(x) = C (x-2024) x(x-2)(x-4)\cdots(x-2022)$

Comparing the expressions for the LHS and RHS, we see they are identical polynomials. Thus, the solution is correct.

### Conclusion

The set of all real polynomials $P(x)$ satisfying the given equation is:
$$ P(x) = C \cdot x(x-2)(x-4)\cdots(x-2022) = C \prod_{k=0}^{1011} (x-2k) $$
for any arbitrary real constant $C$.