Let the limit be $L$. We are asked to find
$$ L = \lim_{k\to 0} \frac 1k \int_0^k (1+\tan(x))^{\frac 1x}\, dx $$
Let $f(x) = (1+\tan(x))^{\frac 1x}$.
Let $F(k) = \int_0^k f(x) dx$.
Then the limit can be written as
$$ L = \lim_{k\to 0} \frac{F(k)}{k} $$
As $k \to 0$, the numerator $F(k) = \int_0^k f(x) dx \to \int_0^0 f(x) dx = 0$. The denominator $k \to 0$.
Since the limit is in the indeterminate form $\frac 00$, we can apply L'Hopital's Rule, provided the limit of the ratio of the derivatives exists.
$$ L = \lim_{k\to 0} \frac{\frac{d}{dk} F(k)}{\frac{d}{dk} k} $$
By the Fundamental Theorem of Calculus Part 1, if $f(x)$ is continuous on an interval containing 0, then $F'(k) = f(k)$. Let's examine the continuity of $f(x)$ at $x=0$.
The function $f(x) = (1+\tan(x))^{\frac 1x}$ is not defined at $x=0$. We need to evaluate the limit of $f(x)$ as $x \to 0$.
$$ \lim_{x\to 0} f(x) = \lim_{x\to 0} (1+\tan(x))^{\frac 1x} $$
This limit is of the indeterminate form $1^\infty$, since $\tan(x) \to 0$ as $x \to 0$.
Let $y = (1+\tan(x))^{\frac 1x}$. To evaluate the limit, we consider the natural logarithm of $y$:
$$ \ln y = \ln \left( (1+\tan(x))^{\frac 1x} \right) = \frac 1x \ln(1+\tan(x)) $$
We want to find $\lim_{x\to 0} \ln y$:
$$ \lim_{x\to 0} \ln y = \lim_{x\to 0} \frac{\ln(1+\tan(x))}{x} $$
This limit is of the form $\frac 00$, since $\ln(1+\tan(0)) = \ln(1) = 0$. We can use L'Hopital's Rule:
$$ \lim_{x\to 0} \frac{\frac{d}{dx} \ln(1+\tan(x))}{\frac{d}{dx} x} = \lim_{x\to 0} \frac{\frac{1}{1+\tan(x)} \cdot \sec^2(x)}{1} $$
Now, substitute $x=0$:
$$ \frac{\frac{1}{1+\tan(0)} \cdot \sec^2(0)}{1} = \frac{\frac{1}{1+0} \cdot 1^2}{1} = \frac{1}{1} = 1 $$
So, $\lim_{x\to 0} \ln y = 1$.
Therefore, the limit of $f(x)$ as $x \to 0$ is:
$$ \lim_{x\to 0} f(x) = \lim_{x\to 0} y = e^1 = e $$
Since $\lim_{x\to 0} f(x)$ exists, the function $f(x)$ has a removable singularity at $x=0$. Let us define $\tilde{f}(x)$ such that $\tilde{f}(x) = f(x)$ for $x \ne 0$ and $\tilde{f}(0) = e$. Then $\tilde{f}(x)$ is continuous at $x=0$.
The integral $\int_0^k f(x) dx$ is equal to $\int_0^k \tilde{f}(x) dx$, because the value of the integrand at a single point does not change the value of the integral.
Let $F(k) = \int_0^k \tilde{f}(x) dx$. Since $\tilde{f}(x)$ is continuous, by FTC Part 1, $F'(k) = \tilde{f}(k)$.
Now we can apply L'Hopital's Rule to the original limit $L$:
$$ L = \lim_{k\to 0} \frac{F'(k)}{1} = \lim_{k\to 0} \tilde{f}(k) $$
Since $\tilde{f}(x)$ is continuous at $x=0$, this limit is simply $\tilde{f}(0)$.
$$ L = \tilde{f}(0) = e $$

Alternatively, using the Mean Value Theorem for Integrals:
Let $f(x) = (1+\tan x)^{1/x}$ for $x \neq 0$, and $f(0)=e$. $f(x)$ is continuous.
By the Mean Value Theorem for Integrals, for $k > 0$, there exists $c_k \in (0, k)$ such that
$$ \int_0^k f(x) dx = f(c_k) (k - 0) = k f(c_k) $$
Then, $\frac 1k \int_0^k f(x) dx = f(c_k)$.
As $k \to 0^+$, since $0 < c_k < k$, we must have $c_k \to 0$.
Since $f(x)$ is continuous at $x=0$,
$$ \lim_{k\to 0^+} \frac 1k \int_0^k f(x) dx = \lim_{k\to 0^+} f(c_k) = f(\lim_{k\to 0^+} c_k) = f(0) = e $$
If $k < 0$, let $k=-h$ where $h>0$.
$$ \frac 1k \int_0^k f(x) dx = \frac{1}{-h} \int_0^{-h} f(x) dx = \frac{1}{-h} \left( - \int_{-h}^0 f(x) dx \right) = \frac 1h \int_{-h}^0 f(x) dx $$
By MVT for integrals, there exists $d_h \in (-h, 0)$ such that $\int_{-h}^0 f(x) dx = f(d_h) (0 - (-h)) = h f(d_h)$.
$$ \frac 1h \int_{-h}^0 f(x) dx = \frac 1h (h f(d_h)) = f(d_h) $$
As $k \to 0^-$, $h \to 0^+$. Since $-h < d_h < 0$, we have $d_h \to 0$.
$$ \lim_{k\to 0^-} \frac 1k \int_0^k f(x) dx = \lim_{h\to 0^+} f(d_h) = f(\lim_{h\to 0^+} d_h) = f(0) = e $$
Since the limit from both sides is $e$, the limit exists and is equal to $e$.

Final Answer: The final answer is $\boxed{e}$