Below is one acceptable solution. One may show that the sum
\[
S:=\sum_{k=1}^n \; \sum_{1\le i_1<\cdots<i_k\le n}(-1)^k\frac{m_{i_1,\dots,i_k}^{\,2N+i_1+\cdots+i_k-1}}{i_1+\cdots+i_k+N}
\]
satisfies \(S\le0\). (Any answer equivalent to the answer below is correct.)

We begin by writing each term using an integral representation. Recall that for a positive number \(s\) and any \(a>0\) one has
\[
\frac{a^{\,s}}{s}=\int_0^a t^{\,s-1}\,dt.
\]
In our case, for each nonempty index set
\[
I=\{i_1,i_2,\dots,i_k\}\subset\{1,2,\dots,n\},
\]
we have
\[
\frac{m_I^{\,2N+\sum_{i\in I} i-1}}{\sum_{i\in I} i+N}
=\int_0^{\,m_I} t^{\,2N+\sum_{i\in I} i-1}\,dt,
\]
where we write
\[
m_I:=\min\{r_i: i\in I\}.
\]

Thus our sum may be written as
\[
S=\sum_{\emptyset\neq I\subset\{1,\dots,n\}}(-1)^{|I|}
\int_0^{\,m_I}t^{\,2N+\sum_{i\in I} i-1}dt.
\]
Since all of the numbers \(r_i\) lie in \((0,1)\) we may change the order of summation and integration. To this end, for each \(t\in[0,1]\) define
\[
A(t):=\{i\in\{1,2,\dots,n\} \mid t\le r_i\}.
\]
Notice that for any nonempty \(I\subset\{1,\dots,n\}\) we have
\[
t\le m_I \quad\Longleftrightarrow\quad I\subset A(t).
\]
Thus upon interchanging the order of summation and integration we find
\[
S=\int_0^1 t^{\,2N-1} \left[\sum_{\emptyset\neq I\subset A(t)}(-1)^{|I|}t^{\sum_{i\in I}i}\right]dt.
\]
But for any finite set \(A\) one may sum over all its subsets to obtain
\[
\sum_{I\subset A}(-1)^{|I|}t^{\sum_{i\in I}i}=\prod_{i\in A}(1-t^i).
\]
Since the empty set contributes \(1\) we deduce that
\[
\sum_{\emptyset\neq I\subset A(t)}(-1)^{|I|}t^{\sum_{i\in I}i}
=\prod_{i\in A(t)}(1-t^i)-1.
\]
Thus,
\[
S=\int_0^1 t^{\,2N-1}\Biggl[\prod_{i\in A(t)}(1-t^i)-1\Biggr]dt.
\]

Now, for every \(t\in[0,1]\) and each \(i\in A(t)\) the factor \((1-t^i)\) satisfies
\[
0\le 1-t^i\le1.
\]
Hence, 
\[
\prod_{i\in A(t)}(1-t^i)\le1.
\]
It follows that 
\[
\prod_{i\in A(t)}(1-t^i)-1\le0.
\]
Since also \(t^{2N-1}\ge0\) for \(t\in[0,1]\), the integrand is always nonpositive. Consequently,
\[
S=\int_0^1 t^{2N-1}\Biggl[\prod_{i\in A(t)}(1-t^i)-1\Biggr]dt\le0.
\]

This is what we wanted to prove.

Below is the complete solution in Markdown with LaTeX:

---

```markdown
# Solution

We wish to show that for any \(N\in\mathbb{N}\) and \(r_i\in(0,1)\) (for \(1\le i\le n\)) the inequality
\[
\sum_{k=1}^n \; \sum_{1\le i_1<\cdots<i_k\le n} (-1)^k \frac{m_{i_1,\dots,i_k}^{\,2N+i_1+\cdots+i_k-1}}{i_1+\cdots+i_k+N}\le 0,
\]
holds, where for any nonempty subset \(I=\{i_1,\dots,i_k\}\) we define
\[
m_I=m_{i_1,\dots,i_k}:=\min\{r_{i_1},r_{i_2},\dots,r_{i_k}\}.
\]

### Step 1. Integral Representation

For any \(a>0\) and \(s>0\) one has
\[
\frac{a^{\,s}}{s}=\int_0^a t^{s-1}\,dt.
\]
Thus, with
\[
s=2N+\sum_{i\in I} i,
\]
we may write
\[
\frac{m_I^{\,2N+\sum_{i\in I} i-1}}{\sum_{i\in I} i+N}=\int_0^{m_I}t^{\,2N+\sum_{i\in I} i-1}\,dt.
\]

### Step 2. Exchanging Sum and Integral

Write the sum as
\[
S=\sum_{\emptyset\neq I\subset\{1,\dots,n\}}(-1)^{|I|}\int_0^{m_I} t^{\,2N+\sum_{i\in I} i-1}\,dt.
\]
Since the integration intervals satisfy \(0\le t\le m_I\le 1\) (because \(r_i\in(0,1)\)), we may reverse the sum and the integral:
\[
S=\int_0^1 t^{\,2N-1}\left[\sum_{\substack{\emptyset\neq I\subset\{1,\dots,n\}\\ t\le m_I}} (-1)^{|I|}t^{\sum_{i\in I} i}\right]dt.
\]
For any fixed \(t\in[0,1]\), define
\[
A(t):=\{i\in\{1,2,\dots,n\} \mid t\le r_i\}.
\]
Note that \(t\le m_I\) if and only if \(I\subset A(t)\). Therefore, we may write
\[
S=\int_0^1 t^{\,2N-1}\left[\sum_{\emptyset\neq I\subset A(t)} (-1)^{|I|}t^{\sum_{i\in I} i}\right]dt.
\]

### Step 3. Summing over Subsets

A standard combinatorial identity tells us that for any finite set \(A\)
\[
\sum_{I\subset A}(-1)^{|I|}t^{\sum_{i\in I} i}=\prod_{i\in A}(1-t^i).
\]
Since the empty set contributes \(1\), it follows that
\[
\sum_{\emptyset\neq I\subset A(t)}(-1)^{|I|}t^{\sum_{i\in I} i}=\prod_{i\in A(t)}(1-t^i)-1.
\]
Thus,
\[
S=\int_0^1 t^{\,2N-1}\Bigl[\prod_{i\in A(t)}(1-t^i)-1\Bigr]dt.
\]

### Step 4. Nonpositivity of the Integrand

For any \(t\in[0,1]\) and any \(i\), we have \(0\le 1-t^i\le 1\). Hence,
\[
\prod_{i\in A(t)}(1-t^i)\le 1,
\]
so that
\[
\prod_{i\in A(t)}(1-t^i)-1\le 0.
\]
Since \(t^{2N-1}\ge 0\) for \(t\ge0\), the integrand in the expression for \(S\) is nonpositive. Consequently,
\[
S=\int_0^1 t^{\,2N-1}\Bigl[\prod_{i\in A(t)}(1-t^i)-1\Bigr]dt\le 0.
\]

This completes the proof.
```

---

Any answer which shows that
\[
\sum_{k=1}^n\sum_{1\le i_1<\cdots<i_k\le n} (-1)^k\frac{m_{i_1,\dots,i_k}^{\,2N+i_1+\cdots+i_k-1}}{i_1+\cdots+i_k+N}=\int_0^1t^{2N-1}\Bigl[\prod_{i\in A(t)}(1-t^i)-1\Bigr]dt\le 0
\]
is correct.
  
Feel free to use the above solution or any equivalent argument.