Of course. Here is a detailed, step-by-step solution to the problem.

### **Problem Statement**

Show that any prime divisor $p>2$ of the number $a^{2^k}+b^{2^k}$ is of the form $p=2^{d}m+1$, where $d\geq k+1$, $m$ is an odd positive integer, and $k$, $a$ and $b$ are positive integers with $\gcd(a,b)=1$.

---

### **Solution**

Let $N = a^{2^k}+b^{2^k}$. We are given that $p$ is a prime divisor of $N$ and $p > 2$.

#### **Step 1: Set up the congruence and show that $p$ does not divide $a$ or $b$.**

The condition that $p$ divides $N$ can be written as a congruence in modular arithmetic:
$$a^{2^k} + b^{2^k} \equiv 0 \pmod{p}$$
This is equivalent to:
$$a^{2^k} \equiv -b^{2^k} \pmod{p}$$

Now, let's consider the possibility that $p$ divides $a$ or $b$.
Suppose $p$ divides $b$. Then $b \equiv 0 \pmod{p}$. The congruence becomes:
$$a^{2^k} \equiv -0^{2^k} \pmod{p} \implies a^{2^k} \equiv 0 \pmod{p}$$
Since $p$ is prime, if $p$ divides $a^{2^k}$, then $p$ must divide $a$.
So, if $p|b$, then $p|a$. This means that $p$ is a common divisor of $a$ and $b$.

However, we are given that $\gcd(a, b) = 1$. This means that $a$ and $b$ share no common prime divisors. Therefore, our assumption that $p$ divides $b$ must be false.
By a symmetric argument, if we assume $p$ divides $a$, the congruence implies $p$ divides $b$, which again contradicts $\gcd(a,b)=1$.

Thus, we can conclude that $p \nmid a$ and $p \nmid b$.

#### **Step 2: Simplify the congruence.**

Since $p \nmid b$, $b$ has a multiplicative inverse modulo $p$. Let's denote this inverse by $b^{-1}$. Multiplying both sides of the congruence $a^{2^k} \equiv -b^{2^k} \pmod{p}$ by $(b^{-1})^{2^k}$, we get:
$$a^{2^k} (b^{-1})^{2^k} \equiv -b^{2^k} (b^{-1})^{2^k} \pmod{p}$$
$$(ab^{-1})^{2^k} \equiv -1 \pmod{p}$$
Let's define $x = ab^{-1}$. Our congruence simplifies to:
$$x^{2^k} \equiv -1 \pmod{p}$$

#### **Step 3: Determine the order of $x$ modulo $p$.**

Let $t = \text{ord}_p(x)$ be the order of $x$ modulo $p$. The order is the smallest positive integer such that $x^t \equiv 1 \pmod{p}$.

From the congruence $x^{2^k} \equiv -1 \pmod{p}$, we can make two important observations:

1.  Since $p > 2$, we know that $1 \not\equiv -1 \pmod{p}$. Therefore, $x^{2^k} \not\equiv 1 \pmod{p}$. This implies that the order $t$ cannot be a divisor of $2^k$.

2.  If we square both sides of $x^{2^k} \equiv -1 \pmod{p}$, we get:
    $$(x^{2^k})^2 \equiv (-1)^2 \pmod{p}$$
    $$x^{2 \cdot 2^k} \equiv 1 \pmod{p}$$
    $$x^{2^{k+1}} \equiv 1 \pmod{p}$$

By the definition of order, since $x^{2^{k+1}} \equiv 1 \pmod{p}$, the order $t$ must divide $2^{k+1}$. This means that $t$ must be a power of 2. So, $t = 2^j$ for some integer $j \leq k+1$.

Combining our two observations:
*   $t$ must be of the form $2^j$ for some $j \leq k+1$.
*   $t$ does not divide $2^k$, which means $j$ cannot be less than or equal to $k$.

The only possibility that satisfies both conditions is $j = k+1$.
Therefore, the order of $x$ modulo $p$ is precisely:
$$\text{ord}_p(x) = 2^{k+1}$$

#### **Step 4: Apply Fermat's Little Theorem.**

Since $p \nmid a$ and $p \nmid b$, it follows that $p \nmid ab^{-1}$ (if $p$ were to divide $ab^{-1}$, it would have to divide $a$, which we've shown is not the case). So, $x \not\equiv 0 \pmod{p}$.

Fermat's Little Theorem states that for any integer $x$ not divisible by a prime $p$, we have:
$$x^{p-1} \equiv 1 \pmod{p}$$
A fundamental property of the order of an element is that if $x^n \equiv 1 \pmod{p}$, then the order of $x$ must divide $n$. In our case, this means that $\text{ord}_p(x)$ must divide $p-1$.

Substituting the order we found in Step 3:
$$2^{k+1} \mid (p-1)$$

#### **Step 5: Express $p$ in the required form.**

The statement $2^{k+1} \mid (p-1)$ means that $p-1$ is a multiple of $2^{k+1}$. So, we can write:
$$p-1 = c \cdot 2^{k+1}$$
for some positive integer $c$.

We want to show that $p$ is of the form $2^d m + 1$ with $d \ge k+1$ and $m$ odd.
Any positive integer $c$ can be uniquely written as a product of a power of 2 and an odd number. Let $c = 2^s \cdot m$, where $m$ is a positive odd integer and $s \ge 0$ is an integer.

Substituting this into our expression for $p-1$:
$$p-1 = (2^s \cdot m) \cdot 2^{k+1}$$
$$p-1 = m \cdot 2^{k+1+s}$$

Let $d = k+1+s$. Since $s \ge 0$, we have $d \ge k+1$.
Now we can write:
$$p-1 = m \cdot 2^d$$
where $m$ is a positive odd integer and $d \ge k+1$.

This gives the final form for $p$:
$$p = 2^d m + 1$$

This is exactly the form required by the problem statement.

### **Conclusion**

We have shown, through a sequence of logical steps, that any prime divisor $p > 2$ of $a^{2^k} + b^{2^k}$ must be of the form $p = 2^d m + 1$, where $m$ is a positive odd integer and $d \ge k+1$. The proof relies on fundamental concepts of number theory, including modular arithmetic, the order of an element, and Fermat's Little Theorem, along with the crucial initial condition that $\gcd(a,b)=1$.

**Q.E.D.**