Solution:
Let the sequence be defined by $x_{n+1} = \beta x_n + \lfloor \alpha x_n \rfloor$ for $n \geq 0$, where $x_0 \in \mathbb{N}$, $\beta \in \mathbb{N}$, $\alpha \in (0, \infty) \setminus \mathbb{Q}$, $\beta - \alpha \in (0, 1)$, and $\alpha^2 = K \in \mathbb{N}$. We want to compute the limit $L = \lim_{n\to\infty} \frac{x_n}{(\alpha + \beta)^n}$.

Let $\gamma = \beta + \alpha$. Let $\delta_n = \{ \alpha x_n \} = \alpha x_n - \lfloor \alpha x_n \rfloor$. The recurrence relation can be written as
$$ x_{n+1} = \beta x_n + \alpha x_n - \{ \alpha x_n \} = (\beta + \alpha) x_n - \delta_n = \gamma x_n - \delta_n $$
Since $0 \le \delta_n < 1$ and $\gamma = \beta + \alpha > 1$ (as $\beta \ge 1$ and $\alpha > 0$), we can show that the limit $L = \lim_{n\to\infty} x_n/\gamma^n$ exists.
From the recurrence $x_{n+1} = \gamma x_n - \delta_n$, we can write
$$ x_n = \gamma^n x_0 - \sum_{k=0}^{n-1} \gamma^{n-1-k} \delta_k $$
Dividing by $\gamma^n$, we get
$$ \frac{x_n}{\gamma^n} = x_0 - \sum_{k=0}^{n-1} \frac{\delta_k}{\gamma^{k+1}} $$
Taking the limit as $n \to \infty$, we have
$$ L = x_0 - \sum_{k=0}^{\infty} \frac{\delta_k}{\gamma^{k+1}} $$
This expresses the limit $L$ in terms of an infinite sum involving the terms $\delta_k = \{\alpha x_k\}$. To find $L$, we need to evaluate this sum.

Let $y_n = \lfloor \alpha x_n \rfloor$. Since $x_0 \in \mathbb{N}$, $\beta \in \mathbb{N}$, and $\lfloor \alpha x_n \rfloor \in \mathbb{Z}$, it follows by induction that $x_n \in \mathbb{N}$ for all $n \ge 0$. Thus $y_n \in \mathbb{N}_0$.
Consider the associated linear recurrence system defined by:
$$ x'_{n+1} = \beta x'_n + y'_n $$
$$ y'_{n+1} = K x'_n + \beta y'_n $$
where $K = \alpha^2 \in \mathbb{N}$.
Let the initial conditions for this system be $x'_0 = x_0$ and $y'_0 = y_0 = \lfloor \alpha x_0 \rfloor$. Since $x_0 \in \mathbb{N}$ and $y_0 \in \mathbb{Z}$, and $K, \beta \in \mathbb{N}$, it follows that $x'_n, y'_n \in \mathbb{Z}$ for all $n \ge 0$.

The characteristic equation of the matrix $M = \begin{pmatrix} \beta & 1 \\ K & \beta \end{pmatrix}$ is $(\beta-\lambda)^2 - K = 0$, which gives $\lambda = \beta \pm \sqrt{K} = \beta \pm \alpha$. The eigenvalues are $\gamma = \beta + \alpha$ and $\bar{\gamma} = \beta - \alpha$.
The general solution for $x'_n$ is $x'_n = A \gamma^n + B \bar{\gamma}^n$.
The coefficients $A, B$ are determined by the initial conditions $x'_0=x_0$ and $x'_1 = \beta x'_0 + y'_0 = \beta x_0 + y_0$.
$x'_0 = A + B = x_0$.
$x'_1 = A \gamma + B \bar{\gamma} = \beta x_0 + y_0$.
Substituting $B = x_0 - A$: $A \gamma + (x_0 - A) \bar{\gamma} = \beta x_0 + y_0$.
$A(\gamma - \bar{\gamma}) + x_0 \bar{\gamma} = \beta x_0 + y_0$.
$A(2\alpha) = \beta x_0 + y_0 - x_0 \bar{\gamma} = \beta x_0 + y_0 - x_0 (\beta - \alpha) = y_0 + x_0 \alpha$.
$A = \frac{x_0 \alpha + y_0}{2\alpha} = \frac{x_0 + y_0/\alpha}{2}$.
$B = x_0 - A = x_0 - \frac{x_0 \alpha + y_0}{2\alpha} = \frac{2x_0 \alpha - x_0 \alpha - y_0}{2\alpha} = \frac{x_0 \alpha - y_0}{2\alpha}$.
Note that $y_0 = \lfloor \alpha x_0 \rfloor$, so $x_0 \alpha - y_0 = \{ \alpha x_0 \} = \delta_0$. Thus $B = \frac{\delta_0}{2\alpha}$.

The solution for the linear recurrence is $x'_n = \left(\frac{x_0 + y_0/\alpha}{2}\right) \gamma^n + \left(\frac{\delta_0}{2\alpha}\right) \bar{\gamma}^n$.
We are given $\bar{\gamma} = \beta - \alpha \in (0, 1)$. Also $\gamma = \beta + \alpha > \beta \ge 1$. Thus $0 < \bar{\gamma}/\gamma < 1$, and $(\bar{\gamma}/\gamma)^n \to 0$ as $n \to \infty$.
So, $\lim_{n\to\infty} \frac{x'_n}{\gamma^n} = \lim_{n\to\infty} \left( A + B \left(\frac{\bar{\gamma}}{\gamma}\right)^n \right) = A = \frac{x_0 + y_0/\alpha}{2}$.

Now, we show that the sequence $x_n$ is identical to the sequence $x'_n$. Let $d_n = x_n - x'_n$ and $e_n = y_n - y'_n = \lfloor \alpha x_n \rfloor - y'_n$.
$d_0 = x_0 - x'_0 = 0$. $e_0 = y_0 - y'_0 = \lfloor \alpha x_0 \rfloor - \lfloor \alpha x_0 \rfloor = 0$.
$x_{n+1} = \beta x_n + \lfloor \alpha x_n \rfloor$.
$x'_{n+1} = \beta x'_n + y'_n$.
$d_{n+1} = x_{n+1} - x'_{n+1} = \beta (x_n - x'_n) + (\lfloor \alpha x_n \rfloor - y'_n) = \beta d_n + e_n$.
We need to find a recurrence for $e_n$.
$e_{n+1} = y_{n+1} - y'_{n+1} = \lfloor \alpha x_{n+1} \rfloor - y'_{n+1}$.
We have shown in the scratchpad that $y'_n = A\alpha \gamma^n - B\alpha \bar{\gamma}^n$. This implies $x'_n \alpha - y'_n = (A \gamma^n + B \bar{\gamma}^n)\alpha - (A\alpha \gamma^n - B\alpha \bar{\gamma}^n) = 2 B \alpha \bar{\gamma}^n = \delta_0 \bar{\gamma}^n$.
So $\alpha x'_n = y'_n + \delta_0 \bar{\gamma}^n$. Since $x'_n, y'_n$ are integers, this holds for all $n$.
$e_{n+1} = \lfloor \alpha (x'_{n+1} + d_{n+1}) \rfloor - y'_{n+1} = \lfloor \alpha x'_{n+1} + \alpha d_{n+1} \rfloor - y'_{n+1}$.
$e_{n+1} = \lfloor y'_{n+1} + \delta_0 \bar{\gamma}^{n+1} + \alpha d_{n+1} \rfloor - y'_{n+1}$.
Since $y'_{n+1}$ is an integer, $e_{n+1} = \lfloor \delta_0 \bar{\gamma}^{n+1} + \alpha d_{n+1} \rfloor$.

We proceed by induction to show $d_n = 0$ and $e_n = 0$ for all $n$.
Base case: $d_0 = 0, e_0 = 0$.
Inductive step: Assume $d_k = 0$ and $e_k = 0$ for $0 \le k \le n$.
$d_{n+1} = \beta d_n + e_n = \beta(0) + 0 = 0$.
$e_{n+1} = \lfloor \delta_0 \bar{\gamma}^{n+1} + \alpha d_{n+1} \rfloor = \lfloor \delta_0 \bar{\gamma}^{n+1} + \alpha(0) \rfloor = \lfloor \delta_0 \bar{\gamma}^{n+1} \rfloor$.
Since $0 \le \delta_0 = \{\alpha x_0\} < 1$ and $0 < \bar{\gamma} = \beta - \alpha < 1$, we have $0 \le \delta_0 \bar{\gamma}^{n+1} < 1$.
Therefore, $e_{n+1} = \lfloor \delta_0 \bar{\gamma}^{n+1} \rfloor = 0$.
By induction, $d_n = 0$ and $e_n = 0$ for all $n$.
This means $x_n = x'_n$ for all $n$.

Hence, the limit is
$$ L = \lim_{n\to\infty} \frac{x_n}{\gamma^n} = \lim_{n\to\infty} \frac{x'_n}{\gamma^n} = A = \frac{x_0 + y_0/\alpha}{2} $$
Substituting $y_0 = \lfloor \alpha x_0 \rfloor$:
$$ L = \frac{x_0 + \lfloor \alpha x_0 \rfloor / \alpha}{2} $$
We can also express this using $\delta_0 = \{ \alpha x_0 \} = \alpha x_0 - \lfloor \alpha x_0 \rfloor$.
$$ L = \frac{x_0 + (\alpha x_0 - \delta_0)/\alpha}{2} = \frac{x_0 + x_0 - \delta_0/\alpha}{2} = \frac{2x_0 - \delta_0/\alpha}{2} = x_0 - \frac{\delta_0}{2\alpha} $$
So the limit is
$$ L = x_0 - \frac{\{\alpha x_0\}}{2\alpha} $$

Final answer is expressed in terms of $x_0$ and $\alpha$. $\beta$ is implicitly used via the conditions.

The limit is:
$$ \lim_{n\to\infty} \frac{x_n}{(\alpha + \beta)^n} = \frac{x_0 + \lfloor \alpha x_0 \rfloor / \alpha}{2} = x_0 - \frac{\{\alpha x_0\}}{2\alpha} $$

Final answer in markdown:
The sequence is defined by $x_{n+1} = \beta x_n + \lfloor \alpha x_n \rfloor$. Let $\gamma = \alpha + \beta$. We want to compute $L = \lim_{n\to\infty} \frac{x_n}{\gamma^n}$.
Let $y_n = \lfloor \alpha x_n \rfloor$. The recurrence can be written as $x_{n+1} = \beta x_n + y_n$.
Let $\delta_n = \{ \alpha x_n \} = \alpha x_n - y_n$. Then $x_{n+1} = \beta x_n + \alpha x_n - \delta_n = \gamma x_n - \delta_n$.
Consider the linear recurrence system $x'_{n+1} = \beta x'_n + y'_n$ and $y'_{n+1} = K x'_n + \beta y'_n$, where $K=\alpha^2$. Let the initial conditions be $x'_0 = x_0$ and $y'_0 = y_0 = \lfloor \alpha x_0 \rfloor$. The sequences $x'_n, y'_n$ consist of integers.
The characteristic equation is $\lambda^2 - 2\beta \lambda + (\beta^2-K) = 0$, with roots $\lambda_{1,2} = \beta \pm \sqrt{K} = \beta \pm \alpha$. Let $\gamma = \beta+\alpha$ and $\bar{\gamma} = \beta-\alpha$.
The general solution for $x'_n$ is $x'_n = A \gamma^n + B \bar{\gamma}^n$.
Using initial conditions, we find $A = \frac{x_0 + y_0/\alpha}{2}$ and $B = \frac{x_0 - y_0/\alpha}{2} = \frac{\alpha x_0 - y_0}{2\alpha} = \frac{\{\alpha x_0\}}{2\alpha}$.
Let $d_n = x_n - x'_n$. We showed by induction that $d_n = 0$ for all $n$, which means $x_n = x'_n$ for all $n$.
The limit is $L = \lim_{n\to\infty} \frac{x_n}{\gamma^n} = \lim_{n\to\infty} \frac{x'_n}{\gamma^n}$.
$$ \frac{x'_n}{\gamma^n} = A + B \left(\frac{\bar{\gamma}}{\gamma}\right)^n $$
We are given $\bar{\gamma} = \beta - \alpha \in (0, 1)$. Since $\beta \in \mathbb{N}$, $\beta \ge 1$. If $\beta=1$, $1-\alpha \in (0,1)$, so $0 < \alpha < 1$. $\alpha^2=K \in \mathbb{N}$, so $K=0$, impossible. Thus $\beta \ge 2$. Then $\gamma = \beta + \alpha > \beta \ge 2$.
Since $0 < \bar{\gamma} < 1$ and $\gamma > 1$, we have $0 < \bar{\gamma}/\gamma < 1$. Thus, $\lim_{n\to\infty} (\bar{\gamma}/\gamma)^n = 0$.
$$ L = \lim_{n\to\infty} \frac{x'_n}{\gamma^n} = A = \frac{x_0 + y_0/\alpha}{2} = \frac{x_0 + \lfloor \alpha x_0 \rfloor / \alpha}{2} $$
This can be rewritten using $\{\alpha x_0\} = \alpha x_0 - \lfloor \alpha x_0 \rfloor$:
$$ L = \frac{x_0 + (\alpha x_0 - \{\alpha x_0\})/\alpha}{2} = \frac{x_0 + x_0 - \{\alpha x_0\}/\alpha}{2} = x_0 - \frac{\{\alpha x_0\}}{2\alpha} $$

Final Result: The final result is
$$ \lim_{n\to\infty} \frac{x_n}{(\alpha + \beta)^n} = \frac{x_0 + \lfloor \alpha x_0 \rfloor / \alpha}{2} = x_0 - \frac{\{\alpha x_0\}}{2\alpha} $$

```markdown
Let the sequence be defined by $x_{n+1} = \beta x_n + \lfloor \alpha x_n \rfloor$ for $n \geq 0$.
Let $\gamma = \alpha + \beta$. We are interested in the limit $L = \lim_{n\to\infty} \frac{x_n}{\gamma^n}$.
Let $y_n = \lfloor \alpha x_n \rfloor$. The recurrence is $x_{n+1} = \beta x_n + y_n$.
Let $\delta_n = \{ \alpha x_n \} = \alpha x_n - \lfloor \alpha x_n \rfloor$. The recurrence can be written as $x_{n+1} = \gamma x_n - \delta_n$.

Consider the associated linear recurrence system defined by:
$$ x'_{n+1} = \beta x'_n + y'_n $$
$$ y'_{n+1} = K x'_n + \beta y'_n $$
where $K = \alpha^2 \in \mathbb{N}$. Let the initial conditions be $x'_0 = x_0$ and $y'_0 = y_0 = \lfloor \alpha x_0 \rfloor$. Since $x_0, \beta, K$ are integers and $y_0$ is an integer, it follows that $x'_n, y'_n$ are integers for all $n \ge 0$.

The characteristic equation for the system is $\lambda^2 - 2\beta \lambda + (\beta^2 - K) = 0$. The roots are $\lambda_{1,2} = \beta \pm \sqrt{K} = \beta \pm \alpha$. Let $\gamma = \beta + \alpha$ and $\bar{\gamma} = \beta - \alpha$.
The general solution for $x'_n$ is $x'_n = A \gamma^n + B \bar{\gamma}^n$.
The coefficients $A, B$ are determined by the initial conditions $x'_0=x_0$ and $x'_1 = \beta x_0 + y_0$.
We find $A = \frac{x_0 \alpha + y_0}{2\alpha} = \frac{x_0 + y_0/\alpha}{2}$ and $B = \frac{x_0 \alpha - y_0}{2\alpha} = \frac{\{\alpha x_0\}}{2\alpha}$.

Let $d_n = x_n - x'_n$. We show by induction that $d_n = 0$ for all $n$.
The base case $d_0 = x_0 - x'_0 = 0$ holds.
We have the relations $d_{n+1} = \beta d_n + e_n$ and $e_{n+1} = \lfloor \delta_0 \bar{\gamma}^{n+1} + \alpha d_{n+1} \rfloor$, where $e_n = y_n - y'_n = \lfloor \alpha x_n \rfloor - y'_n$ and $\delta_0 = \{\alpha x_0\}$.
Since $d_0=0$ and $e_0=0$, we compute $d_1 = \beta(0)+0 = 0$. Then $e_1 = \lfloor \delta_0 \bar{\gamma} + \alpha(0) \rfloor = \lfloor \delta_0 \bar{\gamma} \rfloor$.
Since $0 \le \delta_0 < 1$ and $0 < \bar{\gamma} < 1$ (given $\beta - \alpha \in (0,1)$), we have $0 \le \delta_0 \bar{\gamma} < 1$. So $e_1=0$.
Inductively, if $d_n=0$ and $e_n=0$, then $d_{n+1}=0$, and $e_{n+1} = \lfloor \delta_0 \bar{\gamma}^{n+1} \rfloor = 0$ because $0 \le \delta_0 \bar{\gamma}^{n+1} < 1$.
Thus $x_n = x'_n$ for all $n$.

The limit is $L = \lim_{n\to\infty} \frac{x_n}{\gamma^n} = \lim_{n\to\infty} \frac{x'_n}{\gamma^n}$.
$$ \frac{x'_n}{\gamma^n} = A + B \left(\frac{\bar{\gamma}}{\gamma}\right)^n $$
Since $0 < \bar{\gamma} < 1$ and $\gamma = \beta+\alpha > 1$, we have $0 < |\bar{\gamma}/\gamma| < 1$. Therefore, $\lim_{n\to\infty} (\bar{\gamma}/\gamma)^n = 0$.
$$ L = A = \frac{x_0 + y_0/\alpha}{2} = \frac{x_0 + \lfloor \alpha x_0 \rfloor / \alpha}{2} $$
This can be rewritten using $\{\alpha x_0\} = \alpha x_0 - \lfloor \alpha x_0 \rfloor$:
$$ L = \frac{x_0 + (\alpha x_0 - \{\alpha x_0\})/\alpha}{2} = \frac{x_0 + x_0 - \{\alpha x_0\}/\alpha}{2} = x_0 - \frac{\{\alpha x_0\}}{2\alpha} $$

The final result is:
$$ \lim_{n\to\infty} \frac{x_n}{(\alpha + \beta)^n} = \frac{x_0 + \lfloor \alpha x_0 \rfloor / \alpha}{2} = x_0 - \frac{\{\alpha x_0\}}{2\alpha} $$
```