# Solution

To solve this problem, I need to compute the integral $\int_{B(0,1)} |x_1|^{2k} \, dx$ and show it satisfies the given inequality.

## Step 1: Express the integral using spherical coordinates

In $n$-dimensional spherical coordinates, I have $x_1 = r\cos\theta_1$ where $r$ is the distance from the origin and $\theta_1$ is the angle between the position vector and the $x_1$-axis.

The volume element in spherical coordinates is:
$$dx = r^{n-1} \sin^{n-2}\theta_1 \sin^{n-3}\theta_2 \cdots \sin\theta_{n-2} \, dr \, d\theta_1 \, d\theta_2 \, \cdots \, d\theta_{n-1}$$

The integral becomes:
\begin{align}
\int_{B(0,1)} |x_1|^{2k} \, dx &= \int_0^1 \int_{S^{n-1}} |r\cos\theta_1|^{2k} r^{n-1} \, d\omega \, dr\\
&= \int_0^1 r^{2k} r^{n-1} \, dr \times \int_{S^{n-1}} |\cos\theta_1|^{2k} \, d\omega
\end{align}

where $d\omega$ represents the surface element on the unit sphere $S^{n-1}$.

## Step 2: Evaluate the radial integral

For the radial part:
$$\int_0^1 r^{2k+n-1} \, dr = \frac{1}{2k+n}$$

## Step 3: Evaluate the angular integral

For the angular part, I'll use the fact that for a function $f(\omega) = g(\omega_1)$ that depends only on the first coordinate:
$$\int_{S^{n-1}} f(\omega) \, d\omega = \omega_{n-1} \int_{-1}^1 g(t)(1-t^2)^{\frac{n-3}{2}} \, dt$$

In our case, $g(t) = |t|^{2k}$. Since both $|t|^{2k}$ and $(1-t^2)^{\frac{n-3}{2}}$ are even functions, I can write:
$$\int_{S^{n-1}} |\cos\theta_1|^{2k} \, d\omega = 2\omega_{n-1} \int_0^1 t^{2k}(1-t^2)^{\frac{n-3}{2}} \, dt$$

Making the substitution $u = t^2$, I get:
$$\int_0^1 t^{2k}(1-t^2)^{\frac{n-3}{2}} \, dt = \frac{1}{2}\int_0^1 u^{k-\frac{1}{2}}(1-u)^{\frac{n-3}{2}} \, du = \frac{1}{2}B\left(k+\frac{1}{2}, \frac{n-1}{2}\right)$$

where $B$ is the beta function. Using $B(a,b) = \frac{\Gamma(a)\Gamma(b)}{\Gamma(a+b)}$, I have:
$$\int_{S^{n-1}} |\cos\theta_1|^{2k} \, d\omega = \omega_{n-1} \frac{\Gamma(k+\frac{1}{2})\Gamma(\frac{n-1}{2})}{\Gamma(k+\frac{n}{2})}$$

## Step 4: Combine the results

Using $\omega_{n-1} = \frac{2\pi^{\frac{n-1}{2}}}{\Gamma(\frac{n-1}{2})}$, my integral becomes:
$$\int_{B(0,1)} |x_1|^{2k} \, dx = \frac{1}{2k+n} \times \frac{2\pi^{\frac{n-1}{2}}\Gamma(k+\frac{1}{2})}{\Gamma(k+\frac{n}{2})}$$

## Step 5: Prove the inequality

I need to show that:
$$\frac{1}{2k+n} \times \frac{2\pi^{\frac{n-1}{2}}\Gamma(k+\frac{1}{2})}{\Gamma(k+\frac{n}{2})} \geq \frac{\omega_n}{n^k(2k+n)}$$

Using $\omega_n = \frac{2\pi^{\frac{n}{2}}}{\Gamma(\frac{n}{2})}$, this is equivalent to proving:
$$\frac{2\pi^{\frac{n-1}{2}}\Gamma(k+\frac{1}{2})}{\Gamma(k+\frac{n}{2})} \geq \frac{2\pi^{\frac{n}{2}}}{n^k\Gamma(\frac{n}{2})}$$

After some algebraic manipulation, this is equivalent to:
$$\frac{\Gamma(k+\frac{1}{2})\Gamma(\frac{n}{2})}{\pi^{\frac{1}{2}}\Gamma(k+\frac{n}{2})} \geq \frac{1}{n^k}$$

Using the recursion formula for the gamma function and the fact that $\Gamma(\frac{1}{2}) = \sqrt{\pi}$, I can express:
$$\Gamma(k+\frac{1}{2}) = (k-\frac{1}{2})(k-\frac{3}{2})\cdots(\frac{1}{2})\sqrt{\pi}$$
$$\Gamma(k+\frac{n}{2}) = (k+\frac{n}{2}-1)(k+\frac{n}{2}-2)\cdots(\frac{n}{2})\Gamma(\frac{n}{2})$$

The inequality becomes:
$$\prod_{j=0}^{k-1} \frac{k-j-\frac{1}{2}}{\frac{n}{2}+k-j-1} \geq \frac{1}{n^k}$$

Multiplying both numerator and denominator by 2:
$$\prod_{j=0}^{k-1} \frac{2k-2j-1}{n+2k-2j-2} \geq \frac{1}{n^k}$$

## Step 6: Final proof

For $j = 0, 1, ..., k-1$, the function $f(j) = \frac{2k-2j-1}{n+2k-2j-2}$ is decreasing in $j$. Therefore:
$$\frac{2k-2j-1}{n+2k-2j-2} \geq \frac{1}{n} \text{ for all } j = 0, 1, ..., k-1$$

This can be verified algebraically. As a result:
$$\prod_{j=0}^{k-1} \frac{2k-2j-1}{n+2k-2j-2} \geq \prod_{j=0}^{k-1} \frac{1}{n} = \frac{1}{n^k}$$

This proves the inequality:
$$\int_{B(0,1)} |x_1|^{2k} \, dx \geq \frac{\omega_n}{n^k(2k+n)}$$

for any $k \geq 1$.