

To prove that $\lceil (\sqrt{11} + 3)^{2n} \rceil$ is divisible by $2^{n+1}$ for any $n \geq 1$, we analyze the sequence $S_n = (\sqrt{11} + 3)^{2n} + (3 - \sqrt{11})^{2n}$, which equals $\lceil (\sqrt{11} + 3)^{2n} \rceil$ since $(3 - \sqrt{11}) \in (-1, 0)$. The key steps are:

### Key Steps:

1. **Define Conjugate Terms**:
   Let $x = \sqrt{11} + 3$ and $y = 3 - \sqrt{11}$. These satisfy the quadratic equation $t^2 - 6t - 2 = 0$.

2. **Recurrence Relation**:
   The sequence $S_n = x^{2n} + y^{2n}$ follows the recurrence:
   $$
   S_n = 6S_{n-1} + 2S_{n-2}
   $$
   with initial conditions $S_0 = 2$ and $S_1 = 40$.

3. **Inductive Proof**:
   Use mathematical induction to show $2^{n+1} \mid S_n$:
   - **Base Case**: For $n=1$, $S_1 = 40$ is divisible by $2^{1+1} = 4$.
   - **Inductive Step**: Assume $2^{k+1} \mid S_k$ and $2^{k} \mid S_{k-1}$. Show $2^{k+2} \mid S_{k+1}$ by analyzing the recurrence relation modulo $2^{k+2}$.

4. **Divisibility Analysis**:
   - $T_{2k+1} = x^{2k+1} + y^{2k+1}$ is shown to have $v_2(T_{2k+1}) = k+1$ via induction.
   - This ensures $6T_{2k+1}$ contributes sufficiently to the divisibility of $S_{k+1}$.

### Final Proof:
By induction, $S_n$ is divisible by $2^{n+1}$ for all $n \geq 1$. Hence, $\lceil (\sqrt{11} + 3)^{2n} \rceil = S_n$ is divisible by $2^{n+1}$.

```markdown
**Proof:**

Let \( x = 3 + \sqrt{11} \) and \( y = 3 - \sqrt{11} \). These roots satisfy \( t^2 - 6t - 2 = 0 \). Define \( S_n = x^{2n} + y^{2n} \).

**Recurrence Relation:**
Using the minimal polynomial, \( S_n \) satisfies:
\[
S_n = 6S_{n-1} + 2S_{n-2}, \quad S_0 = 2, \quad S_1 = 40
\]

**Induction on \( n \):**
- **Base Case (\( n = 1 \)):** 
  \[
  S_1 = 40 = 2^{2} \cdot 10 \implies 2^{1+1} \mid S_1
  \]
  
- **Inductive Step:**
  Assume \( 2^{k+1} \mid S_k \) and \( 2^{k} \mid S_{k-1} \). For \( S_{k+1} \):
  \[
  S_{k+1} = 6T_{2k+1} + 2S_k
  \]
  where \( T_{2k+1} = x^{2k+1} + y^{2k+1} \). By lemma, \( v_2(T_{2k+1}) = k+1 \), so:
  \[
  6T_{2k+1} \equiv 0 \mod 2^{k+2}, \quad 2S_k \equiv 0 \mod 2^{k+2}
  \]
  Thus, \( S_{k+1} \equiv 0 \mod 2^{k+2} \).

Hence, by induction, \( 2^{n+1} \mid S_n \) for all \( n \geq 1 \). Since \( \lceil x^{2n} \rceil = S_n \), the result follows.
```