Solution step (worth 2 points):
Let $f: (0,\infty)\to \mathbb{R}$ and $g: (0,\infty)\to \mathbb{R}$ be defined by
$$
f(t)=\int_0^{\infty}\frac{e^{-tx}}{1+x^2}dx \;\;\text{ and }\;\;g(t)=\int_0^{\infty}\frac{\cos x}{t+x}dx.
$$
Then
$$
f(2)=\int_0^{\infty}\frac{e^{-2x}}{1+x^2}dx\;\; \text{ and }\;\;g(2)=\int_0^{\infty}\frac{\cos x}{2+x}dx.
$$
We will show that $f(t)-g(t)\equiv 0$,  meaning that it is identically zero (i.e., a constant function).

Solution step (worth 6 points):
We calculate the first and second derivative of $f(t)$:
$$
f'(t)=\frac{d}{dt}\int_0^{\infty}\frac{e^{-tx}}{1+x^2}dx=-\int_0^{\infty}\frac{xe^{-tx}}{1+x^2}dx.
$$
Observe that
$$
0\leq \int_0^{\infty}\frac{xe^{-tx}}{1+x^2}dx=\int_0^{\infty}\frac{x}{1+x^2}\cdot e^{-tx}dx\leq \int_0^{\infty}1\cdot e^{-tx}dx=
\left.-\frac{1}{t}e^{-tx}\right|_0^{\infty}=\frac{1}{t}.
$$
Thus
$$
\lim_{t\to\infty} f'(t)=0.
$$
Moreover, we have
$$
\begin{aligned}
f''(t)&=\frac{d}{dt}\int_0^{\infty}\frac{-xe^{-tx}}{1+x^2}dx=\int_0^{\infty}\frac{x^2e^{-tx}}{1+x^2}dx\\
&=\int_0^{\infty}\frac{1+x^2-1}{1+x^2}e^{-tx}dx\\
&=\int_0^{\infty}e^{-tx}dx-\int_0^{\infty}\frac{e^{-tx}}{1+x^2}dx\\
&=\left.-\frac{1}{t}e^{-tx}\right|_0^{\infty}-\int_0^{\infty}\frac{e^{-tx}}{1+x^2}dx\\
&=\frac{1}{t}-f(t).
\end{aligned}
$$

On the other hand, the first and second derivatives of the function $g(t)$ are expressed as follows:
$$
g'(t)=\frac{d}{dt}\int_0^{\infty}\frac{\cos x}{t+x}dx=-\int_0^{\infty}\frac{\cos x}{(t+x)^2}dx.
$$
We have
$$
0\leq \left|\int_0^{\infty}\frac{\cos x}{(t+x)^2}dx\right|\leq \int_0^{\infty}\frac{1}{(t+x)^2}dx=-\left.\frac{1}{t+x}\right|_0^{\infty}=\frac{1}{t}.
$$
Hence, we obtain that
$$
\lim_{t\to\infty} g'(t)=0.
$$
Furthermore, we have
$$
\begin{aligned}
g''(t)&=2\int_0^{\infty}\frac{\cos x}{(t+x)^3}dx=\left.-\frac{\cos x}{(t+x)^2}\right|_0^{\infty}-\int_0^{\infty}\frac{\sin x}{(t+x)^2}dx=\\
&=\frac{1}{t}-\int_0^{\infty}\frac{\sin x}{(t+x)^2}dx=\\
&=\frac{1}{t}-\left(\left.-\frac{\sin x}{t+x}\right|_0^{\infty}+\int_0^{\infty}\frac{\cos x}{t+x}dx\right)=\\
&=\frac{1}{t}-\int_0^{\infty}\frac{\cos x}{t+x}dx=\frac{1}{t}-g(t).
\end{aligned}
$$

Solution step (worth 2 points):
Since
$$
(f(t)-g(t))''-(f(t)-g(t))=0,
$$
it follows that the function $f(t)-g(t)$ is a solution of the linear differential equation:
$$
y''(t)-y(t)=0.
$$
On the other hand, the general solution $y(t)$ of the equation $y''(t)-y(t)=0$ has the form:
$$
y(t)=A\cos(t)+B\sin(t).
$$
Hence
$$
f(t)-g(t)=A\cos(t)+B\sin(t)
$$
for some real constants $A$ and $B$. Now we need show that $A=B=0$. To this end, we have
$$
f'(t)-g'(t)=-A\sin(t)+B\cos(t)
$$
and
$$
\lim_{t\to\infty}(f'(t)-g'(t))=0.
$$
This condition can only hold if $A=B=0$. Therefore, we conclude that $f(t)=g(t)$ for all $t\in (0,\infty)$, and in particular, $f(2)=g(2)$.
