 Notice that the inequality is equivalent to:
$$\frac{a \sqrt{a}+2 \sqrt{2}}{\sqrt{2a}} \leq \sqrt{a}+\sqrt{2}$$
\noindent if and only if $a \sqrt{a}+2 \sqrt{2} \leq a \sqrt{2} + 2 \sqrt{a}$
\noindent and we can factorize and obtain  $(a-2)(\sqrt{a}-\sqrt{2}) \leq 0$. Since the square root is a non-decreasing function, we obtain that both factors at left have the same sign. Hence $(a-2)(\sqrt{a}-\sqrt{2}) \geq 0$ so we obtain $(a-2)(\sqrt{a}-\sqrt{2}) = 0$ and the solution is unique: $a=2$ and we are done.