Here is a detailed, step-by-step solution to the problem.

### **1. Preliminary Analysis and Simplification of the Recurrence Relation**

The given recurrence relation is $a_{n+2}=4a_{n+1}-3a_n+\frac{3^n}{a_n}$ for $n\geq 1$.
The homogeneous part of this recurrence is $a_{n+2} - 4a_{n+1} + 3a_n = 0$. The characteristic equation is $r^2 - 4r + 3 = 0$, which factors as $(r-1)(r-3)=0$. The roots are $r_1=1$ and $r_2=3$. This suggests that the terms $a_n$, $a_{n+1}$, and $a_{n+2}$ are related in a way that involves factors of 3.

Let's rearrange the recurrence relation:
$$ a_{n+2} - 3a_{n+1} = a_{n+1} - 3a_n + \frac{3^n}{a_n} $$
This form is much simpler. Let us define a new sequence $(c_n)$ by $c_n = a_{n+1} - 3a_n$ for $n \geq 1$.
The recurrence relation then becomes:
$$ c_{n+1} = c_n + \frac{3^n}{a_n} \quad \text{for } n \geq 1 $$
We can express $c_n$ as a sum. Let's find the first term, $c_1$:
$c_1 = a_2 - 3a_1 = 10 - 3(3) = 1$.

Using the recurrence for $c_n$, we can write:
$c_2 = c_1 + \frac{3^1}{a_1} = 1 + \frac{3}{3} = 2$.
$c_3 = c_2 + \frac{3^2}{a_2} = 2 + \frac{9}{10} = \frac{29}{10}$.
In general, by repeatedly substituting, we get a sum formula for $c_n$:
$$ c_n = c_1 + \sum_{k=1}^{n-1} \frac{3^k}{a_k} = 1 + \sum_{k=1}^{n-1} \frac{3^k}{a_k} \quad \text{for } n \geq 2 $$
For $n=1$, $c_1=1$. The formula holds if we adopt the convention that the empty sum is 0.

### **2. Introducing the Sequence of Interest and Proving its Monotonicity**

We are interested in the limit of $b_n = \frac{a_n}{3^n}$. Let's express the relation $c_n = a_{n+1} - 3a_n$ in terms of $b_n$.
Dividing by $3^{n+1}$:
$$ \frac{c_n}{3^{n+1}} = \frac{a_{n+1}}{3^{n+1}} - \frac{3a_n}{3^{n+1}} = \frac{a_{n+1}}{3^{n+1}} - \frac{a_n}{3^n} $$
$$ b_{n+1} - b_n = \frac{c_n}{3^{n+1}} $$
To show that the limit of $(b_n)$ exists, we can use the Monotone Convergence Theorem, which requires proving that the sequence is both monotonic and bounded.

**Monotonicity:**
Let's find the sign of $b_{n+1} - b_n$. This depends on the sign of $c_n$.
$c_n = 1 + \sum_{k=1}^{n-1} \frac{3^k}{a_k}$.
To determine the sign of $c_n$, we first need to determine the sign of the terms $a_k$.

**Proof that $a_n > 0$ for all $n \geq 1$ by induction:**
*   **Base cases:** $a_1=3 > 0$ and $a_2=10 > 0$.
*   **Inductive hypothesis:** Assume $a_k > 0$ for all $k$ from $1$ to $n+1$ for some $n \geq 1$.
*   **Inductive step:** We want to show $a_{n+2} > 0$.
    From our previous work, $c_k = a_{k+1} - 3a_k$. By the inductive hypothesis, $a_k > 0$ for $1 \le k \le n$. This implies that the sum $\sum_{k=1}^{n} \frac{3^k}{a_k}$ consists of positive terms.
    Therefore, for $n \ge 1$, $c_{n+1} = 1 + \sum_{k=1}^{n} \frac{3^k}{a_k} > 1$.
    Since $c_n = a_{n+1} - 3a_n$, we have $c_n > 1$ for $n \ge 2$, and $c_1=1$. So $c_n \geq 1$ for all $n \geq 1$.
    The recurrence relation for $a_n$ is $a_{n+2} = 4a_{n+1} - 3a_n + \frac{3^n}{a_n}$.
    We can write this as $a_{n+2} = a_{n+1} + 3(a_{n+1}-3a_n) + \frac{3^n}{a_n} + 3a_n = a_{n+1} + 3c_n + \frac{3^n}{a_n}$. This is not the right way.
    Let's use $a_{n+2} = (a_{n+2}-3a_{n+1}) + 3a_{n+1} = c_{n+1} + 3a_{n+1}$.
    Using the inductive hypothesis, $a_{n+1} > 0$. Also, we've shown that $c_{n+1} = 1 + \sum_{k=1}^{n} \frac{3^k}{a_k} > 0$.
    Thus, $a_{n+2} = c_{n+1} + 3a_{n+1} > 0$.
    By the principle of mathematical induction, $a_n > 0$ for all $n \geq 1$.

Since $a_k > 0$ for all $k$, it follows that $c_n = 1 + \sum_{k=1}^{n-1} \frac{3^k}{a_k} > 0$ for all $n \geq 1$.
This means $b_{n+1} - b_n = \frac{c_n}{3^{n+1}} > 0$.
So, the sequence $(b_n)$ is strictly increasing.

### **3. Proving the Sequence is Bounded Above**

To prove convergence, we now need to show that $(b_n)$ is bounded above.
We can express $b_n$ as a sum:
$$ b_n = b_1 + \sum_{j=1}^{n-1} (b_{j+1} - b_j) = b_1 + \sum_{j=1}^{n-1} \frac{c_j}{3^{j+1}} $$
$b_1 = \frac{a_1}{3^1} = \frac{3}{3} = 1$.
So, $b_n = 1 + \sum_{j=1}^{n-1} \frac{1}{3^{j+1}} \left(1 + \sum_{k=1}^{j-1} \frac{3^k}{a_k}\right)$.

To find an upper bound for $b_n$, we need a lower bound for $a_k$.
We have shown that $c_n = a_{n+1} - 3a_n \geq 1$ for all $n \geq 1$.
This implies $a_{n+1} \geq 3a_n + 1$.
Let's use this to establish a lower bound for $a_n$:
$a_1 = 3$.
$a_2 \geq 3a_1+1 = 3(3)+1 = 10$. This matches the given $a_2=10$.
$a_3 \geq 3a_2+1 = 3(10)+1 = 31$. (In fact, $a_3=4(10)-3(3)+3/3 = 32$).
Let's find a general formula for this lower bound. Let a sequence $(u_n)$ be defined by $u_1=3$ and $u_{n+1}=3u_n+1$.
$u_n = A \cdot 3^n + B$. $A \cdot 3^{n+1}+B = 3(A \cdot 3^n + B) + 1 = A \cdot 3^{n+1} + 3B + 1$. So $B = 3B+1 \implies -2B=1 \implies B=-1/2$.
$u_n = A \cdot 3^n - 1/2$.
$u_1=3 \implies 3A-1/2 = 3 \implies 3A = 7/2 \implies A=7/6$.
So $u_n = \frac{7}{6}3^n - \frac{1}{2} = \frac{7 \cdot 3^{n-1} - 1}{2}$.
By induction, we can show $a_n \geq u_n$. Since $u_n = \frac{7}{6}3^n - \frac{1}{2} > 3^n$ for $n \ge 1$, we have $a_n > 3^n$ for $n \ge 2$. For $n=1$, $a_1=3^1$.
Thus, $a_n \ge 3^n$ for all $n \ge 1$.

Now we can bound $c_n$:
$$ c_n = 1 + \sum_{k=1}^{n-1} \frac{3^k}{a_k} $$
Since $a_k \ge 3^k$, we have $\frac{1}{a_k} \le \frac{1}{3^k}$, so $\frac{3^k}{a_k} \le \frac{3^k}{3^k} = 1$.
Therefore,
$$ c_n \le 1 + \sum_{k=1}^{n-1} 1 = 1 + (n-1) = n $$
Now, we can bound $b_n$:
$$ b_n = b_1 + \sum_{j=1}^{n-1} (b_{j+1} - b_j) = 1 + \sum_{j=1}^{n-1} \frac{c_j}{3^{j+1}} \le 1 + \sum_{j=1}^{n-1} \frac{j}{3^{j+1}} $$
The terms in the sum are positive, so the sequence $S_n = \sum_{j=1}^{n-1} \frac{j}{3^{j+1}}$ is increasing. To show $b_n$ is bounded, we can show the infinite series $\sum_{j=1}^{\infty} \frac{j}{3^{j+1}}$ converges.
$$ \sum_{j=1}^{\infty} \frac{j}{3^{j+1}} < \sum_{j=1}^{\infty} \frac{j}{3^j} $$
The series $\sum_{j=1}^{\infty} jx^j$ converges for $|x|<1$. By the ratio test, $\lim_{j\to\infty} \frac{(j+1)/3^{j+1}}{j/3^j} = \lim_{j\to\infty} \frac{j+1}{j} \frac{1}{3} = \frac{1}{3} < 1$.
So the series converges, and the sequence $(b_n)$ is bounded above.

### **4. Existence and Value of the Limit**

Since $(b_n)$ is a strictly increasing sequence and is bounded above, the Monotone Convergence Theorem guarantees that the limit $L = \lim_{n\to\infty} b_n$ exists.

Now we need to prove that $L \le \frac{7}{4}$.
The upper bound for $b_n$ for any $n$ is also an upper bound for the limit $L$.
$$ L \le 1 + \sum_{j=1}^{\infty} \frac{j}{3^{j+1}} $$
Let's compute the value of this infinite sum. Consider the geometric series formula for $|x|<1$:
$$ \sum_{j=0}^{\infty} x^j = \frac{1}{1-x} $$
Differentiating with respect to $x$:
$$ \sum_{j=1}^{\infty} jx^{j-1} = \frac{1}{(1-x)^2} $$
Multiplying by $x$:
$$ \sum_{j=1}^{\infty} jx^j = \frac{x}{(1-x)^2} $$
Our sum is $\sum_{j=1}^{\infty} \frac{j}{3^{j+1}} = \frac{1}{3} \sum_{j=1}^{\infty} j \left(\frac{1}{3}\right)^j$.
Let $x=1/3$. The sum is:
$$ \frac{1}{3} \cdot \frac{1/3}{(1-1/3)^2} = \frac{1}{3} \cdot \frac{1/3}{(2/3)^2} = \frac{1}{3} \cdot \frac{1/3}{4/9} = \frac{1}{3} \cdot \frac{1}{3} \cdot \frac{9}{4} = \frac{1}{9} \cdot \frac{9}{4} = \frac{1}{4} $$
So, we have the upper bound for the limit $L$:
$$ L = \lim_{n\to\infty} b_n \le 1 + \frac{1}{4} = \frac{5}{4} $$
The problem asks to prove that the limit is not greater than $\frac{7}{4}$.
Since $\frac{5}{4} = 1.25$ and $\frac{7}{4} = 1.75$, we have:
$$ L \le \frac{5}{4} < \frac{7}{4} $$
This completes the proof.

### **Summary of the Proof**

1.  **Transform the Recurrence:** The original recurrence relation $a_{n+2}=4a_{n+1}-3a_n+\frac{3^n}{a_n}$ was rewritten for the sequence $c_n=a_{n+1}-3a_n$ as $c_{n+1}=c_n+\frac{3^n}{a_n}$, with $c_1=1$.
2.  **Define Target Sequence:** The sequence of interest $b_n = a_n/3^n$ was shown to follow the relation $b_{n+1}-b_n = c_n/3^{n+1}$.
3.  **Prove Monotonicity:** We proved by induction that $a_n > 0$ for all $n$. This implies $c_n > 0$, and therefore $b_{n+1}-b_n > 0$. Thus, the sequence $(b_n)$ is strictly increasing.
4.  **Prove Boundedness:** We established the lower bound $a_n \ge 3^n$ for all $n \ge 1$. This led to an upper bound $c_n \le n$. Consequently, we found that $b_n \le 1 + \sum_{j=1}^{n-1} \frac{j}{3^{j+1}}$.
5.  **Establish Existence of Limit:** Since $(b_n)$ is increasing and bounded above (as the series $\sum \frac{j}{3^{j+1}}$ converges), the limit $L = \lim_{n\to\infty} b_n$ exists by the Monotone Convergence Theorem.
6.  **Bound the Limit:** By finding the exact sum of the infinite series, $\sum_{j=1}^{\infty} \frac{j}{3^{j+1}} = \frac{1}{4}$, we found that $L \le 1 + \frac{1}{4} = \frac{5}{4}$.
7.  **Conclusion:** As $\frac{5}{4} < \frac{7}{4}$, we have proven that the limit exists and is not greater than $\frac{7}{4}$.