Of course. Here is a detailed, step-by-step solution to the problem.

### **Problem Statement**

Let $\alpha, \beta > 0$. Find the equation of the parabola tangent to the lines $y=0$ (the x-axis) and $x=0$ (the y-axis) at the points $(\alpha, 0)$ and $(0, \beta)$, respectively.

### **Analysis of the Problem**

We are looking for the equation of a parabola. Let's visualize the given information:
*   The parabola is tangent to the x-axis at point $A(\alpha, 0)$.
*   The parabola is tangent to the y-axis at point $B(0, \beta)$.

Since $\alpha > 0$ and $\beta > 0$, these points of tangency are on the positive x and y axes. A sketch reveals that the parabola is "tilted", meaning its axis of symmetry is not parallel to either the x-axis or the y-axis. Therefore, the standard forms $y = ax^2+bx+c$ or $x=ay^2+by+c$ are not suitable. We must use a more general form for the conic section.

We will present two methods to solve this problem. The first is based on the general equation of a second-degree curve, and the second uses a more elegant parametric approach.

---

### **Method 1: Using the General Equation of a Conic Section**

**Step 1: The General Equation of a Conic**
The general equation of a conic section is given by:
$$Ax^2 + Bxy + Cy^2 + Dx + Ey + F = 0$$
For this equation to represent a parabola, the discriminant must be zero:
$$B^2 - 4AC = 0$$

**Step 2: Apply the Tangency Conditions**
The problem states that the parabola is tangent to the line $y=0$ at the point $(\alpha, 0)$.
Let's substitute $y=0$ into the general equation:
$$Ax^2 + D x + F = 0$$
For the parabola to be tangent to the line $y=0$ at a single point $x=\alpha$, this quadratic equation in $x$ must have a double root at $x=\alpha$. This means the quadratic must be equivalent to the form $k(x-\alpha)^2=0$ for some constant $k$. We can set $k=A$ without loss of generality.
$$A(x-\alpha)^2 = Ax^2 - 2A\alpha x + A\alpha^2 = 0$$
By comparing the coefficients of this with $Ax^2+Dx+F=0$, we get:
1.  $D = -2A\alpha$
2.  $F = A\alpha^2$

Similarly, the parabola is tangent to the line $x=0$ at the point $(0, \beta)$.
Let's substitute $x=0$ into the general equation:
$$Cy^2 + Ey + F = 0$$
This quadratic in $y$ must have a double root at $y=\beta$. So, it must be of the form $C(y-\beta)^2=0$.
$$C(y-\beta)^2 = Cy^2 - 2C\beta y + C\beta^2 = 0$$
By comparing the coefficients with $Cy^2+Ey+F=0$, we get:
3.  $E = -2C\beta$
4.  $F = C\beta^2$

**Step 3: Synthesize the Conditions and Solve for Coefficients**
From our findings, we have a system of relationships between the coefficients:
*   $D = -2A\alpha$
*   $F = A\alpha^2 \implies A = F/\alpha^2$
*   $E = -2C\beta$
*   $F = C\beta^2 \implies C = F/\beta^2$
*   $B^2 - 4AC = 0$

Now, substitute the expressions for $A$ and $C$ in terms of $F$ into the parabola condition:
$$B^2 - 4\left(\frac{F}{\alpha^2}\right)\left(\frac{F}{\beta^2}\right) = 0$$
$$B^2 = \frac{4F^2}{\alpha^2\beta^2}$$
Taking the square root, we get:
$$B = \pm \frac{2F}{\alpha\beta}$$
The physical arrangement of the parabola (curving away from the origin between the tangency points) suggests a particular sign choice. Let's proceed and see. Let's choose $B = - \frac{2F}{\alpha\beta}$ (we will verify this choice later).

Now we can express all coefficients in terms of $F$ (assuming $F \neq 0$):
*   $A = F/\alpha^2$
*   $B = -2F/(\alpha\beta)$
*   $C = F/\beta^2$
*   $D = -2A\alpha = -2(F/\alpha^2)\alpha = -2F/\alpha$
*   $E = -2C\beta = -2(F/\beta^2)\beta = -2F/\beta$

Substitute these into the general conic equation:
$$\left(\frac{F}{\alpha^2}\right)x^2 - \left(\frac{2F}{\alpha\beta}\right)xy + \left(\frac{F}{\beta^2}\right)y^2 - \left(\frac{2F}{\alpha}\right)x - \left(\frac{2F}{\beta}\right)y + F = 0$$
We can divide the entire equation by $F$ (since $F=A\alpha^2$ and $A$ cannot be zero for a parabola):
$$\frac{x^2}{\alpha^2} - \frac{2xy}{\alpha\beta} + \frac{y^2}{\beta^2} - \frac{2x}{\alpha} - \frac{2y}{\beta} + 1 = 0$$
This is a valid Cartesian equation for the parabola.

**Step 4: Simplify the Equation**
The equation can be written in a more elegant and well-known form. Let's rearrange the terms:
$$\left(\frac{x^2}{\alpha^2} - \frac{2xy}{\alpha\beta} + \frac{y^2}{\beta^2}\right) = \frac{2x}{\alpha} + \frac{2y}{\beta} - 1$$
The left side is a perfect square:
$$\left(\frac{x}{\alpha} - \frac{y}{\beta}\right)^2 = 2\left(\frac{x}{\alpha} + \frac{y}{\beta}\right) - 1$$
This is correct, but we can simplify it even further towards a canonical form. Let's go back to the polynomial form:
$$\frac{x^2}{\alpha^2} - \frac{2xy}{\alpha\beta} + \frac{y^2}{\beta^2} - \frac{2x}{\alpha} - \frac{2y}{\beta} + 1 = 0$$
This equation is equivalent to:
$$\left(\frac{x}{\alpha} + \frac{y}{\beta} - 1\right)^2 = \frac{4xy}{\alpha\beta}$$
To see this, expand the left side:
$$\left(\frac{x}{\alpha}\right)^2 + \left(\frac{y}{\beta}\right)^2 + 1 + \frac{2xy}{\alpha\beta} - \frac{2x}{\alpha} - \frac{2y}{\beta} = \frac{4xy}{\alpha\beta}$$
Subtracting $\frac{4xy}{\alpha\beta}$ from both sides gives the polynomial we derived.

From $(\frac{x}{\alpha} + \frac{y}{\beta} - 1)^2 = \frac{4xy}{\alpha\beta}$, we can take the square root of both sides:
$$\frac{x}{\alpha} + \frac{y}{\beta} - 1 = \pm 2\sqrt{\frac{xy}{\alpha\beta}}$$
For the arc of the parabola between the tangency points $(\alpha, 0)$ and $(0, \beta)$, the points $(x,y)$ lie "below" the line $\frac{x}{\alpha}+\frac{y}{\beta}=1$. Thus, for these points, $\frac{x}{\alpha}+\frac{y}{\beta}-1 < 0$. We must choose the negative sign:
$$\frac{x}{\alpha} + \frac{y}{\beta} - 1 = -2\sqrt{\frac{x}{\alpha}}\sqrt{\frac{y}{\beta}}$$
Rearranging the terms:
$$\frac{x}{\alpha} + 2\sqrt{\frac{x}{\alpha}}\sqrt{\frac{y}{\beta}} + \frac{y}{\beta} = 1$$
The left side is now a perfect square:
$$\left(\sqrt{\frac{x}{\alpha}} + \sqrt{\frac{y}{\beta}}\right)^2 = 1$$
Since $x,y,\alpha,\beta$ are all positive, the terms inside the square root are positive. We take the positive square root of both sides:
$$\sqrt{\frac{x}{\alpha}} + \sqrt{\frac{y}{\beta}} = 1$$

This is the most common and elegant form of the equation for this parabola.

---

### **Method 2: Parametric (Bézier Curve) Approach**

This problem can be modeled beautifully using a quadratic Bézier curve.

**Step 1: Relate the Problem to a Bézier Curve**
A quadratic Bézier curve is a parametric curve defined by three control points: a start point $P_0$, a control point $P_1$, and an end point $P_2$. The curve is tangent to the line segment $P_0P_1$ at $P_0$ and to the line segment $P_1P_2$ at $P_2$.

In our problem:
*   The start point of the parabolic arc can be $P_0 = (\alpha, 0)$.
*   The end point can be $P_2 = (0, \beta)$.
*   The tangent at $P_0$ is the x-axis ($y=0$).
*   The tangent at $P_2$ is the y-axis ($x=0$).
*   The control point $P_1$ is the intersection of the tangent lines. The intersection of $y=0$ and $x=0$ is the origin, so $P_1 = (0, 0)$.

**Step 2: Write the Parametric Equations**
The formula for a quadratic Bézier curve is:
$$P(t) = (1-t)^2 P_0 + 2t(1-t) P_1 + t^2 P_2, \quad \text{for } t \in [0, 1]$$
Substituting our points $P_0=(\alpha,0)$, $P_1=(0,0)$, and $P_2=(0,\beta)$:
$$P(t) = (x(t), y(t)) = (1-t)^2 (\alpha, 0) + 2t(1-t) (0, 0) + t^2 (0, \beta)$$
This gives us the parametric equations for $x$ and $y$:
$$x(t) = \alpha(1-t)^2$$
$$y(t) = \beta t^2$$

**Step 3: Eliminate the Parameter `t`**
Our goal is to find a Cartesian equation, so we must eliminate the parameter $t$.
From the equation for $y(t)$:
$$t^2 = \frac{y}{\beta} \implies t = \sqrt{\frac{y}{\beta}} \quad (\text{since } t \ge 0)$$
From the equation for $x(t)$:
$$(1-t)^2 = \frac{x}{\alpha} \implies 1-t = \sqrt{\frac{x}{\alpha}} \quad (\text{since } 1-t \ge 0 \text{ for } t \in [0,1])$$
Now we have two expressions, one for $t$ and one for $1-t$. We know that $t + (1-t) = 1$. Substituting our expressions:
$$\sqrt{\frac{y}{\beta}} + \sqrt{\frac{x}{\alpha}} = 1$$

Rearranging gives the same beautiful equation:
$$\sqrt{\frac{x}{\alpha}} + \sqrt{\frac{y}{\beta}} = 1$$

---

### **Conclusion**

Both methods lead to the same result. The equation of the parabola tangent to the x-axis at $(\alpha,0)$ and the y-axis at $(0,\beta)$ is:
$$ \sqrt{\frac{x}{\alpha}} + \sqrt{\frac{y}{\beta}} = 1 $$
This equation can also be written in the polynomial form derived in Method 1:
$$ \left(\frac{x}{\alpha} + \frac{y}{\beta} - 1\right)^2 = \frac{4xy}{\alpha\beta} $$
or
$$ \frac{x^2}{\alpha^2} - \frac{2xy}{\alpha\beta} + \frac{y^2}{\beta^2} - \frac{2x}{\alpha} - \frac{2y}{\beta} + 1 = 0 $$