# Solution

I'll solve this system of equations by finding all positive solutions $(x_1,x_2,\ldots,x_n)$.

First, let's see if there's an obvious solution. If I set $x_i = 1$ for all $i$, then:
- $\ln x_i = 0$ for all $i$
- Each equation becomes: $1^2 + (1-0)^2 = 2(1) - 2(0) \Rightarrow 1 + 1 = 2$

This checks out, so $(1,1,\ldots,1)$ is a solution. Now I'll prove it's the only solution.

## Step 1: Sum all equations

I'll add up all $n$ equations in the system:

$$\sum_{i=1}^n x_i^2 + \sum_{i=1}^n (1 - x_{i+1} \ln x_{i+1})^2 = \sum_{i=1}^n 2x_{i+1} - \sum_{i=1}^n 2 x_{i+2}^2 \ln x_{i+2}$$

Since the indices are cyclic modulo $n$, we can reindex the sums:

$$\sum_{i=1}^n x_i^2 + \sum_{i=1}^n (1 - x_i \ln x_i)^2 = \sum_{i=1}^n 2x_i - \sum_{i=1}^n 2 x_i^2 \ln x_i$$

## Step 2: Rearrange and expand

Expanding $(1 - x_i \ln x_i)^2 = 1 - 2x_i \ln x_i + (x_i \ln x_i)^2$:

$$\sum_{i=1}^n x_i^2 + \sum_{i=1}^n [1 - 2x_i \ln x_i + (x_i \ln x_i)^2] = \sum_{i=1}^n 2x_i - \sum_{i=1}^n 2 x_i^2 \ln x_i$$

Rearranging:

$$\sum_{i=1}^n x_i^2 + n - \sum_{i=1}^n 2x_i \ln x_i + \sum_{i=1}^n (x_i \ln x_i)^2 + \sum_{i=1}^n 2 x_i^2 \ln x_i = \sum_{i=1}^n 2x_i$$

Further simplification yields:

$$\sum_{i=1}^n (x_i - 1)^2 + \sum_{i=1}^n (x_i \ln x_i)^2 + \sum_{i=1}^n 2 x_i \ln x_i (x_i - 1) = 0$$

## Step 3: Analyze each term

For all $x_i > 0$:
1. $(x_i - 1)^2 \geq 0$ with equality iff $x_i = 1$
2. $(x_i \ln x_i)^2 \geq 0$ with equality iff $x_i = 1$ (since $x_i \ln x_i = 0$ only when $x_i = 1$ for $x_i > 0$)
3. For the term $2x_i \ln x_i (x_i - 1)$:
   - If $x_i > 1$: then $\ln x_i > 0$ and $(x_i - 1) > 0$, so the term is positive
   - If $0 < x_i < 1$: then $\ln x_i < 0$ and $(x_i - 1) < 0$, so the term is positive
   - If $x_i = 1$: then $\ln x_i = 0$, so the term equals zero

Therefore, each term in the sum is non-negative, and their sum equals zero. This is only possible when each term equals zero, which happens if and only if $x_i = 1$ for all $i$.

## Conclusion

The only solution to the given system is $(x_1, x_2, \ldots, x_n) = (1, 1, \ldots, 1)$.