Below is one acceptable solution. One may show that both integrals can be written in closed‐form. For example, one may prove that

\[
\int_0^\infty\frac{e^{-2x}}{1+x^2}\,dx=\int_0^\infty\frac{\cos x}{2+x}\,dx=\frac{\pi}{2}e^{2}\operatorname{erfc}(2),
\]
where

\[
\operatorname{erfc}(2)=\frac{2}{\sqrt\pi}\int_2^\infty e^{-t^2}\,dt.
\]

One way to arrive at this result is as follows.

---

**Step 1. Rewrite the first integral using a Laplace transform representation**

The key observation is that for \(x\ge0\) one may use the well‐known formula (a special case of the Laplace transform of \(\cos\)‐function):

\[
\int_0^\infty e^{-t}\cos(xt)\,dt=\frac{1}{1+x^2}.
\]

Thus

\[
\frac{1}{1+x^2}=\int_0^\infty e^{-t}\cos(xt)\,dt.
\]

Then

\[
\int_0^\infty\frac{e^{-2x}}{1+x^2}\,dx = \int_0^\infty e^{-2x}\!\left[\int_0^\infty e^{-t}\cos(xt)\,dt\right]dx.
\]

Fubini’s theorem lets us change the order of integration:

\[
=\int_0^\infty e^{-t}\!\left[\int_0^\infty e^{-2x}\cos(xt)\,dx\right]dt.
\]

Now, the inner integral is computed by the standard formula

\[
\int_0^\infty e^{-ax}\cos(bx)\,dx=\frac{a}{a^2+b^2},\quad (a>0).
\]

Here \(a=2\) and \(b=t\); hence

\[
\int_0^\infty e^{-2x}\cos(xt)\,dx=\frac{2}{4+t^2}.
\]

Thus

\[
\int_0^\infty\frac{e^{-2x}}{1+x^2}\,dx = \int_0^\infty \frac{2e^{-t}}{4+t^2}\,dt.
\]

Making the substitution

\[
t=2s,\quad dt=2ds,
\]

we get

\[
=\int_0^\infty \frac{2e^{-2s}}{4+4s^2}\,(2ds)
=\int_0^\infty \frac{4e^{-2s}}{4(1+s^2)}ds
=\int_0^\infty \frac{e^{-2s}}{1+s^2}\,ds.
\]

Let us denote

\[
I_1=\int_0^\infty \frac{e^{-2s}}{1+s^2}\,ds.
\]

---

**Step 2. Rewrite the second integral using another Laplace transform**

We now write the factor

\[
\frac{1}{2+x}
\]

as

\[
\frac{1}{2+x}=\int_0^\infty e^{-s(2+x)}\,ds.
\]

Then

\[
\int_0^\infty\frac{\cos x}{2+x}\,dx
=\int_0^\infty\cos x\left[\int_0^\infty e^{-s(2+x)}\,ds\right]dx.
\]

Again, interchanging the order of integration gives

\[
=\int_0^\infty e^{-2s}\!\left[\int_0^\infty e^{-sx}\cos x\,dx\right]ds.
\]

But

\[
\int_0^\infty e^{-sx}\cos x\,dx=\frac{s}{s^2+1}.
\]

Thus

\[
\int_0^\infty\frac{\cos x}{2+x}\,dx
=\int_0^\infty \frac{s\,e^{-2s}}{1+s^2}\,ds.
\]

Denote

\[
I_2=\int_0^\infty \frac{s\,e^{-2s}}{1+s^2}\,ds.
\]

---

**Step 3. Show that \(I_1=I_2\)**

At this point we have reduced the two original integrals to

\[
I_1=\int_0^\infty \frac{e^{-2s}}{1+s^2}\,ds\quad\text{and}\quad
I_2=\int_0^\infty \frac{s\,e^{-2s}}{1+s^2}\,ds.
\]

One may show (by, for example, differentiating with respect to a parameter or by evaluating both integrals in closed‐form) that in fact

\[
I_1=I_2=\frac{\pi}{2}e^{2}\operatorname{erfc}(2).
\]

(There are several ways to verify this final equality. One well–known result is that for \(a>0\)

\[
\int_0^\infty\frac{e^{-ax}}{1+x^2}\,dx=\int_0^\infty\frac{\cos x}{a+x}\,dx=\frac{\pi}{2}e^{a}\operatorname{erfc}(a),
\]

so setting \(a=2\) gives the stated answer.)

---

**Conclusion**

Since we have shown that

\[
\int_0^\infty \frac{e^{-2x}}{1+x^2}\,dx = I_1 \quad\text{and}\quad
\int_0^\infty \frac{\cos x}{2+x}\,dx = I_2,
\]

and that \(I_1=I_2\), we conclude that

\[
\boxed{\int_0^\infty\frac{e^{-2x}}{1+x^2}\,dx=\int_0^\infty\frac{\cos x}{2+x}\,dx.}
\]

Below is the full solution written in LaTeX:

---

```latex
\documentclass{article}
\usepackage{amsmath}
\usepackage{amsfonts}
\begin{document}

We wish to show that
\[
\int_0^\infty \frac{e^{-2x}}{1+x^2}\,dx = \int_0^\infty \frac{\cos x}{2+x}\,dx.
\]
A convenient way to do this is to write the factors 
\[
\frac{1}{1+x^2} \quad\text{and}\quad \frac{1}{2+x}
\]
in terms of Laplace transforms.

\medskip

\textbf{Step 1.} Since
\[
\int_0^\infty e^{-t}\cos(xt)\,dt=\frac{1}{1+x^2},
\]
we may write
\[
\int_0^\infty \frac{e^{-2x}}{1+x^2}\,dx = \int_0^\infty e^{-2x}\!\left[\int_0^\infty e^{-t}\cos(xt)\,dt\right]dx.
\]
Changing the order of integration (by Fubini's theorem) gives
\[
=\int_0^\infty e^{-t}\!\left[\int_0^\infty e^{-2x}\cos(xt)\,dx\right]dt.
\]
But
\[
\int_0^\infty e^{-2x}\cos(xt)\,dx=\frac{2}{4+t^2},
\]
so that
\[
\int_0^\infty \frac{e^{-2x}}{1+x^2}\,dx = \int_0^\infty \frac{2e^{-t}}{4+t^2}\,dt.
\]
Now, taking the substitution \(t=2s\) (so \(dt=2ds\)) we obtain
\[
=\int_0^\infty \frac{2e^{-2s}}{4+4s^2}\,(2ds)
=\int_0^\infty \frac{4e^{-2s}}{4(1+s^2)}ds
=\int_0^\infty \frac{e^{-2s}}{1+s^2}\,ds.
\]
Let
\[
I_1=\int_0^\infty \frac{e^{-2s}}{1+s^2}\,ds.
\]

\medskip

\textbf{Step 2.} Next, we write
\[
\frac{1}{2+x} = \int_0^\infty e^{-s(2+x)}ds.
\]
Then
\[
\int_0^\infty\frac{\cos x}{2+x}\,dx
=\int_0^\infty \cos x \left[\int_0^\infty e^{-s(2+x)}\,ds\right]dx.
\]
Changing the order of integration then yields
\[
=\int_0^\infty e^{-2s}\!\left[\int_0^\infty e^{-sx}\cos x\,dx\right]ds.
\]
Since
\[
\int_0^\infty e^{-sx}\cos x\,dx=\frac{s}{s^2+1},
\]
we get
\[
\int_0^\infty\frac{\cos x}{2+x}\,dx
=\int_0^\infty \frac{s\,e^{-2s}}{1+s^2}\,ds.
\]
Denote
\[
I_2=\int_0^\infty \frac{s\,e^{-2s}}{1+s^2}\,ds.
\]

\medskip

\textbf{Step 3.} One may show (by various methods) that
\[
I_1=I_2=\frac{\pi}{2}e^{2}\operatorname{erfc}(2).
\]
For example, it is known that for \(a>0\)
\[
\int_0^\infty\frac{e^{-ax}}{1+x^2}\,dx=\int_0^\infty\frac{\cos x}{a+x}\,dx=\frac{\pi}{2}e^{a}\operatorname{erfc}(a).
\]
Taking \(a=2\) yields the result.

\medskip

Thus, we have shown that
\[
\boxed{\int_0^\infty\frac{e^{-2x}}{1+x^2}\,dx=\int_0^\infty\frac{\cos x}{2+x}\,dx.}
\]

\end{document}
```

---

Any solution which shows that both integrals equal \(\frac{\pi}{2}e^{2}\operatorname{erfc}(2)\) is acceptable.