 Notice that $a$,$b$, $c$ have to be positive. If the triple $a$, $b$, $c$ satisfies this system of equation, then w.l.o.g. we can assume that $a \leqslant b \leqslant c$. But then
    \begin{displaymath}
        (b+c)^{2024} \geqslant (a+c)^{2024} \geqslant (a+b)^{2024},
    \end{displaymath}
    so $4a \geqslant 4b \geqslant 4c$. Thus $a = b = c$. Substituting this to for example the first equation, we obtain $(2a)^{2024} = 4a$. Dividing both sides by $4a$, we obtain $2^{2022}a^{2023} = 1$, thus $a = 2^{\frac{-2022}{2023}}$. So the sum of all of those numbers is $\frac{3}{2^{\frac{2022}{2023}}}$, and thus $x+y = 5$.