Of course. Here is a detailed, step-by-step solution to the problem.

### **Methodology**

The problem asks us to prove that $\lceil (\sqrt {11}+3)^{2n}\rceil$ is divisible by $2^{n+1}$ for any integer $n\geq 1$.

Our strategy will be as follows:
1.  **Simplify the Expression:** The ceiling function $\lceil x \rceil$ and the irrational term $(\sqrt{11}+3)^{2n}$ are difficult to work with directly. We will introduce the conjugate term $(\sqrt{11}-3)^{2n}$ to create an integer expression, which will allow us to eliminate the ceiling function.
2.  **Establish a Recurrence Relation:** We will define a sequence $S_n$ based on our new integer expression and find a linear recurrence relation that it satisfies. This is a powerful technique for proving properties of sequences.
3.  **Prove Divisibility by Induction:** Using the recurrence relation, we will use the principle of mathematical induction to prove that the terms of the sequence have the desired divisibility property.

---

### **Step 1: Simplifying the Expression and Eliminating the Ceiling Function**

Let the expression inside the ceiling function be $A_n = (\sqrt{11}+3)^{2n}$.
To handle the irrationality and the ceiling function, we introduce its conjugate pair. Let $B_n = (\sqrt{11}-3)^{2n}$.

Let's analyze the sum $A_n + B_n$:
$A_n + B_n = (\sqrt{11}+3)^{2n} + (\sqrt{11}-3)^{2n}$.

We can expand each term using the binomial theorem:
$(x+y)^k = \sum_{j=0}^{k} \binom{k}{j} x^{k-j} y^j$.

For $A_n$, let $x=\sqrt{11}$, $y=3$, and $k=2n$:
$(\sqrt{11}+3)^{2n} = \sum_{j=0}^{2n} \binom{2n}{j} (\sqrt{11})^{2n-j} 3^j$.

For $B_n$, let $x=\sqrt{11}$, $y=-3$, and $k=2n$:
$(\sqrt{11}-3)^{2n} = \sum_{j=0}^{2n} \binom{2n}{j} (\sqrt{11})^{2n-j} (-3)^j$.

When we add these two expansions, the terms where $j$ is odd will have opposite signs and cancel out.
- If $j$ is odd, the term from $A_n$ is $\binom{2n}{j} (\sqrt{11})^{2n-j} 3^j$.
- If $j$ is odd, the term from $B_n$ is $\binom{2n}{j} (\sqrt{11})^{2n-j} (-3)^j = - \binom{2n}{j} (\sqrt{11})^{2n-j} 3^j$.

The terms where $j$ is even will be identical and will be doubled.
- If $j$ is even, the term from $A_n$ is $\binom{2n}{j} (\sqrt{11})^{2n-j} 3^j$.
- If $j$ is even, the term from $B_n$ is $\binom{2n}{j} (\sqrt{11})^{2n-j} (-3)^j = \binom{2n}{j} (\sqrt{11})^{2n-j} 3^j$.

In the sum $A_n+B_n$, all terms with an odd power of $\sqrt{11}$ (which corresponds to an odd value of $2n-j$, meaning $j$ is odd) are eliminated. The remaining terms have even powers of $\sqrt{11}$, which are integers. Thus, $A_n + B_n$ is an integer. Let's call this integer $I_n$.
$I_n = A_n + B_n = 2 \sum_{j=0, j \text{ even}}^{2n} \binom{2n}{j} (\sqrt{11})^{2n-j} 3^j$.
Since all terms in the sum are integers, $I_n$ is an integer.

Now, let's analyze the magnitude of $B_n = (\sqrt{11}-3)^{2n}$.
We know that $\sqrt{9} < \sqrt{11} < \sqrt{16}$, which means $3 < \sqrt{11} < 4$.
Subtracting 3, we get $0 < \sqrt{11}-3 < 1$.
Since $n \ge 1$, we raise this inequality to the power of $2n$:
$0 < (\sqrt{11}-3)^{2n} < 1^{2n}$, which simplifies to $0 < B_n < 1$.

We have the relation $A_n + B_n = I_n$, where $I_n$ is an integer.
Rearranging for $A_n$, we get $A_n = I_n - B_n$.
Since $0 < B_n < 1$, we can write the inequality for $A_n$:
$I_n - 1 < A_n < I_n$.

Since $A_n = (\sqrt{11}+3)^{2n}$ is not an integer, and it lies strictly between two consecutive integers $I_n-1$ and $I_n$, the smallest integer greater than or equal to $A_n$ must be $I_n$.
Therefore, $\lceil A_n \rceil = \lceil (\sqrt{11}+3)^{2n} \rceil = I_n$.

The problem is now reduced to proving that $I_n = (\sqrt{11}+3)^{2n} + (\sqrt{11}-3)^{2n}$ is divisible by $2^{n+1}$ for $n \ge 1$.

---

### **Step 2: Establish a Recurrence Relation**

Let $S_n = (\sqrt{11}+3)^{2n} + (\sqrt{11}-3)^{2n}$.
To find a simpler recurrence, let's group the exponent differently:
$S_n = [(\sqrt{11}+3)^2]^n + [(\sqrt{11}-3)^2]^n$.

Let's compute the base terms:
$\alpha = (\sqrt{11}+3)^2 = (\sqrt{11})^2 + 2(3)\sqrt{11} + 3^2 = 11 + 6\sqrt{11} + 9 = 20 + 6\sqrt{11}$.
$\beta = (\sqrt{11}-3)^2 = (\sqrt{11})^2 - 2(3)\sqrt{11} + 3^2 = 11 - 6\sqrt{11} + 9 = 20 - 6\sqrt{11}$.

So, our sequence is $S_n = \alpha^n + \beta^n$.
This is a standard form for a sequence that satisfies a linear homogeneous recurrence relation with constant coefficients. The characteristic equation for such a recurrence has roots $\alpha$ and $\beta$.
The equation is $(x-\alpha)(x-\beta)=0$, which expands to $x^2 - (\alpha+\beta)x + \alpha\beta = 0$.

Let's compute the coefficients:
- Sum of the roots: $\alpha+\beta = (20+6\sqrt{11}) + (20-6\sqrt{11}) = 40$.
- Product of the roots: $\alpha\beta = (20+6\sqrt{11})(20-6\sqrt{11}) = 20^2 - (6\sqrt{11})^2 = 400 - 36(11) = 400 - 396 = 4$.

So, the characteristic equation is $x^2 - 40x + 4 = 0$.
The sequence $S_n$ satisfies the recurrence relation:
$S_{n+2} = 40 S_{n+1} - 4 S_n$.

---

### **Step 3: Prove Divisibility by Induction**

We want to prove that $S_n$ is divisible by $2^{n+1}$ for all $n \ge 1$.
Let $P(n)$ be the statement "$S_n$ is divisible by $2^{n+1}$".

**Base Cases:**
We need to establish the first two cases because our recurrence relation is of order 2.

- **For n=1:**
$S_1 = \alpha^1 + \beta^1 = 40$.
We need to check if $S_1$ is divisible by $2^{1+1} = 2^2 = 4$.
$40 = 4 \times 10$. So, $S_1$ is divisible by 4.
Thus, $P(1)$ is true.

- **For n=2:**
We can calculate $S_2$ using the recurrence: $S_2 = 40 S_1 - 4 S_0$.
First, we need $S_0 = \alpha^0 + \beta^0 = 1+1 = 2$.
$S_2 = 40(S_1) - 4(S_0) = 40(40) - 4(2) = 1600 - 8 = 1592$.
We need to check if $S_2$ is divisible by $2^{2+1} = 2^3 = 8$.
$1592 \div 8 = 199$. So, $S_2$ is divisible by 8.
Thus, $P(2)$ is true.

**Inductive Hypothesis:**
Assume that for some integer $k \ge 2$, $P(m)$ is true for all integers $m$ such that $1 \le m \le k$.
Specifically, we assume:
- $P(k): S_k$ is divisible by $2^{k+1}$. So, $S_k = a \cdot 2^{k+1}$ for some integer $a$.
- $P(k-1): S_{k-1}$ is divisible by $2^{(k-1)+1} = 2^k$. So, $S_{k-1} = b \cdot 2^k$ for some integer $b$.

**Inductive Step:**
We want to prove $P(k+1)$, which is the statement that $S_{k+1}$ is divisible by $2^{(k+1)+1} = 2^{k+2}$.
Using our recurrence relation:
$S_{k+1} = 40 S_k - 4 S_{k-1}$.

Substitute the expressions from our inductive hypothesis:
$S_{k+1} = 40 (a \cdot 2^{k+1}) - 4 (b \cdot 2^k)$.

Now, let's analyze the powers of 2:
$S_{k+1} = (5 \cdot 8) (a \cdot 2^{k+1}) - (2^2) (b \cdot 2^k)$
$S_{k+1} = (5 \cdot 2^3) (a \cdot 2^{k+1}) - (b \cdot 2^2 \cdot 2^k)$
$S_{k+1} = 5a \cdot 2^{k+1+3} - b \cdot 2^{k+2}$
$S_{k+1} = 5a \cdot 2^{k+4} - b \cdot 2^{k+2}$

Now, we can factor out the term $2^{k+2}$:
$S_{k+1} = 2^{k+2} (5a \cdot 2^2 - b)$
$S_{k+1} = 2^{k+2} (20a - b)$

Since $a$ and $b$ are integers, $(20a - b)$ is also an integer.
This shows that $S_{k+1}$ is an integer multiple of $2^{k+2}$.
Therefore, $S_{k+1}$ is divisible by $2^{k+2}$.
This proves that $P(k+1)$ is true.

### **Conclusion**

By the principle of strong mathematical induction, the statement $P(n)$ is true for all integers $n \ge 1$.
We have already shown that $\lceil (\sqrt {11}+3)^{2n}\rceil = S_n$.
Therefore, $\lceil (\sqrt {11}+3)^{2n}\rceil$ is divisible by $2^{n+1}$ for any $n\geq 1$.

---
**Final Summary of Proof:**
1.  We let $A_n = (\sqrt{11}+3)^{2n}$ and $B_n = (\sqrt{11}-3)^{2n}$. We showed that their sum $S_n = A_n+B_n$ is an integer.
2.  We showed that $0 < B_n < 1$, which implies that $\lceil A_n \rceil = S_n$.
3.  The problem was reduced to proving that $S_n$ is divisible by $2^{n+1}$.
4.  We defined $\alpha = (20+6\sqrt{11})$ and $\beta = (20-6\sqrt{11})$ so that $S_n = \alpha^n + \beta^n$.
5.  We derived the recurrence relation $S_{n+2} = 40 S_{n+1} - 4 S_n$ for the sequence.
6.  We used strong induction to prove that $S_n$ is divisible by $2^{n+1}$ for all $n \ge 1$, successfully completing the proof.