An expert mathematician's response to the problem would involve not only verifying the result but also ensuring that every step in the reasoning is logically sound and rigorously justified. The provided solution sketch arrives at the correct answer, but it relies on an intuitive leap that should be formalized.

### Problem Statement
Compute the limit:
$$ L = \lim_{n\to\infty} \frac{1}{n^2}\sum_{k=1}^n\sum_{l=1}^k e^{l/k} $$

### Analysis of the Provided Solution

The solution starts by defining the inner sum as $S_k = \sum_{l=1}^k e^{l/k}$. This is a finite geometric series with first term $a = e^{1/k}$ and common ratio $r = e^{1/k}$. The sum is correctly calculated as:
$$ S_k = a \frac{r^k - 1}{r - 1} = e^{1/k} \frac{(e^{1/k})^k - 1}{e^{1/k} - 1} = e^{1/k} \frac{e - 1}{e^{1/k} - 1} $$
The next step in the provided solution uses the asymptotic approximation $S_k \sim k(e-1)$ for large $k$. This is derived from the Taylor expansion $e^x \approx 1+x$ for small $x$. Letting $x=1/k$, we have:
$$ S_k = \frac{e^{1/k}(e-1)}{e^{1/k}-1} \approx \frac{(1+1/k)(e-1)}{(1+1/k)-1} = \frac{(1+1/k)(e-1)}{1/k} = (k+1)(e-1) \sim k(e-1) $$
The crucial step is then replacing $S_k$ with its asymptotic form inside the summation:
$$ \sum_{k=1}^n S_k \sim \sum_{k=1}^n k(e-1) = (e-1)\frac{n(n+1)}{2} $$
While this leads to the correct final answer, this step is a heuristic that is not always valid. Replacing terms in a sum with their asymptotic equivalents requires justification. We will now provide a rigorous proof.

### Rigorous Solution using the Stolz-Cesàro Theorem

A powerful tool for limits of this form is the Stolz-Cesàro theorem. The theorem states that if $(b_n)_{n\ge 1}$ is a strictly monotone and divergent sequence (i.e., $b_n \to \infty$), and the limit
$$ \lim_{n\to\infty} \frac{a_n - a_{n-1}}{b_n - b_{n-1}} = L $$
exists, then the limit $\lim_{n\to\infty} \frac{a_n}{b_n}$ also exists and is equal to $L$.

Let's apply this to our problem. Define:
- $a_n = \sum_{k=1}^n S_k = \sum_{k=1}^n \sum_{l=1}^k e^{l/k}$
- $b_n = n^2$

The sequence $b_n = n^2$ is strictly increasing and diverges to $\infty$. Now we compute the limit of the ratio of differences:
$$ \frac{a_n - a_{n-1}}{b_n - b_{n-1}} = \frac{\left(\sum_{k=1}^n S_k\right) - \left(\sum_{k=1}^{n-1} S_k\right)}{n^2 - (n-1)^2} = \frac{S_n}{n^2 - (n^2 - 2n + 1)} = \frac{S_n}{2n-1} $$
Now we need to compute the limit of this expression as $n \to \infty$:
$$ \lim_{n\to\infty} \frac{S_n}{2n-1} = \lim_{n\to\infty} \frac{1}{2n-1} \left( \frac{e^{1/n}(e-1)}{e^{1/n}-1} \right) $$
To evaluate this limit, we rearrange the terms:
$$ = (e-1) \lim_{n\to\infty} \left( \frac{n}{2n-1} \cdot \frac{e^{1/n}}{n(e^{1/n}-1)} \right) $$
We can evaluate the limits of the individual parts:
1.  $\lim_{n\to\infty} \frac{n}{2n-1} = \lim_{n\to\infty} \frac{1}{2 - 1/n} = \frac{1}{2}$
2.  $\lim_{n\to\infty} e^{1/n} = e^0 = 1$
3.  $\lim_{n\to\infty} n(e^{1/n}-1)$. Let $x = 1/n$. As $n\to\infty$, $x\to 0$. The limit becomes $\lim_{x\to 0} \frac{e^x-1}{x}$. This is the definition of the derivative of $e^x$ at $x=0$, which is $e^0=1$.

Combining these results, we get:
$$ \lim_{n\to\infty} \frac{S_n}{2n-1} = (e-1) \cdot \left( \frac{1}{2} \cdot \frac{1}{1} \right) = \frac{e-1}{2} $$
By the Stolz-Cesàro theorem, the original limit is the same:
$$ L = \lim_{n\to\infty} \frac{1}{n^2}\sum_{k=1}^n\sum_{l=1}^k e^{l/k} = \frac{e-1}{2} $$

### Rigorous Solution using Asymptotic Expansion

This method justifies the heuristic by analyzing the error terms.
We found $S_k = (e-1) \frac{e^{1/k}}{e^{1/k}-1}$. Let $x=1/k$. For $k\to\infty$, $x\to 0$. We find a more precise expansion of $\frac{e^x}{e^x-1}$:
$$ \frac{e^x}{e^x-1} = \frac{1+x+\frac{x^2}{2}+O(x^3)}{x+\frac{x^2}{2}+\frac{x^3}{6}+O(x^4)} = \frac{1}{x} \cdot \frac{1+x+\frac{x^2}{2}+O(x^3)}{1+\frac{x}{2}+\frac{x^2}{6}+O(x^3)} $$
By performing polynomial long division or using Taylor series manipulation:
$$ \frac{1+x+x^2/2}{1+x/2} = 1 + \frac{x}{2} + O(x^2) $$
So, $\frac{e^x}{e^x-1} = \frac{1}{x} \left(1 + \frac{x}{2} + O(x^2)\right) = \frac{1}{x} + \frac{1}{2} + O(x)$.
Substituting back $x=1/k$:
$$ S_k = (e-1)\left(k + \frac{1}{2} + O\left(\frac{1}{k}\right)\right) = k(e-1) + \frac{e-1}{2} + O\left(\frac{1}{k}\right) $$
Now, we sum this expression from $k=1$ to $n$:
$$ \sum_{k=1}^n S_k = \sum_{k=1}^n \left( k(e-1) + \frac{e-1}{2} + O\left(\frac{1}{k}\right) \right) $$
$$ = (e-1)\sum_{k=1}^n k + \frac{e-1}{2}\sum_{k=1}^n 1 + \sum_{k=1}^n O\left(\frac{1}{k}\right) $$
We evaluate each term:
- $\sum_{k=1}^n k = \frac{n(n+1)}{2} = \frac{n^2}{2} + \frac{n}{2}$
- $\sum_{k=1}^n 1 = n$
- $\sum_{k=1}^n O(\frac{1}{k}) = O(\sum_{k=1}^n \frac{1}{k}) = O(\ln n)$ (since the harmonic series grows logarithmically)

Substituting these back:
$$ \sum_{k=1}^n S_k = (e-1)\left(\frac{n^2}{2} + \frac{n}{2}\right) + \frac{e-1}{2}n + O(\ln n) $$
$$ = \frac{e-1}{2}n^2 + \frac{e-1}{2}n + \frac{e-1}{2}n + O(\ln n) = \frac{e-1}{2}n^2 + (e-1)n + O(\ln n) $$
Finally, we divide by $n^2$ and take the limit:
$$ \lim_{n\to\infty} \frac{1}{n^2}\sum_{k=1}^n S_k = \lim_{n\to\infty} \frac{1}{n^2}\left(\frac{e-1}{2}n^2 + (e-1)n + O(\ln n)\right) $$
$$ = \lim_{n\to\infty} \left(\frac{e-1}{2} + \frac{e-1}{n} + O\left(\frac{\ln n}{n^2}\right)\right) = \frac{e-1}{2} $$
This method confirms the result and demonstrates that the error terms introduced by the approximation $S_k \approx k(e-1)$ do not affect the final limit.

### Conclusion
The heuristic argument provided in the problem description, while insightful, skips over a crucial justification. Both the Stolz-Cesàro theorem and the method of asymptotic expansion provide rigorous pathways to the same result. They confirm that the dominant behavior of the sum is dictated by the leading term in the asymptotic expansion of $S_k$.

The final answer is:
$$ \lim_{n\to\infty} \frac{1}{n^2}\sum_{k=1}^n\sum_{l=1}^k e^{l/k} = \frac{e-1}{2} $$