Of course. Here is a detailed, step-by-step solution to the problem.

### Introduction
The problem asks us to prove the inequality $\sum_{i=1}^n \left( a_i + \frac{1}{a_i} \right)^p \geq \frac{(n^2+1)^p}{n^{p-1}}$ given that $a_i > 0$ for all $i$, $\sum_{i=1}^n a_i = 1$, and $p > 0$.

This inequality has a structure that is highly suggestive of **Jensen's Inequality**. Jensen's inequality relates the value of a convex function of an integral to the integral of the convex function. For a discrete set of points, it states that if a function $f$ is convex, then for any points $x_1, \ldots, x_n$ in its domain,
$$ \frac{1}{n} \sum_{i=1}^n f(x_i) \geq f\left(\frac{1}{n}\sum_{i=1}^n x_i\right). $$

Let's define the function $f(x) = \left(x + \frac{1}{x}\right)^p$. The left side of our inequality is $\sum_{i=1}^n f(a_i)$. Our strategy will be to prove that $f(x)$ is a convex function on the domain of interest for the $a_i$ and then apply Jensen's inequality.

### Step 1: Determine the Domain of Interest
The variables $a_i$ are positive and sum to 1. This implies that for $n > 1$, we must have $0 < a_i < 1$ for all $i$. If $n=1$, then $a_1=1$. Therefore, all $a_i$ values lie in the interval $(0, 1]$. Our goal is to prove that $f(x)$ is convex on this interval.

A function is convex on an interval if its second derivative, $f''(x)$, is non-negative on that interval.

### Step 2: Prove Convexity of $f(x) = \left(x + \frac{1}{x}\right)^p$ on $(0, 1]$

We need to compute $f''(x)$ and analyze its sign. The analysis differs slightly depending on the value of $p$, so we will consider two cases: $p \geq 1$ and $0 < p < 1$.

**Case 1: $p \geq 1$**

For this case, we can prove convexity using the properties of composite functions.
Let $k(x) = x + \frac{1}{x}$ and $h(u) = u^p$. Then $f(x) = h(k(x))$.

1.  **Analyze $k(x) = x + \frac{1}{x}$:**
    $k'(x) = 1 - \frac{1}{x^2}$
    $k''(x) = \frac{2}{x^3}$
    Since $x > 0$, $k''(x) > 0$. Thus, $k(x)$ is a convex function for all $x>0$.

2.  **Analyze $h(u) = u^p$ for $p \geq 1$:**
    $h'(u) = pu^{p-1}$
    $h''(u) = p(p-1)u^{p-2}$
    Since $p \geq 1$ and the argument $u = x+1/x \geq 2 > 0$, we have $h''(u) \geq 0$. Thus, $h(u)$ is a convex function. Furthermore, for $u>0$, $h'(u) > 0$, so $h(u)$ is an increasing function.

3.  **Composition:**
    A key theorem in calculus states that the composition of a convex, increasing function with a convex function is convex. Since $h(u)$ is convex and increasing for $u > 0$, and $k(x)$ is convex for $x > 0$, their composition $f(x) = h(k(x))$ is convex for all $x > 0$. This includes our interval of interest, $(0, 1]$.

**Case 2: $0 < p < 1$**

In this case, the function $h(u)=u^p$ is concave, so the composition argument does not work. We must directly compute and analyze the sign of $f''(x)$.

1.  **First Derivative:**
    Using the chain rule:
    $f'(x) = p\left(x + \frac{1}{x}\right)^{p-1} \cdot \left(1 - \frac{1}{x^2}\right)$

2.  **Second Derivative:**
    Using the product rule $[g(x)h(x)]' = g'(x)h(x) + g(x)h'(x)$:
    $f''(x) = p(p-1)\left(x + \frac{1}{x}\right)^{p-2}\left(1 - \frac{1}{x^2}\right)^2 + p\left(x + \frac{1}{x}\right)^{p-1}\left(\frac{2}{x^3}\right)$

    Let's factor out common terms to simplify the expression:
    $f''(x) = p\left(x + \frac{1}{x}\right)^{p-2} \left[ (p-1)\left(1 - \frac{1}{x^2}\right)^2 + \left(x + \frac{1}{x}\right)\left(\frac{2}{x^3}\right) \right]$

    For $x>0$, the term $p\left(x + \frac{1}{x}\right)^{p-2}$ is positive. So the sign of $f''(x)$ is determined by the sign of the term in the brackets. Let's call this term $B(x)$:
    $B(x) = (p-1)\left(1 - \frac{1}{x^2}\right)^2 + \left(x + \frac{1}{x}\right)\left(\frac{2}{x^3}\right)$
    $B(x) = (p-1)\frac{(x^2-1)^2}{x^4} + \frac{x^2+1}{x} \frac{2}{x^3} = \frac{(p-1)(x^4 - 2x^2 + 1) + 2(x^2+1)}{x^4}$
    $B(x) = \frac{(p-1)x^4 + (-2p+2)x^2 + p-1 + 2x^2 + 2}{x^4}$
    $B(x) = \frac{(p-1)x^4 + (4-2p)x^2 + p+1}{x^4}$

    The denominator $x^4$ is positive. Let $Q(x^2)$ be the numerator. Let $y = x^2$. We need to analyze the sign of the quadratic polynomial $Q(y) = (p-1)y^2 + (4-2p)y + (p+1)$ for $y \in (0, 1]$ (since $x \in (0, 1]$).

    Since $0 < p < 1$, the leading coefficient $(p-1)$ is negative, so $Q(y)$ is a downward-opening parabola. A downward-opening parabola is non-negative between its roots. Let's find the roots of $Q(y)=0$:
    $y = \frac{-(4-2p) \pm \sqrt{(4-2p)^2 - 4(p-1)(p+1)}}{2(p-1)}$
    $y = \frac{2p-4 \pm \sqrt{16-16p+4p^2 - 4(p^2-1)}}{2(p-1)}$
    $y = \frac{2p-4 \pm \sqrt{20-16p}}{2(p-1)} = \frac{p-2 \pm \sqrt{5-4p}}{p-1}$

    Let the two roots be $y_1$ and $y_2$.
    $y_1 = \frac{p-2 - \sqrt{5-4p}}{p-1}$ and $y_2 = \frac{p-2 + \sqrt{5-4p}}{p-1}$.

    For $0 < p < 1$:
    - The denominator $p-1$ is negative.
    - The numerator of $y_1$: $p-2$ is negative and $-\sqrt{5-4p}$ is negative, so the numerator is negative. Thus, $y_1 > 0$.
    - The numerator of $y_2$: Let's compare $(p-2)^2$ and $(\sqrt{5-4p})^2$. $(p-2)^2 - (5-4p) = p^2-4p+4 - 5+4p = p^2-1 < 0$. So $|p-2| < \sqrt{5-4p}$, which means $2-p < \sqrt{5-4p}$. This implies $p-2 > -\sqrt{5-4p}$, so $p-2+\sqrt{5-4p} > 0$. The numerator is positive. Thus, $y_2 < 0$.

    So we have a downward-opening parabola $Q(y)$ with a negative root $y_2$ and a positive root $y_1$. This means $Q(y) \geq 0$ for $y \in [y_2, y_1]$.
    We need to check if our domain of interest, $(0, 1]$, is contained within this interval. Since $y_2 < 0$, we just need to show that $1 \leq y_1$.
    $1 \leq \frac{p-2 - \sqrt{5-4p}}{p-1}$
    Since $p-1 < 0$, multiplying by it reverses the inequality:
    $p-1 \geq p-2 - \sqrt{5-4p}$
    $-1 \geq -2 - \sqrt{5-4p}$
    $1 \geq -\sqrt{5-4p}$
    This is always true, as the right side is negative and the left side is positive.

    So, we have shown that $y_1 \geq 1$. Therefore, for any $y \in (0, 1]$, we have $y_2 < 0 < y \leq 1 \leq y_1$, which means $y$ is in the interval where $Q(y) \geq 0$.
    This implies that the numerator of $B(x)$ is non-negative for $x \in (0, 1]$.
    Therefore, $f''(x) \geq 0$ for all $x \in (0, 1]$.

**Conclusion of Step 2:** For all $p>0$, the function $f(x) = (x+1/x)^p$ is convex on the interval $(0, 1]$.

### Step 3: Apply Jensen's Inequality

Since $f(x)$ is convex on $(0, 1]$ and all $a_i \in (0, 1]$ (as shown in Step 1), we can apply Jensen's inequality:
$$ \frac{1}{n} \sum_{i=1}^n f(a_i) \geq f\left(\frac{1}{n}\sum_{i=1}^n a_i\right) $$
Substituting $f(x) = (x+1/x)^p$ and $\sum_{i=1}^n a_i = 1$:
$$ \frac{1}{n} \sum_{i=1}^n \left(a_i + \frac{1}{a_i}\right)^p \geq f\left(\frac{1}{n}\right) $$
Now we evaluate $f(1/n)$:
$$ f\left(\frac{1}{n}\right) = \left(\frac{1}{n} + \frac{1}{1/n}\right)^p = \left(\frac{1}{n} + n\right)^p = \left(\frac{1+n^2}{n}\right)^p = \frac{(n^2+1)^p}{n^p} $$
Substituting this back into our inequality:
$$ \frac{1}{n} \sum_{i=1}^n \left(a_i + \frac{1}{a_i}\right)^p \geq \frac{(n^2+1)^p}{n^p} $$
Finally, multiply both sides by $n$:
$$ \sum_{i=1}^n \left(a_i + \frac{1}{a_i}\right)^p \geq n \cdot \frac{(n^2+1)^p}{n^p} = \frac{(n^2+1)^p}{n^{p-1}} $$

This is precisely the inequality we wanted to prove.

### Case of Equality
Equality in Jensen's inequality $\frac{1}{n}\sum f(a_i) \geq f(\bar{a})$ holds if and only if $a_1 = a_2 = \ldots = a_n$ or if $f$ is a linear function over the domain containing the $a_i$. Our function $f(x)=(x+1/x)^p$ is not linear (since $f''(x)$ is not identically zero). Thus, equality holds if and only if $a_1 = a_2 = \ldots = a_n$.
Given the constraint $\sum_{i=1}^n a_i = 1$, this implies that equality holds when $a_i = 1/n$ for all $i=1, \ldots, n$.

### Summary of the Proof
1.  We identified the problem as an application of Jensen's inequality for the function $f(x) = (x+1/x)^p$.
2.  We established that the variables $a_i$ must lie in the interval $(0, 1]$.
3.  We proved that $f(x)$ is convex on $(0, 1]$ for all $p > 0$ by showing its second derivative $f''(x)$ is non-negative. This required splitting the proof into two cases: $p \geq 1$ (using properties of composite convex functions) and $0 < p < 1$ (by direct analysis of the second derivative).
4.  With the convexity of $f(x)$ established, we applied Jensen's inequality to the points $a_1, \ldots, a_n$.
5.  Substituting the mean value $\bar{a} = 1/n$ and simplifying the resulting expression yielded the desired inequality.