

The functions \( f : \mathbb{V} \to \mathbb{V} \) satisfying the given functional equation are precisely the linear involutions on \(\mathbb{V}\). A linear involution is a linear transformation \( f \) such that \( f(f(z)) = z \) for all \( z \in \mathbb{V} \).

**Step-by-Step Explanation:**

1. **Injectivity of \( f \):**  
   Suppose \( f(a) = f(b) \). For any \( z_2 \), substituting into the functional equation gives:
   \[
   f(f(a) + z_2) = a + f(z_2) \quad \text{and} \quad f(f(b) + z_2) = b + f(z_2).
   \]
   Since \( f(a) = f(b) \), the left-hand sides are equal, implying \( a = b \). Thus, \( f \) is injective.

2. **Setting \( z_2 = 0 \):**  
   Substituting \( z_2 = 0 \) into the equation:
   \[
   f(f(z_1)) = z_1 + f(0).
   \]
   Let \( c = f(0) \). Then \( f(f(z_1)) = z_1 + c \).

3. **Setting \( z_1 = 0 \):**  
   Substituting \( z_1 = 0 \):
   \[
   f(c + z_2) = f(z_2) \quad \forall z_2 \in \mathbb{V}.
   \]
   Since \( f \) is injective, \( c = 0 \). Hence, \( f(0) = 0 \) and \( f(f(z_1)) = z_1 \), showing \( f \) is a bijection (involution).

4. **Additivity of \( f \):**  
   Substitute \( z_1 = f(x) \) into the original equation:
   \[
   f(f(f(x)) + z_2) = f(x) + f(z_2) \implies f(x + z_2) = f(x) + f(z_2).
   \]
   Thus, \( f \) is additive.

5. **Homogeneity over \( \mathbb{Q} \):**  
   For \( k \in \mathbb{Q} \), using additivity and induction:
   - \( f(nx) = nf(x) \) for integers \( n \).
   - Extend to rationals via \( f\left(\frac{m}{n}x\right) = \frac{m}{n}f(x) \).

6. **Conclusion:**  
   \( f \) is a linear transformation and an involution (\( f^2 = I \)). Conversely, any linear involution satisfies the given functional equation.

**Answer:**  
All solutions are linear involutions. Thus, the functions \( f \) are precisely the linear transformations satisfying \( f(f(z)) = z \) for all \( z \in \mathbb{V} \). In LaTeX:

\[
\boxed{f \text{ is a linear involution on } \mathbb{V}, \text{ i.e., } f \circ f = \mathrm{id}_{\mathbb{V}}}
\]