Solution:
Let $x_n = (\sqrt{11}+3)^{2n}$. We want to prove that $\lceil x_n \rceil$ is divisible by $2^{n+1}$ for any integer $n \ge 1$.

Let $a = \sqrt{11}+3$ and $b = \sqrt{11}-3$.
Consider the quantities $A = a^2$ and $B = b^2$.
$A = (\sqrt{11}+3)^2 = 11 + 6\sqrt{11} + 9 = 20 + 6\sqrt{11}$.
$B = (\sqrt{11}-3)^2 = 11 - 6\sqrt{11} + 9 = 20 - 6\sqrt{11}$.
Then $x_n = A^n$.

Let $S_n = A^n + B^n$.
We find the sum and product of $A$ and $B$:
$A+B = (20 + 6\sqrt{11}) + (20 - 6\sqrt{11}) = 40$.
$AB = (20 + 6\sqrt{11})(20 - 6\sqrt{11}) = 20^2 - (6\sqrt{11})^2 = 400 - 36 \times 11 = 400 - 396 = 4$.

The sequence $S_n$ satisfies a linear recurrence relation with characteristic equation $x^2 - (A+B)x + AB = 0$, which is $x^2 - 40x + 4 = 0$.
Thus, the recurrence relation is $S_{n+2} = 40 S_{n+1} - 4 S_n$.

Let's find the first few terms of the sequence $S_n$.
$S_0 = A^0 + B^0 = 1+1 = 2$.
$S_1 = A^1 + B^1 = A+B = 40$.
$S_2 = 40 S_1 - 4 S_0 = 40(40) - 4(2) = 1600 - 8 = 1592$.

Since $S_0=2$ and $S_1=40$ are integers, and the coefficients of the recurrence relation are integers, all $S_n$ are integers for $n \ge 0$.
Alternatively, let $A^n = u_n + v_n \sqrt{11}$ for integers $u_n, v_n$. This holds for $n=1$ with $u_1=20, v_1=6$. Assume it holds for $n=k$. Then $A^{k+1} = A^k \cdot A = (u_k + v_k \sqrt{11})(20 + 6\sqrt{11}) = (20u_k + 66v_k) + (6u_k + 20v_k)\sqrt{11}$. Since $u_k, v_k$ are integers, $u_{k+1}=20u_k + 66v_k$ and $v_{k+1}=6u_k + 20v_k$ are integers. By induction, $u_n, v_n$ are integers for all $n \ge 1$.
Similarly, $B^n = (20 - 6\sqrt{11})^n = u_n - v_n \sqrt{11}$.
So $S_n = A^n + B^n = (u_n + v_n \sqrt{11}) + (u_n - v_n \sqrt{11}) = 2u_n$. Since $u_n$ is an integer, $S_n$ is an integer.

Now we relate $S_n$ to $\lceil x_n \rceil = \lceil A^n \rceil$.
$B = 20 - 6\sqrt{11}$. We know $3^2 = 9$ and $4^2 = 16$, so $3 < \sqrt{11} < 4$.
$3.3^2 = 10.89$, $3.32^2 = 11.0224$. So $3.31 < \sqrt{11} < 3.32$.
$6 \times 3.31 = 19.86$. $6 \times 3.32 = 19.92$.
So $19.86 < 6\sqrt{11} < 19.92$.
Then $20 - 19.92 < B < 20 - 19.86$, which means $0.08 < B < 0.14$.
Since $0 < B < 1$, we have $0 < B^n < 1$ for all $n \ge 1$.

We have $A^n = S_n - B^n$.
Since $S_n$ is an integer and $0 < B^n < 1$, we have $S_n - 1 < A^n < S_n$.
$A^n = (\sqrt{11}+3)^{2n}$ is irrational for $n \ge 1$, since $A^n = u_n + v_n \sqrt{11}$ and $v_n \ne 0$.
Therefore, $A^n$ is not an integer.
The ceiling function $\lceil A^n \rceil$ is the smallest integer greater than or equal to $A^n$.
Since $S_n - 1 < A^n < S_n$, the smallest integer greater than or equal to $A^n$ is $S_n$.
So, $\lceil A^n \rceil = \lceil (\sqrt{11}+3)^{2n} \rceil = S_n$.

The problem now reduces to proving that $S_n$ is divisible by $2^{n+1}$ for $n \ge 1$.
We will use induction on $n$. Let $P(n)$ be the statement "$S_n$ is divisible by $2^{n+1}$".

Base cases:
For $n=1$: $S_1 = 40$. We need to check if $S_1$ is divisible by $2^{1+1} = 2^2 = 4$. $40 = 4 \times 10$. So $P(1)$ is true.
For $n=2$: $S_2 = 1592$. We need to check if $S_2$ is divisible by $2^{2+1} = 2^3 = 8$. $1592 = 8 \times 199$. So $P(2)$ is true.

Inductive hypothesis: Assume $P(k)$ and $P(k+1)$ are true for some integer $k \ge 1$.
That is, assume $S_k$ is divisible by $2^{k+1}$ and $S_{k+1}$ is divisible by $2^{k+2}$.
So, $S_k = p \cdot 2^{k+1}$ for some integer $p$, and $S_{k+1} = m \cdot 2^{k+2}$ for some integer $m$.

Inductive step: We want to show $P(k+2)$ is true, i.e., $S_{k+2}$ is divisible by $2^{k+3}$.
We use the recurrence relation $S_{k+2} = 40 S_{k+1} - 4 S_k$.
Substitute the expressions for $S_k$ and $S_{k+1}$ from the inductive hypothesis:
$S_{k+2} = 40 (m \cdot 2^{k+2}) - 4 (p \cdot 2^{k+1})$
$S_{k+2} = (5 \times 2^3) (m \cdot 2^{k+2}) - 2^2 (p \cdot 2^{k+1})$
$S_{k+2} = 5m \cdot 2^{k+5} - p \cdot 2^{k+3}$
Factor out $2^{k+3}$:
$S_{k+2} = 5m \cdot 2^2 \cdot 2^{k+3} - p \cdot 2^{k+3}$
$S_{k+2} = (20m) \cdot 2^{k+3} - p \cdot 2^{k+3}$
$S_{k+2} = (20m - p) \cdot 2^{k+3}$.

Since $m$ and $p$ are integers, $20m - p$ is an integer.
Therefore, $S_{k+2}$ is divisible by $2^{k+3}$. This proves $P(k+2)$.

By the principle of strong induction, the statement $P(n)$ is true for all integers $n \ge 1$.
Thus, $S_n$ is divisible by $2^{n+1}$ for all $n \ge 1$.

Since we established that $\lceil (\sqrt{11}+3)^{2n} \rceil = S_n$, we conclude that $\lceil (\sqrt{11}+3)^{2n} \rceil$ is divisible by $2^{n+1}$ for all $n \ge 1$.

Final Answer: The final answer is $\boxed{\lceil (\sqrt {11}+3)^{2n}\rceil \text{ is divisible by } 2^{n+1} \text{ for any } n\geq 1}$