Solution:
Let $X_i = (R_i, S_i, T_i)$ be the sequence of independent random variables. Each $X_i$ is uniformly distributed on the set of permutations of $(1, 2, 3)$. Let this set be $S_3$. $|S_3| = 3! = 6$. The possible values for $X_i$ are $(1,2,3), (1,3,2), (2,1,3), (2,3,1), (3,1,2), (3,2,1)$. Each value has probability $1/6$.
Note that $R_i+S_i+T_i = 1+2+3 = 6$ for all $i$.
Let $\hat X_n = (\hat R_n, \hat S_n, \hat T_n) = \sum_{i=1}^n X_i = (\sum R_i, \sum S_i, \sum T_i)$.
The sum of the components of $\hat X_n$ is $\hat R_n + \hat S_n + \hat T_n = \sum_{i=1}^n (R_i+S_i+T_i) = \sum_{i=1}^n 6 = 6n$.

We are given $p_n = P(\hat R_n = \hat S_n = \hat T_n)$. If $\hat R_n = \hat S_n = \hat T_n$, then $3 \hat R_n = 6n$, which implies $\hat R_n = 2n$. So $p_n = P(\hat R_n = 2n, \hat S_n = 2n, \hat T_n = 2n)$.

We are given $q_n = P(\hat R_n, \hat S_n, \hat T_n \in \{2n-1, 2n, 2n+1\}, \hat R_n \neq \hat S_n)$.
Let $E_n$ be the event that $\hat R_n, \hat S_n, \hat T_n \in \{2n-1, 2n, 2n+1\}$. Let the state be $(r, s, t)$. We must have $r, s, t \in \{2n-1, 2n, 2n+1\}$ and $r+s+t=6n$.
Let $r=2n+a, s=2n+b, t=2n+c$ where $a,b,c \in \{-1, 0, 1\}$. Then $(2n+a)+(2n+b)+(2n+c) = 6n + (a+b+c)$. So we must have $a+b+c=0$.
The possible combinations for $(a,b,c)$ are:
1. $(0,0,0)$: This corresponds to $(r,s,t) = (2n, 2n, 2n)$. In this case $\hat R_n = \hat S_n = 2n$. This outcome is excluded by the condition $\hat R_n \neq \hat S_n$.
2. Permutations of $(1, -1, 0)$: This corresponds to $(r,s,t)$ being a permutation of $(2n+1, 2n-1, 2n)$. There are $3! = 6$ such permutations. For any permutation $\sigma$ of $(2n+1, 2n-1, 2n)$, the components are distinct. In particular, $\hat R_n \neq \hat S_n$.
Therefore, the event defining $q_n$ is precisely the event that $(\hat R_n, \hat S_n, \hat T_n)$ is a permutation of $(2n+1, 2n-1, 2n)$.
$q_n = P(\{(\hat R_n, \hat S_n, \hat T_n) \text{ is a permutation of } (2n+1, 2n-1, 2n)\})$.

Let $Y_i = X_i - (2,2,2) = (R_i-2, S_i-2, T_i-2)$. Let $Y_i = (U_i, V_i, W_i)$. The possible values for $Y_i$ are the permutations of $(-1, 0, 1)$, each with probability $1/6$.
The values are: $(-1,0,1), (-1,1,0), (0,-1,1), (0,1,-1), (1,-1,0), (1,0,-1)$.
Note that $U_i+V_i+W_i = (R_i-2)+(S_i-2)+(T_i-2) = (R_i+S_i+T_i) - 6 = 6-6=0$.
Let $\hat Y_n = \sum_{i=1}^n Y_i = (\sum U_i, \sum V_i, \sum W_i) = (\hat R_n-2n, \hat S_n-2n, \hat T_n-2n)$. Let $\hat Y_n = (U_n, V_n, W_n)$.
Then $p_n = P(U_n=0, V_n=0, W_n=0)$. Since $W_n = -U_n-V_n$, this is $p_n = P(U_n=0, V_n=0)$.
And $q_n = P(\{(U_n, V_n, W_n) \text{ is a permutation of } (1, -1, 0)\})$. The possible states are $(1,-1,0), (1,0,-1), (-1,1,0), (0,1,-1), (-1,0,1), (0,-1,1)$.

The random vector $\hat Y_n$ is a sum of i.i.d. random vectors $Y_i$ with $E[Y_i] = (0,0,0)$. The vectors $Y_i$ lie in the plane $u+v+w=0$. This is a 2-dimensional lattice $L = \{(u,v,w) \in \mathbb{Z}^3 : u+v+w=0\}$.
We can choose a basis for this lattice, for example $e_1 = (1,-1,0)$ and $e_2 = (0,1,-1)$. Any vector $y \in L$ can be written as $y = k_1 e_1 + k_2 e_2 = (k_1, -k_1+k_2, -k_2)$ for unique integers $k_1, k_2$.
Let $Y_i = K_{i1} e_1 + K_{i2} e_2$. Let $Z'_i = (K_{i1}, K_{i2})$. The possible values for $Z'_i$ corresponding to the 6 values of $Y_i$ are:
$(-1,0,1) \rightarrow (-1,-1)$
$(-1,1,0) \rightarrow (-1,0)$
$(0,-1,1) \rightarrow (0,-1)$
$(0,1,-1) \rightarrow (0,1)$
$(1,-1,0) \rightarrow (1,0)$
$(1,0,-1) \rightarrow (1,1)$
Each vector $z'_k$ occurs with probability $1/6$. Let $S' = \{(-1,-1), (-1,0), (0,-1), (0,1), (1,0), (1,1)\}$.
Let $\hat Z'_n = \sum_{i=1}^n Z'_i = (K_n, L_n)$. This is a 2D random walk on $\mathbb{Z}^2$.
$E[Z'_i] = (1/6) \sum_{z' \in S'} z' = (1/6) ((-1)+(-1)+0+0+1+1, (-1)+0+(-1)+1+0+1) = (0,0)$.
The covariance matrix $\Sigma' = E[Z'_i (Z'_i)^T]$ is:
$E[K_{i1}^2] = (1/6) ((-1)^2+(-1)^2+0^2+0^2+1^2+1^2) = 4/6 = 2/3$.
$E[K_{i2}^2] = (1/6) ((-1)^2+0^2+(-1)^2+1^2+0^2+1^2) = 4/6 = 2/3$.
$E[K_{i1}K_{i2}] = (1/6) ((-1)(-1)+(-1)(0)+0(-1)+0(1)+1(0)+1(1)) = (1/6)(1+0+0+0+0+1) = 2/6 = 1/3$.
$\Sigma' = \begin{pmatrix} 2/3 & 1/3 \\ 1/3 & 2/3 \end{pmatrix}$.
$\det(\Sigma') = (2/3)(2/3) - (1/3)(1/3) = 4/9 - 1/9 = 3/9 = 1/3$. Since $\det(\Sigma') \neq 0$, the covariance matrix is non-singular.
The random walk $\hat Z'_n$ takes place on the lattice $\mathbb{Z}^2$. The possible steps are $S'$. The lattice generated by $S'$ is $\mathbb{Z}^2$. The greatest common divisor of the step lengths is 1 (viewed in $\mathbb{Z}^2$). The walk is aperiodic because steps with odd and even coordinate sums exist (e.g., $(-1,0)$ sum is $-1$, $(-1,-1)$ sum is $-2$).
The conditions for the Local Central Limit Theorem (LCLT) for lattice random walks are satisfied. For $x' \in \mathbb{Z}^2$, as $n \to \infty$:
$P(\hat Z'_n = x') = \frac{1}{2\pi n \sqrt{\det \Sigma'}} \exp\left(-\frac{1}{2n} x'^T (\Sigma')^{-1} x'\right) (1 + o(1))$.
Here $d=2$ and $\det \Sigma' = 1/3$.
$p_n = P(\hat Z'_n = (0,0))$. For $x'=(0,0)$, the quadratic form $Q(x') = x'^T (\Sigma')^{-1} x'$ is $Q(0)=0$.
$p_n = \frac{1}{2\pi n \sqrt{1/3}} e^0 (1+o(1)) = \frac{\sqrt{3}}{2\pi n} (1+o(1))$.
$q_n = P(\hat Y_n \in \text{Permutations of } (1,-1,0))$. This corresponds to $\hat Z'_n \in S'$.
$q_n = \sum_{x' \in S'} P(\hat Z'_n = x')$.
Let's compute $Q(x')$ for $x' \in S'$.
$(\Sigma')^{-1} = \frac{1}{1/3} \begin{pmatrix} 2/3 & -1/3 \\ -1/3 & 2/3 \end{pmatrix} = 3 \begin{pmatrix} 2/3 & -1/3 \\ -1/3 & 2/3 \end{pmatrix} = \begin{pmatrix} 2 & -1 \\ -1 & 2 \end{pmatrix}$.
For $x'=(1,0)$: $Q((1,0)) = (1,0) \begin{pmatrix} 2 & -1 \\ -1 & 2 \end{pmatrix} \begin{pmatrix} 1 \\ 0 \end{pmatrix} = (1,0) \begin{pmatrix} 2 \\ -1 \end{pmatrix} = 2$.
For $x'=(0,1)$: $Q((0,1)) = (0,1) \begin{pmatrix} 2 & -1 \\ -1 & 2 \end{pmatrix} \begin{pmatrix} 0 \\ 1 \end{pmatrix} = (0,1) \begin{pmatrix} -1 \\ 2 \end{pmatrix} = 2$.
For $x'=(1,1)$: $Q((1,1)) = (1,1) \begin{pmatrix} 2 & -1 \\ -1 & 2 \end{pmatrix} \begin{pmatrix} 1 \\ 1 \end{pmatrix} = (1,1) \begin{pmatrix} 1 \\ 1 \end{pmatrix} = 2$.
For $x'=(-1,0)$: $Q((-1,0)) = (-1,0) \begin{pmatrix} 2 & -1 \\ -1 & 2 \end{pmatrix} \begin{pmatrix} -1 \\ 0 \end{pmatrix} = (-1,0) \begin{pmatrix} -2 \\ 1 \end{pmatrix} = 2$.
For $x'=(0,-1)$: $Q((0,-1)) = (0,-1) \begin{pmatrix} 2 & -1 \\ -1 & 2 \end{pmatrix} \begin{pmatrix} 0 \\ -1 \end{pmatrix} = (0,-1) \begin{pmatrix} 1 \\ -2 \end{pmatrix} = 2$.
For $x'=(-1,-1)$: $Q((-1,-1)) = (-1,-1) \begin{pmatrix} 2 & -1 \\ -1 & 2 \end{pmatrix} \begin{pmatrix} -1 \\ -1 \end{pmatrix} = (-1,-1) \begin{pmatrix} -1 \\ -1 \end{pmatrix} = 2$.
So $Q(x')=2$ for all $x' \in S'$.
The LCLT gives, for any $x' \in S'$:
$P(\hat Z'_n = x') = \frac{1}{2\pi n \sqrt{1/3}} e^{-2/(2n)} (1+o(1)) = \frac{\sqrt{3}}{2\pi n} e^{-1/n} (1+o(1))$.
$q_n = \sum_{x' \in S'} P(\hat Z'_n = x') = 6 \times \frac{\sqrt{3}}{2\pi n} e^{-1/n} (1+o(1))$.

We want to show that $4p_n < q_n$ for infinitely many $n$. Let's examine the ratio $q_n / p_n$:
$$ \frac{q_n}{p_n} = \frac{6 \frac{\sqrt{3}}{2\pi n} e^{-1/n} (1+o(1))}{\frac{\sqrt{3}}{2\pi n} (1+o(1))} = 6 e^{-1/n} \frac{1+o(1)}{1+o(1)} $$
As $n \to \infty$, $e^{-1/n} \to e^0 = 1$. The term $\frac{1+o(1)}{1+o(1)} \to 1$.
Therefore, $\lim_{n \to \infty} \frac{q_n}{p_n} = 6$.
Since the limit is 6, for any $\epsilon > 0$, there exists $N$ such that for all $n \ge N$, $|q_n/p_n - 6| < \epsilon$.
Choose $\epsilon = 1$. Then for $n \ge N$, $q_n/p_n > 6 - 1 = 5$.
Since $5 > 4$, we have $q_n/p_n > 4$ for all $n \ge N$.
This means $q_n > 4p_n$ for all sufficiently large $n$.
The condition "for sufficiently large $n$" implies that the inequality holds for infinitely many $n$.

Final check: The LCLT approximation is valid for large $n$. The calculation implies that the inequality $4p_n < q_n$ holds for all $n$ greater than some $N_0$. This is a stronger result than needed, but it implies the desired conclusion. Explicit calculations showed the inequality holds for $n=1, 3$ but fails for $n=2$, confirming that it may not hold for small $n$.

Thus, based on the Local Central Limit Theorem, we have shown that $q_n/p_n \to 6$ as $n \to \infty$. Since $6 > 4$, it follows that $q_n > 4p_n$ for all sufficiently large $n$, which implies that $4p_n < q_n$ holds for infinitely many $n$.

```markdown
Solution:
Let $X_i = (R_i, S_i, T_i)$ be the sequence of independent random variables, where each $X_i$ is uniformly distributed on the set $S_3$ of permutations of $(1, 2, 3)$. The size of $S_3$ is $3! = 6$. For any $i$, $R_i+S_i+T_i = 1+2+3 = 6$.
Let $\hat X_n = (\hat R_n, \hat S_n, \hat T_n) = \sum_{i=1}^n X_i$. The sum of the components is $\hat R_n + \hat S_n + \hat T_n = \sum_{i=1}^n (R_i+S_i+T_i) = 6n$.

We are given $p_n = P(\hat R_n = \hat S_n = \hat T_n)$. The condition $\hat R_n = \hat S_n = \hat T_n$ implies $3\hat R_n = 6n$, so $\hat R_n = 2n$. Thus, $p_n = P(\hat R_n = 2n, \hat S_n = 2n, \hat T_n = 2n)$.

We are given $q_n = P(\hat R_n, \hat S_n, \hat T_n \in \{2n-1, 2n, 2n+1\}, \hat R_n \neq \hat S_n)$. Let the state be $(r, s, t)$. The condition implies $r, s, t \in \{2n-1, 2n, 2n+1\}$ and $r+s+t=6n$. Let $r=2n+a, s=2n+b, t=2n+c$ where $a,b,c \in \{-1, 0, 1\}$. The sum condition $r+s+t=6n$ implies $a+b+c=0$. The possible values for $(a,b,c)$ are $(0,0,0)$ and permutations of $(1,-1,0)$.
The case $(a,b,c)=(0,0,0)$ corresponds to $(r,s,t)=(2n,2n,2n)$. In this case $\hat R_n = \hat S_n = 2n$, which violates the condition $\hat R_n \neq \hat S_n$.
The permutations of $(1,-1,0)$ correspond to $(r,s,t)$ being a permutation of $(2n+1, 2n-1, 2n)$. In this case, the components $r,s,t$ are distinct values $2n+1, 2n-1, 2n$. In particular, $\hat R_n \neq \hat S_n$ is always satisfied.
So, $q_n = P(\{(\hat R_n, \hat S_n, \hat T_n) \text{ is a permutation of } (2n+1, 2n-1, 2n)\})$.

Let $Y_i = X_i - (2,2,2) = (R_i-2, S_i-2, T_i-2)$. Let $Y_i = (U_i, V_i, W_i)$. The possible values for $Y_i$ are the 6 permutations of $(-1, 0, 1)$, each with probability $1/6$. Note that $U_i+V_i+W_i = 0$.
Let $\hat Y_n = \sum_{i=1}^n Y_i = (U_n, V_n, W_n) = (\hat R_n-2n, \hat S_n-2n, \hat T_n-2n)$.
Then $p_n = P(U_n=0, V_n=0, W_n=0)$. Since $W_n = -U_n-V_n$, this is $p_n = P(U_n=0, V_n=0)$.
And $q_n = P(\{(U_n, V_n, W_n) \text{ is a permutation of } (1, -1, 0)\})$.

The vector $\hat Y_n$ represents a random walk on the 2-dimensional lattice $L = \{(u,v,w) \in \mathbb{Z}^3 : u+v+w=0\}$. We choose a basis for $L$, e.g., $e_1=(1,-1,0)$ and $e_2=(0,1,-1)$. Any $y \in L$ can be written as $y = k_1 e_1 + k_2 e_2 = (k_1, -k_1+k_2, -k_2)$ for $k_1, k_2 \in \mathbb{Z}$.
Let $Y_i = K_{i1} e_1 + K_{i2} e_2$, and let $Z'_i = (K_{i1}, K_{i2})$. $\hat Z'_n = \sum_{i=1}^n Z'_i = (K_n, L_n)$. This is a 2D random walk on $\mathbb{Z}^2$. The possible steps $Z'_i$ are $S' = \{(-1,-1), (-1,0), (0,-1), (0,1), (1,0), (1,1)\}$, each with probability $1/6$.
$E[Z'_i] = (0,0)$. The covariance matrix is $\Sigma' = E[Z'_i (Z'_i)^T] = \begin{pmatrix} 2/3 & 1/3 \\ 1/3 & 2/3 \end{pmatrix}$. The determinant is $\det(\Sigma') = 1/3$.
The random walk $\hat Z'_n$ is a sum of i.i.d. random variables on $\mathbb{Z}^2$ with mean 0 and non-singular covariance matrix $\Sigma'$. The walk is aperiodic as the lattice generated is $\mathbb{Z}^2$ and the steps don't confine the walk to a coset of a proper sublattice.
The Local Central Limit Theorem (LCLT) applies. For $x' \in \mathbb{Z}^2$, as $n \to \infty$:
$$ P(\hat Z'_n = x') = \frac{1}{(2\pi n)^{2/2} \sqrt{\det \Sigma'}} \exp\left(-\frac{1}{2n} x'^T (\Sigma')^{-1} x'\right) (1 + o(1)) $$
$p_n = P(\hat Z'_n = (0,0))$. The inverse covariance matrix is $(\Sigma')^{-1} = \begin{pmatrix} 2 & -1 \\ -1 & 2 \end{pmatrix}$. The quadratic form $Q(x') = x'^T (\Sigma')^{-1} x'$ is $Q(0)=0$.
$$ p_n = \frac{1}{2\pi n \sqrt{1/3}} e^0 (1+o(1)) = \frac{\sqrt{3}}{2\pi n} (1+o(1)) $$
$q_n = P(\hat Z'_n \in S')$. We calculated $Q(x')=2$ for all $x' \in S'$.
For any $x' \in S'$,
$$ P(\hat Z'_n = x') = \frac{1}{2\pi n \sqrt{1/3}} e^{-2/(2n)} (1+o(1)) = \frac{\sqrt{3}}{2\pi n} e^{-1/n} (1+o(1)) $$
Since this value is the same for all $x' \in S'$, we have
$$ q_n = \sum_{x' \in S'} P(\hat Z'_n = x') = 6 \times \frac{\sqrt{3}}{2\pi n} e^{-1/n} (1+o(1)) $$
Now we examine the ratio $q_n / p_n$ for large $n$:
$$ \frac{q_n}{p_n} = \frac{6 \frac{\sqrt{3}}{2\pi n} e^{-1/n} (1+o(1))}{\frac{\sqrt{3}}{2\pi n} (1+o(1))} = 6 e^{-1/n} \frac{1+o(1)}{1+o(1)} $$
As $n \to \infty$, $e^{-1/n} \to 1$ and $\frac{1+o(1)}{1+o(1)} \to 1$.
$$ \lim_{n \to \infty} \frac{q_n}{p_n} = 6 $$
Since the limit is 6, for any constant $C < 6$, there exists an integer $N$ such that for all $n \ge N$, $q_n/p_n > C$.
Let $C=4$. Since $4 < 6$, there exists $N$ such that for all $n \ge N$, $q_n/p_n > 4$.
This means $q_n > 4p_n$ for all sufficiently large $n$.
Therefore, the inequality $4p_n < q_n$ holds for infinitely many $n$.

```