# Solution

Let's analyze the problem by examining the condition that $\frac{f(x)}{x^n}$ is increasing on $(0,1)$ for all $n \geq 0$, and determine if this implies that all derivatives of $f$ are non-negative.

## Step 1: Express the condition mathematically

For $\frac{f(x)}{x^n}$ to be increasing, its derivative must be non-negative:

$$\frac{d}{dx}\left(\frac{f(x)}{x^n}\right) \geq 0$$

Using the quotient rule, we get:

$$\frac{f'(x)x^n - nx^{n-1}f(x)}{x^{2n}} \geq 0$$

Since $x > 0$ for $x \in (0,1)$, this simplifies to:

$$f'(x) - n\frac{f(x)}{x} \geq 0$$

Or equivalently:

$$f'(x) \geq n\frac{f(x)}{x}$$

This inequality must hold for all $n \geq 0$ and all $x \in (0,1)$.

## Step 2: Show that $f(x) \geq 0$ for all $x \in (0,1)$

For $n = 0$, we have $f'(x) \geq 0$, meaning $f$ is non-decreasing on $(0,1)$.

Suppose there exists $x_0 \in (0,1)$ such that $f(x_0) < 0$. Since $f$ is non-decreasing, we would have $f(x) \leq f(x_0) < 0$ for all $x \in (0,x_0]$.

However, for any such negative value of $f(x)$, the inequality $f'(x) \geq n\frac{f(x)}{x}$ would be violated for sufficiently large $n$, since:
- $f(x) < 0$
- $x > 0$
- $f'(x) \geq 0$

The right side $n\frac{f(x)}{x}$ would become arbitrarily negative as $n$ increases, contradicting $f'(x) \geq 0$.

Therefore, $f(x) \geq 0$ for all $x \in (0,1)$.

## Step 3: Prove by induction that $f^{(m)}(x) \geq 0$ for all $m \geq 0$

Base cases:
- $m = 0$: We've shown $f(x) \geq 0$.
- $m = 1$: We have $f'(x) \geq 0$ from the $n = 0$ case.

Inductive hypothesis: Assume $f^{(k)}(x) \geq 0$ for all $k \leq m$.

We will prove by induction the following stronger statement:

$$f^{(m)}(x) \geq \frac{n(n-1)(n-2)\cdots(n-m+1)f(x)}{x^m}$$

for all $n \geq m-1$ and $x \in (0,1)$.

For $m = 1$, this is precisely our original inequality $f'(x) \geq n\frac{f(x)}{x}$.

Assuming the statement holds for $m$, differentiate both sides with respect to $x$:

$$f^{(m+1)}(x) \geq \frac{d}{dx}\left[\frac{n(n-1)\cdots(n-m+1)f(x)}{x^m}\right]$$

Computing the derivative on the right side and using our original inequality for $f'(x)$, we get:

$$f^{(m+1)}(x) \geq \frac{n(n-1)\cdots(n-m+1)(n-m)f(x)}{x^{m+1}}$$

For $n \geq m$, the coefficient $n(n-1)\cdots(n-m+1)(n-m)$ is non-negative. Since $f(x) \geq 0$ and $x > 0$, we have $f^{(m+1)}(x) \geq 0$.

Since our original condition holds for all $n \geq 0$, we can always choose $n$ large enough to ensure that $f^{(m)}(x) \geq 0$ for any $m$.

## Conclusion

Yes, it is true that $f^{(n)}(x) \geq 0$ for every $n \geq 0$ and all $x \in (0,1)$.