# Solution

I'll find all real polynomials $P$ that satisfy the functional equation $x P(x-2) = (x-2024)P(x)$ for all $x \in \mathbb{R}$.

## First approach: Finding the roots

Let's examine what happens when we substitute specific values of $x$ into the equation.

When $x = 0$:
$$0 \cdot P(-2) = (0-2024)P(0)$$
$$0 = -2024 \cdot P(0)$$

Since $-2024 \neq 0$, we must have $P(0) = 0$.

When $x = 2$:
$$2 \cdot P(0) = (2-2024)P(2)$$
$$2 \cdot 0 = -2022 \cdot P(2)$$

This implies $P(2) = 0$.

When $x = 4$:
$$4 \cdot P(2) = (4-2024)P(4)$$
$$4 \cdot 0 = -2020 \cdot P(4)$$

This implies $P(4) = 0$.

I notice a pattern forming. Let's continue this reasoning for $x = 2k$ where $k$ is a non-negative integer:

$$2k \cdot P(2k-2) = (2k-2024)P(2k)$$

If $P(2k-2) = 0$, then $P(2k) = 0$ as well (assuming $2k \neq 2024$, which is true for $k < 1012$).

Since we already established $P(0) = P(2) = P(4) = 0$, by induction $P(2k) = 0$ for all integers $k$ with $0 \leq k \leq 1011$.

Therefore, $P(x)$ must be divisible by $x(x-2)(x-4)\cdots(x-2022)$.

## Second approach: Finding the general solution

Let's define $P(x) = x \cdot Q(x)$ since we know $P(0) = 0$. Substituting into our functional equation:

$$x(x-2)Q(x-2) = (x-2024)xQ(x)$$

For $x \neq 0$, we can simplify:
$$(x-2)Q(x-2) = (x-2024)Q(x)$$

This is the same form as our original equation but for $Q$. By the same reasoning, $Q(0) = 0$, so $Q(x) = x \cdot R(x)$ for some polynomial $R$.

Continuing this process, we find that:
$$P(x) = x(x-2)(x-4)\cdots(x-2022) \cdot S(x)$$

for some polynomial $S$. Substituting back into the functional equation:

$$x(x-2)(x-4)\cdots(x-2024) \cdot S(x-2) = (x-2024)x(x-2)(x-4)\cdots(x-2022) \cdot S(x)$$

Simplifying:
$$(x-2024) \cdot S(x-2) = (x-2024) \cdot S(x)$$

For $x \neq 2024$, we get:
$$S(x-2) = S(x)$$

This means $S$ is periodic with period 2. Since the only polynomial that is periodic is a constant polynomial, $S(x) = c$ for some constant $c$.

## Conclusion

The general solution to the functional equation $x P(x-2) = (x-2024)P(x)$ is:

$$P(x) = c \cdot \prod_{i=0}^{1011} (x-2i) = c \cdot x(x-2)(x-4)\cdots(x-2022)$$

where $c$ is any real constant.

This is a polynomial of degree 1012.