Of course. Here is a detailed, step-by-step solution to the problem.

### The Problem

Let $a_1,\ldots,a_n$, $b_1,\ldots,b_n$ and $c_1,\ldots, c_n$ be nonnegative real numbers. Show that
$$
\left(\prod_{i=1}^n a_i\right)^\frac 1n+\left(\prod_{i=1}^n b_i\right)^\frac 1n+\left(\prod_{i=1}^n c_i\right)^\frac 1n\leq \left(\prod_{i=1}^n (a_i+b_i+c_i)\right)^\frac 1n.
$$

### Solution

This inequality relates the sum of geometric means of three sequences to the geometric mean of their term-wise sum. We will prove this by first handling a trivial case and then transforming the inequality into a simpler form, which can then be proven using the AM-GM inequality.

**Step 1: Handle the trivial case.**

Let's consider the case where the right-hand side (RHS) of the inequality is zero.
$$
\left(\prod_{i=1}^n (a_i+b_i+c_i)\right)^\frac 1n = 0
$$
Since the product of non-negative numbers is zero if and only if at least one of the numbers is zero, there must exist some index $k \in \{1, 2, \ldots, n\}$ such that $a_k+b_k+c_k=0$.
Given that $a_k, b_k, c_k$ are all non-negative, their sum can only be zero if each term is zero. Thus, for this index $k$, we must have $a_k=0$, $b_k=0$, and $c_k=0$.

If $a_k=0$ for some $k$, then the product $\prod_{i=1}^n a_i = 0$, which implies $\left(\prod_{i=1}^n a_i\right)^\frac 1n = 0$.
Similarly, since $b_k=0$ and $c_k=0$, we have $\left(\prod_{i=1}^n b_i\right)^\frac 1n = 0$ and $\left(\prod_{i=1}^n c_i\right)^\frac 1n = 0$.

In this case, the left-hand side (LHS) of the inequality becomes $0+0+0=0$.
The inequality is $0 \leq 0$, which is true. So, the inequality holds if the RHS is zero.

**Step 2: Normalize the inequality.**

Now, let's assume the RHS is strictly positive:
$$
\left(\prod_{i=1}^n (a_i+b_i+c_i)\right)^\frac 1n > 0
$$
This implies that for all $i \in \{1, 2, \ldots, n\}$, we have $a_i+b_i+c_i > 0$.

Let $S = \left(\prod_{i=1}^n (a_i+b_i+c_i)\right)^\frac 1n$. We can divide both sides of the inequality by $S$ (since $S>0$). The inequality we want to prove is equivalent to:
$$
\frac{\left(\prod_{i=1}^n a_i\right)^\frac 1n}{S} + \frac{\left(\prod_{i=1}^n b_i\right)^\frac 1n}{S} + \frac{\left(\prod_{i=1}^n c_i\right)^\frac 1n}{S} \leq 1
$$
Substituting the expression for $S$:
$$
\frac{\left(\prod_{i=1}^n a_i\right)^\frac 1n}{\left(\prod_{i=1}^n (a_i+b_i+c_i)\right)^\frac 1n} + \frac{\left(\prod_{i=1}^n b_i\right)^\frac 1n}{\left(\prod_{i=1}^n (a_i+b_i+c_i)\right)^\frac 1n} + \frac{\left(\prod_{i=1}^n c_i\right)^\frac 1n}{\left(\prod_{i=1}^n (a_i+b_i+c_i)\right)^\frac 1n} \leq 1
$$
Using the property $(x/y)^{1/n} = x^{1/n}/y^{1/n}$, we can rewrite the LHS:
$$
\left(\prod_{i=1}^n \frac{a_i}{a_i+b_i+c_i}\right)^\frac 1n + \left(\prod_{i=1}^n \frac{b_i}{a_i+b_i+c_i}\right)^\frac 1n + \left(\prod_{i=1}^n \frac{c_i}{a_i+b_i+c_i}\right)^\frac 1n \leq 1
$$

**Step 3: Introduce new variables to simplify the expression.**

To make the expression clearer, let's define three new sequences of variables $x_i, y_i, z_i$ for $i=1, \ldots, n$:
$$
x_i = \frac{a_i}{a_i+b_i+c_i}, \quad y_i = \frac{b_i}{a_i+b_i+c_i}, \quad z_i = \frac{c_i}{a_i+b_i+c_i}
$$
Since $a_i, b_i, c_i$ are non-negative and $a_i+b_i+c_i > 0$, these new variables are also non-negative: $x_i, y_i, z_i \ge 0$.
Furthermore, for each $i$, they sum to 1:
$$
x_i+y_i+z_i = \frac{a_i}{a_i+b_i+c_i} + \frac{b_i}{a_i+b_i+c_i} + \frac{c_i}{a_i+b_i+c_i} = \frac{a_i+b_i+c_i}{a_i+b_i+c_i} = 1
$$
In terms of these new variables, the inequality we need to prove becomes:
$$
\left(\prod_{i=1}^n x_i\right)^\frac 1n + \left(\prod_{i=1}^n y_i\right)^\frac 1n + \left(\prod_{i=1}^n z_i\right)^\frac 1n \leq 1
$$

**Step 4: Apply the Arithmetic Mean - Geometric Mean (AM-GM) Inequality.**

The expressions on the LHS are geometric means of the sequences $(x_i)$, $(y_i)$, and $(z_i)$. The AM-GM inequality states that for any set of non-negative real numbers, their geometric mean is less than or equal to their arithmetic mean.
For the sequence $x_1, \ldots, x_n$:
$$
\left(\prod_{i=1}^n x_i\right)^\frac 1n \leq \frac{1}{n}\sum_{i=1}^n x_i
$$
Similarly, for the sequences $y_1, \ldots, y_n$ and $z_1, \ldots, z_n$:
$$
\left(\prod_{i=1}^n y_i\right)^\frac 1n \leq \frac{1}{n}\sum_{i=1}^n y_i
$$
$$
\left(\prod_{i=1}^n z_i\right)^\frac 1n \leq \frac{1}{n}\sum_{i=1}^n z_i
$$

**Step 5: Combine the inequalities and conclude the proof.**

Let's denote the LHS of our transformed inequality by $L'$. By adding the three AM-GM inequalities from Step 4, we get an upper bound for $L'$:
$$
L' = \left(\prod_{i=1}^n x_i\right)^\frac 1n + \left(\prod_{i=1}^n y_i\right)^\frac 1n + \left(\prod_{i=1}^n z_i\right)^\frac 1n \leq \frac{1}{n}\sum_{i=1}^n x_i + \frac{1}{n}\sum_{i=1}^n y_i + \frac{1}{n}\sum_{i=1}^n z_i
$$
We can combine the sums on the right side:
$$
L' \leq \frac{1}{n} \left( \sum_{i=1}^n x_i + \sum_{i=1}^n y_i + \sum_{i=1}^n z_i \right) = \frac{1}{n} \sum_{i=1}^n (x_i + y_i + z_i)
$$
Now, we use the property of our normalized variables from Step 3, which is that $x_i+y_i+z_i = 1$ for all $i$.
$$
L' \leq \frac{1}{n} \sum_{i=1}^n (1) = \frac{1}{n} \cdot n = 1
$$
So, we have shown that
$$
\left(\prod_{i=1}^n x_i\right)^\frac 1n + \left(\prod_{i=1}^n y_i\right)^\frac 1n + \left(\prod_{i=1}^n z_i\right)^\frac 1n \leq 1
$$
This proves the normalized inequality. Since this inequality is equivalent to the original one (under the assumption that the RHS is not zero), the original inequality is also true.

**Conclusion**

We have shown the inequality holds in both the trivial case (RHS=0) and the main case (RHS>0). Therefore, for any non-negative real numbers $a_1,\ldots,a_n$, $b_1,\ldots,b_n$ and $c_1,\ldots, c_n$, the following inequality is true:
$$
\left(\prod_{i=1}^n a_i\right)^\frac 1n+\left(\prod_{i=1}^n b_i\right)^\frac 1n+\left(\prod_{i=1}^n c_i\right)^\frac 1n\leq \left(\prod_{i=1}^n (a_i+b_i+c_i)\right)^\frac 1n.
$$

**Condition for Equality**
Equality holds if and only if all the inequalities we used are equalities. The AM-GM inequality $\left(\prod x_i\right)^{1/n} \le \frac{1}{n}\sum x_i$ becomes an equality if and only if $x_1=x_2=\dots=x_n$.
For our proof, equality holds if:
1.  $x_1=x_2=\dots=x_n$
2.  $y_1=y_2=\dots=y_n$
3.  $z_1=z_2=\dots=z_n$

Recalling the definitions of $x_i, y_i, z_i$:
$$
\frac{a_1}{a_1+b_1+c_1} = \frac{a_2}{a_2+b_2+c_2} = \dots = \frac{a_n}{a_n+b_n+c_n}
$$
and similarly for the $b_i$ and $c_i$ sequences. This means that the ratio of $a_i$ to the sum $a_i+b_i+c_i$ is constant for all $i$. This is true if and only if the vectors $(a_i, b_i, c_i)$ are all proportional to a single vector $(A, B, C)$. That is, for each $i$, there exists a constant $\lambda_i \ge 0$ such that $(a_i, b_i, c_i) = \lambda_i (A, B, C)$ for some fixed non-negative constants $A, B, C$ not all zero.