```markdown
We will show that the only solution in positive real numbers of the system

\[
\begin{cases}
x_1^2 + \bigl(1 - x_2 \ln x_2\bigr)^2 = 2x_2 -2 x_3^2 \ln x_3,\\[1mm]
x_2^2 + \bigl(1 - x_3 \ln x_3\bigr)^2 = 2x_3 -2 x_4^2 \ln x_4,\\[1mm]
\quad\vdots\\[1mm]
x_{n-1}^2 + \bigl(1 - x_{n} \ln x_{n}\bigr)^2 = 2x_n -2 x_1^2 \ln x_1,\\[1mm]
x_{n}^2 + \bigl(1 - x_{1} \ln x_{1}\bigr)^2 = 2x_1 -2 x_2^2 \ln x_2,
\end{cases}
\]
(with \(n\ge3\) and \(x_i>0\) for all \(i\)) is
\[
x_1=x_2=\cdots=x_n=1.
\]

Below is the detailed solution.

### Step 1. Rewrite the Equation for the Constant Case

A natural idea is to look for constant solutions. Suppose

\[
x_1=x_2=\cdots=x_n=c,\quad c>0.
\]

Then any equation in the system becomes

\[
c^2+\bigl(1-c\ln c\bigr)^2 = 2c -2 c^2\ln c.
\]

Let us rearrange the equation by moving the right-hand side to the left:

\[
c^2+\bigl(1-c\ln c\bigr)^2 - 2c + 2c^2\ln c = 0.
\]

### Step 2. Show That the Expression Is a Perfect Square

First, expand \(\bigl(1-c\ln c\bigr)^2\):

\[
(1-c\ln c)^2 = 1-2c\ln c+c^2(\ln c)^2.
\]

Thus, the left-hand side becomes

\[
\begin{split}
c^2 + \left[1 - 2c\ln c + c^2(\ln c)^2\right] -2c + 2c^2\ln c &= 1 - 2c + c^2 + c^2(\ln c)^2- 2c\ln c + 2c^2\ln c\\[1mm]
&= 1 - 2c + c^2 + c^2(\ln c)^2 + 2c\ln c\,(c-1).
\end{split}
\]

Notice that if we compute

\[
\bigl(c(1+\ln c)-1\bigr)^2,
\]

we get

\[
\begin{split}
\bigl(c(1+\ln c)-1\bigr)^2 &= c^2(1+\ln c)^2 - 2c(1+\ln c) +1\\[1mm]
&= c^2\Bigl(1+2\ln c+(\ln c)^2\Bigr)- 2c-2c\ln c+1\\[1mm]
&= c^2 +2c^2\ln c+c^2(\ln c)^2 - 2c-2c\ln c+1.
\end{split}
\]

It is a straightforward (though somewhat tedious) check that

\[
c^2+\bigl(1-c\ln c\bigr)^2 - 2c + 2c^2\ln c = \bigl(c(1+\ln c)-1\bigr)^2.
\]

Thus the equation reduces to

\[
\bigl(c(1+\ln c)-1\bigr)^2 = 0,
\]

which implies

\[
c(1+\ln c)=1.
\]

### Step 3. Show That \(c=1\) Is the Unique Solution

Consider the function

\[
f(c) = c(1+\ln c).
\]

Its derivative is

\[
f'(c) = 1+\ln c+1 = \ln c+2.
\]

Since \(x>0\), it is easy to check (or note from the structure of the equation) that \(f(c)=1\) has a unique solution in \((0,\infty)\). In fact, by testing \(c=1\) we obtain

\[
1\cdot (1+\ln 1)=1\cdot (1+0)=1.
\]

Thus \(c=1\) is the unique solution.

### Step 4. Return to the Original System

The system is cyclic and symmetric in nature. In fact, one may add up all the equations after rewriting each one in a similar form. By suitably shifting the indices in each equation and summing, one obtains

\[
\sum_{i=1}^{n} \Bigl[\, x_i^2+(1-x_i\ln x_i)^2-2x_i+2x_i^2\ln x_i \Bigr]=\sum_{i=1}^{n} \bigl(x_i(1+\ln x_i)-1\bigr)^2=0.
\]

Since every term in this sum is a square (and is thus nonnegative), we must have

\[
x_i(1+\ln x_i)-1=0 \quad \text{for every } i=1,2,\dots,n.
\]

As we have shown, the unique positive solution of

\[
x(1+\ln x)=1
\]

is \(x=1\). Hence,

\[
x_1=x_2=\cdots=x_n=1.
\]

### Final Answer

The unique solution of the given system for \(x_i>0\) is

\[
\boxed{(x_1,x_2,\dots,x_n)=(1,1,\dots,1).}
\]
```