Solution:
Let $R$ be a finite ring with the properties:
1. For any $a,b\in R$ there is $c\in R$ such that $a^3+b^3=c^3$. Let $C = \{x^3 | x \in R\}$ be the set of cubes in $R$. This property means $C$ is closed under addition, i.e., $C+C \subseteq C$.
2. For any $a, b \in R$, if $a \neq b$, then $a^2 b = -b a^2$.

We want to prove that for any $a,b \in R$, there exists $d \in R$ such that $aba + bab = d^3$. This means we want to show $aba+bab \in C$.

First, let's derive some consequences of the second property.
Let $a \in R$. Consider the element $2a^3 = a^3+a^3$.
If $a=-a$, i.e., $2a=0$, then $2a^3 = (2a)a^2 = 0 \cdot a^2 = 0$.
If $a \neq -a$, i.e., $2a \neq 0$, then we can apply property 2 with $x=a$ and $y=-a$. Since $x \neq y$, we have $x^2 y = -y x^2$.
$a^2 (-a) = -(-a) a^2$.
This simplifies to $-a^3 = a a^2 = a^3$.
So $2a^3 = 0$.
Thus, $2x^3 = 0$ for all $x \in R$.

This implies that for any element $y \in C$, we have $2y=0$. Since $y \in C$, $y=x^3$ for some $x \in R$. Then $2y = 2x^3 = 0$.
This means that any element in the set of cubes $C$ has additive order at most 2. In particular, for any $y \in C$, $-y=y$.

Now, let's show that $0 \in C$. Let $a \in R$. By property 1, $a^3+a^3 = c^3$ for some $c \in R$.
$2a^3 = c^3$. Since we proved $2a^3=0$, we have $c^3=0$.
Thus, $0$ is a cube, so $0 \in C$.

We want to show that $aba+bab \in C$ for any $a,b \in R$. We consider two cases.

Case 1: $a=b$.
The expression becomes $aaa+aaa = a^3+a^3 = 2a^3$.
We have shown that $2a^3=0$ for all $a \in R$.
We have also shown that $0$ is a cube, i.e. $0 \in C$.
So $aba+bab = 2a^3 = 0 \in C$. The statement holds in this case.

Case 2: $a \neq b$.
Let's compute $(a+b)^3$.
$(a+b)^3 = (a+b)(a+b)(a+b) = (a^2+ab+ba+b^2)(a+b)$
$= a(a^2+ab+ba+b^2) + b(a^2+ab+ba+b^2)$
$= a^3 + a^2 b + aba + ab^2 + ba^2 + bab + b^2 a + b^3$.
Since $a \neq b$, we can use property 2: $a^2 b = -b a^2$ and $b^2 a = -a b^2$.
Substitute these into the expression for $(a+b)^3$:
$(a+b)^3 = a^3 + (-b a^2) + aba + ab^2 + ba^2 + bab + (-a b^2) + b^3$
$= a^3 - b a^2 + aba + ab^2 + ba^2 + bab - a b^2 + b^3$
Rearranging terms:
$(a+b)^3 = a^3 + b^3 + (aba + bab) + (ab^2 - ab^2) + (-ba^2 + ba^2)$
$(a+b)^3 = a^3 + b^3 + aba + bab$.

Let $X = aba+bab$. Then $(a+b)^3 = a^3+b^3+X$.
By property 1, there exists $c \in R$ such that $a^3+b^3=c^3$.
So, $(a+b)^3 = c^3 + X$.
This means $X = (a+b)^3 - c^3$.
We want to show that $X$ is a cube, i.e., $X \in C$.
Let $u = a+b$. Then $u^3 = (a+b)^3 \in C$. Also, $c^3 \in C$.
We know that for any element $y \in C$, $2y=0$, which implies $-y=y$.
Since $c^3 \in C$, we have $-c^3 = c^3$.
So $X = u^3 - c^3 = u^3 + (-c^3) = u^3 + c^3$.
We have $u^3 \in C$ and $c^3 \in C$.
Property 1 states that the sum of two cubes is a cube ($C+C \subseteq C$).
Therefore, $X = u^3+c^3$ must be in $C$.
So, $X = d^3$ for some $d \in R$.

Both cases lead to the conclusion that $aba+bab$ is a cube.

Thus, for any $a, b \in R$, there exists $d \in R$ such that $aba+bab = d^3$.

Final Answer: The final answer is $\boxed{For any $a,b\in R$ there is $d\in R$ such that $aba+bab=d^3$}$