

To solve the problem, we analyze the given ratio condition and utilize properties of smooth functions with bounded derivatives.

**Step 1:** Define \( S_n(x) = f(x) + f'(x) + \cdots + f^{(n)}(x) \). The given condition becomes:
\[
\frac{S_n(b_n)}{S_n(a_n)} = e^{b_n - a_n}.
\]
Rewriting, \( S_n(b_n)e^{-b_n} = S_n(a_n)e^{-a_n} \). Let \( T_n(x) = S_n(x)e^{-x} \), so \( T_n(b_n) = T_n(a_n) \).

**Step 2:** By Rolle's Theorem, there exists \( c_n \in (a_n, b_n) \) such that \( T_n'(c_n) = 0 \). Compute \( T_n'(x) \):
\[
T_n'(x) = e^{-x}\left(S_n'(x) - S_n(x)\right).
\]
Since \( S_n'(x) = S_{n+1}(x) - f(x) \), substituting gives:
\[
T_n'(x) = e^{-x}\left(S_{n+1}(x) - f(x) - S_n(x)\right) = e^{-x}\left(f^{(n+1)}(x) - f(x)\right).
\]
Setting \( T_n'(c_n) = 0 \) implies:
\[
f^{(n+1)}(c_n) = f(c_n),
\]
where \( c_n \to c \) as \( n \to \infty \).

**Step 3:** For large \( n \), \( c_{n} \) is close to \( c \). Consider \( f^{(n)}(c) \):
\[
f^{(n)}(c) = f^{(n)}(c_{n-1}) + (c - c_{n-1})f^{(n+1)}(\xi_n),
\]
for some \( \xi_n \) between \( c \) and \( c_{n-1} \). From Step 2, \( f^{(n)}(c_{n-1}) = f(c_{n-1}) \). Thus:
\[
|f^{(n)}(c) - f(c_{n-1})| \leq |c - c_{n-1}| \cdot |f^{(n+1)}(\xi_n)| \leq M|c - c_{n-1}|.
\]
As \( n \to \infty \), \( |c - c_{n-1}| \to 0 \), so:
\[
\lim_{n \to \infty} f^{(n)}(c) = \lim_{n \to \infty} f(c_{n-1}) = f(c).
\]

**Conclusion:** \( \lim_{n \to \infty} f^{(n)}(c) = f(c) \).

```markdown
\boxed{\lim_{n \to \infty} f^{(n)}(c) = f(c)}
```