This step is worth 3 points.
Using the binomial formula we find that
$$
\begin{aligned}
\int_0^1 \frac{(1-\ln(1-x))^n}{n!} \, dx &= \frac{1}{n!} \int_0^1 (1-\ln(1-x))^n \, dx = \frac{1}{n!} \int_0^1 \sum_{k=0}^n {n \choose k} \left( - \ln(1-x) \right)^k \, dx \\
&=  \frac{1}{n!}  \sum_{k=0}^n {n \choose k} \int_0^1 \left( - \ln(1-x) \right)^k \, dx =  \frac{1}{n!}  \sum_{k=0}^n {n \choose k} I_k,
\end{aligned}
$$
where
$$
I_k := \int_0^1 \left( - \ln(1-x) \right)^k \, dx.
$$

This step is worth 5 points.
We will compute $I_k$. First note that
$$
I_0 = \int_0^1 \, dx = 1.
$$
Now, let $k \geq 1$ and we integrate by parts
$$
\begin{aligned}
I_{k} &= \int_0^1 \left( - \ln(1-x) \right)^k \, dx = - \int_0^1 \left( - \ln(1-x) \right)^k \cdot (-1) \, dx \\
&= - \int_0^1 \left( - \ln(1-x) \right)^k \cdot (1-x)' \, dx \\
&= - (1-x) \left( - \ln (1-x) \right)^k \big|_0^1 + \int_0^1 k \left(-\ln (1-x)\right)^{k-1} \cdot \frac{1}{1-x} \cdot (1-x) \, dx \\
&= \lim_{x\to 1^-} \left( (1-x) \left( - \ln (1-x) \right)^k \right) + k \int_0^1 \left(-\ln (1-x)\right)^{k-1} \, dx = k I_{k-1}.
\end{aligned}
$$
Hence $I_k = k!$.

This step is worth 2 points.
It allows us to compute that
$$
\begin{aligned}
\lim_{n\to\infty} \int_0^1 \frac{(1-\ln(1-x))^n}{n!} \, dx &= \lim_{n\to\infty} \frac{1}{n!}  \sum_{k=0}^n {n \choose k} I_k = \lim_{n\to\infty} \frac{1}{n!}  \sum_{k=0}^n {n \choose k} k! \\
&= \lim_{n\to\infty} \sum_{k=0}^n \frac{1}{(n-k)!} = \lim_{n\to\infty} \sum_{k=0}^n \frac{1}{k!} = \sum_{k=0}^\infty \frac{1}{k!} = e.
\end{aligned}
$$
