Solution step (1 point)
We will use the following result:

 **Theorem (Van Dyck's Theorem).** Let $G$ be a group with the presentation $\langle x_1, \ldots, x_n; R \rangle$, where $R$ is a finite set of relations between the generators $x_1, \ldots, x_n$. If a group $G'$ and a set $\{y_1, \ldots, y_n\}$ of its generators have the property that for every relation $x_{i_1}^{a_1} \cdots x_{i_m}^{a_m} \in R$, the equality
$y_{i_1}^{a_1} \cdots y_{i_m}^{a_m} = e'$ holds in $G'$, then the group $G'$ is a homomorphic image of the group $G$.

Solution step (2 points)
From the relations defining the group $G$, it follows that the equalities $x^{-1} = x^{n-1}$, $y^{-1} = y$,
and $yx = x^{n-1}y$ hold. One can show that any element of the group
$G$ can be written in the form $x^k y^l$, where $k \in \mathbb{Z}_n$ and $l \in \mathbb{Z}_2$. Take any element of the group $G$ and write it in the form $x^{a_1} y^{b_1} x^{a_2} y^{b_2} \cdots x^{a_m} y^{b_m} \in G$, where $a_i, b_i \in \mathbb{Z}$ for $i = 1, \ldots, m$. Since the relations $x^n = e$ and $y^2 = e$ hold in $G$, the element can be expressed as
$$
x^{a_1} y^{b_1} x^{a_2} y^{b_2} \cdots x^{a_m} y^{b_m},
$$
where $a_j\in \{0, 1, ...,n-1\}$ and $b_j\in\{0,1\}$ for $j = 1, \ldots, m$.
We have
$$
xyxy=e\Longrightarrow x^nyxy=x^{n-1}\Longrightarrow yxy=x^{n-1}\Longrightarrow yxy^2=x^{n-1}y \Longrightarrow yx=x^{n-1}y.
$$
Hence, by applying the method of induction, we obtain
$$
yx^k=x^{k(n-1)}y \text{ for all }k\in \{1,...,n-1\}.
$$
This allows any factor $y$ preceding a factor $x$ to be "moved" after that $x$. To see this, consider the following example. So, consider such an element
$$
x^{a_1}y^{b_1}x^{a_2}y^{b_2}.
$$
We have to check three cases:
* Case $1$. We assume that $b_1=0$ and $a_2\in \{0,1,2,...,n-1\}$. Then we have
$$
x^{a_1}y^{b_1}x^{a_2}y^{b_2}=x^{a_1}x^{a_2}y^{b_2}=x^{a_1+a_2}y^{b_2}.
$$
* Case 2: We assume that $b_1=1$ and $a_2=0$. Then we have
$$
x^{a_1}y^{b_1}x^{a_2}y^{b_2}=x^{a_1}yy^{b_2}=x^{a_1}y^{1+b_2}.
$$
* Case 3: We assume that $b_1=1$ and $a_2=k\in \{1,...,n-1\}$. Then, in view of the previous equation, we have
$$
x^{a_1}y^{b_1}x^{a_2}y^{b_2}=x^{a_1}yx^ky^{b_2}=x^{a_1}x^{k(n-1)}yy^{b_2}=x^{a_1+k(n-1)}y^{1+b_2}.
$$
Therefore, any element can be written in the form $x^a y^b$, where $a, b \in \mathbb{N} \cup \{0\}$. Since $y^2 = e$, the exponents $a$ and $b$ can be reduced modulo $n$ and $2$, respectively. Consequently, the initial element can be written in the form $x^k y^l$, where $k \in \{0, 1, 2,...,n-1\}$ and $l \in \{0, 1\}$. Thus, $\mathrm{ord}\, G \leq 2n$.

Solution step (7 points)
From the equalities $x^n = y^2 = e$ and $yx = x^{n-1}y$, it follows that for any $k_1, k_2 \in \mathbb{Z}_n$ and $l_1, l_2 \in \mathbb{Z}_2$, the following holds:
$$
x^{k_1}y^{l_1} \cdot x^{k_2}y^{l_2} = x^{k_1 + (-1)^{l_1}k_2}y^{l_1 + l_2}.
$$
Clearly, the exponents of $x$ and $y$ on the right-hand side of equality can be reduced modulo $n$ and $2$, respectively. Let us define in the set $\mathbb{Z}_n \times \mathbb{Z}_2$ an operation given by the formula
$$
(k_1, l_1) \circ (k_2, l_2) = \big(k_1 + (-1)^{l_1}k_2 \mod n, l_1 + l_2 \mod 2\big).
$$
It is easy to verify that $(\mathbb{Z}_n \times \mathbb{Z}_2, \circ)$ is a group. The identity element of this group is the pair $(0, 0)$. Since for every $r \in \mathbb{Z}_n$, the equalities $(1, 0)^r = (r, 0)$ and $(r, 0)\circ (0, 1) = (r, 1)$ hold, it follows that
$\mathbb{Z}_n \times \mathbb{Z}_2$ is generated by two elements  $(1, 0)$ and $(0, 1)$.
It can easily be checked that
$$
(1, 0)^n = (0, 0), \quad (0, 1)^2 = (0, 0), \quad (1, 0) \circ (0, 1) \circ (1, 0) \circ (0, 1) = (0, 0).
$$

Furthermore, since $\mathrm{ord}(\mathbb{Z}_n \times \mathbb{Z}_2) = 2n$, it follows from Van Dyck's theorem that $\mathrm{ord}(G) \geq 2n$. We have already shown that $\mathrm{ord}(G) \leq 2n$. As a result, $\mathrm{ord}(G) = 2n$, and therefore the representation of any element of the group $G$ in the form $x^k y^l$, where $k \in \mathbb{Z}_n$ and $l \in \mathbb{Z}_2$, is unique. To prove that the group $G$ is non-abelian, it suffices to note that $yx = x^{n-1}y \neq xy.$