```markdown
**Solution:**

We want to evaluate
\[
S = \sum_{k=0}^{\lfloor n/2 \rfloor} \sum_{\ell=\max\{1,2k\}}^n \frac{1}{4^k} \binom{\ell}{2k}.
\]
A good strategy is to change the order of summation. Notice that for each \(\ell\) (with \(\ell\ge1\)) the inner sum (over \(k\)) runs over all integers \(k\) such that \(0\le k\le \lfloor \ell/2\rfloor\) and is given by
\[
\sum_{k=0}^{\lfloor \ell/2 \rfloor} \frac{1}{4^k} \binom{\ell}{2k}.
\]
Changing the index by letting \(j=2k\) (so that \(k = j/2\)), this becomes a sum over even indices:
\[
\sum_{\substack{j=0 \\ j\text{ even}}}^{\ell} \binom{\ell}{j} \left(\frac{1}{2}\right)^{j},
\]
since
\[
\frac{1}{4^k} = \left(\frac{1}{4}\right)^k = \left(\frac{1}{2}\right)^{2k} = \left(\frac{1}{2}\right)^{j}.
\]

A well-known identity tells us that
\[
\sum_{\substack{j=0 \\ j\text{ even}}}^{\ell} \binom{\ell}{j} x^{j} = \frac{(1+x)^\ell + (1-x)^\ell}{2}.
\]
In our case we take \(x=\frac{1}{2}\) to find
\[
\sum_{k=0}^{\lfloor \ell/2 \rfloor} \frac{1}{4^k} \binom{\ell}{2k} = \frac{1}{2}\left[\left(1+\frac{1}{2}\right)^\ell + \left(1-\frac{1}{2}\right)^\ell\right]
=\frac{1}{2}\left[\left(\frac{3}{2}\right)^\ell + \left(\frac{1}{2}\right)^\ell\right].
\]

Thus, we can rewrite the original sum \(S\) by interchanging the order of summation:
\[
S = \sum_{\ell=1}^{n} \frac{1}{2}\left[\left(\frac{3}{2}\right)^\ell + \left(\frac{1}{2}\right)^\ell\right]
=\frac{1}{2}\sum_{\ell=1}^{n} \left[\left(\frac{3}{2}\right)^\ell + \left(\frac{1}{2}\right)^\ell\right].
\]

Now, we compute the two geometric sums separately.

1. For the first sum:
   \[
   \sum_{\ell=1}^{n} \left(\frac{3}{2}\right)^\ell
   = \frac{\frac{3}{2}\left[\left(\frac{3}{2}\right)^n - 1\right]}{\frac{3}{2}-1}
   = \frac{\frac{3}{2}\left[\left(\frac{3}{2}\right)^n - 1\right]}{\frac{1}{2}}
   = 3\left[\left(\frac{3}{2}\right)^n - 1\right].
   \]

2. For the second sum:
   \[
   \sum_{\ell=1}^{n} \left(\frac{1}{2}\right)^\ell
   = \frac{\frac{1}{2}\left[1-\left(\frac{1}{2}\right)^n\right]}{1-\frac{1}{2}}
   = \frac{\frac{1}{2}\left[1-\left(\frac{1}{2}\right)^n\right]}{\frac{1}{2}}
   = 1-\left(\frac{1}{2}\right)^n.
   \]

Substitute these back into the expression for \(S\):
\[
S = \frac{1}{2}\left[3\left(\left(\frac{3}{2}\right)^n - 1\right) + 1-\left(\frac{1}{2}\right)^n\right].
\]

Simplify the expression:
\[
S = \frac{1}{2}\left[3\left(\frac{3}{2}\right)^n - 3 + 1 - \left(\frac{1}{2}\right)^n\right]
= \frac{3\left(\frac{3}{2}\right)^n - \left(\frac{1}{2}\right)^n - 2}{2}.
\]

Thus, the final answer is:
\[
\boxed{ \frac{3\left(\frac{3}{2}\right)^n - \left(\frac{1}{2}\right)^n - 2}{2} }.
\]
```