An elegant way to prove this identity is by using integral representations of the terms in the summation.

Our goal is to prove the identity:
$$ \sum_{k=0}^n \binom{n}{k}\frac{(-1)^k}{(k+1)^3}=\frac{1}{n+1}\sum_{k=0}^n\sum_{j=0}^k\frac{1}{k+1}\cdot \frac{1}{j+1} $$

Let's denote the left-hand side as LHS and the right-hand side as RHS.

### Step 1: Express the LHS using an integral representation

The key idea is to represent the term $\frac{1}{(k+1)^3}$ as an integral. We know the basic identity:
$$ \int_0^1 x^k \, dx = \left[ \frac{x^{k+1}}{k+1} \right]_0^1 = \frac{1}{k+1} $$
To get a cubic term in the denominator, we can use a triple integral:
\begin{align*}
\frac{1}{(k+1)^3} &= \left(\frac{1}{k+1}\right) \cdot \left(\frac{1}{k+1}\right) \cdot \left(\frac{1}{k+1}\right) \\
&= \left(\int_0^1 x^k \, dx\right) \left(\int_0^1 y^k \, dy\right) \left(\int_0^1 z^k \, dz\right) \\
&= \int_0^1 \int_0^1 \int_0^1 x^k y^k z^k \, dx \, dy \, dz \\
&= \int_0^1 \int_0^1 \int_0^1 (xyz)^k \, dx \, dy \, dz
\end{align*}
Now, we can substitute this integral representation into the LHS sum:
$$ \text{LHS} = \sum_{k=0}^n \binom{n}{k} (-1)^k \left( \int_0^1 \int_0^1 \int_0^1 (xyz)^k \, dx \, dy \, dz \right) $$
Since the summation is finite, we can interchange the order of summation and integration:
$$ \text{LHS} = \int_0^1 \int_0^1 \int_0^1 \left( \sum_{k=0}^n \binom{n}{k} (-1)^k (xyz)^k \right) \, dx \, dy \, dz $$
The expression inside the parentheses is a binomial expansion. Recall the binomial theorem: $(a+b)^n = \sum_{k=0}^n \binom{n}{k} a^{n-k} b^k$. A variation is $(1+u)^n = \sum_{k=0}^n \binom{n}{k} u^k$.
Let $u = -xyz$. The sum becomes:
$$ \sum_{k=0}^n \binom{n}{k} (-xyz)^k = (1 - xyz)^n $$
Substituting this back into the expression for the LHS, we get a compact integral form:
$$ \text{LHS} = \int_0^1 \int_0^1 \int_0^1 (1 - xyz)^n \, dx \, dy \, dz $$

### Step 2: Evaluate the triple integral

We will now evaluate this integral iteratively.

**A. Integrate with respect to x:**
Let's first compute the innermost integral with respect to $x$:
\begin{align*}
\int_0^1 (1 - xyz)^n \, dx
\end{align*}
Let $u = 1 - xyz$, so $du = -yz \, dx$. The limits of integration for $u$ are from $1$ (when $x=0$) to $1-yz$ (when $x=1$).
\begin{align*}
\int_1^{1-yz} u^n \left(\frac{-du}{yz}\right) &= \frac{1}{yz} \int_{1-yz}^1 u^n \, du \\
&= \frac{1}{yz} \left[ \frac{u^{n+1}}{n+1} \right]_{1-yz}^1 \\
&= \frac{1}{yz(n+1)} \left( 1^{n+1} - (1-yz)^{n+1} \right) \\
&= \frac{1 - (1-yz)^{n+1}}{yz(n+1)}
\end{align*}
Substituting this back into the expression for the LHS:
$$ \text{LHS} = \frac{1}{n+1} \int_0^1 \int_0^1 \frac{1 - (1-yz)^{n+1}}{yz} \, dy \, dz $$

**B. Integrate with respect to y:**
Now we focus on the integral with respect to $y$:
$$ I_y = \int_0^1 \frac{1 - (1-yz)^{n+1}}{yz} \, dy = \frac{1}{z} \int_0^1 \frac{1 - (1-yz)^{n+1}}{y} \, dy $$
Let's analyze the inner integral. We use the identity for a finite geometric series:
$$ \frac{1-a^{m}}{1-a} = 1 + a + a^2 + \dots + a^{m-1} $$
Let $a = 1-yz$ and $m = n+1$. Then $1-a = yz$. The integrand is:
$$ \frac{1 - (1-yz)^{n+1}}{yz} = \frac{1}{z} \cdot \frac{1-(1-yz)^{n+1}}{y} $$
This doesn't seem to simplify directly. Let's try a different approach for the integral with respect to $y$. Let $v=1-y$. Then $y=1-v$ and $dy=-dv$.
$$ \int_0^1 \frac{1 - (1-(1-v)z)^{n+1}}{(1-v)z} \, dv $$
This also looks complicated. Let's go back to the expression and use the geometric series identity in a different way.
Let $a = 1-yz$.
$$ \frac{1-a^{n+1}}{1-a} = \sum_{j=0}^n a^j = \sum_{j=0}^n (1-yz)^j $$
The integral $I_y$ has a denominator of $y$, not $1-a=yz$.
Let's try a substitution $v=yz$.
No, the key is recognizing the structure of $\frac{1-A^{N}}{A}$.

Let's use the finite geometric sum identity on $\frac{1-u^{n+1}}{1-u} = \sum_{j=0}^n u^j$.
Consider the integral $I_y = \int_0^1 \frac{1 - (1-yz)^{n+1}}{y} \, dy$. Let $v=y z$. $dv = z dy$.
This substitution seems problematic. Let's try to expand $(1 - (1-yz)^{n+1})$.

A more direct way is to recognize the form of the integral. Let $F(z) = \int_0^1 \frac{1-(1-yz)^{n+1}}{y} dy$.
Let $t = yz$. Then $y=t/z$, $dy = dt/z$. Limits for $t$ are from $0$ to $z$.
$$ F(z) = \int_0^z \frac{1-(1-t)^{n+1}}{t/z} \frac{dt}{z} = \int_0^z \frac{1-(1-t)^{n+1}}{t} dt $$
Now, we use the finite geometric series identity $\frac{1-x^{n+1}}{1-x} = \sum_{j=0}^n x^j$.
$$ \frac{1-(1-t)^{n+1}}{t} = \frac{1-(1-t)^{n+1}}{1-(1-t)} = \sum_{j=0}^n (1-t)^j $$
So,
\begin{align*}
F(z) &= \int_0^z \left( \sum_{j=0}^n (1-t)^j \right) dt \\
&= \sum_{j=0}^n \int_0^z (1-t)^j dt \\
&= \sum_{j=0}^n \left[ -\frac{(1-t)^{j+1}}{j+1} \right]_0^z \\
&= \sum_{j=0}^n \left( -\frac{(1-z)^{j+1}}{j+1} - \left(-\frac{(1-0)^{j+1}}{j+1}\right) \right) \\
&= \sum_{j=0}^n \frac{1 - (1-z)^{j+1}}{j+1}
\end{align*}
Substituting this back into the expression for LHS:
$$ \text{LHS} = \frac{1}{n+1} \int_0^1 \frac{1}{z} F(z) \, dz = \frac{1}{n+1} \int_0^1 \frac{1}{z} \left( \sum_{j=0}^n \frac{1 - (1-z)^{j+1}}{j+1} \right) dz $$
Again, we can swap the finite sum and the integral:
$$ \text{LHS} = \frac{1}{n+1} \sum_{j=0}^n \frac{1}{j+1} \int_0^1 \frac{1 - (1-z)^{j+1}}{z} dz $$

**C. Evaluate the final integral:**
The remaining integral is of the exact same form as the one we just evaluated for $F(z)$, but with $n$ replaced by $j$ and the integration variable being $z$ over the interval $[0,1]$.
Let's define $G(m) = \int_0^1 \frac{1 - (1-z)^{m+1}}{z} dz$.
Using the same steps as for $F(z)$:
\begin{align*}
G(m) &= \int_0^1 \left( \sum_{i=0}^m (1-z)^i \right) dz \\
&= \sum_{i=0}^m \int_0^1 (1-z)^i dz \\
&= \sum_{i=0}^m \left[ -\frac{(1-z)^{i+1}}{i+1} \right]_0^1 \\
&= \sum_{i=0}^m \left( -\frac{0}{i+1} - \left(-\frac{1}{i+1}\right) \right) \\
&= \sum_{i=0}^m \frac{1}{i+1}
\end{align*}
So, the integral in our expression for LHS is $G(j)$:
$$ \int_0^1 \frac{1 - (1-z)^{j+1}}{z} dz = \sum_{i=0}^j \frac{1}{i+1} $$

### Step 3: Final Assembly and Comparison with RHS

Substituting this result back into our expression for the LHS:
$$ \text{LHS} = \frac{1}{n+1} \sum_{j=0}^n \frac{1}{j+1} \left( \sum_{i=0}^j \frac{1}{i+1} \right) $$
This expression can be written as a double summation:
$$ \text{LHS} = \frac{1}{n+1} \sum_{j=0}^n \sum_{i=0}^j \frac{1}{j+1} \cdot \frac{1}{i+1} $$
Now let's examine the RHS of the original identity:
$$ \text{RHS} = \frac{1}{n+1}\sum_{k=0}^n\sum_{j=0}^k\frac{1}{k+1}\cdot \frac{1}{j+1} $$
By simply relabeling the summation indices in our final expression for the LHS (letting the outer index $j$ be $k$, and the inner index $i$ be $j$), we see that the LHS is identical to the RHS.

$$ \text{LHS} = \frac{1}{n+1} \sum_{k=0}^n \sum_{j=0}^k \frac{1}{k+1} \cdot \frac{1}{j+1} = \text{RHS} $$

Thus, the identity is proven.

---
**Summary of the Proof:**

1.  We represented the term $\frac{1}{(k+1)^3}$ on the LHS as a triple integral: $\int_0^1\int_0^1\int_0^1 (xyz)^k \,dx\,dy\,dz$.
2.  We substituted this into the sum and interchanged summation and integration.
3.  We used the binomial theorem to simplify the sum $\sum_{k=0}^n \binom{n}{k}(-xyz)^k$ to $(1-xyz)^n$.
4.  This transformed the LHS into the triple integral $\int_0^1\int_0^1\int_0^1 (1-xyz)^n \,dx\,dy\,dz$.
5.  We evaluated the integral iteratively. Each step of the integration revealed a structure of the form $\int \frac{1-A^N}{B} d\dots$, which was simplified using the formula for a finite geometric series.
6.  The first integration (w.r.t. $x$) yielded $\frac{1-(1-yz)^{n+1}}{yz(n+1)}$.
7.  The second integration (w.r.t. $y$) simplified to $\frac{1}{z(n+1)} \sum_{j=0}^n \frac{1-(1-z)^{j+1}}{j+1}$.
8.  The third integration (w.r.t. $z$) led to the final expression for the LHS: $\frac{1}{n+1} \sum_{j=0}^n \frac{1}{j+1} \left(\sum_{i=0}^j \frac{1}{i+1}\right)$.
9.  This expression is identical to the RHS of the given equation, thus completing the proof.