```markdown
**Solution.**

We start from the given ODE
\[
(u')^2(1+u^2)\;=\;1 - u\,u''\,,\qquad u(0)=0.
\]
Define the auxiliary function
\[
g(x)\;=\;u(x)\,u'(x).
\]
Then
\[
g'(x)
\;=\;\frac{d}{dx}\bigl(u\,u'\bigr)
\;=\;u'^2 \;+\;u\,u''
\;=\;u'^2 \;+\;\bigl[\,1 - (u')^2(1+u^2)\bigr]
\;=\;1 - (u\,u')^2
\;=\;1 - g(x)^2.
\]
Since \(g(0)=u(0)u'(0)=0\), the unique solution of
\[
g'(x)=1 - g(x)^2,\quad g(0)=0
\]
is
\[
g(x)\;=\;\tanh(x)\,.
\]
Hence
\[
u(x)\,u'(x)\;=\;\tanh(x),
\qquad
\frac{d}{dx}\bigl(u(x)^2\bigr)
\;=\;2\,u\,u'
\;=\;2\,\tanh(x).
\]
Integrating from \(0\) to \(x\) gives
\[
u(x)^2
\;=\;\int_0^x 2\,\tanh(s)\,ds
\;=\;2\int_0^x \tanh(s)\,ds
\;=\;2\ln\!\bigl(\cosh x\bigr).
\]
Since for \(x>0\) one has \(\cosh x<e^x\) and hence \(\ln\cosh x<x\), we obtain
\[
u(x)^2
\;=\;2\ln\!\bigl(\cosh x\bigr)
\;<\;2x,
\]
or equivalently
\[
\bigl|u(x)\bigr|\;<\;\sqrt{2x},
\qquad x>0.
\]
This completes the proof. \(\qed\)
```