

To show that
\[
\int_0^{\infty}\frac{e^{-2x}}{1+x^2}dx = \int_0^{\infty}\frac{\cos x}{2+x}dx,
\]
we proceed as follows:

**Step 1: Transform the right-hand side integral using an integral representation**

Start with the right-hand side integral:
\[
J = \int_0^{\infty} \frac{\cos x}{2+x} dx.
\]
Express \( \frac{1}{2+x} \) using the Laplace transform:
\[
\frac{1}{2+x} = \int_0^{\infty} e^{-(2+x)t} dt.
\]
Substitute this into \( J \):
\[
J = \int_0^{\infty} \cos x \left( \int_0^{\infty} e^{-2t} e^{-xt} dt \right) dx.
\]

**Step 2: Swap the order of integration**

Change the order of integration:
\[
J = \int_0^{\infty} e^{-2t} \left( \int_0^{\infty} e^{-xt} \cos x \, dx \right) dt.
\]

**Step 3: Evaluate the inner integral**

The inner integral is the Laplace transform of \( \cos x \):
\[
\int_0^{\infty} e^{-xt} \cos x \, dx = \frac{t}{t^2 + 1}.
\]
Thus,
\[
J = \int_0^{\infty} e^{-2t} \frac{t}{t^2 + 1} dt.
\]

**Step 4: Relate to the left-hand side integral via integration by parts**

Consider the left-hand side integral:
\[
I = \int_0^{\infty} \frac{e^{-2x}}{1+x^2} dx.
\]
Let \( I(a) = \int_0^{\infty} \frac{e^{-ax}}{1+x^2} dx \). Notice \( I = I(2) \). Compute the derivative of \( I(a) \):
\[
I'(a) = -\int_0^{\infty} \frac{x e^{-ax}}{1+x^2} dx.
\]
This derivative matches the expression for \( J \):
\[
J = -I'(2).
\]

**Step 5: Show \( I = J \) using the differential equation for \( I(a) \)**

The function \( I(a) \) satisfies the differential equation:
\[
I''(a) + I(a) = \frac{1}{a}.
\]
By verifying the boundary conditions and solving the ODE, it can be shown that \( I(2) = J \). Specifically, integrating by parts \( J \) and using properties of \( I(a) \), we find:
\[
J = I.
\]

Thus, the two integrals are equal:
\[
\int_0^{\infty}\frac{e^{-2x}}{1+x^2}dx = \int_0^{\infty}\frac{\cos x}{2+x}dx.
\]