# Solution

I will prove the inequality 
$$\left(\prod_{i=1}^n a_i\right)^\frac{1}{n}+\left(\prod_{i=1}^n b_i\right)^\frac{1}{n}+\left(\prod_{i=1}^n c_i\right)^\frac{1}{n} \leq \left(\prod_{i=1}^n (a_i+b_i+c_i)\right)^\frac{1}{n}$$
where $a_1,\ldots,a_n$, $b_1,\ldots,b_n$, and $c_1,\ldots,c_n$ are non-negative real numbers.

## Step 1: Make a substitution

Define:
$$x_i = \frac{a_i}{a_i+b_i+c_i}, \quad y_i = \frac{b_i}{a_i+b_i+c_i}, \quad z_i = \frac{c_i}{a_i+b_i+c_i}$$

Note that $x_i, y_i, z_i \geq 0$ and $x_i + y_i + z_i = 1$ for all $i$.

With this substitution, we have:
$$a_i = (a_i+b_i+c_i)x_i, \quad b_i = (a_i+b_i+c_i)y_i, \quad c_i = (a_i+b_i+c_i)z_i$$

## Step 2: Rewrite the inequality

Substituting these expressions:
$$\begin{align*}
\left(\prod_{i=1}^n a_i\right)^\frac{1}{n} &= \left(\prod_{i=1}^n (a_i+b_i+c_i)x_i\right)^\frac{1}{n} \\
&= \left(\prod_{i=1}^n (a_i+b_i+c_i)\right)^\frac{1}{n} \cdot \left(\prod_{i=1}^n x_i\right)^\frac{1}{n}
\end{align*}$$

Similarly for the other terms. The original inequality becomes:
$$\left(\prod_{i=1}^n (a_i+b_i+c_i)\right)^\frac{1}{n}\left[\left(\prod_{i=1}^n x_i\right)^\frac{1}{n}+\left(\prod_{i=1}^n y_i\right)^\frac{1}{n}+\left(\prod_{i=1}^n z_i\right)^\frac{1}{n}\right] \leq \left(\prod_{i=1}^n (a_i+b_i+c_i)\right)^\frac{1}{n}$$

Dividing both sides by $\left(\prod_{i=1}^n (a_i+b_i+c_i)\right)^\frac{1}{n}$, we need to prove:
$$\left(\prod_{i=1}^n x_i\right)^\frac{1}{n}+\left(\prod_{i=1}^n y_i\right)^\frac{1}{n}+\left(\prod_{i=1}^n z_i\right)^\frac{1}{n} \leq 1$$

## Step 3: Apply the AM-GM inequality

By the AM-GM inequality, for any sequence of non-negative real numbers, the arithmetic mean is greater than or equal to the geometric mean:
$$\frac{1}{n}\sum_{i=1}^n x_i \geq \left(\prod_{i=1}^n x_i\right)^\frac{1}{n}$$
$$\frac{1}{n}\sum_{i=1}^n y_i \geq \left(\prod_{i=1}^n y_i\right)^\frac{1}{n}$$
$$\frac{1}{n}\sum_{i=1}^n z_i \geq \left(\prod_{i=1}^n z_i\right)^\frac{1}{n}$$

Adding these three inequalities:
$$\frac{1}{n}\sum_{i=1}^n (x_i + y_i + z_i) \geq \left(\prod_{i=1}^n x_i\right)^\frac{1}{n} + \left(\prod_{i=1}^n y_i\right)^\frac{1}{n} + \left(\prod_{i=1}^n z_i\right)^\frac{1}{n}$$

Since $x_i + y_i + z_i = 1$ for all $i$, we have:
$$\frac{1}{n}\sum_{i=1}^n 1 = 1 \geq \left(\prod_{i=1}^n x_i\right)^\frac{1}{n} + \left(\prod_{i=1}^n y_i\right)^\frac{1}{n} + \left(\prod_{i=1}^n z_i\right)^\frac{1}{n}$$

This proves the original inequality.