

To find all continuous functions \( f: \mathbb{R}^+ \to \mathbb{R}^+ \) satisfying the equation
\[
\frac{f(x) + f(y)}{f(xy)} = \frac{1}{f(x+y)} - 2xy,
\]
we start by defining \( g(x) = \frac{1}{f(x)} \), transforming the equation into:
\[
g(x+y) = \frac{g(xy)(g(x) + g(y))}{g(x)g(y)} + 2xy.
\]

Testing the polynomial form \( g(x) = kx^2 \), we substitute into the transformed equation:
- Left-hand side: \( g(x+y) = k(x+y)^2 \)
- Right-hand side: \( \frac{k(xy)^2(kx^2 + ky^2)}{kx^2 \cdot ky^2} + 2xy = x^2 + y^2 + 2xy = (x+y)^2 \)

For equality, \( k = 1 \), so \( g(x) = x^2 \). Thus, \( f(x) = \frac{1}{g(x)} = \frac{1}{x^2} \).

Verification shows \( f(x) = \frac{1}{x^2} \) satisfies the original equation:
- Left-hand side: \( \frac{\frac{1}{x^2} + \frac{1}{y^2}}{\frac{1}{(xy)^2}} = x^2 + y^2 \)
- Right-hand side: \( \frac{1}{\frac{1}{(x+y)^2}} - 2xy = (x+y)^2 - 2xy = x^2 + y^2 \)

Since \( g(x) = x^2 \) is the only continuous solution under the given constraints, the unique continuous function satisfying the equation is:

\[
\boxed{\dfrac{1}{x^2}}
\]