

To show that \( |u(x)| < \sqrt{2x} \) for all \( x > 0 \) given the differential equation \( (u')^2 (1 + u^2) = 1 - u'' u \) with \( u(0) = 0 \), follow these steps:

**Step 1: Introduce Energy Function**  
Define \( E(x) = u(x)^2 \). Compute its derivatives:
\[
E'(x) = 2u u', \quad E''(x) = 2(u')^2 + 2u u''.
\]
Substitute \( u u'' \) from the original equation:
\[
u u'' = 1 - (u')^2 (1 + u^2).
\]
Thus,
\[
E'' = 2(u')^2 + 2\left[1 - (u')^2 (1 + u^2)\right] = 2 - 2(u')^2 u^2.
\]

**Step 2: Relate \( E'' \) to \( E' \)**  
Express \( (u')^2 u^2 \) in terms of \( E \) and \( E' \):
\[
(u')^2 u^2 = \frac{(E')^2}{4}.
\]
Substitute into \( E'' \):
\[
E'' = 2 - \frac{(E')^2}{2}.
\]

**Step 3: Solve the Riccati Equation**  
Let \( F = E' \), so \( F' = 2 - \frac{F^2}{2} \). This integrates to:
\[
\frac{dF}{2 - \frac{F^2}{2}} = dx \implies \frac{2}{4 - F^2} dF = dx.
\]
Integrate using partial fractions and apply initial conditions \( E(0) = 0 \) and \( E'(0) = 0 \):
\[
F(x) = 2 \tanh(x).
\]

**Step 4: Integrate \( E' = 2 \tanh(x) \)**  
Integrate \( F(x) = E'(x) \):
\[
E(x) = 2 \int_0^x \tanh(t) \, dt = 2 \ln(\cosh(x)).
\]
Thus,
\[
u(x)^2 = 2 \ln(\cosh(x)).
\]

**Step 5: Establish the Inequality**  
For \( x > 0 \), \( \cosh(x) < e^x \) implies:
\[
\ln(\cosh(x)) < x.
\]
Therefore,
\[
u(x)^2 = 2 \ln(\cosh(x)) < 2x \implies |u(x)| < \sqrt{2x}.
\]

**Conclusion**  
For all \( x > 0 \), \( |u(x)| < \sqrt{2x} \).

```markdown
\boxed{|u(x)| < \sqrt{2x} \quad \text{for all } x > 0}
```