Of course. Here is a detailed, step-by-step solution to the problem.

### **Problem Statement**
Prove that the sequence $(a_n)$ where
$$
a_n=\frac{\left(1+\frac 1n\right)^{3n+2}}{\left(1+\frac 1n\right)^n+\left(1+\frac 1n\right)^{n+1}+\left(1+\frac 1n\right)^{n+2}}
$$
is strictly increasing.

### **Solution**

To prove that the sequence $(a_n)$ is strictly increasing, we must show that $a_{n+1} > a_n$ for all integers $n \geq 1$.

**Step 1: Simplify the expression for $a_n$**

Let's simplify the expression for $a_n$. Let $x_n = 1 + \frac{1}{n}$. The expression becomes:
$$
a_n = \frac{x_n^{3n+2}}{x_n^n + x_n^{n+1} + x_n^{n+2}}
$$
We can factor out $x_n^n$ from the denominator:
$$
a_n = \frac{x_n^{3n+2}}{x_n^n(1 + x_n + x_n^2)} = \frac{x_n^{2n+2}}{1 + x_n + x_n^2}
$$
The denominator is a finite geometric series sum $1 + x_n + x_n^2 = \frac{x_n^3 - 1}{x_n - 1}$.
Let's substitute $x_n = 1 + \frac{1}{n}$ back into the denominator expression:
$$
1 + \left(1 + \frac{1}{n}\right) + \left(1 + \frac{1}{n}\right)^2 = 1 + \frac{n+1}{n} + \frac{(n+1)^2}{n^2}
$$
Putting everything over a common denominator $n^2$:
$$
= \frac{n^2}{n^2} + \frac{n(n+1)}{n^2} + \frac{(n+1)^2}{n^2} = \frac{n^2 + n^2+n + n^2+2n+1}{n^2} = \frac{3n^2+3n+1}{n^2}
$$
Now, let's work on the numerator of $a_n$:
$$
x_n^{2n+2} = \left(1 + \frac{1}{n}\right)^{2n+2} = \left(\frac{n+1}{n}\right)^{2n+2} = \frac{(n+1)^{2n+2}}{n^{2n+2}}
$$
Combining the simplified numerator and denominator:
$$
a_n = \frac{\frac{(n+1)^{2n+2}}{n^{2n+2}}}{\frac{3n^2+3n+1}{n^2}} = \frac{(n+1)^{2n+2}}{n^{2n+2}} \cdot \frac{n^2}{3n^2+3n+1} = \frac{(n+1)^{2n+2}}{n^{2n}(3n^2+3n+1)}
$$
So we have the simplified expression for the general term of the sequence:
$$
a_n = \frac{(n+1)^{2n+2}}{n^{2n}(3n^2+3n+1)}
$$

**Step 2: Define a continuous function and use calculus**

To prove that $a_{n+1} > a_n$, we can define a continuous function $f(x)$ for $x \geq 1$ such that $f(n) = a_n$. If we can show that $f(x)$ is strictly increasing for $x \geq 1$, i.e., $f'(x) > 0$, it will imply that $f(n+1) > f(n)$ for all integers $n \geq 1$.

Let the function $f(x)$ be:
$$
f(x) = \frac{(x+1)^{2x+2}}{x^{2x}(3x^2+3x+1)}
$$

**Step 3: Use logarithmic differentiation**

The expression for $f(x)$ is complex to differentiate directly. We will use logarithmic differentiation. Let $g(x) = \ln(f(x))$. If we show that $g'(x) > 0$, then $f'(x) = f(x)g'(x)$ will also be positive since $f(x) > 0$ for $x \geq 1$.

$$
g(x) = \ln\left(\frac{(x+1)^{2x+2}}{x^{2x}(3x^2+3x+1)}\right)
$$
Using the properties of logarithms:
$$
g(x) = \ln((x+1)^{2x+2}) - \ln(x^{2x}) - \ln(3x^2+3x+1)
$$
$$
g(x) = (2x+2)\ln(x+1) - 2x\ln(x) - \ln(3x^2+3x+1)
$$

**Step 4: Compute the derivative $g'(x)$**

Now, we differentiate $g(x)$ with respect to $x$ using the product rule for the first two terms:
$$
\frac{d}{dx}((2x+2)\ln(x+1)) = 2\ln(x+1) + (2x+2)\frac{1}{x+1} = 2\ln(x+1) + 2
$$
$$
\frac{d}{dx}(2x\ln(x)) = 2\ln(x) + 2x\frac{1}{x} = 2\ln(x) + 2
$$
$$
\frac{d}{dx}(\ln(3x^2+3x+1)) = \frac{6x+3}{3x^2+3x+1}
$$
Combining these results to find $g'(x)$:
$$
g'(x) = (2\ln(x+1) + 2) - (2\ln(x) + 2) - \frac{6x+3}{3x^2+3x+1}
$$
$$
g'(x) = 2\ln(x+1) - 2\ln(x) - \frac{6x+3}{3x^2+3x+1}
$$
$$
g'(x) = 2\ln\left(\frac{x+1}{x}\right) - \frac{3(2x+1)}{3x^2+3x+1}
$$
$$
g'(x) = 2\ln\left(1+\frac{1}{x}\right) - \frac{3(2x+1)}{3x^2+3x+1}
$$

**Step 5: Prove that $g'(x) > 0$ for $x \geq 1$**

We need to show that for $x \geq 1$:
$$
2\ln\left(1+\frac{1}{x}\right) > \frac{3(2x+1)}{3x^2+3x+1}
$$
To prove this, we will use a well-known inequality for the natural logarithm: for any $t > 0$,
$$
\ln(1+t) > \frac{2t}{2+t}
$$
Let's first prove this auxiliary inequality. Let $h(t) = \ln(1+t) - \frac{2t}{2+t}$. We want to show $h(t) > 0$ for $t > 0$.
First, $h(0) = \ln(1) - 0 = 0$.
Now, let's find the derivative of $h(t)$:
$$
h'(t) = \frac{1}{1+t} - \frac{2(2+t) - 2t(1)}{(2+t)^2} = \frac{1}{1+t} - \frac{4+2t-2t}{(2+t)^2} = \frac{1}{1+t} - \frac{4}{(2+t)^2}
$$
Combining the fractions:
$$
h'(t) = \frac{(2+t)^2 - 4(1+t)}{(1+t)(2+t)^2} = \frac{4+4t+t^2 - 4-4t}{(1+t)(2+t)^2} = \frac{t^2}{(1+t)(2+t)^2}
$$
For $t>0$, $t^2 > 0$, $1+t > 0$, and $(2+t)^2 > 0$. Thus, $h'(t) > 0$ for all $t > 0$.
Since $h(0)=0$ and $h(t)$ is strictly increasing for $t>0$, it follows that $h(t) > h(0)=0$ for all $t>0$.
This confirms that $\ln(1+t) > \frac{2t}{2+t}$ for $t>0$.

Now, let $t = 1/x$. Since we are considering $x \geq 1$, we have $0 < t \leq 1$. The inequality holds.
Substituting $t=1/x$ into the inequality $\ln(1+t) > \frac{2t}{2+t}$:
$$
\ln\left(1+\frac{1}{x}\right) > \frac{2(1/x)}{2+(1/x)} = \frac{2/x}{(2x+1)/x} = \frac{2}{2x+1}
$$
Multiplying by 2, we get a lower bound for the first term of $g'(x)$:
$$
2\ln\left(1+\frac{1}{x}\right) > \frac{4}{2x+1}
$$
Now, we need to show that this lower bound is greater than the second term of $g'(x)$:
$$
\frac{4}{2x+1} > \frac{3(2x+1)}{3x^2+3x+1}
$$
Since $x \geq 1$, both denominators are positive, so we can cross-multiply without changing the inequality direction:
$$
4(3x^2+3x+1) > 3(2x+1)(2x+1)
$$
$$
12x^2+12x+4 > 3(4x^2+4x+1)
$$
$$
12x^2+12x+4 > 12x^2+12x+3
$$
$$
4 > 3
$$
This last inequality is clearly true.

**Step 6: Conclusion**

We have successfully shown that for all $x \geq 1$:
$$
g'(x) = 2\ln\left(1+\frac{1}{x}\right) - \frac{3(2x+1)}{3x^2+3x+1} > \frac{4}{2x+1} - \frac{3(2x+1)}{3x^2+3x+1} > 0
$$
Since $g'(x) > 0$ for $x \geq 1$, the function $g(x)=\ln(f(x))$ is strictly increasing on $[1, \infty)$.
Because the exponential function $e^x$ is strictly increasing, $f(x) = e^{g(x)}$ is also strictly increasing on $[1, \infty)$.
Therefore, for any integer $n \geq 1$, we have $f(n+1) > f(n)$.
Since $a_n = f(n)$, it follows that $a_{n+1} > a_n$ for all $n \geq 1$.

This completes the proof that the sequence $(a_n)$ is strictly increasing.