Solution:
Let the given sum be $S$. The sum is
\begin{equation*}
S = \sum_{n=1}^{\infty}\frac{48n^2+44n+9}{n(2n+1)(4n+1)(4n+3)}.
\end{equation*}
Let $a_n$ be the general term of the series:
\begin{equation*}
a_n = \frac{48n^2+44n+9}{n(2n+1)(4n+1)(4n+3)}.
\end{equation*}
We perform a partial fraction decomposition of $a_n$. We look for constants $A, B, C, D$ such that
\begin{equation*}
\frac{48n^2+44n+9}{n(2n+1)(4n+1)(4n+3)} = \frac{A}{n} + \frac{B}{2n+1} + \frac{C}{4n+1} + \frac{D}{4n+3}.
\end{equation*}
Using the cover-up method:
\begin{itemize}
    \item For $A$, multiply by $n$ and set $n=0$: $A = \frac{9}{1 \cdot 1 \cdot 3} = 3$.
    \item For $B$, multiply by $2n+1$ and set $n=-1/2$: $B = \frac{48(-1/2)^2+44(-1/2)+9}{(-1/2)(4(-1/2)+1)(4(-1/2)+3)} = \frac{12-22+9}{(-1/2)(-1)(1)} = \frac{-1}{1/2} = -2$.
    \item For $C$, multiply by $4n+1$ and set $n=-1/4$: $C = \frac{48(-1/4)^2+44(-1/4)+9}{(-1/4)(2(-1/4)+1)(4(-1/4)+3)} = \frac{3-11+9}{(-1/4)(1/2)(2)} = \frac{1}{-1/4} = -4$.
    \item For $D$, multiply by $4n+3$ and set $n=-3/4$: $D = \frac{48(-3/4)^2+44(-3/4)+9}{(-3/4)(2(-3/4)+1)(4(-3/4)+1)} = \frac{27-33+9}{(-3/4)(-1/2)(-2)} = \frac{3}{-3/4} = -4$.
\end{itemize}
Thus, the partial fraction decomposition is
\begin{equation*}
a_n = \frac{3}{n} - \frac{2}{2n+1} - \frac{4}{4n+1} - \frac{4}{4n+3}.
\end{equation*}
We can rewrite $a_n$ as:
\begin{equation*}
a_n = \frac{3}{n} - \frac{1}{n+1/2} - \frac{1}{n+1/4} - \frac{1}{n+3/4}.
\end{equation*}
We can group the terms as follows:
\begin{equation*}
a_n = \left(\frac{1}{n} - \frac{1}{n+1/2}\right) + \left(\frac{1}{n} - \frac{1}{n+1/4}\right) + \left(\frac{1}{n} - \frac{1}{n+3/4}\right).
\end{equation*}
The sum $S$ can be written as
\begin{equation*}
S = \sum_{n=1}^{\infty} a_n = \sum_{n=1}^{\infty} \left(\frac{1}{n} - \frac{1}{n+1/2}\right) + \sum_{n=1}^{\infty} \left(\frac{1}{n} - \frac{1}{n+1/4}\right) + \sum_{n=1}^{\infty} \left(\frac{1}{n} - \frac{1}{n+3/4}\right).
\end{equation*}
This decomposition is valid because $a_n \sim \frac{48n^2}{128n^4} = \frac{3}{8n^2}$ for large $n$, so the sum $\sum a_n$ converges absolutely, and the individual sums also converge.
We use the identity related to the digamma function $\psi(x)$:
\begin{equation*}
\sum_{n=1}^{\infty} \left(\frac{1}{n} - \frac{1}{n+a}\right) = \psi(1+a) + \gamma,
\end{equation*}
where $\gamma$ is the Euler-Mascheroni constant.
Let $S_a = \sum_{n=1}^{\infty} \left(\frac{1}{n} - \frac{1}{n+a}\right)$. Then
\begin{equation*}
S = S_{1/2} + S_{1/4} + S_{3/4}.
\end{equation*}
We have:
\begin{itemize}
    \item $S_{1/2} = \psi(1+1/2) + \gamma = \psi(3/2) + \gamma$.
    \item $S_{1/4} = \psi(1+1/4) + \gamma = \psi(5/4) + \gamma$.
    \item $S_{3/4} = \psi(1+3/4) + \gamma = \psi(7/4) + \gamma$.
\end{itemize}
Using the property $\psi(x+1) = \psi(x) + 1/x$:
\begin{itemize}
    \item $\psi(3/2) = \psi(1/2+1) = \psi(1/2) + \frac{1}{1/2} = \psi(1/2) + 2$.
    \item $\psi(5/4) = \psi(1/4+1) = \psi(1/4) + \frac{1}{1/4} = \psi(1/4) + 4$.
    \item $\psi(7/4) = \psi(3/4+1) = \psi(3/4) + \frac{1}{3/4} = \psi(3/4) + 4/3$.
\end{itemize}
We use the known values of the digamma function:
\begin{itemize}
    \item $\psi(1/2) = -\gamma - 2\ln 2$.
    \item $\psi(1/4) = -\gamma - \frac{\pi}{2} - 3\ln 2$.
    \item $\psi(3/4) = -\gamma + \frac{\pi}{2} - 3\ln 2$. (This can be derived from $\psi(1/4)$ using the reflection formula $\psi(1-x)-\psi(x)=\pi\cot(\pi x)$ with $x=1/4$).
\end{itemize}
Now substitute these values back:
\begin{itemize}
    \item $S_{1/2} = (-\gamma - 2\ln 2) + 2 + \gamma = 2 - 2\ln 2$.
    \item $S_{1/4} = (-\gamma - \frac{\pi}{2} - 3\ln 2) + 4 + \gamma = 4 - \frac{\pi}{2} - 3\ln 2$.
    \item $S_{3/4} = (-\gamma + \frac{\pi}{2} - 3\ln 2) + 4/3 + \gamma = \frac{4}{3} + \frac{\pi}{2} - 3\ln 2$.
\end{itemize}
Finally, we sum these results:
\begin{align*} S &= S_{1/2} + S_{1/4} + S_{3/4} \\ &= (2 - 2\ln 2) + (4 - \frac{\pi}{2} - 3\ln 2) + (\frac{4}{3} + \frac{\pi}{2} - 3\ln 2) \\ &= (2 + 4 + \frac{4}{3}) + (-2 - 3 - 3)\ln 2 + (-\frac{\pi}{2} + \frac{\pi}{2}) \\ &= (6 + \frac{4}{3}) - 8\ln 2 + 0 \\ &= (\frac{18}{3} + \frac{4}{3}) - 8\ln 2 \\ &= \frac{22}{3} - 8\ln 2 \end{align*}

Alternatively, using the integral representation $\sum_{n=1}^{\infty} (\frac{1}{n} - \frac{1}{n+a}) = \int_0^1 \frac{1-t^a}{1-t} dt$:
\begin{align*} S &= \int_0^1 \frac{1-t^{1/2}}{1-t} dt + \int_0^1 \frac{1-t^{1/4}}{1-t} dt + \int_0^1 \frac{1-t^{3/4}}{1-t} dt \\ &= \int_0^1 \frac{(1-t^{1/2}) + (1-t^{1/4}) + (1-t^{3/4})}{1-t} dt \\ &= \int_0^1 \frac{3 - t^{1/2} - t^{1/4} - t^{3/4}}{1-t} dt \end{align*}
Let $t=u^4$, $dt = 4u^3 du$.
\begin{align*} S &= \int_0^1 \frac{3 - u^2 - u - u^3}{1-u^4} 4u^3 du \\ &= \int_0^1 \frac{3 - u - u^2 - u^3}{(1-u)(1+u)(1+u^2)} 4u^3 du\end{align*}
Factor the numerator: $3 - u - u^2 - u^3 = (1-u)(3+2u+u^2)$.
\begin{align*} S &= \int_0^1 \frac{(1-u)(3+2u+u^2)}{(1-u)(1+u)(1+u^2)} 4u^3 du \\ &= \int_0^1 \frac{4u^3(3+2u+u^2)}{(1+u)(1+u^2)} du \\ &= \int_0^1 \frac{12u^3+8u^4+4u^5}{1+u+u^2+u^3} du \end{align*}
Performing polynomial division: $4u^5+8u^4+12u^3 = (4u^2+4u+4)(u^3+u^2+u+1) - (12u^2+8u+4)$.
So the integrand is $4u^2+4u+4 - \frac{12u^2+8u+4}{(1+u)(1+u^2)}$.
\begin{align*} S &= \int_0^1 (4u^2+4u+4) du - \int_0^1 \frac{12u^2+8u+4}{(1+u)(1+u^2)} du \\ &= \left[\frac{4u^3}{3} + 2u^2 + 4u\right]_0^1 - \int_0^1 \left(\frac{4}{1+u} + \frac{8u}{1+u^2}\right) du \\ &= (\frac{4}{3}+2+4) - \left[4\ln(1+u) + 4\ln(1+u^2)\right]_0^1 \\ &= \frac{22}{3} - [ (4\ln 2 + 4\ln 2) - (4\ln 1 + 4\ln 1) ] \\ &= \frac{22}{3} - 8\ln 2 \end{align*}

Final Answer: The final answer is $\boxed{\frac{22}{3} - 8\ln 2}$