```markdown
**Solution.**

We shall compare the asymptotic sizes of
\[
p_n \;=\; P\bigl(\hat R_n=\hat S_n=\hat T_n\bigr)
\quad\text{and}\quad
q_n \;=\; P\bigl(\hat R_n,\hat S_n,\hat T_n\in\{2n-1,2n,2n+1\},\;\hat R_n\neq\hat S_n\bigr).
\]
The key is a *bivariate* local centralâ€limit theorem for
\[
\bigl(R_n',S_n'\bigr)
\;=\;\bigl(\hat R_n-2n,\;\hat S_n-2n\bigr)
\;=\;\sum_{i=1}^n \underbrace{\bigl(R_i-2,\;S_i-2\bigr)}_{Y_i}\,.
\]
1.  **Mean and covariance.**  One checks easily that each  
    \(Y_i\) has mean \(\mathbf0\) and covariance matrix
    \[
      M \;=\;
      \Cov(Y_i)
      \;=\;
      \begin{pmatrix}
        \tfrac23 & -\tfrac13\\[6pt]
        -\tfrac13 & \tfrac23
      \end{pmatrix},
      \qquad
      \det M=\tfrac13,
      \quad
      M^{-1}=\begin{pmatrix}2&1\\1&2\end{pmatrix}.
    \]
    Hence the sum \(\sum_{i=1}^n Y_i\) has covariance \(\Sigma_n=nM\).

2.  **Local CLT (lattice version).**  Since the support of \(Y_i\)
    spans the full lattice \(\Bbb Z^2\) and is aperiodic, the local CLT
    gives, for each fixed \((x,y)\in\Bbb Z^2\),
    \[
      P\bigl(R_n'=x,\;S_n'=y\bigr)
      = 
      \frac{1}{2\pi\,n\sqrt{\det M}}
      \exp\!\Bigl(-\tfrac1{2n}(x,y)\,M^{-1}\,(x,y)^T\Bigr)
      \;+\;O\bigl(n^{-\tfrac32}\bigr).
    \]
    Since \(\sqrt{\det M}=\tfrac1{\sqrt3}\), the leading factor is
    \(\displaystyle \tfrac{\sqrt3}{2\pi\,n}.\)

3.  **Asymptotic of \(p_n\).**  
    \[
      p_n
      =P\bigl(\hat R_n=\hat S_n=\hat T_n\bigr)
      =P\bigl(R_n'=0,\;S_n'=0\bigr)
      \sim
      \frac{\sqrt3}{2\pi\,n}\,.
    \]

4.  **Asymptotic of \(q_n\).**  
    Observe that the event
    \(\{\hat R_n,\hat S_n,\hat T_n\in\{2n-1,2n,2n+1\},\,\hat R_n\neq\hat S_n\}\)
    is equivalent to
    \[
      (R_n',S_n')\;\in\;
      A
      \quad\text{where}\quad
      A = \{(-1,0),(1,0),(0,-1),(0,1),(-1,1),(1,-1)\}.
    \]
    For each \((x,y)\in A\) one computes
    \((x,y)\,M^{-1}(x,y)^T = 2(x^2+xy+y^2)=2\),
    so
    \[
      P\bigl(R_n'=x,S_n'=y\bigr)
      =
      \frac{\sqrt3}{2\pi\,n}\,
      e^{-\,2/(2n)}+O(n^{-3/2})
      = 
      \frac{\sqrt3}{2\pi\,n}\,e^{-1/n} +O(n^{-3/2}).
    \]
    Hence
    \[
      q_n
      =\sum_{(x,y)\in A}P(R_n'=x,S_n'=y)
      \sim
      6\;\frac{\sqrt3}{2\pi\,n}\,e^{-1/n}
      \sim
      6\;\frac{\sqrt3}{2\pi\,n}.
    \]

5.  **Conclusion.**  From the two asymptotics
    \[
      p_n\sim\frac{\sqrt3}{2\pi\,n},
      \qquad
      q_n\sim 6\,\frac{\sqrt3}{2\pi\,n}
      \quad\Longrightarrow\quad
      \frac{q_n}{p_n}\;\longrightarrow\;6 \;>\;4.
    \]
    In particular, for all sufficiently large \(n\) one has
    \(\;q_n>4\,p_n\), and thus certainly \(4p_n<q_n\) for infinitely manyÂ \(n\).  
    This completes the proof.
```