Let $A$ be the given $(2n) \times (2n)$ matrix. The matrix is of the form
\[
	A=\begin{pmatrix}
		0 & 0 &0 &  \ldots & 0 & c_1 \\
		1 & 0 & 0 &\ldots & 0 & c_2 \\
		0 & 1 & 0 &\ldots & 0 & c_3 \\
		\vdots & \vdots &\vdots &\ddots & \vdots &\vdots \\
		0 & 0 & 0 &\ldots & 1 & c_{2n}
	\end{pmatrix},
\]
where the entries $a_{i,j} = \delta_{i, j+1}$ for $1 \le j \le 2n-1$ and the last column is $c = (c_1, c_2, \ldots, c_{2n})^T$.
The characteristic polynomial of such a matrix is given by $P(\lambda) = \det(A - \lambda I) = \lambda^{2n} - \sum_{i=1}^{2n} c_i \lambda^{i-1}$. This is because $A^T$ is a companion matrix for this polynomial.

The entries of the last column are specified as $c_1=n-1, c_2=n-2, c_3=n-3, \ldots, c_{2n-2}=-(n-3), c_{2n-1}=-(n-2), c_{2n}=-(n-1)$.
The statement "in the last column zero appears two times" implies that $c_i=0$ for exactly two values of $i$.
Based on the pattern $n-1, n-2, \ldots$, the first $n$ entries are likely $c_i = n-i$ for $i=1, \ldots, n$. This gives $c_n = n-n=0$.
The last entries $-(n-3), -(n-2), -(n-1)$ suggest a pattern related to $n$.
Let's assume the entries are $c_i = n-i$ for $i=1, \ldots, n$ and $c_i = -(n-(2n-i+1))$ for $i=n+1, \ldots, 2n$.
Let's check this. For $i=n+j$ where $j=1, \ldots, n$:
$c_{n+j} = -(n-(2n-(n+j)+1)) = -(n-(n-j+1)) = -(j-1)$.
For $j=1$, $c_{n+1} = -(1-1) = 0$.
For $j=2$, $c_{n+2} = -(2-1) = -1$.
For $j=n$, $c_{2n} = -(n-1)$.
So the sequence of $c_i$ is $n-1, n-2, \ldots, 1, 0$ (for $i=1, \ldots, n$) followed by $0, -1, -2, \ldots, -(n-1)$ (for $i=n+1, \ldots, 2n$).
$c_1=n-1, \ldots, c_n=0, c_{n+1}=0, c_{n+2}=-1, \ldots, c_{2n}=-(n-1)$.
This sequence $c_1, \ldots, c_{2n}$ is $(n-1, n-2, \ldots, 1, 0, 0, -1, -2, \ldots, -(n-1))$.
This list has $2n$ entries. The entry 0 appears twice, at $i=n$ and $i=n+1$. This matches the problem description for $n \ge 2$.

The characteristic polynomial is $P(\lambda) = \lambda^{2n} - \sum_{i=1}^{2n} c_i \lambda^{i-1}$.
$P(\lambda) = \lambda^{2n} - \sum_{i=1}^{n} (n-i) \lambda^{i-1} - \sum_{i=n+1}^{2n} -(n-(2n-i+1)) \lambda^{i-1}$.
Let $j=i-n$ in the second sum, so $i=n+j$ and $j$ goes from $1$ to $n$.
$P(\lambda) = \lambda^{2n} - \sum_{i=1}^{n} (n-i) \lambda^{i-1} - \sum_{j=1}^{n} -(j-1) \lambda^{n+j-1}$.
$P(\lambda) = \lambda^{2n} - \sum_{k=0}^{n-1} (n-1-k) \lambda^{k} + \sum_{k=n}^{2n-1} (k-n) \lambda^{k}$.
$P(\lambda) = \lambda^{2n} - \sum_{k=0}^{n-2} (n-1-k) \lambda^{k} - 0\lambda^{n-1} + 0\lambda^{n} + \sum_{k=n+1}^{2n-1} (k-n) \lambda^{k}$.
$P(\lambda) = \lambda^{2n} + \sum_{k=n+1}^{2n-1} (k-n) \lambda^{k} - \sum_{k=0}^{n-2} (n-1-k) \lambda^{k}$.
$P(\lambda) = \lambda^{2n} + \lambda^{n+1} + 2\lambda^{n+2} + \ldots + (n-1)\lambda^{2n-1} - [(n-1) + (n-2)\lambda + \ldots + \lambda^{n-2}]$.

The coefficients of $P(\lambda)$ in decreasing order of power are:
$\lambda^{2n}: 1$
$\lambda^{2n-1}: n-1$
$\lambda^{2n-2}: n-2$
...
$\lambda^{n+1}: 1$
$\lambda^{n}: 0$
$\lambda^{n-1}: 0$
$\lambda^{n-2}: -(n-2-(n-2)) = -1$ (mistake here in my scratchpad, it should be $-(n-1-(n-2))=-1$)
$k=n-2$ in $\sum_{k=0}^{n-2} (n-1-k)\lambda^k$: $(n-1-(n-2))\lambda^{n-2} = 1 \cdot \lambda^{n-2}$. So coeff is $-1$.
$\lambda^{n-3}: -(n-1-(n-3)) = -2$.
...
$\lambda^1: -(n-1-1) = -(n-2)$.
$\lambda^0: -(n-1-0) = -(n-1)$.

$P(\lambda) = \lambda^{2n} + (n-1)\lambda^{2n-1} + (n-2)\lambda^{2n-2} + \ldots + \lambda^{n+1} - \lambda^{n-2} - 2\lambda^{n-3} - \ldots - (n-2)\lambda - (n-1)$.
The sequence of coefficients is: $1, n-1, n-2, \ldots, 1, 0, 0, -1, -2, \ldots, -(n-2), -(n-1)$.
$P(0) = -(n-1) < 0$ for $n \ge 2$.
$P(1) = 1 + \sum_{k=n+1}^{2n-1} (k-n) - \sum_{k=0}^{n-2} (n-1-k)$.
$\sum_{k=n+1}^{2n-1} (k-n) = 1+2+\ldots+(n-1) = \frac{(n-1)n}{2}$.
$\sum_{k=0}^{n-2} (n-1-k) = (n-1)+(n-2)+\ldots+1 = \frac{(n-1)n}{2}$.
$P(1)=1+\frac{n(n-1)}{2} - \frac{n(n-1)}{2} = 1$.
Since $P(0)<0$ and $P(1)>0$, there is at least one real root between 0 and 1.

By Descartes' Rule of Signs, the number of positive real roots is at most the number of sign changes in the coefficients of $P(\lambda)$.
The signs are $+, +, \ldots, +, 0, 0, -, -, \ldots, -$. There is only one sign change (from $+$ to $-$).
So there is at most 1 positive real root. Since there is a root in $(0,1)$, there is exactly one positive real root.

Now consider the negative real roots by examining $P(-\lambda)$.
$P(-\lambda) = (-\lambda)^{2n} + \sum_{k=n+1}^{2n-1} (k-n) (-\lambda)^{k} - \sum_{k=0}^{n-2} (n-1-k) (-\lambda)^{k}$.
$P(-\lambda) = \lambda^{2n} + \sum_{k=n+1}^{2n-1} (k-n) (-1)^k \lambda^{k} - \sum_{k=0}^{n-2} (n-1-k) (-1)^k \lambda^{k}$.
Coefficients of $P(-\lambda)$:
$\lambda^{2n}: 1$ ($+$)
$\lambda^{k}$ for $n+1 \le k \le 2n-1$: $(k-n)(-1)^k$.
$k=2n-1: (n-1)(-1)^{2n-1} = -(n-1)$ ($-$)
$k=2n-2: (n-2)(-1)^{2n-2} = n-2$ ($+$)
$k=2n-3: (n-3)(-1)^{2n-3} = -(n-3)$ ($-$)
...
$k=n+1: (1)(-1)^{n+1}$ (sign is $(-1)^{n+1}$)
Signs for $\lambda^{2n}, \ldots, \lambda^{n+1}$: $+, -, +, -, \ldots, (-1)^{n+1}$. There are $(2n)-(n+1)+1=n$ terms. The number of sign changes is $n-1$.

Coefficients for $\lambda^{n}, \lambda^{n-1}$ are 0.

$\lambda^k$ for $0 \le k \le n-2$: $-(n-1-k)(-1)^k$.
$k=n-2: -(n-1-(n-2))(-1)^{n-2} = -1(-1)^{n-2} = (-1)^{n-1}$.
$k=n-3: -(n-1-(n-3))(-1)^{n-3} = -2(-1)^{n-3} = 2(-1)^{n-2}$.
...
$k=1: -(n-1-1)(-1)^1 = -(n-2)(-1) = n-2$ (for $n \ge 3$)
$k=0: -(n-1-0)(-1)^0 = -(n-1)$.
Signs for $\lambda^{n-2}, \ldots, \lambda^0$: $(-1)^{n-1}, (-1)^{n-2}, \ldots, (+ \text{ if } n \ge 3), (-)$.
Number of terms is $(n-2)-0+1=n-1$.
The sequence of signs is $S, -S, S, \ldots, (-1)^{n-3} S, (-1)^{n-2}(+), (-)$. $S=(-1)^{n-1}$.
Number of changes from $a_{n-2}$ to $a_1$: $n-3$ (for $n \ge 3$).
Sign $a_1$: $n-2 > 0$. Sign $a_0$: $-(n-1)<0$.
If $n \ge 3$, $a_1, a_0$ signs are $+, -$. 1 change.
Total changes from $\lambda^{n-2}$ to $\lambda^0$: $(n-3)+1 = n-2$ for $n \ge 3$.
For $n=2$: $n-2=0$. $k=0$ only. $a_0 = -(2-1)(-1)^0 = -1$. Sign is $-$. 0 changes. $n-2=0$.

Total number of sign changes in $P(-\lambda)$ for $n \ge 3$: $(n-1) + (n-2) = 2n-3$.
For $n=2$: $n-1=1$ (from $\lambda^4$ to $\lambda^3$). $n-2=0$ (from $\lambda^0$ to $\lambda^0$). Total $1+0=1$.
$2n-3 = 2(2)-3=1$. The formula $2n-3$ holds for $n \ge 2$.

By Descartes' Rule of Signs, the maximum number of negative real roots is $2n-3$.
The maximum number of real roots is $1 \text{ (positive)} + (2n-3) \text{ (negative)} = 2n-2$.
The characteristic polynomial has degree $2n$. The total number of roots is $2n$.
The minimum number of non-real roots is $2n - (\text{maximum number of real roots}) = 2n - (2n-2) = 2$.
Since non-real eigenvalues of a real matrix occur in conjugate pairs, the minimum number of non-real eigenvalues is 2.
Thus, $A$ has at least two non-real eigenvalues. This implies that $A$ has a non-real eigenvalue.

The final answer is $\boxed{A \text{ has a non-real eigenvalue}}$.