Of course. Here is a detailed, step-by-step solution to the problem. We will explore two common methods to arrive at the solution.

### **Problem Statement**

The roots of the cubic equation $x^3 + a x^2 + b x + c = 0$ are $\alpha,$ $\beta,$ and $\gamma$. We need to find the cubic polynomial whose roots are $\alpha^2$, $\beta^2$, and $\gamma^2$.

Let the original polynomial be $P(x) = x^3 + a x^2 + b x + c$.
Let the new polynomial be $Q(y)$, and its roots are $\alpha^2, \beta^2, \gamma^2$.

---

### **Method 1: Using Vieta's Formulas**

This method involves finding the coefficients of the new polynomial by expressing them in terms of the coefficients of the original polynomial.

**Step 1: Write down Vieta's formulas for the original polynomial.**

For the polynomial $P(x) = x^3 + a x^2 + b x + c = 0$ with roots $\alpha, \beta, \gamma$, Vieta's formulas give us the following relationships between the roots and coefficients:
1.  Sum of the roots: $\alpha + \beta + \gamma = -a$
2.  Sum of the products of the roots taken two at a time: $\alpha\beta + \beta\gamma + \gamma\alpha = b$
3.  Product of the roots: $\alpha\beta\gamma = -c$

**Step 2: Define the structure of the new polynomial.**

Let the new polynomial be $Q(y) = y^3 + A y^2 + B y + C = 0$. Its roots are $\alpha^2, \beta^2, \gamma^2$.
Using Vieta's formulas for $Q(y)$, its coefficients $A, B, C$ are given by:
*   $-A = \alpha^2 + \beta^2 + \gamma^2$ (Sum of the new roots)
*   $B = (\alpha^2)(\beta^2) + (\beta^2)(\gamma^2) + (\gamma^2)(\alpha^2)$ (Sum of the products of the new roots taken two at a time)
*   $-C = (\alpha^2)(\beta^2)(\gamma^2)$ (Product of the new roots)

Our goal is to find $A, B,$ and $C$ in terms of $a, b,$ and $c$.

**Step 3: Calculate the coefficient A.**

We need to compute $-A = \alpha^2 + \beta^2 + \gamma^2$. We can express this sum of squares using the identity:
$(\alpha + \beta + \gamma)^2 = \alpha^2 + \beta^2 + \gamma^2 + 2(\alpha\beta + \beta\gamma + \gamma\alpha)$

Rearranging this identity to solve for the sum of squares:
$\alpha^2 + \beta^2 + \gamma^2 = (\alpha + \beta + \gamma)^2 - 2(\alpha\beta + \beta\gamma + \gamma\alpha)$

Now, substitute the values from Step 1:
$\alpha^2 + \beta^2 + \gamma^2 = (-a)^2 - 2(b) = a^2 - 2b$

So, $-A = a^2 - 2b$, which means $A = -(a^2 - 2b) = 2b - a^2$.

**Step 4: Calculate the coefficient B.**

We need to compute $B = \alpha^2\beta^2 + \beta^2\gamma^2 + \gamma^2\alpha^2$. We can use a similar algebraic identity. Consider the square of the sum of products:
$(\alpha\beta + \beta\gamma + \gamma\alpha)^2 = (\alpha\beta)^2 + (\beta\gamma)^2 + (\gamma\alpha)^2 + 2(\alpha\beta\cdot\beta\gamma + \beta\gamma\cdot\gamma\alpha + \gamma\alpha\cdot\alpha\beta)$
$(\alpha\beta + \beta\gamma + \gamma\alpha)^2 = \alpha^2\beta^2 + \beta^2\gamma^2 + \gamma^2\alpha^2 + 2(\alpha\beta^2\gamma + \alpha\beta\gamma^2 + \alpha^2\beta\gamma)$

We can factor out $\alpha\beta\gamma$ from the last term:
$(\alpha\beta + \beta\gamma + \gamma\alpha)^2 = \alpha^2\beta^2 + \beta^2\gamma^2 + \gamma^2\alpha^2 + 2\alpha\beta\gamma(\beta + \gamma + \alpha)$

Rearranging to solve for the expression we need:
$\alpha^2\beta^2 + \beta^2\gamma^2 + \gamma^2\alpha^2 = (\alpha\beta + \beta\gamma + \gamma\alpha)^2 - 2\alpha\beta\gamma(\alpha + \beta + \gamma)$

Now, substitute the values from Step 1:
$B = (b)^2 - 2(-c)(-a) = b^2 - 2ac$

**Step 5: Calculate the coefficient C.**

We need to compute $-C = \alpha^2\beta^2\gamma^2$.
This can be written as:
$-C = (\alpha\beta\gamma)^2$

Substitute the value from Step 1:
$-C = (-c)^2 = c^2$

So, $C = -c^2$.

**Step 6: Assemble the new polynomial.**

Now we substitute the calculated coefficients $A, B,$ and $C$ into the form of our new polynomial $Q(y)$:
$Q(y) = y^3 + Ay^2 + By + C = 0$
$Q(y) = y^3 + (2b - a^2)y^2 + (b^2 - 2ac)y - c^2 = 0$

---

### **Method 2: Algebraic Manipulation**

This method is more direct. We start with the original equation and manipulate it to form a new equation whose variable is the square of the original variable.

**Step 1: Start with the given equation.**
We are given that $x$ is a root of $x^3 + a x^2 + b x + c = 0$.
The roots are $\alpha, \beta, \gamma$.

**Step 2: Let $y = x^2$.**
We want to find a polynomial in $y$. Our goal is to eliminate $x$ from the original equation and express it solely in terms of $y$.
From $y=x^2$, we have $x = \sqrt{y}$. Substituting this directly would introduce radicals, which we want to avoid. A better approach is to rearrange the equation to isolate terms with odd and even powers of $x$.

**Step 3: Rearrange the equation.**
Group terms with even powers of $x$ on one side and terms with odd powers on the other.
$x^3 + a x^2 + b x + c = 0$
$(x^3 + bx) + (ax^2 + c) = 0$
$x(x^2 + b) + (ax^2 + c) = 0$

Substitute $x^2 = y$:
$x(y + b) + (ay + c) = 0$

Now, isolate the term containing the single power of $x$:
$x(y + b) = -(ay + c)$

**Step 4: Square both sides to eliminate x.**
To eliminate the remaining $x$, we can square both sides of the equation. This is valid because if $u=v$, then $u^2=v^2$.
$[x(y + b)]^2 = [-(ay + c)]^2$
$x^2 (y + b)^2 = (ay + c)^2$

**Step 5: Substitute $x^2 = y$ and expand.**
Now substitute $x^2 = y$ into the left side:
$y(y + b)^2 = (ay + c)^2$

This is the polynomial whose roots are $\alpha^2, \beta^2, \gamma^2$. We just need to expand it and write it in standard form.
$y(y^2 + 2by + b^2) = a^2y^2 + 2acy + c^2$
$y^3 + 2by^2 + b^2y = a^2y^2 + 2acy + c^2$

**Step 6: Collect terms to write the polynomial in standard form.**
Move all terms to one side:
$y^3 + 2by^2 - a^2y^2 + b^2y - 2acy - c^2 = 0$
$y^3 + (2b - a^2)y^2 + (b^2 - 2ac)y - c^2 = 0$

This result matches the one obtained from Method 1.

---

### **Final Answer**

The cubic polynomial whose roots are $\alpha^2$, $\beta^2$, and $\gamma^2$ is:
$$ y^3 + (2b - a^2)y^2 + (b^2 - 2ac)y - c^2 = 0 $$
Or, written in terms of a variable $x$:
$$ x^3 + (2b - a^2)x^2 + (b^2 - 2ac)x - c^2 = 0 $$