# Solution

Let's prove that for any $a, b \in R$, there exists $d \in R$ such that $aba + bab = d^3$.

We'll split our proof into two cases: $a \neq b$ and $a = b$.

## Case 1: $a \neq b$

First, let's expand $(a+b)^3$:

$$(a+b)^3 = (a+b)(a+b)(a+b)$$

Expanding this expression:
$$(a+b)^3 = a^3 + a^2b + aba + ab^2 + ba^2 + bab + b^2a + b^3$$

By Property 2, when $a \neq b$, we have $a^2b = -ba^2$, which means $a^2b + ba^2 = 0$.
Similarly, applying Property 2 with roles reversed, $b^2a = -ab^2$, giving $b^2a + ab^2 = 0$.

Substituting these into our expansion:
\begin{align}
(a+b)^3 &= a^3 + (a^2b + ba^2) + aba + (ab^2 + b^2a) + bab + b^3 \\
&= a^3 + 0 + aba + 0 + bab + b^3 \\
&= a^3 + b^3 + aba + bab
\end{align}

By Property 1, there exists $c \in R$ such that $a^3 + b^3 = c^3$. Therefore:
\begin{align}
(a+b)^3 &= c^3 + aba + bab \\
\Rightarrow aba + bab &= (a+b)^3 - c^3
\end{align}

Applying Property 1 again with elements $(a+b)$ and $-c$, there exists $d \in R$ such that $(a+b)^3 + (-c)^3 = d^3$. Since $(-c)^3 = -c^3$ in any ring, we have:
$$(a+b)^3 - c^3 = d^3$$

Therefore, $aba + bab = d^3$ for some $d \in R$ when $a \neq b$.

## Case 2: $a = b$

If $a = b$, then:
\begin{align}
aba + bab &= aba + aba \\
&= 2(aba) \\
&= 2(aaa) \quad \text{(since $a = b$)} \\
&= 2a^3
\end{align}

By Property 1, for elements $a$ and $a$, there exists $e \in R$ such that $a^3 + a^3 = e^3$. This gives us $2a^3 = e^3$. 

Therefore, when $a = b$, we have $aba + bab = 2a^3 = e^3$ for some $e \in R$.

Combining both cases, we conclude that for any $a, b \in R$, there exists $d \in R$ such that $aba + bab = d^3$.