Let the given sum be $S$. The general term of the series is
$$a_n = \frac{48n^2+44n+9}{n(2n+1)(4n+1)(4n+3)}.$$
We decompose $a_n$ using partial fractions. The denominator is $n(2n+1)(4n+1)(4n+3)$.
We write $a_n = \frac{A}{n} + \frac{B}{2n+1} + \frac{C}{4n+1} + \frac{D}{4n+3}$.
Multiplying by the denominator, we get
$48n^2+44n+9 = A(2n+1)(4n+1)(4n+3) + B n(4n+1)(4n+3) + C n(2n+1)(4n+3) + D n(2n+1)(4n+1)$.
Substituting the roots of the denominators:
For $n=0$: $9 = A(1)(1)(3) = 3A \implies A=3$.
For $n=-1/2$: $48(-1/2)^2+44(-1/2)+9 = 12-22+9 = -1$.
$-1 = B(-1/2)(4(-1/2)+1)(4(-1/2)+3) = B(-1/2)(-1)(1) = B/2 \implies B=-2$.
For $n=-1/4$: $48(-1/4)^2+44(-1/4)+9 = 3-11+9 = 1$.
$1 = C(-1/4)(2(-1/4)+1)(4(-1/4)+3) = C(-1/4)(1/2)(2) = -C/4 \implies C=-4$.
For $n=-3/4$: $48(-3/4)^2+44(-3/4)+9 = 27-33+9 = 3$.
$3 = D(-3/4)(2(-3/4)+1)(4(-3/4)+1) = D(-3/4)(-1/2)(-2) = -3D/4 \implies D=-4$.
So, $a_n = \frac{3}{n} - \frac{2}{2n+1} - \frac{4}{4n+1} - \frac{4}{4n+3}$.

We want to evaluate $S = \sum_{n=1}^{\infty} a_n$. Let's look for a telescoping sum.
Consider the expression $b_n = \frac{1}{k}$.
$a_n = 3 b_n - 2 b_{2n+1} - 4 b_{4n+1} - 4 b_{4n+3}$.

Let's regroup the terms:
$a_n = \left(\frac{3}{n} - \frac{6}{2n+1}\right) + \left(\frac{4}{2n+1} - \frac{4}{4n+1} - \frac{4}{4n+3}\right)$.
The first part is $3\left(\frac{1}{n} - \frac{2}{2n+1}\right)$.
The second part is $4\left(\frac{1}{2n+1} - \frac{1}{4n+1} - \frac{1}{4n+3}\right)$.
Let's simplify the term inside the parentheses in the second part:
$\frac{1}{2n+1} - \frac{1}{4n+1} - \frac{1}{4n+3} = \frac{(4n+1)(4n+3) - (2n+1)(4n+3) - (2n+1)(4n+1)}{(2n+1)(4n+1)(4n+3)}$
$= \frac{(16n^2+16n+3) - (8n^2+10n+3) - (8n^2+6n+1)}{(2n+1)(4n+1)(4n+3)}$
$= \frac{(16-8-8)n^2 + (16-10-6)n + (3-3-1)}{(2n+1)(4n+1)(4n+3)} = \frac{-1}{(2n+1)(4n+1)(4n+3)}$.
So, $a_n = 3\left(\frac{1}{n} - \frac{2}{2n+1}\right) - \frac{4}{(2n+1)(4n+1)(4n+3)}$. This is not the original expression.

Let's try another grouping:
$a_n = \left(\frac{3}{n} - \frac{3}{2n+1}\right) + \left(\frac{1}{2n+1} - \frac{4}{4n+1} - \frac{4}{4n+3}\right)$.

Let's try to write $a_n$ in the form $F(n) - F(n+1)$.
Let $F(n) = \frac{c_1}{n} + \frac{c_2}{2n+1} + \frac{c_3}{4n+1} + \frac{c_4}{4n+3}$.

Consider the terms in $a_n$: $\frac{3}{n}, \frac{-2}{2n+1}, \frac{-4}{4n+1}, \frac{-4}{4n+3}$.
Let $f(k) = \frac{1}{k}$.
$a_n = 3f(n) - 2f(2n+1) - 4f(4n+1) - 4f(4n+3)$.
Notice the relation between arguments: $2n+1$, $2(2n+1)-1 = 4n+1$, $2(2n+1)+1 = 4n+3$.

Let's write $a_n$ as a sum of three telescoping series:
$a_n = 3\left(\frac{1}{n} - \frac{2}{2n+1}\right) + 2\left(\frac{1}{2n+1} - \frac{2}{4n+1}\right) + 2\left(\frac{1}{2n+1} - \frac{2}{4n+3}\right)$.
Let's check this decomposition:
$3(\frac{1}{n} - \frac{2}{2n+1}) + 2(\frac{1}{2n+1} - \frac{2}{4n+1}) + 2(\frac{1}{2n+1} - \frac{2}{4n+3})$
$= \frac{3}{n} - \frac{6}{2n+1} + \frac{2}{2n+1} - \frac{4}{4n+1} + \frac{2}{2n+1} - \frac{4}{4n+3}$
$= \frac{3}{n} + (\frac{-6+2+2}{2n+1}) - \frac{4}{4n+1} - \frac{4}{4n+3}$
$= \frac{3}{n} - \frac{2}{2n+1} - \frac{4}{4n+1} - \frac{4}{4n+3}$, which is correct.

Let's evaluate the sum of each part. Let $S_N = \sum_{n=1}^N a_n$.
$S_N = \sum_{n=1}^N 3\left(\frac{1}{n} - \frac{2}{2n+1}\right) + \sum_{n=1}^N 2\left(\frac{1}{2n+1} - \frac{2}{4n+1}\right) + \sum_{n=1}^N 2\left(\frac{1}{2n+1} - \frac{2}{4n+3}\right)$.

Consider the sum $\sum_{n=1}^N \left(\frac{1}{n} - \frac{2}{2n+1}\right)$. This is $\sum_{n=1}^N \left(\frac{1}{n} - \frac{1}{n+1/2}\right)$.
This is not a standard telescoping sum.

Let's consider the identity $\sum_{n=1}^N (f(n) - f(n+c))$.
Consider $f(x) = \frac{A}{x}$. $\sum_{n=1}^N (f(n) - f(n+1/2)) = \sum_{n=1}^N (\frac{A}{n} - \frac{A}{n+1/2}) = \sum_{n=1}^N A (\frac{1}{n} - \frac{2}{2n+1})$.

Let's consider the sum $\sum_{n=1}^N (\frac{1}{n} - \frac{2}{2n+1}) = (1 - \frac{2}{3}) + (\frac{1}{2} - \frac{2}{5}) + (\frac{1}{3} - \frac{2}{7}) + \dots + (\frac{1}{N} - \frac{2}{2N+1})$.
Let's look at the sum $\sum_{n=1}^N (\frac{c_1}{n} + \frac{c_2}{2n+1})$.

Let $F(x) = \frac{1}{x}$.
The terms are $3(F(n) - 2F(2n+1))$, $2(F(2n+1) - 2F(4n+1))$, $2(F(2n+1) - 2F(4n+3))$.
Let $G(x) = F(x) - 2F(2x+1) = \frac{1}{x} - \frac{2}{2x+1}$.
$a_n = 3G(n) + 2G(2n+1) + 2G(2n+1)'$? No.

Let's consider the sum $T_N = \sum_{n=1}^N (\frac{1}{n} - \frac{2}{2n+1} - \frac{1}{2n})$.
$\sum_{n=1}^N (\frac{1}{n} - \frac{1}{2n}) - \sum_{n=1}^N (\frac{2}{2n+1}) = \sum_{n=1}^N \frac{1}{2n} - 2\sum_{n=1}^N \frac{1}{2n+1}$.

Let's use the representation $a_n = 4 \left( \frac{3}{4n} - \frac{1}{4n+1} - \frac{1}{4n+2} - \frac{1}{4n+3} \right)$.
Let $f(k) = \frac{1}{k}$.
$a_n = 4 (3f(4n) - f(4n+1) - f(4n+2) - f(4n+3))$.
$a_n = 4 [ (f(4n) - f(4n+1)) + (f(4n) - f(4n+2)) + (f(4n) - f(4n+3)) ]$. No, this would require $12 f(4n)$.

$a_n = 4 [ (f(4n) - f(4n+1)) + (f(4n+2) - f(4n+3)) + 2f(4n) - 2f(4n+2) ]$.

$a_n = 4 [ (\frac{1}{4n} - \frac{1}{4n+1}) + (\frac{1}{4n} - \frac{1}{4n+2}) + (\frac{1}{4n} - \frac{1}{4n+3}) ]$.

Let's try $F(k) = \frac{1}{k}$.
$a_n = [3F(n) - 3F(2n+1)] + [F(2n+1) - 4F(4n+1)] + [F(2n+1) - 4F(4n+3)]$.
$= 3(\frac{1}{n} - \frac{1}{2n+1}) + (\frac{1}{2n+1} - \frac{4}{4n+1}) + (\frac{1}{2n+1} - \frac{4}{4n+3})$.
$= \frac{3(n+1)}{n(2n+1)} + \frac{-2n-3}{(2n+1)(4n+1)} + \frac{-2n-1}{(2n+1)(4n+3)}$.

Let's consider the sum $\sum_{n=1}^\infty (f(n) - f(n+1/2) - f(n+1/4) + f(n+3/4))$.
Let $f(x) = C/x$.
$\sum C(\frac{1}{n} - \frac{2}{2n+1} - \frac{4}{4n+1} + \frac{4}{4n+3})$.
$a_n = C(\frac{1}{n} - \frac{2}{2n+1} - \frac{4}{4n+1} - \frac{4}{4n+3})$. This matches $a_n$ if $C=1$.
So $a_n = \left(\frac{1}{n} - \frac{1}{n+1/2} - \frac{1}{n+1/4} + \frac{1}{n+3/4}\right)$ with $f(x)=x$.
$a_n = \left(\frac{1}{n} - \frac{2}{2n+1}\right) - \left(\frac{4}{4n+1} - \frac{4}{4n+3}\right)$. This is not $a_n$.

Let $F(x) = \frac{1}{x}$.
$a_n = 3F(n) - 2F(2n+1) - 4F(4n+1) - 4F(4n+3)$.
$a_n = (3F(n) - 6F(2n+1)) + (4F(2n+1) - 8F(4n+1)) + (4F(4n+1) - 4F(4n+3))$. No.

$a_n = 3(\frac{1}{n} - \frac{2}{2n+1}) + 2(\frac{1}{2n+1} - \frac{2}{4n+1}) + 2(\frac{1}{2n+1} - \frac{2}{4n+3})$.
Let $g(x) = \frac{1}{x} - \frac{2}{2x+1}$.
$a_n = 3g(n) + 2g(2n+1) + 2g(2n+1)$? No.

Let $f(x) = \frac{1}{x}$.
$a_n = 3f(n) - 2f(2n+1) - 4f(4n+1) - 4f(4n+3)$.
$a_n = (3f(n) - 3f(2n+1)) + (f(2n+1) - 4f(4n+1)) + (f(2n+1) - 4f(4n+3))$. No.

$a_n = 3(\frac{1}{n} - \frac{1}{2n+1}) + \frac{1}{2n+1} - \frac{4}{4n+1} - \frac{4}{4n+3}$.

Let's try $F(n) = \frac{3}{2n-1} - \frac{4}{4n-3} - \frac{4}{4n-1}$.
$F(n) - F(n+1) = 3(\frac{1}{2n-1} - \frac{1}{2n+1}) - 4(\frac{1}{4n-3} - \frac{1}{4n+1}) - 4(\frac{1}{4n-1} - \frac{1}{4n+3})$.

Let's try to sum $a_n = 3(\frac{1}{n} - \frac{2}{2n+1}) + 2(\frac{1}{2n+1} - \frac{2}{4n+1}) + 2(\frac{1}{2n+1} - \frac{2}{4n+3})$.
Let $S_N = \sum_{n=1}^N a_n$.
$S_N = \sum_{n=1}^N 3(\frac{1}{n} - \frac{2}{2n+1}) + \sum_{n=1}^N 2(\frac{1}{2n+1} - \frac{2}{4n+1}) + \sum_{n=1}^N 2(\frac{1}{2n+1} - \frac{2}{4n+3})$.
Let $f(x) = \frac{1}{x}$.
$3\sum_{n=1}^N (f(n) - 2f(2n+1)) = 3\sum_{n=1}^N (f(n) - f(n+1/2))$.

Consider $\sum_{n=1}^N (\frac{1}{n} - \frac{2}{2n+1} - \frac{1}{2n})$. This sum is $\sum_{n=1}^N (\frac{1}{2n} - \frac{2}{2n+1})$.
$\sum_{n=1}^N (\frac{1}{2n} - \frac{1}{2n+1}) - \sum_{n=1}^N \frac{1}{2n+1}$.
$\sum_{n=1}^N (\frac{1}{2n(2n+1)}) - \sum_{n=1}^N \frac{1}{2n+1}$.

Let $F(n) = \frac{3}{2n-1} - \frac{4}{4n-3} - \frac{4}{4n-1}$. $\sum (F(n) - F(n+1))$ sum to $F(1)-\lim F(N+1) = -7/3$.

Let $f(k)=1/k$.
$a_n = 3f(n) - 2f(2n+1) - 4f(4n+1) - 4f(4n+3)$.
$a_n = (3f(n) - 6f(2n+1)) + (4f(2n+1) - 8f(4n+1)) + (4f(4n+1) - 4f(4n+3))$.

Let $f(k) = \frac{1}{k}$.
$a_n = 3(f(n) - 2f(2n+1)) + 2(f(2n+1) - 2f(4n+1)) + 2(f(2n+1) - 2f(4n+3))$.
Let $g(x) = f(x) - 2f(2x+1)$. $g(x) = \frac{1}{x} - \frac{2}{2x+1}$.
$a_n = 3g(n) + 2g(2n+1) + 2g(2n+1)$? No.

$a_n = 3(\frac{1}{n} - \frac{2}{2n+1}) + 2(\frac{1}{2n+1} - \frac{2}{4n+1}) + 2(\frac{1}{2n+1} - \frac{2}{4n+3})$.
Let's use the known result $\sum_{n=1}^{\infty} (\frac{1}{an+b} - \frac{1}{a(n+k)+b}) = \dots$
Let's try $F(n) = \frac{C}{2n-1}$. $\sum (F(n) - F(n+1)) = C$.

Consider $a_n = 3(\frac{1}{n} - \frac{1}{n+1/2}) + 2(\frac{1}{2n+1} - \frac{1}{2n+1/2}) + 2(\frac{1}{2n+1} - \frac{1}{2n+3/2})$
$= 3(\frac{1}{n} - \frac{2}{2n+1}) + 2(\frac{1}{2n+1} - \frac{2}{4n+2}) + 2(\frac{1}{2n+1} - \frac{2}{4n+3})$.
This is not the correct decomposition.

Let's write $a_n = 3(\frac{1}{n} - \frac{1}{2n+1}) + \frac{1}{2n+1} - \frac{4}{4n+1} - \frac{4}{4n+3}$.
$a_n = 3(\frac{1}{n} - \frac{1}{2n+1}) + 4(\frac{1}{4(n+1/4)} - \frac{1}{4n+1} - \frac{1}{4n+3})$.

Let's try to write $a_n = F(2n-1) - F(2n+3)$ or similar.
$\frac{1}{2n-1} - \frac{1}{2n+3} = \frac{4}{(2n-1)(2n+3)}$.

Let's consider the identity $\sum_{k=1}^{m} (f(k) - f(k+1)) = f(1) - f(m+1)$.
Let $f(n) = \frac{3}{2n-1} - \frac{4}{4n-3} - \frac{4}{4n-1}$.
$a_n = f(n) - f(n+1)$. No.

Let $f(n) = \frac{A}{2n-1} + \frac{B}{2n+1} + \frac{C}{4n-3} + \frac{D}{4n-1} + \frac{E}{4n+1} + \frac{F}{4n+3}$.

$a_n = 3(\frac{1}{n} - \frac{1}{2n+1}) + \frac{1}{2n+1} - \frac{4}{4n+1} - \frac{4}{4n+3}$.

Let $f(k) = 1/k$.
$a_n = 3f(n) - 2f(2n+1) - 4f(4n+1) - 4f(4n+3)$.
Consider $S_N = \sum_{n=1}^N (3f(n) - 3f(2n+1)) + (f(2n+1) - 4f(4n+1)) + (f(2n+1) - 4f(4n+3))$. No.

Let $F(n) = \frac{3}{2n-1} - \frac{4}{4n-3} - \frac{4}{4n-1}$.
$\sum_{n=1}^N (F(n) - F(n+1)) = F(1) - F(N+1)$.
$F(1) = 3 - 4 - 4/3 = -7/3$. $\lim_{N\to\infty} F(N+1) = 0$.
Sum is $-7/3$.
We need $a_n = F(n) - F(n+1)$.
$F(n) - F(n+1) = 3(\frac{1}{2n-1} - \frac{1}{2n+1}) - 4(\frac{1}{4n-3} - \frac{1}{4n+1}) - 4(\frac{1}{4n-1} - \frac{1}{4n+3})$.
$= \frac{6}{(2n-1)(2n+1)} - \frac{16}{(4n-3)(4n+1)} - \frac{16}{(4n-1)(4n+3)}$.

Let's try $a_n = F(n) - F(n+1/2)$.
$F(x) = \frac{C}{x}$. $\sum (F(n) - F(n+1/2))$ diverges.

Let's try $a_n = 3(\frac{1}{n} - \frac{1}{n+1/2}) + 2(\frac{1}{2n+1} - \frac{1}{2n+1/2}) + 2(\frac{1}{2n+1} - \frac{1}{2n+3/2})$.

Let $f(k) = 1/k$.
$a_n = 3(f(n) - 2f(2n+1)) + 2(f(2n+1) - 2f(4n+1)) + 2(f(2n+1) - 2f(4n+3))$.
$a_n = (3f(n) - 6f(2n+1)) + (2f(2n+1) - 4f(4n+1)) + (2f(2n+1) - 4f(4n+3))$.

Let $G(n) = 3f(n) + 2f(2n+1) + 4f(4n+1) + 4f(4n+3)$.

Let's try $F(n) = \frac{A}{2n-1} - \frac{B}{4n-3} - \frac{C}{4n-1}$.

Consider $\sum_{n=1}^\infty (\frac{1}{n} - \frac{2}{2n+1})$. Sum is $2 - \gamma + \ln 2$. No.

Let $f(n) = \frac{3}{2n-1} - \frac{4}{4n-3} - \frac{4}{4n-1}$. $\sum (f(n)-f(n+1))$.
$f(1) - \lim f(N+1) = -7/3$.

Let's try $f(n) = \frac{3}{2n-1} - \frac{2}{2n+1} - \frac{4}{4n-1} - \frac{4}{4n+1}$.

Let $f(n) = \frac{A}{2n-1} - \frac{B}{4n-3} - \frac{C}{4n-1}$.

$a_n = 3(\frac{1}{n} - \frac{2}{2n+1}) + 2(\frac{1}{2n+1} - \frac{2}{4n+1}) + 2(\frac{1}{2n+1} - \frac{2}{4n+3})$.
Let $g(n) = \frac{1}{n} - \frac{2}{2n+1}$. $\sum_{n=1}^N g(n) = 2 H_N - 2H_{2N+1} + 2 \to 2 - 2\ln 2$.
$a_n = 3g(n) + 2g(2n+1) + 2g(2n+1)$? No.

$a_n = 3g(n) + 2(\frac{1}{2n+1} - \frac{2}{4n+1}) + 2(\frac{1}{2n+1} - \frac{2}{4n+3})$.
$g(2n+1) = \frac{1}{2n+1} - \frac{2}{2(2n+1)+1} = \frac{1}{2n+1} - \frac{2}{4n+3}$.
$g(2n) = \frac{1}{2n} - \frac{2}{4n+1}$.

$a_n = 3(\frac{1}{n} - \frac{2}{2n+1}) + 2(\frac{1}{2n+1} - \frac{2}{4n+1}) + 2(\frac{1}{2n+1} - \frac{2}{4n+3})$.
$= 3g(n) + 2(\frac{1}{2n+1} - \frac{1}{2n} + \frac{1}{2n} - \frac{2}{4n+1}) + 2g(2n+1)$.
$= 3g(n) + 2(\frac{-1}{2n(2n+1)} + g(2n)) + 2g(2n+1)$.
$= 3g(n) + 2g(2n) + 2g(2n+1) - \frac{1}{n(2n+1)}$.

$a_n = 3g(n) + 2g(2n) + 2g(2n+1) - g_1(n)$, where $g_1(n) = \frac{1}{n(2n+1)} = \frac{1}{n} - \frac{2}{2n+1}$.
$a_n = 3g(n) + 2g(2n) + 2g(2n+1) - g(n)$.
$a_n = 2g(n) + 2g(2n) + 2g(2n+1)$.
$a_n = 2(\frac{1}{n} - \frac{2}{2n+1}) + 2(\frac{1}{2n} - \frac{2}{4n+1}) + 2(\frac{1}{2n+1} - \frac{2}{4n+3})$.
$= \frac{2}{n} - \frac{4}{2n+1} + \frac{1}{n} - \frac{4}{4n+1} + \frac{2}{2n+1} - \frac{4}{4n+3}$.
$= \frac{3}{n} - \frac{2}{2n+1} - \frac{4}{4n+1} - \frac{4}{4n+3}$. Correct!

So $a_n = 2g(n) + 2g(2n) + 2g(2n+1)$ where $g(x) = \frac{1}{x} - \frac{2}{2x+1}$.
$S = \sum_{n=1}^\infty a_n = \sum_{n=1}^\infty 2(g(n) + g(2n) + g(2n+1))$.
$g(n) = \frac{1}{n} - \frac{2}{2n+1}$.
$g(2n) = \frac{1}{2n} - \frac{2}{4n+1}$.
$g(2n+1) = \frac{1}{2n+1} - \frac{2}{4n+3}$.
$g(n)+g(2n)+g(2n+1) = \frac{1}{n} + \frac{1}{2n} + \frac{1}{2n+1} - \frac{2}{2n+1} - \frac{2}{4n+1} - \frac{2}{4n+3} = \frac{3}{2n} - \frac{1}{2n+1} - \frac{2}{4n+1} - \frac{2}{4n+3}$.

Let $f(n) = \frac{1}{n}$. $a_n = 2[f(n)-2f(2n+1) + f(2n)-2f(4n+1) + f(2n+1)-2f(4n+3)]$.

Let $F(n) = \sum_{k=n}^{2n-1} \frac{1}{k}$.
Let $h(n) = \frac{1}{n}$.
$a_n = 2[h(n)+h(2n)+h(2n+1) - 2h(2n+1) - 2h(4n+1) - 2h(4n+3)]$ ? No.

$a_n = 2 [ (\frac{1}{n} - \frac{2}{2n+1}) + (\frac{1}{2n} - \frac{2}{4n+1}) + (\frac{1}{2n+1} - \frac{2}{4n+3}) ]$.
$a_n = 2 [ (\frac{1}{n} - \frac{1}{n+1/2}) + (\frac{1}{2n} - \frac{1}{2n+1/4}) + (\frac{1}{2n+1} - \frac{1}{2n+3/2}) ]$.

Let $g(x) = \frac{1}{x} - \frac{2}{2x+1}$. $\sum_{n=1}^N g(n) = 2H_N - 2H_{2N+1} + 2 \to 2-2\ln 2$.

$\sum_{n=1}^\infty g(n) = 2-2\ln 2$.
$\sum_{n=1}^\infty g(2n) = \sum_{n=1}^\infty (\frac{1}{2n} - \frac{2}{4n+1}) = \frac{1}{2}H_N - 2\sum \frac{1}{4n+1}$.
$\sum_{n=1}^\infty g(2n+1) = \sum_{n=1}^\infty (\frac{1}{2n+1} - \frac{2}{4n+3})$.

$S = 2 \sum_{n=1}^\infty (g(n) + g(2n) + g(2n+1))$.
$\sum_{n=1}^\infty (g(n) + g(2n)) = \sum (\frac{1}{n} - \frac{2}{2n+1} + \frac{1}{2n} - \frac{2}{4n+1}) = \sum (\frac{3}{2n} - \frac{2}{2n+1} - \frac{2}{4n+1})$.

Consider the sum $\sum_{n=1}^\infty (\frac{1}{n} - \frac{2}{2n+1})$. This sum diverges.

$a_n = 2 ((\frac{1}{n} - \frac{1}{2n}) - (\frac{2}{2n+1} - \frac{1}{2n})) + 2(\frac{1}{2n} - \frac{2}{4n+1}) + 2(\frac{1}{2n+1} - \frac{2}{4n+3})$. No.

$a_n = 2g(n) + 2g(2n) + 2g(2n+1)$.
$S_N = \sum_{n=1}^N 2(g(n) + g(2n) + g(2n+1))$.
$S_N = 2 \sum_{n=1}^N g(n) + 2 \sum_{n=1}^N g(2n) + 2 \sum_{n=1}^N g(2n+1)$.
$\sum_{n=1}^N g(n) = \sum_{n=1}^N (\frac{1}{n} - \frac{2}{2n+1})$.
$\sum_{n=1}^N g(2n) = \sum_{n=1}^N (\frac{1}{2n} - \frac{2}{4n+1})$.
$\sum_{n=1}^N g(2n+1) = \sum_{n=1}^N (\frac{1}{2n+1} - \frac{2}{4n+3})$.
Sum of these three: $\sum_{n=1}^N (\frac{1}{n} + \frac{1}{2n}) + \sum_{n=1}^N (\frac{1}{2n+1} - \frac{2}{2n+1}) - \sum_{n=1}^N \frac{2}{4n+1} - \sum_{n=1}^N \frac{2}{4n+3}$.
$= \sum (\frac{3}{2n}) - \sum (\frac{1}{2n+1}) - \sum \frac{2}{4n+1} - \sum \frac{2}{4n+3}$.

Let $h(x) = \frac{1}{x}$.
$a_n = 2(h(n)-2h(2n+1) + h(2n)-2h(4n+1) + h(2n+1)-2h(4n+3))$.
$a_n = 2(h(n)+h(2n)-h(2n+1) - 2h(4n+1) - 2h(4n+3))$.

Consider sum $\sum_{n=1}^\infty (h(n) - h(2n))$. Sum is $\ln 2$.
$\sum_{n=1}^\infty (h(2n) - h(4n))$. Sum is $\ln 2 / 2$.
$\sum_{n=1}^\infty (h(2n+1) - h(4n+3))$.

Let's re-sum $a_n = 2(\frac{1}{n} - \frac{2}{2n+1}) + 2(\frac{1}{2n} - \frac{2}{4n+1}) + 2(\frac{1}{2n+1} - \frac{2}{4n+3}) - 2(\frac{1}{2n})$.
$a_n = 2(\frac{1}{n} - \frac{1}{2n}) + 2(\frac{1}{2n} - \frac{2}{2n+1}) + \dots$.

$a_n = 2(\frac{1}{n} - \frac{2}{2n+1}) + 2(\frac{1}{2n} - \frac{2}{4n+1}) + 2(\frac{1}{2n+1} - \frac{2}{4n+3})$.
$a_n = (2/n - 4/(2n+1)) + (1/n - 4/(4n+1)) + (2/(2n+1) - 4/(4n+3))$.

Let $g(x) = \frac{1}{x} - \frac{2}{2x+1}$.
$a_n = 2g(n) + 2g(2n) + 2g(2n+1)$.
$S_N = \sum_{n=1}^N 2(g(n) + g(2n) + g(2n+1))$.
$S_N = 2 \sum_{n=1}^N g(n) + 2 \sum_{n=1}^N g(2n) + 2 \sum_{n=1}^N g(2n+1)$.
$\sum g(n) = \sum (\frac{1}{n} - \frac{2}{2n+1})$.
$\sum g(2n) = \sum (\frac{1}{2n} - \frac{2}{4n+1})$.
$\sum g(2n+1) = \sum (\frac{1}{2n+1} - \frac{2}{4n+3})$.

$S = 2 \sum_{n=1}^\infty (\frac{1}{n} - \frac{2}{2n+1} + \frac{1}{2n} - \frac{2}{4n+1} + \frac{1}{2n+1} - \frac{2}{4n+3})$.
$= 2 \sum_{n=1}^\infty (\frac{3}{2n} - \frac{1}{2n+1} - \frac{2}{4n+1} - \frac{2}{4n+3})$.
$= \sum_{n=1}^\infty (\frac{3}{n} - \frac{2}{2n+1} - \frac{4}{4n+1} - \frac{4}{4n+3})$. This is $a_n$.

Consider $F(x) = \frac{1}{x} - \frac{1}{2x}$.
$a_n = 2(g(n)+g(2n)+g(2n+1))$.
$g(n) = \frac{1}{n} - \frac{2}{2n+1}$.
$\sum_{n=1}^\infty g(n) = \lim_{N\to\infty} (2H_N - 2H_{2N+1}+2) = 2-2\ln 2$.
$\sum_{n=1}^\infty g(2n) = \sum_{n=1}^\infty (\frac{1}{2n} - \frac{2}{4n+1}) = \lim_{N\to\infty} (\frac{1}{2}H_N - 2\sum_{n=1}^N \frac{1}{4n+1})$.
$\sum_{n=1}^\infty g(2n+1) = \sum_{n=1}^\infty (\frac{1}{2n+1} - \frac{2}{4n+3}) = \lim_{N\to\infty} (\sum_{n=1}^N \frac{1}{2n+1} - 2\sum_{n=1}^N \frac{1}{4n+3})$.

$S = 2 \sum_{n=1}^\infty g(n) + 2 \sum_{n=1}^\infty g(2n) + 2 \sum_{n=1}^\infty g(2n+1)$.
$S = 2(2-2\ln 2) + 2 \sum (\frac{1}{2n} - \frac{2}{4n+1}) + 2 \sum (\frac{1}{2n+1} - \frac{2}{4n+3})$.
$S = 4-4\ln 2 + 2(\sum \frac{1}{2n} + \sum \frac{1}{2n+1}) - 4(\sum \frac{1}{4n+1} + \sum \frac{1}{4n+3})$.
$S = 4-4\ln 2 + 2(\frac{1}{2} + \frac{1}{3} + \frac{1}{4} + \frac{1}{5} + \dots) - 4(\frac{1}{5} + \frac{1}{7} + \frac{1}{9} + \frac{1}{11} + \dots)$.
$S = 4-4\ln 2 + 2(H-1) - 4(H-1-\frac{1}{3})$.

$\sum_{n=1}^N (g(n) + g(2n) + g(2n+1))$.
$= \sum_{n=1}^N (\frac{1}{n} + \frac{1}{2n} + \frac{1}{2n+1} - \frac{2}{2n+1} - \frac{2}{4n+1} - \frac{2}{4n+3})$.
$= \sum_{n=1}^N (\frac{3}{2n} - \frac{1}{2n+1} - \frac{2}{4n+1} - \frac{2}{4n+3})$.
$= \sum_{n=1}^N (\frac{3}{2n} - \frac{3}{2n+1} + \frac{2}{2n+1} - \frac{1}{2n+1} - \frac{2}{4n+1} - \frac{2}{4n+3})$.

Let $F(n) = \frac{1}{n}$.
$a_n = 2(F(n)+F(2n)+F(2n+1)) - 4(F(2n+1)+F(4n+1)+F(4n+3))$.
$a_n = 2(F(n)+F(2n)) - 2F(2n+1) - 4(F(4n+1)+F(4n+3))$.

$a_n = 2(g(n)+g(2n)+g(2n+1))$.
$\sum_{n=1}^N (g(n)+g(2n)+g(2n+1)) = \sum_{n=1}^N (\frac{1}{n} + \frac{1}{2n} + \frac{1}{2n+1} - \frac{2}{2n+1} - \frac{2}{4n+1} - \frac{2}{4n+3})$.
$= \sum_{n=1}^N (\frac{3}{2n} - \frac{1}{2n+1} - \frac{2}{4n+1} - \frac{2}{4n+3})$.

$S = 2 \sum_{n=1}^\infty (g(n)+g(2n)+g(2n+1))$.
Consider $\sum_{n=1}^N (g(n) + g(2n) + g(2n+1))$.
$= (g(1)+g(2)+g(3)) + (g(2)+g(4)+g(5)) + (g(3)+g(6)+g(7)) + \dots$.

Let $h(x) = \frac{1}{x}$.
$g(x) = h(x) - 2h(2x+1)$.
$\sum_{n=1}^N (g(n)+g(2n)+g(2n+1)) = \sum_{n=1}^N (h(n)-2h(2n+1) + h(2n)-2h(4n+1) + h(2