

To solve the problem, we utilize the Cayley-Hamilton theorem. Given that $1$ is an eigenvalue of $M$ with algebraic multiplicity $3$, the characteristic polynomial of $M$ is $(\lambda - 1)^3 = \lambda^3 - 3\lambda^2 + 3\lambda - 1$. By Cayley-Hamilton, $M$ satisfies its own characteristic equation:

\[
M^3 = 3M^2 - 3M + I_3.
\]

We seek coefficients $a_m, b_m, c_m$ such that $M^m = a_m M^2 + b_m M + c_m I_3$ for $m \geq 3$. Using the recurrence relation from the characteristic equation, we derive:

\[
M^m = 3M^{m-1} - 3M^{m-2} + M^{m-3}.
\]

Expressing each power in terms of $M^2$, $M$, and $I_3$, we derive a system of recurrence relations for the coefficients:

\[
\begin{cases}
a_m = 3a_{m-1} + b_{m-1}, \\
b_m = -3a_{m-1} + c_{m-1}, \\
c_m = a_{m-1}.
\end{cases}
\]

By solving these recurrences with initial conditions from lower powers, we find the closed-form expressions:

\[
a_m = \frac{m(m-1)}{2}, \quad b_m = -m(m-2), \quad c_m = \frac{(m-1)(m-2)}{2}.
\]

**Final Answer:**

For any natural number \( m \geq 3 \), the coefficients are:

\[
a_m = \boxed{\frac{m(m-1)}{2}}, \quad b_m = \boxed{-m(m-2)}, \quad c_m = \boxed{\frac{(m-1)(m-2)}{2}}.
\]