# Solution

I'll solve this problem by analyzing the recurrence relation step-by-step and determining the asymptotic behavior of the sequence.

## Initial Analysis

Given information:
- $x_0 \in \mathbb{N}$
- $\beta \in \mathbb{N}$
- $\alpha \in (0,\infty) \setminus \mathbb{Q}$ (positive irrational)
- $\beta - \alpha \in (0,1)$
- $\alpha^2 \in \mathbb{N}$
- Recurrence relation: $x_{n+1} = \beta x_n + \lfloor \alpha x_n \rfloor$ for $n \geq 0$

Let's define $y_n = \{\alpha x_n\} = \alpha x_n - \lfloor \alpha x_n \rfloor$, which represents the fractional part of $\alpha x_n$.

## Deriving a Simplified Recurrence

Using the identity $\lfloor \alpha x_n \rfloor = \alpha x_n - \{\alpha x_n\} = \alpha x_n - y_n$, we can rewrite the recurrence relation:

$$x_{n+1} = \beta x_n + \lfloor \alpha x_n \rfloor = \beta x_n + \alpha x_n - y_n = (\alpha + \beta)x_n - y_n$$

This gives us a cleaner form to work with.

## Finding a Recurrence for $y_n$

Now, let's determine how $y_n$ evolves:

$$y_{n+1} = \{\alpha x_{n+1}\} = \{\alpha((\alpha + \beta)x_n - y_n)\} = \{\alpha^2 x_n + \alpha\beta x_n - \alpha y_n\}$$

Since $\alpha^2 \in \mathbb{N}$ and $x_n \in \mathbb{N}$, we have $\alpha^2 x_n \in \mathbb{N}$, so $\{\alpha^2 x_n\} = 0$.

Therefore:
$$y_{n+1} = \{\alpha\beta x_n - \alpha y_n\}$$

We can write $\alpha x_n = \lfloor \alpha x_n \rfloor + y_n$, which gives:
$$\alpha\beta x_n = \beta(\lfloor \alpha x_n \rfloor + y_n) = \beta\lfloor \alpha x_n \rfloor + \beta y_n$$

Since $\beta\lfloor \alpha x_n \rfloor \in \mathbb{N}$, its fractional part is zero. This simplifies to:
$$y_{n+1} = \{\beta y_n - \alpha y_n\} = \{(\beta - \alpha)y_n\}$$

Since $\beta - \alpha \in (0,1)$ and $y_n \in [0,1)$, we know $(\beta - \alpha)y_n \in [0,1)$, so:
$$y_{n+1} = (\beta - \alpha)y_n$$

Solving this recurrence relation, we get:
$$y_n = (\beta - \alpha)^n y_0 = (\beta - \alpha)^n \{\alpha x_0\}$$

## Computing the Limit

Let's define $z_n = \frac{x_n}{(\alpha + \beta)^n}$ to express our target limit.

From our simplified recurrence, we have:
$$x_{n+1} = (\alpha + \beta)x_n - y_n$$

Dividing by $(\alpha + \beta)^{n+1}$:
$$\frac{x_{n+1}}{(\alpha + \beta)^{n+1}} = \frac{(\alpha + \beta)x_n}{(\alpha + \beta)^{n+1}} - \frac{y_n}{(\alpha + \beta)^{n+1}}$$

$$z_{n+1} = z_n - \frac{y_n}{(\alpha + \beta)^{n+1}}$$

Expanding recursively:
$$z_n = z_0 - \sum_{i=0}^{n-1} \frac{y_i}{(\alpha + \beta)^{i+1}} = x_0 - \sum_{i=0}^{n-1} \frac{(\beta - \alpha)^i\{\alpha x_0\}}{(\alpha + \beta)^{i+1}}$$

As $n \to \infty$, this becomes:
$$\lim_{n \to \infty} z_n = x_0 - \{\alpha x_0\}\sum_{i=0}^{\infty} \frac{(\beta - \alpha)^i}{(\alpha + \beta)^{i+1}}$$

This sum is a geometric series with first term $\frac{1}{\alpha + \beta}$ and ratio $\frac{\beta - \alpha}{\alpha + \beta}$. Since $0 < \beta - \alpha < 1$ and $\alpha + \beta > 1$, this ratio is between 0 and 1, ensuring convergence.

The sum equals:
$$\sum_{i=0}^{\infty} \frac{(\beta - \alpha)^i}{(\alpha + \beta)^{i+1}} = \frac{1}{\alpha + \beta}\cdot\frac{1}{1-\frac{\beta-\alpha}{\alpha+\beta}} = \frac{1}{\alpha + \beta}\cdot\frac{\alpha+\beta}{2\alpha} = \frac{1}{2\alpha}$$

Therefore:
$$\lim_{n \to \infty} \frac{x_n}{(\alpha + \beta)^n} = x_0 - \frac{\{\alpha x_0\}}{2\alpha}$$

## Final Answer

$$\boxed{\lim_{n\to\infty} \frac{x_n}{(\alpha + \beta)^n} = x_0 - \frac{\{\alpha x_0\}}{2\alpha}}$$