Let the given equation be
$$x P(x-2) = (x-2024)P(x) \quad (*)$$
This equation must hold for all $x \in \mathbb{R}$. $P(x)$ is a real polynomial.

First, let's test some specific values for $x$.
Setting $x=0$ in $(*)$, we get $0 \cdot P(-2) = (0-2024) P(0)$, which simplifies to $0 = -2024 P(0)$. This implies $P(0)=0$.
Since $x=0$ is a root of $P(x)$, we can write $P(x) = x P_1(x)$ for some polynomial $P_1(x)$.
Substituting this into $(*)$:
$x [(x-2) P_1(x-2)] = (x-2024) [x P_1(x)]$
For $x \neq 0$, we can divide by $x$:
$(x-2) P_1(x-2) = (x-2024) P_1(x)$
Since this polynomial equation holds for all $x \neq 0$, it must hold for all $x \in \mathbb{R}$.

Setting $x=2$ in this new equation, we get $(2-2) P_1(2-2) = (2-2024) P_1(2)$, which simplifies to $0 \cdot P_1(0) = -2022 P_1(2)$. This implies $0 = -2022 P_1(2)$, so $P_1(2)=0$.
Since $x=2$ is a root of $P_1(x)$, we can write $P_1(x) = (x-2) P_2(x)$ for some polynomial $P_2(x)$.
Substituting this into the equation for $P_1(x)$:
$(x-2) [(x-2-2) P_2(x-2)] = (x-2024) [(x-2) P_2(x)]$
$(x-2)(x-4) P_2(x-2) = (x-2024)(x-2) P_2(x)$
For $x \neq 2$, we can divide by $(x-2)$:
$(x-4) P_2(x-2) = (x-2024) P_2(x)$
This equation must hold for all $x \in \mathbb{R}$.

We can see a pattern emerging. Let's state it formally.
Let $P_0(x) = P(x)$. We have $P_k(x)$ satisfying $(x-2k) P_k(x-2) = (x-2024) P_k(x)$.
We showed $P_0(0)=0$. From the equation for $P_k$, setting $x=2k$, we get $(2k-2k) P_k(2k-2) = (2k-2024) P_k(2k)$, which is $0 = (2k-2024) P_k(2k)$.
If $2k \neq 2024$, this implies $P_k(2k)=0$.
So, $P_1(2)=0$, $P_2(4)=0$, ..., $P_{1011}(2022)=0$.
Since $P_k(2k)=0$ (for $k \neq 1012$), we can write $P_k(x) = (x-2k) P_{k+1}(x)$.
Substituting this into the equation for $P_k$:
$(x-2k) [(x-2-2k) P_{k+1}(x-2)] = (x-2024) [(x-2k) P_{k+1}(x)]$
For $x \neq 2k$, we divide by $(x-2k)$:
$(x-2(k+1)) P_{k+1}(x-2) = (x-2024) P_{k+1}(x)$
This confirms the recursive structure of the equation for $P_{k+1}$.

This process continues as long as $k \neq 1012$. We have
$P(x) = P_0(x) = x P_1(x) = x(x-2) P_2(x) = \dots = x(x-2)\dots(x-2k) P_{k+1}(x)$.
Let's apply this up to $k=1011$.
$P(x) = x(x-2)(x-4)\dots(x-2020) P_{1011}(x)$.
The equation for $P_{1011}(x)$ is
$(x-2(1011)) P_{1011}(x-2) = (x-2024) P_{1011}(x)$
$(x-2022) P_{1011}(x-2) = (x-2024) P_{1011}(x)$.
We also know $P_{1011}(2 \cdot 1011) = P_{1011}(2022)=0$.
Since $P_{1011}(2022)=0$, we can write $P_{1011}(x) = (x-2022) P_{1012}(x)$ for some polynomial $P_{1012}(x)$.
Substituting this into the equation for $P_{1011}(x)$:
$(x-2022) [(x-2-2022) P_{1012}(x-2)] = (x-2024) [(x-2022) P_{1012}(x)]$
$(x-2022)(x-2024) P_{1012}(x-2) = (x-2024)(x-2022) P_{1012}(x)$
For $x \neq 2022$ and $x \neq 2024$, we can divide by $(x-2022)(x-2024)$:
$P_{1012}(x-2) = P_{1012}(x)$
Since this holds for infinitely many $x$, it must hold for all $x \in \mathbb{R}$.
A polynomial $Q(x)$ satisfying $Q(x-a)=Q(x)$ for a non-zero constant $a$ must be a constant polynomial. If $Q(x)$ is not constant, $\deg(Q) \ge 1$. Let $Q(x) = c_n x^n + \dots + c_0$ with $c_n \neq 0$.
$Q(x-a) = c_n(x-a)^n + \dots = c_n(x^n - nax^{n-1} + \dots) + \dots = c_n x^n - c_n n a x^{n-1} + \dots$.
$Q(x-a)=Q(x)$ implies $c_n x^n - c_n n a x^{n-1} + \dots = c_n x^n + \dots$.
Comparing coefficients of $x^{n-1}$, we must have $-c_n n a = c_{n-1}$ on the LHS and $c_{n-1}$ on the RHS. So $-c_n n a x^{n-1} = 0$ for all $x$. If $n \ge 1$ and $a \neq 0$, then $c_n = 0$, which contradicts $c_n \neq 0$. So we must have $n=0$.
Thus, $P_{1012}(x)$ must be a constant polynomial. Let $P_{1012}(x) = C$ for some real constant $C$.

Now we can reconstruct $P(x)$.
$P_{1011}(x) = (x-2022) P_{1012}(x) = C(x-2022)$.
$P(x) = x(x-2)\dots(x-2020) P_{1011}(x)$
$P(x) = C x(x-2)(x-4)\dots(x-2020)(x-2022)$.
This can be written in product notation as:
$$P(x) = C \prod_{k=0}^{1011} (x-2k)$$
where $C$ is an arbitrary real constant.

Let's check this solution.
$P(x) = C \prod_{k=0}^{1011} (x-2k)$.
$P(x-2) = C \prod_{k=0}^{1011} (x-2-2k) = C \prod_{k=0}^{1011} (x-2(k+1))$.
Let $j=k+1$. The product runs from $j=1$ to $j=1012$.
$P(x-2) = C \prod_{j=1}^{1012} (x-2j) = C (x-2)(x-4)\dots(x-2022)(x-2024)$.
The LHS of $(*)$ is $x P(x-2) = C x (x-2)(x-4)\dots(x-2022)(x-2024)$.
The RHS of $(*)$ is $(x-2024) P(x) = (x-2024) [C x(x-2)\dots(x-2020)(x-2022)]$.
Rearranging the terms on the RHS:
$(x-2024) P(x) = C x (x-2)\dots(x-2020)(x-2022)(x-2024)$.
Comparing LHS and RHS, we see they are identical.
So the solution is indeed of the form $P(x) = C \prod_{k=0}^{1011} (x-2k)$.

The solution includes the zero polynomial $P(x)=0$ when $C=0$.
If $P(x)$ is not the zero polynomial, its degree is $1012$. This matches the degree analysis using coefficients comparison: comparing the coefficients of $x^n$ in $x P(x-2) = (x-2024)P(x)$ implies $a_n (a_{n-1} - 2n a_n) = a_n(a_{n-1} - 2024 a_n)$, which leads to $2n = 2024$ or $n=1012$ if $a_n \neq 0$.

Final Answer: The final answer is $\boxed{P(x) = C \prod_{k=0}^{1011} (x-2k) \text{ for any real constant } C}$