An expert mathematician's solution follows.

This is a beautiful inequality that can be solved by transforming it into a sum of known non-negative quantities. The main idea is to use a convexity-type property of the factorial function.

### Step 1: Rearrange the inequality
Let's move all terms to the left-hand side (LHS). The inequality we want to prove is equivalent to
\begin{align*}
&x \cdot (2n)! + y \cdot (2m)! + z \cdot (2k)! \\
& - (x-y+z) \cdot (n+k)! - (-x+y+z) \cdot (m+k)! - (x+y-z) \cdot (n+m)! \geq 0.
\end{align*}
Let's call the expression on the LHS, $E(x,y,z,n,m,k)$.

### Step 2: A Key Lemma based on convexity
Let's establish a fundamental inequality for factorials that stems from the convexity of related functions.
**Lemma:** For any natural numbers $a, b \in \mathbb{N}$, the following inequality holds:
$$(2a)! + (2b)! \ge 2(a+b)!$$
**Proof of Lemma:**
Without loss of generality, assume $a \ge b$. Let $a = b+d$ for some integer $d \ge 0$. The inequality becomes:
$$(2b+2d)! + (2b)! \ge 2(2b+d)!$$
Let's define a function $f(d)$ for a fixed $b$ and integer $d \ge 0$:
$$f(d) = (2b+2d)! + (2b)! - 2(2b+d)!$$
We want to show that $f(d) \ge 0$ for all $d \ge 0$.
For $d=0$, we have $f(0) = (2b)! + (2b)! - 2(2b)! = 0$.
Now consider the difference $f(d+1) - f(d)$:
\begin{align*} f(d+1) - f(d) &= [(2b+2d+2)! - 2(2b+d+1)!] - [(2b+2d)! - 2(2b+d)!] \\ &= [(2b+2d+2)! - (2b+2d)!] - 2[(2b+d+1)! - (2b+d)!] \\ &= (2b+2d)!((2b+2d+2)(2b+2d+1)-1) - 2(2b+d)!((2b+d+1)-1) \\ &= (2b+2d)!((2b+2d+1)^2-1+2b+2d+1) - 2(2b+d)!(2b+d) \end{align*}
While this discrete approach works, a proof using continuous analogues and derivatives is more elegant. Considering the integers as points on the real line, the function $g(t)=(2t)! = \Gamma(2t+1)$ grows much faster than $h(t)=(t+c)! = \Gamma(t+c+1)$. The inequality essentially follows from the convexity of $t \mapsto (2t)!$. More formally, the function $\log \Gamma(x)$ is convex, a result by Gauss. By Jensen's inequality for the convex function $\phi(t) = \log((2t)!)$:
$$\frac{\log((2a)!) + \log((2b)!)}{2} \ge \log\left(\left(2\frac{a+b}{2}\right)!\right) = \log((a+b)!)$$
Exponentiating both sides gives $\sqrt{(2a)!(2b)!} \ge (a+b)!$.
By the AM-GM inequality, $\frac{(2a)!+(2b)!}{2} \ge \sqrt{(2a)!(2b)!}$.
Combining these two results, we get $\frac{(2a)!+(2b)!}{2} \ge (a+b)!$, which is the desired lemma.

### Step 3: Decomposing the main expression
Let's define the following quantities based on our lemma:
\begin{align*} I_{nm} &= (2n)! + (2m)! - 2(n+m)! \ge 0 \\ I_{mk} &= (2m)! + (2k)! - 2(m+k)! \ge 0 \\ I_{kn} &= (2k)! + (2n)! - 2(k+n)! \ge 0 \end{align*}
The core of the proof is to show that the expression $E(x,y,z,n,m,k)$ from Step 1 can be written as a linear combination of these non-negative terms. Let's try to write $E$ as $c_1 I_{nm} + c_2 I_{mk} + c_3 I_{kn}$.
\begin{align*} c_1 &I_{nm} + c_2 I_{mk} + c_3 I_{kn} \\ &= c_1((2n)! + (2m)! - 2(n+m)!) \\ &+ c_2((2m)! + (2k)! - 2(m+k)!) \\ &+ c_3((2k)! + (2n)! - 2(k+n)!) \\ &= (c_1+c_3)(2n)! + (c_1+c_2)(2m)! + (c_2+c_3)(2k)! \\ & -2c_1(n+m)! -2c_2(m+k)! -2c_3(k+n)! \end{align*}
We want this to be identical to our target expression $E$. By comparing the coefficients of the factorial terms, we get a system of linear equations for $c_1, c_2, c_3$:
\begin{itemize}
    \item Coeff of $(2n)!$: $c_1+c_3 = x$
    \item Coeff of $(2m)!$: $c_1+c_2 = y$
    \item Coeff of $(2k)!$: $c_2+c_3 = z$
    \item Coeff of $(n+m)!$: $-2c_1 = -(x+y-z)$
    \item Coeff of $(m+k)!$: $-2c_2 = -(-x+y+z)$
    \item Coeff of $(k+n)!$: $-2c_3 = -(x-y+z)$
\end{itemize}
Solving the last three equations gives:
$$ c_1 = \frac{x+y-z}{2}, \quad c_2 = \frac{-x+y+z}{2}, \quad c_3 = \frac{x-y+z}{2} $$
Let's check if these satisfy the first three equations:
\begin{itemize}
    \item $c_1+c_3 = \frac{x+y-z}{2} + \frac{x-y+z}{2} = \frac{2x}{2} = x$. (Correct)
    \item $c_1+c_2 = \frac{x+y-z}{2} + \frac{-x+y+z}{2} = \frac{2y}{2} = y$. (Correct)
    \item $c_2+c_3 = \frac{-x+y+z}{2} + \frac{x-y+z}{2} = \frac{2z}{2} = z$. (Correct)
\end{itemize}
The coefficients are consistent. Thus, we have established the following algebraic identity:
$$ E(x,y,z,n,m,k) = \frac{x+y-z}{2} I_{nm} + \frac{-x+y+z}{2} I_{mk} + \frac{x-y+z}{2} I_{kn} $$

### Step 4: Analyzing the coefficients
The inequality is proven if we can show that the RHS of the identity is non-negative. We already know $I_{nm}, I_{mk}, I_{kn} \ge 0$. The signs of the coefficients $c_1, c_2, c_3$ depend on $x,y,z$.
The conditions $1 \le x,y,z \le 4$ are given.

**Case 1: The coefficients $c_1, c_2, c_3$ are all non-negative.**
This happens if $x+y \ge z$, $y+z \ge x$, and $x+z \ge y$. This is the triangle inequality condition. If it holds, then we have a sum of non-negative terms, which is clearly non-negative. $E \ge 0$.

**Case 2: At least one coefficient is negative.**
The variables $x,y,z$ are positive, so at most one of the sums $x+y-z, y+z-x, z+x-y$ can be negative. For example, if $x+y-z<0$ and $y+z-x<0$, then $z>x+y$ and $x>y+z$. Adding these gives $x+z > x+2y+z$, which implies $2y<0$, a contradiction since $y \ge 1$.
So, we can assume, without loss of generality, that at most one coefficient is negative. Let's say $c_1 < 0$, which implies $z > x+y$. Then $c_2$ and $c_3$ must be positive:
\begin{itemize}
    \item $c_2 = \frac{-x+y+z}{2} = \frac{z-x+y}{2} > \frac{(x+y)-x+y}{2} = y \ge 1 > 0$.
    \item $c_3 = \frac{x-y+z}{2} = \frac{z+x-y}{2} > \frac{(x+y)+x-y}{2} = x \ge 1 > 0$.
\end{itemize}
The expression to prove non-negative is $S = c_1 I_{nm} + c_2 I_{mk} + c_3 I_{kn}$. Let's rewrite the coefficients in terms of $|c_1| = \frac{z-x-y}{2}$:
\begin{itemize}
    \item $c_2 = \frac{-x+y+z}{2} = \frac{z-x-y+2y}{2} = |c_1| + y$
    \item $c_3 = \frac{x-y+z}{2} = \frac{z-x-y+2x}{2} = |c_1| + x$
\end{itemize}
Substituting this back into the expression for $S$:
\begin{align*} S &= -|c_1| I_{nm} + (|c_1|+y) I_{mk} + (|c_1|+x) I_{kn} \\ &= |c_1|(I_{kn} + I_{mk} - I_{nm}) + y \cdot I_{mk} + x \cdot I_{kn} \end{align*}
Since $x,y \ge 1$ and $I_{mk}, I_{kn} \ge 0$, the terms $y \cdot I_{mk}$ and $x \cdot I_{kn}$ are non-negative. To prove $S \ge 0$, we just need to show that $I_{kn} + I_{mk} - I_{nm} \ge 0$.

### Step 5: Proving the final sub-inequality
We need to show $I_{kn} + I_{mk} - I_{nm} \ge 0$.
$$ I_{kn} + I_{mk} - I_{nm} = [(2k)!+(2n)! - 2(k+n)!] + [(2m)!+(2k)! - 2(m+k)!] - [(2n)!+(2m)! - 2(n+m)!] $$
$$ = 2(2k)! - 2(k+n)! - 2(m+k)! + 2(n+m)! = 2 \cdot C $$
where $C = (2k)! + (n+m)! - (k+n)! - (m+k)!$.
The sign of $C$ depends on the relative order of $n, m, k$. Let's prove $I_{kn} + I_{mk} - I_{nm} \ge 0$ by ordering the $I$ terms.

Let's assume, without loss of generality, $n \ge m \ge k$. We will show that $I_{kn} \ge I_{nm}$.
$$ I_{kn} - I_{nm} = [(2k)!+(2n)!-2(k+n)!] - [(2n)!+(2m)!-2(n+m)!] $$
$$ = (2k)! - (2m)! - 2(k+n)! + 2(n+m)! = 2((n+m)! - (n+k)!) - ((2m)! - (2k)!) $$
Since $n \ge m \ge k$, we have $n+m \ge n+k$ and $2m \ge 2k$. Thus $(n+m)! \ge (n+k)!$ and $(2m)! \ge (2k)!$. The first term is non-negative, the second term is non-negative. The sign of the difference is not immediately obvious.

Let's analyze the function $h(t) = 2(n+t)! - (2t)!$ for $t \in [k,m]$.
Its continuous analogue would have derivative (using $\psi(z) = \frac{d}{dz}\ln \Gamma(z)$):
$h'(t) = 2(n+t)!\psi(n+t+1) - 2(2t)!\psi(2t+1)$.
The function $u!\psi(u+1)$ is increasing for $u \ge 1$.
For $t \le n$, we have $n+t \ge 2t$. Thus, $(n+t)!\psi(n+t+1) \ge (2t)!\psi(2t+1)$, which means $h'(t) \ge 0$.
Since $h(t)$ is increasing for $t \le n$, and we have $m \ge k$ (and both are $\le n$), it follows that $h(m) \ge h(k)$.
$$ 2(n+m)! - (2m)! \ge 2(n+k)! - (2k)! $$
$$ \iff 2((n+m)! - (n+k)!) \ge (2m)! - (2k)! $$
This proves that $I_{kn} - I_{nm} \ge 0$. So, $I_{kn} \ge I_{nm}$.

Now we can return to the expression $I_{kn} + I_{mk} - I_{nm}$.
Since $I_{kn} \ge I_{nm}$, we have $I_{kn} - I_{nm} \ge 0$.
As $I_{mk} \ge 0$, it follows that
$$ (I_{kn} - I_{nm}) + I_{mk} \ge 0 $$
This establishes that $I_{kn} + I_{mk} - I_{nm} \ge 0$.

### Step 6: Conclusion
We have shown that the original inequality is equivalent to proving $S = c_1 I_{nm} + c_2 I_{mk} + c_3 I_{kn} \ge 0$.
\begin{itemize}
    \item If $c_1, c_2, c_3 \ge 0$, the inequality is trivially true.
    \item If one coefficient is negative (WLOG, $c_1 < 0$), the expression can be written as $S = |c_1|(I_{kn} + I_{mk} - I_{nm}) + y \cdot I_{mk} + x \cdot I_{kn}$.
\end{itemize}
We proved that $I_{kn} + I_{mk} - I_{nm} \ge 0$ (by assuming WLOG $n \ge m \ge k$; the final expression is symmetric with respect to permutations of $(n,m,k)$ so this assumption is valid for proving this sub-inequality). The terms $y \cdot I_{mk}$ and $x \cdot I_{kn}$ are non-negative because $x,y \ge 1$ and the $I$ terms are non-negative.
Therefore, $S \ge 0$ in all cases.

The given condition $1 \le x, y, z \le 4$ ensures $x,y,z$ are positive real numbers. The logic holds for any positive $x,y,z$.

Thus, the original inequality is true.