Let $N = 2025$ be the number of boxes. The boxes are numbered $k = 0, 1, \ldots, N-1 = 2024$.
Box $k$ contains $k$ white balls (W) and $(N-1)-k = 2024-k$ black balls (B).
The total number of balls in each box is $k + (2024-k) = 2024 = N-1$.

Maria chooses a box randomly. Let $C$ be the random variable representing the index of the chosen box. Since the choice is random, we assume a uniform probability distribution over the boxes.
The probability of choosing box $k$ is $P(C=k) = \frac{1}{N} = \frac{1}{2025}$ for $k = 0, 1, \ldots, 2024$.

After choosing box $k$, Maria draws 3 balls with replacement.
Let $E$ be the event that all 3 drawn balls are white. We want to find the probability $P(E)$.

We can use the law of total probability, conditioning on the chosen box $C$. The events $\{C=k\}$ for $k=0, \ldots, N-1$ form a partition of the sample space.
$$P(E) = \sum_{k=0}^{N-1} P(E | C=k) P(C=k)$$

First, let's calculate the conditional probability $P(E | C=k)$.
Given that box $k$ is chosen, there are $k$ white balls and $N-1-k$ black balls, for a total of $N-1$ balls.
The probability of drawing a white ball from box $k$ is $p_k = \frac{k}{N-1}$.
Since the draws are made with replacement, the outcomes of the three draws are independent given the chosen box $k$.
The probability of drawing 3 white balls in a row from box $k$ is:
$$P(E | C=k) = p_k \times p_k \times p_k = \left(\frac{k}{N-1}\right)^3$$
This formula holds for all $k=0, 1, \ldots, N-1$. Note that for $k=0$, $P(E|C=0) = (0/(N-1))^3 = 0$, which is correct as box 0 contains no white balls.

Now substitute this into the formula for $P(E)$:
$$P(E) = \sum_{k=0}^{N-1} \left(\frac{k}{N-1}\right)^3 P(C=k)$$
Since $P(C=k) = \frac{1}{N}$ for all $k$:
$$P(E) = \sum_{k=0}^{N-1} \left(\frac{k}{N-1}\right)^3 \frac{1}{N} = \frac{1}{N(N-1)^3} \sum_{k=0}^{N-1} k^3$$

We need to compute the sum of the first $N-1$ cubes: $\sum_{k=0}^{N-1} k^3$.
Since $0^3=0$, this is the same as $\sum_{k=1}^{N-1} k^3$.
The formula for the sum of the first $m$ cubes is $\sum_{k=1}^{m} k^3 = \left(\frac{m(m+1)}{2}\right)^2$.
In our case, $m = N-1$. So,
$$\sum_{k=0}^{N-1} k^3 = \sum_{k=1}^{N-1} k^3 = \left(\frac{(N-1)((N-1)+1)}{2}\right)^2 = \left(\frac{(N-1)N}{2}\right)^2 = \frac{N^2(N-1)^2}{4}$$

Now substitute this sum back into the expression for $P(E)$:
$$P(E) = \frac{1}{N(N-1)^3} \frac{N^2(N-1)^2}{4}$$
Simplify the expression:
$$P(E) = \frac{N^2 (N-1)^2}{4 N (N-1)^3} = \frac{N}{4(N-1)}$$

The problem gives $N=2025$. So $N-1=2024$.
Substitute this value into the formula for $P(E)$:
$$P(E) = \frac{2025}{4(2024)} = \frac{2025}{8096}$$

To check if the fraction can be simplified, we find the prime factorization of the numerator and the denominator.
$2025 = 25 \times 81 = 5^2 \times 3^4$.
$8096 = 4 \times 2024 = 4 \times 8 \times 253 = 32 \times 11 \times 23 = 2^5 \times 11 \times 23$.
The numerator and the denominator do not share any common prime factors. Thus, the fraction $\frac{2025}{8096}$ is in its simplest form.

Final Answer: The final answer is $\boxed{\frac{2025}{8096}}$