# Solution

To find the limit
$$\lim_{n\to\infty} \int_0^1 \frac{(1-\ln(1-x))^n}{n!} \, dx$$

I'll use a substitution approach to transform this integral into a more manageable form.

## Step 1: Apply a substitution
Let $y = 1-\ln(1-x)$. Then:
- $\ln(1-x) = 1-y$
- $1-x = e^{1-y}$
- $x = 1-e^{1-y}$
- $dx = e^{1-y}\,dy$

For the limits of integration:
- When $x = 0$: $1-e^{1-y} = 0 \implies e^{1-y} = 1 \implies y = 1$
- When $x = 1$: $1-x \to 0^+ \implies \ln(1-x) \to -\infty \implies y \to \infty$

So our integral becomes:
$$\int_0^1 \frac{(1-\ln(1-x))^n}{n!} \, dx = \int_1^{\infty} \frac{y^n}{n!} \cdot e^{1-y} \, dy = \frac{e}{n!} \int_1^{\infty} y^n e^{-y} \, dy$$

## Step 2: Relate to the gamma function
The integral $\int_0^{\infty} y^n e^{-y} \, dy = n!$ is a standard result related to the gamma function.

So we can write:
$$\int_1^{\infty} y^n e^{-y} \, dy = \int_0^{\infty} y^n e^{-y} \, dy - \int_0^1 y^n e^{-y} \, dy = n! - \int_0^1 y^n e^{-y} \, dy$$

Therefore:
$$\int_0^1 \frac{(1-\ln(1-x))^n}{n!} \, dx = e\left(1 - \frac{\int_0^1 y^n e^{-y} \, dy}{n!}\right)$$

## Step 3: Estimate the remaining integral
Let's denote $\gamma_L(n+1,1) = \int_0^1 y^n e^{-y} \, dy$, which is the lower incomplete gamma function.

Since $e^{-y}$ is bounded on $[0,1]$ with $e^{-1} \leq e^{-y} \leq 1$, we have:
$$\frac{e^{-1}}{n+1} \leq \gamma_L(n+1,1) \leq \frac{1}{n+1}$$

Therefore:
$$\frac{e^{-1}}{(n+1)!} \leq \frac{\gamma_L(n+1,1)}{n!} \leq \frac{1}{(n+1)!}$$

As $n \to \infty$, both bounds approach 0, so by the Squeeze Theorem:
$$\lim_{n\to\infty} \frac{\gamma_L(n+1,1)}{n!} = 0$$

## Step 4: Calculate the final limit
$$\lim_{n\to\infty} \int_0^1 \frac{(1-\ln(1-x))^n}{n!} \, dx = \lim_{n\to\infty} e\left(1 - \frac{\gamma_L(n+1,1)}{n!}\right) = e \cdot (1-0) = e$$

Therefore, the value of the limit is $e$.