```markdown
**Solution.**

Let  
\[
S \;=\;\{\,x^3 : x\in R\}
\]  
be the set of all cubes in \(R\).  We first observe that:

1.  **\(S\) is an additive subgroup of \((R,+)\).**  
    By the first hypothesis, for any \(x,y\in R\) there exists \(c\in R\) with
    \[
      x^3 + y^3 \;=\; c^3,
    \]
    so \(S\) is closed under addition.  Taking \(y=-z\) (which lies in \(R\) since \(R\) is a ring), we get
    \[
      x^3 - z^3 \;=\; x^3 +(-z)^3 \;\in\; S,
    \]
    so it is also closed under additive inverses.  Finally \(0=0^3\in S\).

---

We must show that for any \(a,b\in R\) there is \(d\in R\) with
\[
 aba + bab \;=\; d^3.
\]
We split into two cases.

---

### Case 1: \(a=b\)

Then
\[
  aba + bab \;=\; a^2a + a\,a^2 \;=\; 2\,a^3.
\]
By the first hypothesis applied to \((a,a)\), there is an element \(d\in R\) with
\[
  d^3 \;=\; a^3 + a^3 \;=\; 2\,a^3 \;=\; aba + bab,
\]
as required.

---

### Case 2: \(a\neq b\)

1.  **Expand \((a+b)^3\).**  In a general (not necessarily commutative) ring one has
    \[
      (a+b)^3
      \;=\;
      a^3 + a^2b + aba + ba^2
      + ab^2 + bab + b^2a + b^3.
    \]
2.  **Use \(a^2b=-\,ba^2\) and \(b^2a=-\,ab^2\).**  Since \(a\neq b\), the second hypothesis gives
    \[
      a^2b + ba^2 \;=\; 0,
      \quad
      ab^2 + b^2a \;=\; 0.
    \]
    Hence all those “mixed” terms cancel, leaving
    \[
      (a+b)^3
      \;=\;
      a^3 + b^3 \;+\; (aba + bab).
    \]
    Therefore
    \[
      aba + bab
      \;=\;
      (a+b)^3 \;-\;(a^3 + b^3).
    \]
3.  **Conclude it is a cube.**  By the first hypothesis there is some
    \(c\in R\) with
    \[
      c^3 \;=\; a^3 + b^3.
    \]
    Since \(S\) is an additive subgroup, the difference
    \(\,(a+b)^3 - c^3\)
    also lies in \(S\).  Hence there exists \(d\in R\) such that
    \[
      d^3 \;=\; (a+b)^3 - c^3
             \;=\; aba + bab.
    \]

---

In both cases we have exhibited \(d\in R\) with
\[
  aba + bab \;=\; d^3,
\]
completing the proof.  \(\boxed{}\)
```