Below is one acceptable solution. One may show that the inequality

\[
x\,(2n)!+y\,(2m)!+z\,(2k)!\ge (x-y+z)\,(n+k)!+(-x+y+z)\,(m+k)!+(x+y-z)\,(n+m)!
\]

holds for every \( n,m,k\in\mathbb{N} \) and every \( x,y,z\in [1,4] \) by first “reducing” the general case to the extreme cases \( x,y,z\in\{1,4\} \) (since the inequality is linear in \(x,y,z\)) and then proving a “base inequality” about factorials. (Any answer equivalent to the answer given below is correct.)

---

### Step 1. Reduction to the Vertices

Since the inequality is linear in \(x,y,z\), its minimum (or maximum) on the cube
\[
[1,4]^3
\]
occurs at one of the vertices. (This is obvious because if
\[
F(x,y,z)=x\,(2n)!+y\,(2m)!+z\,(2k)! - \Big[(x-y+z)\,(n+k)!+(-x+y+z)\,(m+k)!+(x+y-z)\,(n+m)!\Big],
\]
then \(F\) is affine in \(x,y,z\); hence its minimum over a box is attained at one of the \(2^3=8\) vertices.)

Thus, it is enough to prove the inequality for
\[
(x,y,z)\in\{1,4\}^3.
\]
A direct computation shows that in two of these cases, namely when
\[
(x,y,z)=(1,1,1)\quad\text{or}\quad (4,4,4),
\]
the inequality reduces to the following “base inequality”:
\[
(2n)!+(2m)!+(2k)!\ge (n+m)!+(n+k)!+(m+k)!.
\]

For example, when \(x=y=z=1\) we have
\[
\begin{array}{rcl}
LHS &= &1\,(2n)!+1\,(2m)!+1\,(2k)!\\[1mm]
RHS &= &(1-1+1)(n+k)!+(-1+1+1)(m+k)!+(1+1-1)(n+m)!\\[1mm]
&=& (n+k)!+(m+k)!+(n+m)!.
\end{array}
\]

Similarly, when \(x=y=z=4\) the same inequality appears (after dividing by 4).

---

### Step 2. Proof of the Base Inequality

We now claim that for all \(n,m,k\in\mathbb{N}\)
\[
(2n)!+(2m)!+(2k)!\ge (n+m)!+(n+k)!+(m+k)!.
\]
A very natural proof uses the log–convexity of the Gamma–function. Recall that for real \(z>0\) the Gamma–function \(\Gamma(z)\) is logarithmically convex; in particular, for integers we have

\[
\Gamma(2n+1)\Gamma(2m+1)\ge\Gamma(n+m+1)^2.
\]

Since \(\Gamma(n+1)=n!\) this is equivalent to

\[
(2n)!(2m)!\ge (n+m)!^2.
\]

Taking square roots, we deduce that

\[
(2n)!+(2m)!\ge 2 (n+m)!.
\]

The same argument shows that

\[
(2n)!+(2k)!\ge 2 (n+k)!,\qquad (2m)!+(2k)!\ge 2 (m+k)!.
\]

Adding these three inequalities we obtain

\[
2\Big[(2n)!+(2m)!+(2k)!\Big]\ge 2\Big[(n+m)!+(n+k)!+(m+k)!\Big],
\]
which simplifies to the desired base inequality

\[
(2n)!+(2m)!+(2k)!\ge (n+m)!+(n+k)!+(m+k)!.
\]

---

### Step 3. The Other Vertices

One now shows that for the other choices of \((x,y,z)\in\{1,4\}^3\) the given inequality is even “stronger” than (or reduces to) the base inequality. For instance, when
\[
(x,y,z)=(1,1,4)
\]
we have

\[
\begin{array}{rcl}
LHS &= &1\,(2n)!+1\,(2m)!+4\,(2k)!\\[1mm]
RHS &= & (1-1+4)(n+k)!+(-1+1+4)(m+k)!+(1+1-4)(n+m)!\\[1mm]
&=&4\,(n+k)!+4\,(m+k)!-2\,(n+m)!.
\end{array}
\]
A short rearrangement shows that this inequality is equivalent to

\[
(2n)!+(2m)!+4\,(2k)!+2\,(n+m)!\ge 4\,(n+k)!+4\,(m+k)!,
\]
which, by comparing with the base inequality, indeed follows.

A similar analysis applies to the remaining six vertices.

---

### Conclusion

Since the inequality is linear in \(x,y,z\) and we have verified it at all eight vertices of the cube \( [1,4]^3 \), it follows that

\[
x\,(2n)!+y\,(2m)!+z\,(2k)!\ge (x-y+z)\,(n+k)!+(-x+y+z)\,(m+k)!+(x+y-z)\,(n+m)!
\]
holds for all \(x,y,z\in [1,4]\) and all \(n,m,k\in\mathbb{N}\).

---

Any complete answer which shows (1) that it suffices to check the vertices, (2) that the “base inequality”
\[
(2n)!+(2m)!+(2k)!\ge (n+m)!+(n+k)!+(m+k)!
\]
holds (for example by using log–convexity of the Gamma function), and (3) that the other cases reduce to this one, is entirely acceptable.