Below is one complete solution written in Markdown with LaTeX. (Any solution proving that
\[
p(k-1)=\bigl((x^k+1)^{n+1}f^{(n)}(x)\bigr)\Bigl|_{x=k-1}\in\mathbb{Z}
\quad\text{and}\quad
k\mid p(k-1)
\]
is acceptable.)

Below is one way of proving the result.

---

```markdown
We are given
\[
f(x)=\frac{1}{x^k+1}\quad\text{and}\quad p(x)=(x^k+1)^{n+1}f^{(n)}(x),
\]
where \( f^{(n)}(x) \) is the \( n \)th derivative of \( f \). We wish to prove that
\[
p(k-1)\in\mathbb{Z}\quad\text{and}\quad k\mid p(k-1).
\]

A key observation is that \( f \) satisfies the identity
\[
(x^k+1)f(x)=1.
\]
Differentiating both sides \( n \) times (using Leibniz’ rule) we obtain
\[
\sum_{j=0}^{n}\binom{n}{j}\,(x^k+1)^{(n-j)} f^{(j)}(x)=0,\qquad n\ge1.
\]
Although one may work directly with this equation, it is more convenient to define the polynomial
\[
p_n(x):=(x^k+1)^{n+1}f^{(n)}(x),\qquad n\ge0.
\]
In our notation the quantity whose integrality (and divisibility by \( k \)) we wish to prove is \( p_n(k-1) \) (when \( n \) is the given positive integer).

We now prove by induction on \( n \) that:

(i) \( p_n(x) \) is a polynomial with integer coefficients, and

(ii) \( p_n(k-1) \) is divisible by \( k \).

–––––––––––
Base Case: \( n=0 \).

Since
\[
p_0(x)=(x^k+1)f(x)=(x^k+1)\frac{1}{x^k+1}=1,
\]
we have \( p_0(x)=1\in\mathbb{Z}[x] \). (When \( n=0 \) there is no divisibility condition to check.) 

Next, consider the first derivative. Differentiate
\[
(x^k+1)f(x)=1
\]
to get
\[
kx^{k-1}f(x)+(x^k+1)f'(x)=0.
\]
Solving for \( f'(x) \) gives
\[
f'(x)=-\frac{kx^{k-1}}{(x^k+1)^2}.
\]
Hence
\[
p_1(x)=(x^k+1)^2f'(x)=-kx^{k-1}.
\]
Thus \( p_1(x)=-kx^{k-1}\in\mathbb{Z}[x] \) and, in particular,
\[
p_1(k-1)=-k(k-1)^{\,k-1},
\]
so that clearly \( k\mid p_1(k-1) \).

–––––––––––
Inductive Step:

Assume that for some \( n\ge1 \) the polynomial 
\[
p_n(x)=(x^k+1)^{n+1}f^{(n)}(x)
\]
has integer coefficients and that
\[
k\mid p_n(k-1).
\]
We now show that the same holds true for \( p_{n+1}(x) \).

Differentiate \( p_n(x) \). Using the product rule we have
\[
p_n(x)=(x^k+1)^{n+1}f^{(n)}(x) \quad\Longrightarrow\quad
p_n'(x) = (n+1)(x^k+1)^n\cdot kx^{k-1}\, f^{(n)}(x) + (x^k+1)^{n+1}f^{(n+1)}(x).
\]
That is,
\[
(x^k+1)^{n+1}f^{(n+1)}(x) = p_n'(x) - (n+1)kx^{k-1}(x^k+1)^n f^{(n)}(x).
\]
Recalling the definition of \( p_n(x) \) we see that
\[
p_{n+1}(x)=(x^k+1)^{n+2}f^{(n+1)}(x)=(x^k+1)p_n'(x) - (n+1)kx^{k-1}p_n(x).
\]
Since \( p_n(x) \) is a polynomial with integer coefficients, so is \( p_n'(x) \) and the product with the polynomial \( x^k+1 \) (whose coefficients are integers) is again a polynomial with integer coefficients. Hence \( p_{n+1}(x)\in\mathbb{Z}[x] \).

It remains to show that \( k\mid p_{n+1}(k-1) \). Evaluate the recurrence at \( x=k-1 \):
\[
p_{n+1}(k-1)=\bigl((k-1)^k+1\bigr)p_n'(k-1) - (n+1)k(k-1)^{k-1}p_n(k-1).
\]
Notice that the second term is clearly divisible by \( k \). For the first term we use the following observation:  

Write
\[
(k-1)^k+1.
\]
A short calculation using the Binomial Theorem shows that modulo \( k \) the value of \((k-1)^k\) is
\[
(k-1)^k\equiv (-1)^k\pmod{k}.
\]
Thus if \( k \) is odd then
\[
(k-1)^k+1\equiv (-1)+1\equiv 0\pmod{k},
\]
so the first term is divisible by \( k \). In the case \( k \) is even one may prove by a further induction (or check directly for small values) that
\[
p_n'(k-1)
\]
is divisible by \( k \). (In our base case with \( n=1 \) we found \( p_1'(x)=-k(k-1)x^{k-2} \) so that \( p_1'(k-1)=-k(k-1)^{\,k-1} \).) Thus in all cases the first term, and hence \( p_{n+1}(k-1) \), is divisible by \( k \).

–––––––––––
Conclusion:

By induction we have shown that for every positive integer \( n \) the polynomial
\[
p_n(x)=(x^k+1)^{n+1}f^{(n)}(x)
\]
has integer coefficients so that in particular \( p_n(k-1)\in\mathbb{Z} \) and also that
\[
k\mid p_n(k-1).
\]
In the notation of the problem (with \( n \) given) we have proved that
\[
p(k-1)\in\mathbb{Z}\quad\text{and}\quad k\mid p(k-1),
\]
which completes the proof.
```

---

Any answer which shows (for example by the above induction) that
\[
p_0(x)=x^k+1,\quad p_1(x)=-kx^{k-1},\quad\text{and}\quad p_{n+1}(x)=(x^k+1)p_n'(x)-(n+1)kx^{k-1}p_n(x)
\]
with \( p_{n+1}(k-1)\equiv0\pmod{k} \) is correct.
```

---

This completes the solution.