```markdown
We will prove that
\[
\lceil (3+\sqrt{11})^{2n}\rceil
\]
is divisible by \(2^{n+1}\) for any integer \(n\ge 1\).

### Step 1. Expressing the Ceiling

Let
\[
\alpha = 3+\sqrt{11} \quad \text{and} \quad \beta = 3-\sqrt{11}.
\]
Notice that these are conjugate numbers and that
\[
\alpha \beta = (3+\sqrt{11})(3-\sqrt{11}) = 9-11=-2.
\]
Also, observe that
\[
\alpha + \beta = (3+\sqrt{11})+(3-\sqrt{11}) = 6.
\]
Since \(\sqrt{11}\approx3.316\), we have 
\[
\beta = 3-\sqrt{11}\approx -0.316.
\]
Then, for any \(n\geq 1\),
\[
\beta^{2n} = \left(3-\sqrt{11}\right)^{2n}
\]
is a positive number strictly less than 1 (because \(|\beta|<1\)).

Now, consider the sum
\[
S_n = \alpha^{2n} + \beta^{2n}.
\]
Since \(\alpha\) and \(\beta\) are the roots of the quadratic
\[
x^2 -6x - 2 = 0,
\]
the irrational parts cancel in the sum \(S_n\), so \(S_n\) is an integer. Moreover, since
\[
0 < \beta^{2n} < 1,
\]
we have
\[
S_n - 1 < \alpha^{2n} < S_n.
\]
Thus, the ceiling of \(\alpha^{2n}=(3+\sqrt{11})^{2n}\) is:
\[
\lceil (3+\sqrt{11})^{2n}\rceil = S_n.
\]

### Step 2. Showing \(S_n\) is Divisible by \(2^{n+1}\)

Define
\[
a = \alpha^2 \quad \text{and} \quad b = \beta^2.
\]
Then
\[
S_n = a^n + b^n.
\]
A short calculation gives:
\[
\alpha^2 = (3+\sqrt{11})^2 = 9+6\sqrt{11}+11 = 20+6\sqrt{11},
\]
\[
\beta^2 = (3-\sqrt{11})^2 = 9-6\sqrt{11}+11 = 20-6\sqrt{11}.
\]
Hence, 
\[
a+b = (20+6\sqrt{11})+(20-6\sqrt{11}) = 40 \quad \text{and} \quad ab = \alpha^2\beta^2 = (\alpha\beta)^2 = (-2)^2 = 4.
\]
It follows that the sequence \(\{S_n\}\) satisfies the linear recurrence
\[
S_{n+1} = (a+b)S_n - ab\,S_{n-1} = 40 S_n - 4 S_{n-1},
\]
with initial conditions
\[
S_0 = a^0 + b^0 = 2, \quad S_1 = a+b = 40.
\]

We now prove by induction on \(n\) that
\[
S_n \text{ is divisible by } 2^{n+1}.
\]

#### Base Cases

- For \(n=0\): \(S_0=2\) is divisible by \(2^{0+1}=2\).
- For \(n=1\): \(S_1=40\) is divisible by \(2^{1+1}=4\).

#### Inductive Step

Assume that for some \(n\geq1\), there exist integers \(k\) and \(m\) such that
\[
S_n = 2^{n+1} k \quad \text{and} \quad S_{n-1} = 2^n m.
\]
Then, using the recurrence,
\[
S_{n+1} = 40S_n - 4S_{n-1} = 40(2^{n+1} k) - 4(2^n m) = 2^{n+1}(40k) - 2^{n+2} m.
\]
We can factor out \(2^{n+1}\):
\[
S_{n+1} = 2^{n+1}\left(40k - 2m\right).
\]
Notice that \(40k - 2m\) is an even number (since both terms are even); therefore, we can write
\[
40k - 2m = 2(20k-m).
\]
Thus,
\[
S_{n+1} = 2^{n+1}\cdot 2(20k-m) = 2^{n+2}(20k-m).
\]
This shows that \(S_{n+1}\) is divisible by \(2^{(n+1)+1}\).

By the principle of mathematical induction, for all \(n\geq 0\) the number \(S_n\) is divisible by \(2^{n+1}\).

### Conclusion

Since we have shown that
\[
\lceil (3+\sqrt{11})^{2n}\rceil = S_n
\]
and that \(S_n\) is divisible by \(2^{n+1}\) for all \(n\geq 1\), the proof is complete.
```