Of course. Here is a detailed, step-by-step solution to the problem. We will solve this using two different, powerful methods to demonstrate the result robustly.

### Method 1: Using a Probability Generating Function

This method is very elegant for problems involving sums of probabilities of discrete, independent events.

#### Step 1: Define the probabilities for a single coin
Let $H_m$ be the event that the $m$-th coin lands heads, and $T_m$ be the event that it lands tails.
The probability of heads for the $m$-th coin is given as:
$p_m = P(H_m) = \frac{1}{2m+1}$

The probability of tails for the $m$-th coin is:
$q_m = P(T_m) = 1 - p_m = 1 - \frac{1}{2m+1} = \frac{2m+1-1}{2m+1} = \frac{2m}{2m+1}$

#### Step 2: Construct the generating function
A probability generating function is a polynomial where the coefficient of $x^k$ represents the probability of an event with value $k$. In our case, the value is the number of heads.

For a single coin toss (the $m$-th coin), the outcome is either 0 heads (tails) with probability $q_m$, or 1 head (heads) with probability $p_m$. The generating function for this single toss is:
$G_m(x) = q_m \cdot x^0 + p_m \cdot x^1 = q_m + p_m x$

Since the coin tosses are independent, the generating function for the total experiment of tossing all $n$ coins is the product of the individual generating functions:
$G(x) = \prod_{m=1}^{n} G_m(x) = \prod_{m=1}^{n} (q_m + p_m x)$

If we were to expand this product, we would get a polynomial of degree $n$:
$G(x) = C_0 + C_1 x + C_2 x^2 + \dots + C_n x^n$
where the coefficient $C_k$ is the total probability of getting exactly $k$ heads from the $n$ tosses.

#### Step 3: Extract the desired probability from the generating function
We want to find the probability of getting an even number of heads. This is the sum of the probabilities of getting 0 heads, 2 heads, 4 heads, and so on.
$P(\text{even heads}) = C_0 + C_2 + C_4 + \dots$

There is a standard trick to find this sum. Let's evaluate $G(x)$ at $x=1$ and $x=-1$:
$G(1) = C_0 + C_1 + C_2 + C_3 + \dots + C_n$
$G(-1) = C_0 - C_1 + C_2 - C_3 + \dots + (-1)^n C_n$

Adding these two equations:
$G(1) + G(-1) = (C_0 + C_0) + (C_1 - C_1) + (C_2 + C_2) + \dots = 2C_0 + 2C_2 + 2C_4 + \dots$
$G(1) + G(-1) = 2 (C_0 + C_2 + C_4 + \dots)$

Therefore, the probability of getting an even number of heads is:
$P(\text{even heads}) = \frac{G(1) + G(-1)}{2}$

#### Step 4: Calculate G(1) and G(-1)
First, let's calculate $G(1)$:
$G(1) = \prod_{m=1}^{n} (q_m + p_m)$. Since $q_m + p_m = 1$ for any coin,
$G(1) = \prod_{m=1}^{n} (1) = 1$. This makes sense, as the sum of all probabilities must be 1.

Next, let's calculate $G(-1)$:
$G(-1) = \prod_{m=1}^{n} (q_m - p_m)$.
Let's find the value of the term $(q_m - p_m)$:
$q_m - p_m = \frac{2m}{2m+1} - \frac{1}{2m+1} = \frac{2m-1}{2m+1}$.

Now we can write out the product for $G(-1)$:
$G(-1) = \prod_{m=1}^{n} \frac{2m-1}{2m+1}$

This is a telescoping product. Let's write out the first few terms and the last term to see the cancellation:
For $m=1: \frac{2(1)-1}{2(1)+1} = \frac{1}{3}$
For $m=2: \frac{2(2)-1}{2(2)+1} = \frac{3}{5}$
For $m=3: \frac{2(3)-1}{2(3)+1} = \frac{5}{7}$
...
For $m=n: \frac{2n-1}{2n+1}$

So, $G(-1) = \frac{1}{3} \times \frac{3}{5} \times \frac{5}{7} \times \cdots \times \frac{2n-3}{2n-1} \times \frac{2n-1}{2n+1}$.
The numerator of each term cancels the denominator of the previous term. The only terms that remain are the numerator of the first term and the denominator of the last term.
$G(-1) = \frac{1}{2n+1}$.

#### Step 5: Calculate the final probability
Now we substitute our values for $G(1)$ and $G(-1)$ into the formula:
$P(\text{even heads}) = \frac{G(1) + G(-1)}{2} = \frac{1 + \frac{1}{2n+1}}{2}$

Let's simplify this expression:
$P(\text{even heads}) = \frac{\frac{2n+1}{2n+1} + \frac{1}{2n+1}}{2} = \frac{\frac{2n+2}{2n+1}}{2} = \frac{2n+2}{2(2n+1)} = \frac{n+1}{2n+1}$

---

### Method 2: Using a Recurrence Relation

This method builds the solution up one coin at a time.

#### Step 1: Define the recurrence relation
Let $E_n$ be the probability of getting an even number of heads after tossing the first $n$ coins.
Let $O_n$ be the probability of getting an odd number of heads after tossing the first $n$ coins.
By definition, $E_n + O_n = 1$.

Now, consider the toss of the $(n+1)$-th coin. Its probability of heads is $p_{n+1} = \frac{1}{2(n+1)+1} = \frac{1}{2n+3}$ and its probability of tails is $q_{n+1} = \frac{2(n+1)}{2(n+1)+1} = \frac{2n+2}{2n+3}$.

An even number of heads with $n+1$ coins can be obtained in two ways:
1.  An even number of heads with the first $n$ coins (probability $E_n$), followed by a tail on the $(n+1)$-th coin (probability $q_{n+1}$).
2.  An odd number of heads with the first $n$ coins (probability $O_n$), followed by a head on the $(n+1)$-th coin (probability $p_{n+1}$).

So, we can write a recurrence relation for $E_{n+1}$:
$E_{n+1} = E_n \cdot q_{n+1} + O_n \cdot p_{n+1}$

#### Step 2: Solve the recurrence relation
Substitute $O_n = 1 - E_n$ into the relation:
$E_{n+1} = E_n \cdot q_{n+1} + (1 - E_n) \cdot p_{n+1}$
$E_{n+1} = E_n \cdot q_{n+1} + p_{n+1} - E_n \cdot p_{n+1}$
$E_{n+1} = E_n (q_{n+1} - p_{n+1}) + p_{n+1}$

We previously calculated $q_m - p_m = \frac{2m-1}{2m+1}$. For the $(n+1)$-th coin, this is:
$q_{n+1} - p_{n+1} = \frac{2(n+1)-1}{2(n+1)+1} = \frac{2n+1}{2n+3}$

Substituting this and $p_{n+1}$ back into the recurrence:
$E_{n+1} = E_n \left(\frac{2n+1}{2n+3}\right) + \frac{1}{2n+3}$

#### Step 3: Find the base case and verify the formula
Let's find the probability for $n=1$. "Even heads" means 0 heads, which is a tail on the first coin.
$E_1 = q_1 = \frac{2(1)}{2(1)+1} = \frac{2}{3}$.

Let's test our formula from Method 1: $E_n = \frac{n+1}{2n+1}$.
For $n=1$, the formula gives $E_1 = \frac{1+1}{2(1)+1} = \frac{2}{3}$. This matches the base case.

Let's prove by induction that $E_n = \frac{n+1}{2n+1}$ is the solution to the recurrence. We have already shown the base case is true. Assume the formula holds for $n$, i.e., $E_n = \frac{n+1}{2n+1}$. Let's find $E_{n+1}$ using the recurrence relation:
$E_{n+1} = \left(\frac{n+1}{2n+1}\right) \left(\frac{2n+1}{2n+3}\right) + \frac{1}{2n+3}$

The $(2n+1)$ terms cancel out:
$E_{n+1} = \frac{n+1}{2n+3} + \frac{1}{2n+3}$
$E_{n+1} = \frac{(n+1)+1}{2n+3} = \frac{n+2}{2n+3}$

This is exactly what our formula $E_k = \frac{k+1}{2k+1}$ predicts for $k=n+1$.
$E_{n+1} = \frac{(n+1)+1}{2(n+1)+1} = \frac{n+2}{2n+3}$.
The formula holds for $n+1$. By the principle of mathematical induction, the formula is correct for all $n \ge 1$.

### Conclusion

Both methods lead to the same result. The probability that if each of the $n$ coins is tossed once, one gets an even number of heads is:
$$ \frac{n+1}{2n+1} $$