This is a fascinating problem that, despite its appearance, is not an optimization problem but rather a demonstration of a surprising invariant. We will show that the sum of the numbers in the black cells is constant for any valid coloring.

### 1. Understanding the Grid and Numbering

Let the grid have rows indexed by $i$ from $1$ to $2n$ and columns by $j$ from $1$ to $2n$. A cell is identified by its coordinates $(i, j)$.

The problem specifies a column-major numbering scheme. The number in cell $(i, j)$, which we denote by $N(i, j)$, is determined as follows:
- The first column ($j=1$) contains numbers $1, 2, \dots, 2n$. So, $N(i, 1) = i$.
- The second column ($j=2$) contains numbers $2n+1, 2n+2, \dots, 4n$. So, $N(i, 2) = 2n+i$.
- In general, the $j$-th column starts after the first $j-1$ columns, each containing $2n$ numbers. So, the number at the top of column $j$ is $(j-1)2n + 1$. The number at row $i$ in column $j$ is then:
$N(i, j) = (j-1)2n + i$.

Let's check this formula:
- For $(1, 1)$: $N(1, 1) = (1-1)2n + 1 = 1$. (Correct)
- For $(2n, 2n)$: $N(2n, 2n) = (2n-1)2n + 2n = 4n^2 - 2n + 2n = 4n^2$. (Correct)

### 2. Formalizing the Coloring Constraints

We are given that half the cells in each row and each column are black.
- The total number of cells in the grid is $(2n)^2 = 4n^2$.
- The total number of black cells is $2n^2$.
- Each row has $2n$ cells, so $n$ cells must be black.
- Each column has $2n$ cells, so $n$ cells must be black.

Let's define an indicator variable $C_{ij}$ for the color of cell $(i, j)$:
$C_{ij} = 1$ if cell $(i, j)$ is black.
$C_{ij} = 0$ if cell $(i, j)$ is white.

The constraints can be written as:
- For each row $i \in \{1, \dots, 2n\}$: $\sum_{j=1}^{2n} C_{ij} = n$.
- For each column $j \in \{1, \dots, 2n\}$: $\sum_{i=1}^{2n} C_{ij} = n$.

### 3. Calculating the Sum of Numbers in Black Cells

The sum of the numbers in all the black cells, let's call it $S$, is given by:
$S = \sum_{i=1}^{2n} \sum_{j=1}^{2n} C_{ij} \cdot N(i, j)$

Now, we substitute the formula for $N(i, j)$:
$S = \sum_{i=1}^{2n} \sum_{j=1}^{2n} C_{ij} \cdot ((j-1)2n + i)$

Let's split this sum into two parts:
$S = \sum_{i=1}^{2n} \sum_{j=1}^{2n} C_{ij}(j-1)2n + \sum_{i=1}^{2n} \sum_{j=1}^{2n} C_{ij}i$

Let's analyze each part separately.

**Part 1: $\sum_{i=1}^{2n} \sum_{j=1}^{2n} C_{ij}(j-1)2n$**

We can change the order of summation:
Part 1 = $\sum_{j=1}^{2n} \sum_{i=1}^{2n} C_{ij}(j-1)2n$

The term $(j-1)2n$ is constant with respect to the inner summation (over $i$). We can factor it out:
Part 1 = $\sum_{j=1}^{2n} (j-1)2n \left( \sum_{i=1}^{2n} C_{ij} \right)$

Using the column constraint, $\sum_{i=1}^{2n} C_{ij} = n$:
Part 1 = $\sum_{j=1}^{2n} (j-1)2n \cdot n = 2n^2 \sum_{j=1}^{2n} (j-1)$

The sum $\sum_{j=1}^{2n} (j-1)$ is the sum of integers from $0$ to $2n-1$:
$\sum_{k=0}^{2n-1} k = \frac{(2n-1)(2n-1+1)}{2} = \frac{(2n-1)(2n)}{2} = n(2n-1)$

So, Part 1 = $2n^2 \cdot n(2n-1) = 2n^3(2n-1) = 4n^4 - 2n^3$.

**Part 2: $\sum_{i=1}^{2n} \sum_{j=1}^{2n} C_{ij}i$**

The term $i$ is constant with respect to the inner summation (over $j$). We can factor it out:
Part 2 = $\sum_{i=1}^{2n} i \left( \sum_{j=1}^{2n} C_{ij} \right)$

Using the row constraint, $\sum_{j=1}^{2n} C_{ij} = n$:
Part 2 = $\sum_{i=1}^{2n} i \cdot n = n \sum_{i=1}^{2n} i$

The sum $\sum_{i=1}^{2n} i$ is the sum of integers from $1$ to $2n$:
$\sum_{i=1}^{2n} i = \frac{2n(2n+1)}{2} = n(2n+1)$

So, Part 2 = $n \cdot n(2n+1) = n^2(2n+1) = 2n^3 + n^2$.

**Total Sum S**

Now we add the two parts together:
$S = (4n^4 - 2n^3) + (2n^3 + n^2)$
$S = 4n^4 + n^2$

### 4. Conclusion and Interpretation

The calculation shows that the sum $S$ is a constant value, $4n^4 + n^2$, which depends only on $n$ and not on the specific arrangement of the black cells, as long as the row and column constraints are satisfied.

This is a consequence of the structure of the numbering function $N(i, j) = i + (j-1)2n$, which is a sum of a function of the row index $i$ and a function of the column index $j$. For any such numbering scheme, the total sum over a set of cells with fixed row and column counts will be constant.

Since the sum is the same for *any* valid coloring, the minimal possible sum and the maximal possible sum are identical.

**Minimal Sum = Maximal Sum = $4n^4 + n^2$**

### Example: The case $n=1$

Let's verify this result for the simplest case, $n=1$. The grid is $2 \times 2$.
The numbering is:
$N(1,1) = (1-1)2(1)+1 = 1$
$N(2,1) = (1-1)2(1)+2 = 2$
$N(1,2) = (2-1)2(1)+1 = 3$
$N(2,2) = (2-1)2(1)+2 = 4$
The grid of numbers is:
$$ \begin{pmatrix} 1 & 3 \\ 2 & 4 \end{pmatrix} $$
The constraints require $n=1$ black cell in each row and each column. There are two possible valid colorings:

1.  **Diagonal coloring:** Black cells are $(1,1)$ and $(2,2)$.
    $$ \begin{pmatrix} \blacksquare & \square \\ \square & \blacksquare \end{pmatrix} $$
    The sum of numbers in black cells is $N(1,1) + N(2,2) = 1 + 4 = 5$.

2.  **Anti-diagonal coloring:** Black cells are $(1,2)$ and $(2,1)$.
    $$ \begin{pmatrix} \square & \blacksquare \\ \blacksquare & \square \end{pmatrix} $$
    The sum of numbers in black cells is $N(1,2) + N(2,1) = 3 + 2 = 5$.

In both cases, the sum is 5.
Our formula gives $S = 4(1)^4 + (1)^2 = 4 + 1 = 5$.
This confirms our result for $n=1$.

---
### Final Answer

The sum of the numbers in the black cells is constant for any valid coloring that satisfies the given conditions. This is because the numbering of any cell $(i, j)$ is given by $N(i,j) = (j-1)2n + i$, which is a sum of a function of its row index and a function of its column index.

The sum $S$ is calculated as:
$S = \sum_{i,j \text{ are black}} N(i,j) = 4n^4 + n^2$

Therefore, the minimal and maximal possible sums are the same.

**Minimal possible sum = $4n^4 + n^2$**
**Maximal possible sum = $4n^4 + n^2$**