Let the given system of equations be
$$x_k^2 + (1 - x_{k+1} \ln x_{k+1})^2 = 2x_{k+1} - 2x_{k+2}^2 \ln x_{k+2}, \quad k=1, \ldots, n$$
where indices are taken modulo $n$, i.e., $x_{n+1} = x_1$, $x_{n+2} = x_2$, etc. The variables $x_i$ are positive for all $i \in \{1, 2, \ldots, n\}$.

We can rewrite the $k$-th equation as:
$$x_k^2 - 2x_{k+1} + (1 - x_{k+1} \ln x_{k+1})^2 + 2x_{k+2}^2 \ln x_{k+2} = 0$$
Summing all $n$ equations for $k=1, \ldots, n$:
$$ \sum_{k=1}^n \left[ x_k^2 - 2x_{k+1} + (1 - x_{k+1} \ln x_{k+1})^2 + 2x_{k+2}^2 \ln x_{k+2} \right] = 0 $$
Using the cyclic nature of the indices, we have $\sum_{k=1}^n x_k^2 = \sum_{k=1}^n x_{k+1}^2 = \sum_{k=1}^n x_{k+2}^2$, $\sum_{k=1}^n x_{k+1} = \sum_{k=1}^n x_k$, and $\sum_{k=1}^n x_{k+1} \ln x_{k+1} = \sum_{k=1}^n x_k \ln x_k$, and $\sum_{k=1}^n x_{k+2}^2 \ln x_{k+2} = \sum_{k=1}^n x_k^2 \ln x_k$.
The sum becomes:
$$ \sum_{k=1}^n x_k^2 - 2 \sum_{k=1}^n x_k + \sum_{k=1}^n (1 - x_k \ln x_k)^2 + 2 \sum_{k=1}^n x_k^2 \ln x_k = 0 $$
We can group the terms for each $x_k$:
$$ \sum_{k=1}^n \left[ x_k^2 - 2x_k + (1 - x_k \ln x_k)^2 + 2x_k^2 \ln x_k \right] = 0 $$
Let $g(x) = x^2 - 2x + (1 - x \ln x)^2 + 2x^2 \ln x$. The sum is $\sum_{k=1}^n g(x_k) = 0$.
Let's simplify $g(x)$:
$$ g(x) = x^2 - 2x + 1 - 2x \ln x + (x \ln x)^2 + 2x^2 \ln x $$
$$ g(x) = (x^2 - 2x + 1) + (x \ln x)^2 - 2x \ln x + 2x^2 \ln x $$
$$ g(x) = (x-1)^2 + (x \ln x)^2 + 2(x^2-x) \ln x $$
We can factor $2x(x-1)\ln x$ from the last two terms:
$$ g(x) = (x-1)^2 + x^2 (\ln x)^2 + 2x(x-1) \ln x $$
This expression is in the form $a^2 + b^2 + 2ab$ with $a=x-1$ and $b=x\ln x$? No, it's $(x-1)^2 + (x\ln x)^2 + 2x(x-1)\ln x$.
Let's check if it's a perfect square of the form $(A+B)^2$.
Let $A = x-1$ and $B = x \ln x$.
$(A+B)^2 = (x-1+x\ln x)^2 = (x-1)^2 + 2(x-1)(x\ln x) + (x\ln x)^2$
$$ (x-1+x\ln x)^2 = (x-1)^2 + 2(x^2-x)\ln x + x^2(\ln x)^2 $$
This matches $g(x)$. So, $g(x) = (x-1+x\ln x)^2$.

The sum $\sum_{k=1}^n g(x_k) = 0$ becomes $\sum_{k=1}^n (x_k-1+x_k\ln x_k)^2 = 0$.
Since each term $(x_k-1+x_k\ln x_k)^2$ is non-negative, their sum is zero if and only if each term is zero.
Thus, for each $k \in \{1, \ldots, n\}$, we must have:
$$ x_k-1+x_k\ln x_k = 0 $$
$$ x_k(1+\ln x_k) = 1 $$
Let $f(x) = x(1+\ln x)$ for $x>0$. We need to find the solutions to $f(x)=1$.
Let's analyze the function $f(x)$.
$f(x) = x + x \ln x$.
For $x=1$, $f(1) = 1 + 1 \ln 1 = 1 + 0 = 1$. So $x=1$ is a solution.
Let's check for other solutions by examining the derivative:
$f'(x) = \frac{d}{dx}(x) + \frac{d}{dx}(x \ln x) = 1 + (1 \cdot \ln x + x \cdot \frac{1}{x}) = 1 + \ln x + 1 = 2 + \ln x$.
$f'(x) = 0$ when $2 + \ln x = 0$, which means $\ln x = -2$, so $x = e^{-2}$.
The second derivative is $f''(x) = \frac{d}{dx}(2 + \ln x) = \frac{1}{x}$.
Since $x > 0$, $f''(x) = \frac{1}{x} > 0$. This means $f(x)$ is strictly convex for $x>0$.
A strictly convex function can intersect a horizontal line ($y=1$) at most twice.
The minimum value of $f(x)$ occurs at $x=e^{-2}$:
$f(e^{-2}) = e^{-2}(1 + \ln e^{-2}) = e^{-2}(1 - 2) = -e^{-2}$.
Since $-e^{-2} < 0 < 1$, the minimum value is less than 1.
Let's examine the limits of $f(x)$ as $x \to 0^+$ and $x \to \infty$.
$\lim_{x \to \infty} f(x) = \lim_{x \to \infty} x(1 + \ln x) = \infty \cdot \infty = \infty$.
For the limit as $x \to 0^+$, we have $f(x) = x + x \ln x$. We know $\lim_{x \to 0^+} x = 0$. For $\lim_{x \to 0^+} x \ln x$, let $x=1/y$. As $x \to 0^+$, $y \to \infty$.
$\lim_{y \to \infty} \frac{1}{y} \ln \left(\frac{1}{y}\right) = \lim_{y \to \infty} \frac{-\ln y}{y}$. By L'Hopital's rule, this limit is $\lim_{y \to \infty} \frac{-1/y}{1} = 0$.
So $\lim_{x \to 0^+} f(x) = 0 + 0 = 0$.

The function $f(x)$ starts at 0, decreases to a minimum of $-e^{-2}$ at $x=e^{-2}$, and then increases to $\infty$.
The minimum value $-e^{-2}$ is less than 1.
$f(x)$ decreases from 0 to $-e^{-2}$ on $(0, e^{-2}]$. The values of $f(x)$ in this interval are all less than or equal to 0. Thus, $f(x)=1$ has no solution in $(0, e^{-2}]$.
$f(x)$ increases from $-e^{-2}$ to $\infty$ on $[e^{-2}, \infty)$. In this interval, $f(x)$ takes every value greater than or equal to $-e^{-2}$ exactly once. Since $1 > -e^{-2}$, there is a unique solution to $f(x)=1$ in $[e^{-2}, \infty)$. We already found this solution, $x=1$.

Thus, the only positive solution to $x(1+\ln x)=1$ is $x=1$.
Since $x_k(1+\ln x_k)=1$ must hold for all $k=1, \ldots, n$, it must be that $x_k=1$ for all $k=1, \ldots, n$.

Let's check if $x_i=1$ for all $i$ is indeed a solution to the original system.
If $x_i=1$ for all $i$, then $\ln x_i = \ln 1 = 0$.
The $k$-th equation becomes:
$1^2 + (1 - 1 \ln 1)^2 = 2(1) - 2(1)^2 \ln 1$
$1 + (1 - 0)^2 = 2 - 0$
$1 + 1^2 = 2$
$1 + 1 = 2$, which is $2=2$.
This holds for all $k=1, \ldots, n$.
So, $(x_1, x_2, \ldots, x_n) = (1, 1, \ldots, 1)$ is a solution.

Since we showed that $x_k(1+\ln x_k)=1$ for all $k$ is a necessary condition for any solution $(x_1, \ldots, x_n)$ with $x_i>0$, and we proved that $x=1$ is the unique positive solution to $x(1+\ln x)=1$, the only possible solution is $x_k=1$ for all $k$.

The final answer is $\boxed{(1, 1, \ldots, 1)}$.