```markdown
We will prove that
\[
S(n)=\sum_{k=0}^n (-1)^{\lfloor k(\sqrt3-1)\rfloor}\ge1\quad\text{for all } n\ge0.
\]

Because the summand is defined via the parity of
\[
f(k)=\lfloor k(\sqrt3-1)\rfloor,
\]
it is natural to study the behavior of this floor‐function. (Note that \(\sqrt3-1\approx0.732\) so that every increment
\[
f(k+1)-f(k)
\]
is either \(0\) or \(1\) because
\[
0<\sqrt3-1<1.\])
In fact, by definition of the floor function,
\[
f(k+1)-f(k)=
\begin{cases}
0,&\text{if }\{k(\sqrt3-1)\}<1-(\sqrt3-1)=2-\sqrt3,\\[1mm]
1,&\text{if }\{k(\sqrt3-1)\}\ge2-\sqrt3.
\end{cases}
\]
Thus the sequence \(f(k)\) is nondecreasing with jumps of at most \(1\).

Because the function \(f\) “steps” only by \(0\) or \(1\) we can partition the indices into blocks of consecutive integers where \(f(k)\) remains constant. Define, for each integer \(m\ge0\), the block
\[
B_m=\{k\in\mathbb{N}_0 : \lfloor k(\sqrt3-1)\rfloor=m\}.
\]
Then we may rewrite
\[
S(n)=\sum_{m\ge0}\;\sum_{k\in B_m\cap\{0,1,\dots,n\}} (-1)^m.
\]
In other words, the contribution from all indices in \(B_m\) is simply (number of indices in \(B_m\) up to \(n\)) times \(({-1})^m\).

A short calculation shows that the “length” (or cardinality) of \(B_m\) is given by
\[
|B_m|=\left\lfloor\frac{m+1}{\sqrt3-1}\right\rfloor-\left\lfloor\frac{m}{\sqrt3-1}\right\rfloor.
\]
Since
\[
\frac{1}{\sqrt3-1}=\frac{\sqrt3+1}{2}\approx1.366,
\]
the interval
\[
\left[\frac{m}{\sqrt3-1},\frac{m+1}{\sqrt3-1}\right)
\]
has length about \(1.366\) so that \( |B_m| \) is either \(1\) or \(2\).

A direct check shows that the first few blocks are as follows. For \(m=0\) we have
\[
0\le k(\sqrt3-1)<1\quad\Longrightarrow\quad k<\frac{1}{\sqrt3-1}\approx1.366,
\]
so that \(k=0,1\in B_0\) (hence, \(B_0\) has 2 elements). For \(m=1\), the inequality
\[
1\le k(\sqrt3-1)<2
\]
gives
\[
k\in\left[\frac{1}{\sqrt3-1},\frac{2}{\sqrt3-1}\right)\approx[1.366,2.732),
\]
so that only \(k=2\) belongs to \(B_1\). A similar check shows that typically the even–indexed blocks (i.e. \(m\) even) have 2 elements while the odd–indexed blocks have 1 element. (One may also notice that—with the very mild fluctuations due to the irrationality of \(\sqrt3-1\)—the pattern is forced by the fact that the “step” occurs when the fractional part \(\{k(\sqrt3-1)\}\) exceeds \(2-\sqrt3\); this happens less often than not. In particular, the block \(B_0\) is always of size 2.)

Let us now examine the effect on the partial sum \(S(n)\) when we complete a whole block. Writing
\[
S(n)=\sum_{m=0}^{M-1}\Bigl(|B_m\cap\{0,1,\dots,n\}|\cdot (-1)^m\Bigr)
\]
until all complete blocks (with indices \(m=0,1,\dots,M-1\)) are finished, a brief computation yields:
- After finishing \(B_0\): \(S=\;2\) (since \(2\) terms of \(+1\)).
- After finishing \(B_1\): \(S=2-1=1\).
- After finishing \(B_2\) (which contributes \(+2\)) we have: \(S=1+2=3\).
- After finishing \(B_3\) (which contributes \(-1\)) we have: \(S=3-1=2\).
- After finishing \(B_4\) (usually of size \(1\)) we have: \(S=2-1=1\).

Moreover, if we stop in the middle of a block then the partial sum is either equal to the total at the end of the previous complete block or is larger (by an extra \(+1\) coming from the first term of an even block).

An inductive argument can now be given. The base case \(n=0\) is clear because
\[
S(0)=(-1)^{\lfloor0\cdot(\sqrt3-1)\rfloor}=(-1)^0=1.
\]
For the inductive step, suppose \(S(n)\ge1\) and consider \(S(n+1)=S(n)+(-1)^{\lfloor (n+1)(\sqrt3-1)\rfloor}\). There are two cases:
- If \(\lfloor (n+1)(\sqrt3-1)\rfloor=\lfloor n(\sqrt3-1)\rfloor\) then the \((n+1)\)th term has the same sign as the \(n\)th term and is equal to \(+1\) or \(-1\); in either case the sum increases (or at least does not drop) so that \(S(n+1)\ge S(n)\ge1\).
- If \(\lfloor (n+1)(\sqrt3-1)\rfloor=\lfloor n(\sqrt3-1)\rfloor+1\) then a “step” occurs; however, by the block analysis the step upward (which causes a sign flip) happens only after an even block (of \(+1\)’s) which contributed at least \(+2\) so that
  \[
  S(n)\ge2,
  \]
  and subtracting \(1\) (since the new term is \(-1\)) one still gets \(S(n+1)\ge1\).

Thus, by induction, the inequality
\[
\sum_{k=0}^n (-1)^{\lfloor k(\sqrt3-1)\rfloor}\ge 1
\]
holds for all \(n\ge0\).

---

In summary, the structure of the floor function \(\lfloor k(\sqrt3-1)\rfloor\) forces the \(+1\) terms (coming from the even values) to occur in blocks that are at least as long as needed to “protect” the summation from ever dropping below \(1\).
```