This step is worth 3 points.
The partial fraction decomposition of the expression
$$
\frac{48n^2+44n+9}{n(2n+1)(4n+1)(4n+3)}.
$$
is
$$
\frac{3}{n}-\frac{4}{4n+1}-\frac{4}{4n+2}-\frac{4}{4n+3}.
$$

This step is worth 7 points.
Then, for $N \geq 4$, we have
$$
\begin{aligned}
\sum_{n=1}^{N}\frac{48n^2+44n+9}{n(2n+1)(4n+1)(4n+3)}&=
\sum_{n=1}^{N}\left(\frac{3}{n}-\frac{4}{4n+1}-\frac{4}{4n+2}-\frac{4}{4n+3}\right)\\
&=\sum_{n=1}^{N}\left(\frac{4}{n}-\frac{4}{4n}-\frac{4}{4n+1}-\frac{4}{4n+2}-\frac{4}{4n+3}\right)\\
&=4\sum_{n=1}^{N}\left(\frac{1}{n}-\frac{1}{4n}-\frac{1}{4n+1}-\frac{1}{4n+2}-\frac{1}{4n+3}\right)\\
&=4\left(\sum_{n=1}^N \frac{1}{n}-\sum_{n=4}^{4N+3}\frac{1}{n}\right)\\
&=4\left(1+\frac{1}{2}+\frac{1}{3}-\sum_{n=N+1}^{4N+3}\frac{1}{n}\right)\\
&=4\left(1+\frac{1}{2}+\frac{1}{3}-\sum_{k=1}^{3N+3}\frac{1}{N+k}\right)\\
&=\frac{44}{6}-4\sum_{k=1}^{3N+3}\frac{1}{N+k}\\
&=\frac{44}{6}-4\cdot \frac{1}{N}\sum_{k=1}^{3N+3}\frac{1}{1+\frac{k}{N}}\\
&\xrightarrow[N\rightarrow+\infty]{}
\frac{44}{6}-4\int_0^3\frac{dx}{1+x}\\
&=\frac{44}{6}-4\ln 4=4\left(\frac{11}{6}-\ln 4\right).
\end{aligned}
$$