Let $p$ be a prime divisor of $a^{2^k}+b^{2^k}$ such that $p>2$.
We are given that $k, a, b$ are positive integers and $\gcd(a,b)=1$.
The condition $p | a^{2^k}+b^{2^k}$ means $a^{2^k}+b^{2^k} \equiv 0 \pmod{p}$.
This can be written as $a^{2^k} \equiv -b^{2^k} \pmod{p}$.

Since $\gcd(a,b)=1$, $p$ cannot divide both $a$ and $b$.
If $p|a$, then $a \equiv 0 \pmod{p}$. The congruence becomes $0^{2^k} + b^{2^k} \equiv 0 \pmod{p}$, which implies $b^{2^k} \equiv 0 \pmod{p}$. Since $p$ is prime, this means $p|b$. This contradicts $\gcd(a,b)=1$.
Similarly, if $p|b$, then $p|a$, which is a contradiction.
Thus, $p$ does not divide $a$ and $p$ does not divide $b$.
Since $p$ does not divide $b$, $b$ has a multiplicative inverse modulo $p$. Let $b^{-1}$ be the inverse of $b$ modulo $p$.

Multiply the congruence $a^{2^k} \equiv -b^{2^k} \pmod{p}$ by $(b^{-1})^{2^k}$ on both sides:
$a^{2^k} (b^{-1})^{2^k} \equiv -b^{2^k} (b^{-1})^{2^k} \pmod{p}$
$(ab^{-1})^{2^k} \equiv -(b b^{-1})^{2^k} \pmod{p}$
$(ab^{-1})^{2^k} \equiv -1^{2^k} \pmod{p}$
Let $x = ab^{-1} \pmod{p}$. Then $x^{2^k} \equiv -1 \pmod{p}$.

Since $p>2$, $-1 \not\equiv 1 \pmod{p}$. Thus $x^{2^k} \not\equiv 1 \pmod{p}$.
Squaring both sides of $x^{2^k} \equiv -1 \pmod{p}$, we get:
$(x^{2^k})^2 \equiv (-1)^2 \pmod{p}$
$x^{2^{k+1}} \equiv 1 \pmod{p}$.

Let $\text{ord}_p(x)$ be the order of $x$ modulo $p$.
The congruence $x^{2^{k+1}} \equiv 1 \pmod{p}$ implies that $\text{ord}_p(x)$ must divide $2^{k+1}$. So $\text{ord}_p(x)$ must be of the form $2^j$ for some integer $j$ with $0 \leq j \leq k+1$.
The congruence $x^{2^k} \equiv -1 \pmod{p}$ implies $x^{2^k} \not\equiv 1 \pmod{p}$. This means $\text{ord}_p(x)$ does not divide $2^k$. So $\text{ord}_p(x)$ cannot be of the form $2^j$ for $j \leq k$.
The only possibility remaining is that $\text{ord}_p(x) = 2^{k+1}$.

By Fermat's Little Theorem, since $p$ does not divide $a$ or $b$, $x = ab^{-1} \not\equiv 0 \pmod{p}$. Thus $x^{p-1} \equiv 1 \pmod{p}$.
This implies that $\text{ord}_p(x)$ must divide $p-1$.
So $2^{k+1}$ must divide $p-1$.

This means $p-1 = c \cdot 2^{k+1}$ for some integer $c$.
Thus $p = c \cdot 2^{k+1} + 1$.
Since $p$ is a prime and $p>2$, $p$ is odd. This means $p-1$ is even.
Since $k$ is a positive integer, $k \geq 1$, so $k+1 \geq 2$. Thus $2^{k+1}$ is divisible by 4, and hence even.
For $p = c \cdot 2^{k+1} + 1$ to be a prime greater than 2, $c \cdot 2^{k+1}$ must be a positive even integer. Since $2^{k+1} > 0$, $c$ must be a positive integer.

Any positive integer $c$ can be uniquely written in the form $c = 2^j m$ where $m$ is an odd positive integer and $j \geq 0$ is an integer.
Substitute this form of $c$ into the expression for $p$:
$p = (2^j m) \cdot 2^{k+1} + 1$
$p = m \cdot 2^{j+k+1} + 1$.

Let $d = j+k+1$.
Then $p = m \cdot 2^d + 1$.
We need to verify the conditions on $d$ and $m$.
By construction, $m$ is an odd positive integer.
Since $k$ is a positive integer, $k \geq 1$. Since $j \geq 0$, we have $d = j+k+1 \geq 0+1+1 = 2$.
In particular, $d = j+k+1 \geq k+1$ since $j \geq 0$.

Therefore, any prime divisor $p>2$ of $a^{2^k}+b^{2^k}$ is of the form $p=2^{d}m+1$, where $d\geq k+1$ and $m$ is an odd positive integer.

The final answer is $\boxed{p=2^{d}m+1, \text{ where } d\geq k+1 \text{ and } m \text{ is an odd positive integer}}$.