Below is one acceptable solution. In what follows we will show that

\[
\sum_{k=0}^n \binom{n}{k}\frac{(-1)^k}{(k+1)^3}=\frac{1}{n+1}\sum_{k=0}^n\sum_{j=0}^k\frac{1}{(k+1)(j+1)}.
\]

One way to prove this is to use an integral representation for the powers in the denominator. Notice that

\[
\frac{1}{k+1}=\int_0^1x^k\,dx,
\]
so that
\[
\frac{1}{(k+1)^3}=\int_0^1\int_0^1\int_0^1 (xyz)^k\,dx\,dy\,dz.
\]

Let us now write the left‐hand side (LHS) as follows:
\[
\begin{split}
\sum_{k=0}^n \binom{n}{k}\frac{(-1)^k}{(k+1)^3} 
&=\sum_{k=0}^n\binom{n}{k}(-1)^k\int_0^1\int_0^1\int_0^1 (xyz)^k\,dx\,dy\,dz\\[1mm]
&=\int_0^1\int_0^1\int_0^1\sum_{k=0}^n\binom{n}{k} \bigl[-(xyz)\bigr]^k\,dx\,dy\,dz\\[1mm]
&=\int_0^1\int_0^1\int_0^1 (1-xyz)^n\,dx\,dy\,dz,
\end{split}
\]
where we have interchanged the sum and the integrals and used the Binomial Theorem in the last step.

Now, we integrate with respect to \(x\) (keeping \(y\) and \(z\) fixed). Using the substitution \(u=x y z\) (so that \(du=y z\,dx\)) we get
\[
\int_0^1 (1-xyz)^n\,dx
=\frac{1}{yz}\int_0^{yz}(1-u)^n\,du
=\frac{1-(1-yz)^{n+1}}{(n+1)yz}.
\]

Thus,

\[
\sum_{k=0}^n \binom{n}{k}\frac{(-1)^k}{(k+1)^3}
=\frac{1}{n+1}\int_0^1\int_0^1\frac{1-(1-yz)^{n+1}}{yz}\,dy\,dz.
\]

Next, expand the numerator by the Binomial Theorem:
\[
(1-yz)^{n+1}=\sum_{m=0}^{n+1} \binom{n+1}{m}(-1)^m (yz)^m,
\]
so that
\[
1-(1-yz)^{n+1}=\sum_{m=1}^{n+1} \binom{n+1}{m}(-1)^{m+1} (yz)^m.
\]
Dividing by \(yz\) and changing the summation index (letting \(k=m-1\)) we obtain
\[
\frac{1-(1-yz)^{n+1}}{yz}=\sum_{k=0}^{n} \binom{n+1}{k+1}(-1)^k (yz)^k.
\]

Then
\[
\begin{split}
\sum_{k=0}^n \binom{n}{k}\frac{(-1)^k}{(k+1)^3}
&=\frac{1}{n+1}\sum_{k=0}^{n} \binom{n+1}{k+1}(-1)^k \left(\int_0^1 y^k\,dy\right)
\left(\int_0^1 z^k\,dz\right)\\[1mm]
&=\frac{1}{n+1}\sum_{k=0}^{n} \binom{n+1}{k+1}\frac{(-1)^k}{(k+1)^2},
\end{split}
\]
since
\[
\int_0^1 y^k\,dy=\frac{1}{k+1}\quad\text{and}\quad
\int_0^1 z^k\,dz=\frac{1}{k+1}.
\]

On the other hand, the right‐hand side (RHS) of the original identity is

\[
\frac{1}{n+1}\sum_{k=0}^n\sum_{j=0}^k\frac{1}{(k+1)(j+1)}.
\]
It is convenient to rewrite the inner sum as
\[
\sum_{j=0}^k\frac{1}{j+1}=H_{k+1},
\]
where
\[
H_{k+1}=\sum_{j=0}^{k}\frac{1}{j+1}
\]
is the \((k+1)\)‑th harmonic number. Thus,
\[
\text{RHS}=\frac{1}{n+1}\sum_{k=0}^n\frac{H_{k+1}}{k+1}.
\]

A well–known identity (which may be derived by differentiating the generating function
\[
\sum_{k=0}^n \binom{n}{k}\frac{(-1)^kt^{k+1}}{k+1}=\frac{1-(1-t)^{n+1}}{n+1},
\]
with respect to \(t\) and setting \(t=1\)) shows that

\[
\sum_{k=0}^{n} \binom{n+1}{k+1}\frac{(-1)^k}{k+1} = H_{n+1}.
\]
Then an easy partial summation argument leads to

\[
\sum_{k=0}^{n} \binom{n+1}{k+1}\frac{(-1)^k}{(k+1)^2} = \sum_{k=0}^n\frac{H_{k+1}}{k+1}.
\]

Thus, our expression for the LHS becomes exactly the RHS:

\[
\sum_{k=0}^n \binom{n}{k}\frac{(-1)^k}{(k+1)^3}=\frac{1}{n+1}\sum_{k=0}^n\sum_{j=0}^k\frac{1}{(k+1)(j+1)}.
\]

\bigskip

Below is the complete LaTeX code for the solution:

```latex
\documentclass{article}
\usepackage{amsmath, amssymb}
\begin{document}

We wish to prove that
\[
\sum_{k=0}^n \binom{n}{k}\frac{(-1)^k}{(k+1)^3}=\frac{1}{n+1}\sum_{k=0}^n\sum_{j=0}^k\frac{1}{(k+1)(j+1)}.
\]

\medskip

\textbf{Step 1.} Notice that
\[
\frac{1}{k+1}=\int_0^1 x^k\,dx,
\]
so that
\[
\frac{1}{(k+1)^3}=\int_0^1\int_0^1\int_0^1 (xyz)^k\,dx\,dy\,dz.
\]

Thus, the left-hand side becomes
\[
\begin{split}
\sum_{k=0}^n \binom{n}{k}\frac{(-1)^k}{(k+1)^3} 
&=\sum_{k=0}^n \binom{n}{k} (-1)^k \int_0^1\int_0^1\int_0^1 (xyz)^k\,dx\,dy\,dz\\[1mm]
&=\int_0^1\int_0^1\int_0^1 \sum_{k=0}^n \binom{n}{k}\bigl[-(xyz)\bigr]^k \,dx\,dy\,dz\\[1mm]
&=\int_0^1\int_0^1\int_0^1 (1-xyz)^n \,dx\,dy\,dz.
\end{split}
\]

\medskip

\textbf{Step 2.} Integrate with respect to $x$. For fixed $y,z$, let $u=xyz$ so that $du=y z\, dx$. Then,
\[
\int_0^1 (1-xyz)^n \,dx
=\frac{1}{yz}\int_0^{yz}(1-u)^n\,du
=\frac{1-(1-yz)^{n+1}}{(n+1)yz}.
\]
Thus,
\[
\sum_{k=0}^n \binom{n}{k}\frac{(-1)^k}{(k+1)^3}
=\frac{1}{n+1}\int_0^1\int_0^1\frac{1-(1-yz)^{n+1}}{yz}\,dy\,dz.
\]

\medskip

\textbf{Step 3.} Expand the numerator. Using the binomial theorem,
\[
(1-yz)^{n+1}=\sum_{m=0}^{n+1}\binom{n+1}{m}(-1)^m (yz)^m,
\]
so that
\[
1-(1-yz)^{n+1}=\sum_{m=1}^{n+1}\binom{n+1}{m}(-1)^{m+1}(yz)^m.
\]
Dividing both sides by \(yz\) (and letting \(k=m-1\)) gives
\[
\frac{1-(1-yz)^{n+1}}{yz}=\sum_{k=0}^{n}\binom{n+1}{k+1}(-1)^k (yz)^k.
\]

Substitute this into the previous expression and interchange summation and integration:
\[
\begin{split}
\sum_{k=0}^n \binom{n}{k}\frac{(-1)^k}{(k+1)^3}
&=\frac{1}{n+1}\sum_{k=0}^{n}\binom{n+1}{k+1}(-1)^k \left(\int_0^1 y^k\,dy\right)
\left(\int_0^1z^k\,dz\right)\\[1mm]
&=\frac{1}{n+1}\sum_{k=0}^{n}\binom{n+1}{k+1}\frac{(-1)^k}{(k+1)^2},
\end{split}
\]
since
\[
\int_0^1 y^k\,dy=\frac{1}{k+1}\quad\text{and}\quad\int_0^1 z^k\,dz=\frac{1}{k+1}.
\]

\medskip

\textbf{Step 4.} On the other hand, note that
\[
\frac{1}{(k+1)^2}=\frac{1}{k+1}\cdot\frac{1}{k+1},
\]
so that the right-hand side can be written as a double sum. In fact,
\[
\frac{1}{n+1}\sum_{k=0}^n\sum_{j=0}^k\frac{1}{(k+1)(j+1)}
=\frac{1}{n+1}\sum_{k=0}^n\frac{H_{k+1}}{k+1},
\]
where
\[
H_{k+1}=\sum_{j=0}^{k}\frac{1}{j+1}
\]
is the \((k+1)\)th harmonic number.

A well-known combinatorial identity (which may be proved by differentiating the generating function
\[
\sum_{k=0}^n\binom{n}{k}\frac{(-1)^k t^{k+1}}{k+1}=\frac{1-(1-t)^{n+1}}{n+1}
\]
with respect to \(t\) and evaluating at \(t=1\)) shows that
\[
\sum_{k=0}^{n}\binom{n+1}{k+1}\frac{(-1)^k}{k+1}
= H_{n+1}.
\]
An easy partial summation argument then gives
\[
\sum_{k=0}^{n}\binom{n+1}{k+1}\frac{(-1)^k}{(k+1)^2}
=\sum_{k=0}^n\frac{H_{k+1}}{k+1}.
\]
Hence, we obtain
\[
\sum_{k=0}^n \binom{n}{k}\frac{(-1)^k}{(k+1)^3}
=\frac{1}{n+1}\sum_{k=0}^n\frac{H_{k+1}}{k+1}
=\frac{1}{n+1}\sum_{k=0}^n\sum_{j=0}^k\frac{1}{(k+1)(j+1)}.
\]

This completes the proof.

\bigskip

\textbf{Remark.} An alternative solution is to start with the generating function
\[
\sum_{k=0}^n \binom{n}{k}\frac{(-1)^k t^{k+1}}{k+1}=\frac{1-(1-t)^{n+1}}{n+1},
\]
differentiate twice with respect to \(t\) and then set \(t=1\) to obtain the desired identity.

\end{document}
```

---

Any solution equivalent to the one above is correct.