Here is a detailed, step-by-step solution to the problem.

### Statement of the Problem

Let $f:\mathbb{R}\to\mathbb{R}$ be a real function with a continuous derivative. Assume that for all $x \in \mathbb{R}$, the following inequality holds:
$$|f'(x)|\leq |f(x)-f(0)|$$
Show that $f$ is a constant function.

### Strategy

To show that $f$ is constant, we need to prove that $f(x) = f(0)$ for all $x \in \mathbb{R}$. This is equivalent to showing that $f(x) - f(0) = 0$ for all $x$.

Let's define a new function $g(x) = f(x) - f(0)$. Our goal is to show that $g(x) = 0$ for all $x$. Let's translate the given information in terms of $g(x)$:

1.  **Value at origin:** $g(0) = f(0) - f(0) = 0$.
2.  **Derivative:** Since $f(0)$ is a constant, $g'(x) = f'(x)$.
3.  **The inequality:** Substituting $g'(x)$ and $g(x)$ into the given inequality, we get $|g'(x)| \leq |g(x)|$.

So the problem is reduced to proving the following:
*If $g: \mathbb{R} \to \mathbb{R}$ has a continuous derivative, with $g(0)=0$ and $|g'(x)| \leq |g(x)|$ for all $x$, then $g(x)=0$ for all $x$.*

We will prove this by considering a non-negative auxiliary function $h(x) = g(x)^2$ and analyzing its derivative. This technique is related to Grönwall's inequality. We will handle the cases for $x \geq 0$ and $x < 0$ separately.

---

### Step-by-Step Solution

**Step 1: Define an auxiliary function and analyze its properties**

Let $g(x) = f(x) - f(0)$ as defined above. Now, let's define a second auxiliary function $h(x)$:
$$h(x) = g(x)^2 = (f(x) - f(0))^2$$
Since $f$ has a continuous derivative, $g$ also has a continuous derivative. Therefore, $h(x)$ is also continuously differentiable.

Let's find the properties of $h(x)$:
*   $h(x) \geq 0$ for all $x \in \mathbb{R}$, since it is a square of a real number.
*   $h(0) = g(0)^2 = 0^2 = 0$.
*   The derivative of $h(x)$ is given by the chain rule:
    $$h'(x) = 2g(x)g'(x)$$

**Step 2: Bound the derivative of the auxiliary function**

We are given $|g'(x)| \leq |g(x)|$. Let's use this to find a bound for $h'(x)$.
We can take the absolute value of $h'(x)$:
$$|h'(x)| = |2g(x)g'(x)| = 2|g(x)||g'(x)|$$
Using the inequality $|g'(x)| \leq |g(x)|$, we get:
$$|h'(x)| \leq 2|g(x)||g(x)| = 2g(x)^2$$
Since $h(x) = g(x)^2$, this simplifies to:
$$|h'(x)| \leq 2h(x)$$
This inequality implies that $-2h(x) \leq h'(x) \leq 2h(x)$. We will use these two inequalities for the cases $x < 0$ and $x \geq 0$.

**Step 3: Prove that $g(x) = 0$ for $x \geq 0$**

For this case, we use the inequality $h'(x) \leq 2h(x)$.
Let's rearrange it:
$$h'(x) - 2h(x) \leq 0$$
This form suggests using an integrating factor, $e^{-2x}$. Let's multiply the inequality by $e^{-2x}$. Since $e^{-2x} > 0$ for all $x$, the direction of the inequality is preserved:
$$h'(x)e^{-2x} - 2h(x)e^{-2x} \leq 0$$
The left side is the derivative of $h(x)e^{-2x}$ by the product rule. So, we have:
$$\frac{d}{dx}\left(h(x)e^{-2x}\right) \leq 0$$
This means that the function $k(x) = h(x)e^{-2x}$ is a non-increasing function on $\mathbb{R}$.

Now, let's consider any $x \geq 0$. Since $k(x)$ is non-increasing, for $x \geq 0$, we must have:
$$k(x) \leq k(0)$$
We can calculate $k(0)$ using the fact that $h(0)=0$:
$$k(0) = h(0)e^{-2(0)} = 0 \cdot 1 = 0$$
So, for all $x \geq 0$, we have $k(x) \leq 0$.

On the other hand, we know $h(x) = g(x)^2 \geq 0$ and $e^{-2x} > 0$. Thus, their product must be non-negative:
$$k(x) = h(x)e^{-2x} \geq 0$$
For $x \geq 0$, we have shown both $k(x) \leq 0$ and $k(x) \geq 0$. The only possibility is that $k(x) = 0$ for all $x \geq 0$.
$$h(x)e^{-2x} = 0 \quad \text{for } x \geq 0$$
Since $e^{-2x}$ is never zero, we must have $h(x) = 0$ for all $x \geq 0$.
Because $h(x) = g(x)^2$, this implies $g(x)^2 = 0$, and thus $g(x) = 0$ for all $x \geq 0$.

**Step 4: Prove that $g(x) = 0$ for $x < 0$**

For this case, we use the other part of the inequality we derived in Step 2: $h'(x) \geq -2h(x)$.
Let's rearrange it:
$$h'(x) + 2h(x) \geq 0$$
This time, the integrating factor is $e^{2x}$. Multiplying by $e^{2x}$ (which is always positive), we get:
$$h'(x)e^{2x} + 2h(x)e^{2x} \geq 0$$
The left side is the derivative of $h(x)e^{2x}$:
$$\frac{d}{dx}\left(h(x)e^{2x}\right) \geq 0$$
This means that the function $m(x) = h(x)e^{2x}$ is a non-decreasing function on $\mathbb{R}$.

Now, let's consider any $x < 0$. Since $m(x)$ is non-decreasing, for $x < 0$, we must have:
$$m(x) \leq m(0)$$
We can calculate $m(0)$:
$$m(0) = h(0)e^{2(0)} = 0 \cdot 1 = 0$$
So, for all $x < 0$, we have $m(x) \leq 0$.

Again, we know that $h(x) = g(x)^2 \geq 0$ and $e^{2x} > 0$. Their product must be non-negative:
$$m(x) = h(x)e^{2x} \geq 0$$
For $x < 0$, we have shown both $m(x) \leq 0$ and $m(x) \geq 0$. This forces $m(x) = 0$ for all $x < 0$.
$$h(x)e^{2x} = 0 \quad \text{for } x < 0$$
Since $e^{2x}$ is never zero, we must have $h(x) = 0$ for all $x < 0$.
This implies $g(x)^2 = 0$, and thus $g(x) = 0$ for all $x < 0$.

**Step 5: Conclude the proof**

From Step 3, we have $g(x) = 0$ for all $x \geq 0$.
From Step 4, we have $g(x) = 0$ for all $x < 0$.

Combining these results, we find that $g(x) = 0$ for all $x \in \mathbb{R}$.
Recalling the definition of $g(x)$:
$$g(x) = f(x) - f(0)$$
So, we have shown that:
$$f(x) - f(0) = 0 \quad \text{for all } x \in \mathbb{R}$$
This means:
$$f(x) = f(0) \quad \text{for all } x \in \mathbb{R}$$
Therefore, the function $f$ must be a constant function, with its value equal to $f(0)$ everywhere.

### Final Conclusion

We have successfully shown that if a function $f$ with a continuous derivative satisfies the condition $|f'(x)|\leq |f(x)-f(0)|$ for all real numbers $x$, then $f$ must be a constant function. The proof relied on constructing an auxiliary function $h(x)=(f(x)-f(0))^2$ and using a standard technique for differential inequalities (a proof of Grönwall's lemma) to show that $h(x)$ must be identically zero. This, in turn, implies that $f(x)$ is constant.