```markdown
We start with
\[
f_n(x)=\prod_{k=1}^{n}\cos((2k-1)x).
\]
Using Eulerâ€™s formula,
\[
\cos((2k-1)x)=\frac{e^{i(2k-1)x}+e^{-i(2k-1)x}}{2},
\]
we can write
\[
f_n(x)=\frac{1}{2^n}\prod_{k=1}^{n}\Bigl(e^{i(2k-1)x}+e^{-i(2k-1)x}\Bigr)
=\frac{1}{2^n}\sum_{\epsilon_1,\epsilon_2,\dots,\epsilon_n\in\{-1,1\}}e^{i\left(\sum_{k=1}^{n}\epsilon_k(2k-1)\right)x}.
\]

Next, we integrate over the interval \([0,2\pi]\):
\[
I_n=\int_0^{2\pi}f_n(x)\,dx=\frac{1}{2^n}\sum_{\epsilon_1,\dots,\epsilon_n\in\{-1,1\}}\int_0^{2\pi}e^{i\left(\sum_{k=1}^{n}\epsilon_k(2k-1)\right)x}\,dx.
\]
Recall that
\[
\int_0^{2\pi}e^{imx}\,dx=
\begin{cases}
2\pi,& m=0,\\[1mm]
0,& m\neq 0.
\end{cases}
\]
Thus, only those choices of \((\epsilon_1,\dots,\epsilon_n)\) satisfying
\[
\sum_{k=1}^{n}\epsilon_k(2k-1)=0
\]
contribute to the integral. Denote by \(N_n\) the number of solutions to
\[
\sum_{k=1}^{n}\epsilon_k(2k-1)=0.
\]
Then we have
\[
I_n=\frac{2\pi}{2^n}\,N_n.
\]

A key observation is that
\[
\sum_{k=1}^{n}(2k-1)=n^2.
\]
Hence, when \(n\) is odd the total sum \(n^2\) is odd, and it is impossible to split the odd total into two equal parts; that is, there are no choices of signs giving a zero sum. Therefore, for all odd \(n\) we have
\[
N_n=0\quad\text{and}\quad I_n=0.
\]

Even when \(n\) is even, one may show (using, for example, the local central limit theorem applied to the random sum
\[
S_n=\sum_{k=1}^{n}\epsilon_k(2k-1)
\]
with variance
\[
\sigma_n^2=\sum_{k=1}^{n}(2k-1)^2\sim\frac{4}{3}n^3)
\]
that the number of solutions behaves roughly like
\[
N_n\sim\frac{2^n}{\sqrt{2\pi\,\sigma_n^2}}.
\]
Thus, for even \(n\) we obtain
\[
I_n=\frac{2\pi}{2^n}\,N_n\sim\frac{2\pi}{\sqrt{2\pi\,\sigma_n^2}}\sim\frac{2\pi}{\sqrt{\frac{8\pi}{3}n^3}},
\]
which decays to 0 as \(n\to\infty\).

Since \(I_n=0\) for all odd \(n\) and for even \(n\) the integral tends to 0, we conclude that
\[
\liminf_{n\to\infty}\int_0^{2\pi}f_n(x)\,dx=0.
\]

**Answer:** \(0\).
```