Let the initial sequence be $X^{(0)} = (x_1, x_2, \ldots, x_n)$.
After one action, the sequence becomes $X^{(1)} = (x_1^{(1)}, x_2^{(1)}, \ldots, x_{n-1}^{(1)})$, where $x_i^{(1)} = \sqrt{x_i x_{i+1}}$.
After $k$ actions, the sequence $X^{(k)}$ has $n-k$ elements. The $i$-th element of $X^{(k)}$ is $x_i^{(k)} = \sqrt{x_i^{(k-1)} x_{i+1}^{(k-1)}}$.
The process stops after $n-1$ actions, when the sequence $X^{(n-1)}$ has $n-(n-1)=1$ element. This single element is the result, let's call it $R$. $R = x_1^{(n-1)}$.

The definition of the action, which transforms a sequence of length $m$ into a sequence of length $m-1$, requires $m \ge 2$. The process starts with a sequence of length $n$. The first action requires $n \ge 2$. The $(n-1)$-th action transforms a sequence of length $n-(n-2)=2$ to length $n-(n-1)=1$, which also requires the length to be at least 2 for the action to be applicable. Thus, the problem implicitly assumes $n \ge 2$. For $n=1$, the sequence has length 1, and the action is not applicable as defined. $n-1=0$ actions mean no change, and the result is $x_1$. The inequality $1 < (1+1)/2$ is false. So we consider $n \ge 2$.

Let's express $R$ in terms of the initial elements $x_1, \ldots, x_n$.
$x_i^{(1)} = (x_i x_{i+1})^{1/2} = x_i^{1/2} x_{i+1}^{1/2}$.
$x_i^{(2)} = \sqrt{x_i^{(1)} x_{i+1}^{(1)}} = (x_i^{(1)})^{1/2} (x_{i+1}^{(1)})^{1/2} = (x_i^{1/2} x_{i+1}^{1/2})^{1/2} (x_{i+1}^{1/2} x_{i+2}^{1/2})^{1/2} = x_i^{1/4} x_{i+1}^{1/4} x_{i+1}^{1/4} x_{i+2}^{1/4} = x_i^{1/4} x_{i+1}^{1/2} x_{i+2}^{1/4}$.
In general, it can be shown by induction that $x_i^{(k)} = \prod_{j=i}^{i+k} x_j^{\alpha_{j,i}^{(k)}}$, where $\alpha_{j,i}^{(k)} = \frac{1}{2^k} \binom{k}{j-i}$ for $i \le j \le i+k$, and $\alpha_{j,i}^{(k)}=0$ otherwise.
The base case $k=0$ is $x_i^{(0)} = x_i^1$, so $\alpha_{j,i}^{(0)}=1$ if $j=i$ and 0 otherwise, which matches $\frac{1}{2^0}\binom{0}{j-i}=1$ for $j=i$.
Assume the formula holds for $k$. Then
$x_i^{(k+1)} = \sqrt{x_i^{(k)} x_{i+1}^{(k)}} = \left(\prod_{j=i}^{i+k} x_j^{\alpha_{j,i}^{(k)}}\right)^{1/2} \left(\prod_{j=i+1}^{i+k+1} x_j^{\alpha_{j,i+1}^{(k)}}\right)^{1/2} = \prod_{j=i}^{i+k+1} x_j^{(\alpha_{j,i}^{(k)} + \alpha_{j,i+1}^{(k)})/2}$.
Here we define $\alpha_{j,i}^{(k)}=0$ if $j<i$ or $j>i+k$.
So $\alpha_{j,i}^{(k+1)} = \frac{1}{2}(\alpha_{j,i}^{(k)} + \alpha_{j,i+1}^{(k)})$.
Using the hypothesis: $\alpha_{j,i}^{(k+1)} = \frac{1}{2} \left( \frac{1}{2^k} \binom{k}{j-i} + \frac{1}{2^k} \binom{k}{j-(i+1)} \right) = \frac{1}{2^{k+1}} \left( \binom{k}{j-i} + \binom{k}{j-i-1} \right)$.
By Pascal's identity $\binom{k}{r} + \binom{k}{r-1} = \binom{k+1}{r}$, with $r=j-i$:
$\alpha_{j,i}^{(k+1)} = \frac{1}{2^{k+1}} \binom{k+1}{j-i}$ for $i \le j \le i+k+1$. This completes the induction.

The result is $R = x_1^{(n-1)}$. Here $i=1$ and $k=n-1$. The coefficients are $\alpha_{j,1}^{(n-1)} = \frac{1}{2^{n-1}} \binom{n-1}{j-1}$ for $j=1, \ldots, n$.
So $R = \prod_{j=1}^n x_j^{\frac{\binom{n-1}{j-1}}{2^{n-1}}}$.
The initial sequence is $(1, 2, \ldots, n)$, so $x_j=j$.
$R = \prod_{j=1}^n j^{\frac{\binom{n-1}{j-1}}{2^{n-1}}}$.
Let $w_j = \frac{\binom{n-1}{j-1}}{2^{n-1}}$ for $j=1, \ldots, n$. These are positive weights for $n \ge 2$ and $j \in \{1, \ldots, n\}$.
The sum of the weights is $\sum_{j=1}^n w_j = \sum_{j=1}^n \frac{\binom{n-1}{j-1}}{2^{n-1}} = \frac{1}{2^{n-1}} \sum_{k=0}^{n-1} \binom{n-1}{k} = \frac{1}{2^{n-1}} 2^{n-1} = 1$.
The result $R$ is the weighted geometric mean of the numbers $1, 2, \ldots, n$ with weights $w_j$.

By the AM-GM inequality, for positive numbers $a_1, \ldots, a_m$ and positive weights $w_1, \ldots, w_m$ with $\sum w_i = 1$, we have $\prod a_i^{w_i} \le \sum w_i a_i$.
Applying this to $a_j=j$ and $w_j = \frac{\binom{n-1}{j-1}}{2^{n-1}}$:
$R = \prod_{j=1}^n j^{w_j} \le \sum_{j=1}^n w_j j = \sum_{j=1}^n \frac{\binom{n-1}{j-1}}{2^{n-1}} j$.
Let's calculate the weighted arithmetic mean:
$\sum_{j=1}^n j \frac{\binom{n-1}{j-1}}{2^{n-1}} = \frac{1}{2^{n-1}} \sum_{j=1}^n j \binom{n-1}{j-1}$.
Let $k=j-1$. The sum is $\sum_{k=0}^{n-1} (k+1) \binom{n-1}{k} = \sum_{k=0}^{n-1} k \binom{n-1}{k} + \sum_{k=0}^{n-1} \binom{n-1}{k}$.
The second sum is the binomial expansion of $(1+1)^{n-1}$, which is $2^{n-1}$.
For the first sum, we use the identity $k \binom{m}{k} = m \binom{m-1}{k-1}$.
$\sum_{k=0}^{n-1} k \binom{n-1}{k} = \sum_{k=1}^{n-1} k \binom{n-1}{k}$ (the term for $k=0$ is 0).
$\sum_{k=1}^{n-1} (n-1) \binom{n-2}{k-1}$. Let $l=k-1$.
$\sum_{l=0}^{n-2} (n-1) \binom{n-2}{l} = (n-1) \sum_{l=0}^{n-2} \binom{n-2}{l} = (n-1) 2^{n-2}$.
The weighted arithmetic mean is $\frac{1}{2^{n-1}} ((n-1) 2^{n-2} + 2^{n-1}) = \frac{1}{2^{n-1}} (n-1+2) 2^{n-2} = \frac{n+1}{2^{n-1}} 2^{n-2} = \frac{n+1}{2}$.

So, by AM-GM inequality, $R \le \frac{n+1}{2}$.
The equality in AM-GM holds if and only if all the numbers $a_j$ are equal. In this case, the numbers are $1, 2, \ldots, n$.
For $n \ge 2$, the numbers $1, 2, \ldots, n$ are not all equal.
Therefore, the inequality is strict for $n \ge 2$:
$R < \frac{n+1}{2}$.

The final answer is $\boxed{\text{The result is smaller then } \frac{n+1}2}$.