Below is one complete solution written in LaTeX (inside a Markdown code block). One acceptable answer is to show that the integrand dominates a telescoping logarithmic sum which diverges. In our solution we shall use the following wellâ€known inequality: for any numbers \(a>b>0\) if we set \(u=\frac{a}{b}>1\) then
\[
\frac{a-b}{b}=u-1\ge \ln u=\ln\frac{a}{b}.
\]
We now give one version of the solution.

Below is the full LaTeX code:

```latex
\documentclass{article}
\usepackage{amsmath,amssymb}

\begin{document}

\textbf{Problem.} Let \(\alpha>0\) and \(f:[0,\infty)\to\mathbb{R}\) be a strictly decreasing continuous function such that 
\[
\lim_{x\to\infty}f(x)=0.
\]
Prove that
\[
\int_\alpha^\infty \frac{f(x-\alpha)-f(x+\alpha)}{f(x)}\,dx= \infty.
\]

\bigskip

\textbf{Solution.} 

Since \(f\) is strictly decreasing, for all \(x\ge \alpha\) we have
\[
f(x-\alpha)> f(x)> f(x+\alpha),
\]
so that the numerator \(f(x-\alpha)-f(x+\alpha)\) and the integrand 
\[
\frac{f(x-\alpha)-f(x+\alpha)}{f(x)}
\]
are positive.

We first write
\[
\frac{f(x-\alpha)-f(x+\alpha)}{f(x)}
=\frac{f(x-\alpha)-f(x)}{f(x)}+\frac{f(x)-f(x+\alpha)}{f(x)}.
\]
Since \(f\) is decreasing, we also have \(f(x)\ge f(x+\alpha)\) so that
\[
\frac{f(x)-f(x+\alpha)}{f(x)}\ge \frac{f(x)-f(x+\alpha)}{f(x+\alpha)}.
\]
Altogether,
\[
\frac{f(x-\alpha)-f(x+\alpha)}{f(x)}
\ge \frac{f(x-\alpha)-f(x)}{f(x)}+\frac{f(x)-f(x+\alpha)}{f(x+\alpha)}.
\]
Now, applying the inequality 
\[
\frac{a-b}{b}\ge \ln\frac{a}{b},
\]
first with \(a=f(x-\alpha)\) and \(b=f(x)\) and then with \(a=f(x)\) and \(b=f(x+\alpha)\), we obtain
\[
\frac{f(x-\alpha)-f(x)}{f(x)}\ge \ln\frac{f(x-\alpha)}{f(x)}
\]
and
\[
\frac{f(x)-f(x+\alpha)}{f(x+\alpha)}\ge \ln\frac{f(x)}{f(x+\alpha)}.
\]
Adding these inequalities gives
\[
\frac{f(x-\alpha)-f(x)}{f(x)}+\frac{f(x)-f(x+\alpha)}{f(x+\alpha)}
\ge \ln\left(\frac{f(x-\alpha)}{f(x)}\cdot \frac{f(x)}{f(x+\alpha)}\right)
=\ln\frac{f(x-\alpha)}{f(x+\alpha)}.
\]
Thus, we have shown that
\[
\frac{f(x-\alpha)-f(x+\alpha)}{f(x)}\ge \ln\frac{f(x-\alpha)}{f(x+\alpha)}\quad \text{for all } x\ge \alpha.
\]
It follows that
\[
\int_\alpha^\infty \frac{f(x-\alpha)-f(x+\alpha)}{f(x)}\,dx \ge \int_\alpha^\infty \ln\frac{f(x-\alpha)}{f(x+\alpha)}\,dx.
\]

Next, we perform the substitution \(u=x-\alpha\). Then \(x=u+\alpha\) and \(dx=du\). The new limits are: when \(x=\alpha\) then \(u=0\) and when \(x\to\infty\) then \(u\to\infty\). Hence,
\[
\int_\alpha^\infty \ln\frac{f(x-\alpha)}{f(x+\alpha)}\,dx 
=\int_0^\infty \ln\frac{f(u)}{f(u+2\alpha)}\,du.
\]
This can be written as
\[
\int_0^\infty \left[\ln f(u)-\ln f(u+2\alpha)\right]du.
\]
Now, partition the interval \([0,\infty)\) into segments of length \(2\alpha\). Namely, for any integer \(n\ge 0\) consider the interval 
\[
I_n=[2n\alpha, 2(n+1)\alpha].
\]
Then,
\[
\int_0^{2N\alpha}\left[\ln f(u)-\ln f(u+2\alpha)\right]du
=\sum_{n=0}^{N-1}\int_{2n\alpha}^{2(n+1)\alpha}\Big[\ln f(u)-\ln f(u+2\alpha)\Big]du.
\]
A telescoping sum shows that
\[
\sum_{n=0}^{N-1}\int_{2n\alpha}^{2(n+1)\alpha}\Big[\ln f(u)-\ln f(u+2\alpha)\Big]du
=\int_{0}^{2\alpha}\ln f(u)\,du -\int_{2N\alpha}^{2N\alpha+2\alpha}\ln f(u)\,du.
\]
Since \(f\) is strictly decreasing with \(\lim_{x\to\infty}f(x)=0\), we have \(\ln f(u)\to -\infty\) as \(u\to\infty\). In particular, 
\[
\int_{2N\alpha}^{2N\alpha+2\alpha}\ln f(u)\,du \le 2\alpha\,\ln f(2N\alpha)
\]
tends to \(-\infty\) as \(N\to\infty\). Therefore,
\[
\int_0^{2N\alpha}\left[\ln f(u)-\ln f(u+2\alpha)\right]du\to \infty\quad \text{as } N\to\infty.
\]
Thus, 
\[
\int_0^\infty \ln\frac{f(u)}{f(u+2\alpha)}\,du =\infty,
\]
and hence
\[
\int_\alpha^\infty \frac{f(x-\alpha)-f(x+\alpha)}{f(x)}\,dx=\infty.
\]

\bigskip

\textbf{Conclusion.} The integral diverges:
\[
\int_\alpha^\infty \frac{f(x-\alpha)-f(x+\alpha)}{f(x)}\,dx= \infty.
\]

\end{document}
```

### Explanation of the Main Ideas

1. Since \(f\) is strictly decreasing, the difference \(f(x-\alpha)-f(x+\alpha)\) is positive.
2. We write the difference as the sum of two differences and then use the inequality
   \[
   \frac{a-b}{b}\geq \ln\frac{a}{b}\quad (a>b>0)
   \]
   to bound each term from below.
3. With the substitution \(u=x-\alpha\) the integral becomes a telescoping sum in the logarithms.
4. Because \(\lim_{x\to\infty}f(x)=0\) (so that \(\ln f(x)\to-\infty\)), the telescoped sum diverges to \(+\infty\).

Any solution that shows these steps is acceptable.

Happy TeXing!