Solution:
Let the integral be denoted by $I_n$:
$$
I_n = \int_0^1 \frac{(1-\ln(1-x))^n}{n!} \, dx.
$$
We perform a substitution to simplify the integrand. Let $u = 1-\ln(1-x)$.
Then $\ln(1-x) = 1-u$.
Taking the exponential of both sides, we get $1-x = e^{1-u}$.
This implies $x = 1 - e^{1-u}$.
Differentiating with respect to $u$, we find $dx = -e^{1-u}(-1) du = e^{1-u} du$.

Now we need to change the limits of integration:
When $x=0$, $u = 1-\ln(1-0) = 1-\ln(1) = 1$.
As $x \to 1^-$, $1-x \to 0^+$, so $\ln(1-x) \to -\infty$. Thus, $u = 1 - \ln(1-x) \to 1 - (-\infty) = \infty$.

Substituting $u$ and $dx$ into the integral $I_n$, we get:
$$
I_n = \int_1^\infty \frac{u^n}{n!} e^{1-u} \, du.
$$
We can factor out the constant $e^1 = e$ from the integral:
$$
I_n = e \int_1^\infty \frac{u^n}{n!} e^{-u} \, du.
$$
Let $K_n = \int_1^\infty \frac{u^n}{n!} e^{-u} \, du$. Then $I_n = e K_n$.
We want to find the limit $\lim_{n\to\infty} I_n = e \lim_{n\to\infty} K_n$.

Recall the definition of the Gamma function $\Gamma(z) = \int_0^\infty t^{z-1} e^{-t} dt$.
For positive integers $n$, $\Gamma(n+1) = n!$.
This means $\int_0^\infty u^n e^{-u} du = n!$.
Dividing by $n!$, we have:
$$
\int_0^\infty \frac{u^n}{n!} e^{-u} \, du = 1.
$$
We can split this integral into two parts:
$$
\int_0^\infty \frac{u^n}{n!} e^{-u} \, du = \int_0^1 \frac{u^n}{n!} e^{-u} \, du + \int_1^\infty \frac{u^n}{n!} e^{-u} \, du.
$$
Let $J_n = \int_0^1 \frac{u^n}{n!} e^{-u} \, du$. The second term is $K_n$.
So we have the relation:
$$
1 = J_n + K_n.
$$
To find the limit of $K_n$ as $n\to\infty$, we can analyze the limit of $J_n$.
$$
J_n = \int_0^1 \frac{u^n}{n!} e^{-u} \, du.
$$
For $u \in [0, 1]$, the function $e^{-u}$ is bounded between $e^{-1}$ and $e^0=1$.
Specifically, $e^{-1} \le e^{-u} \le 1$ for $u \in [0, 1]$.
Using these bounds, we can estimate $J_n$:
Lower bound:
$$
J_n \ge \int_0^1 \frac{u^n}{n!} e^{-1} \, du = \frac{e^{-1}}{n!} \int_0^1 u^n \, du = \frac{e^{-1}}{n!} \left[ \frac{u^{n+1}}{n+1} \right]_0^1 = \frac{e^{-1}}{n!(n+1)} = \frac{e^{-1}}{(n+1)!}.
$$
Upper bound:
$$
J_n \le \int_0^1 \frac{u^n}{n!} (1) \, du = \frac{1}{n!} \int_0^1 u^n \, du = \frac{1}{n!} \left[ \frac{u^{n+1}}{n+1} \right]_0^1 = \frac{1}{n!(n+1)} = \frac{1}{(n+1)!}.
$$
So, we have the inequality:
$$
\frac{e^{-1}}{(n+1)!} \le J_n \le \frac{1}{(n+1)!}.
$$
As $n \to \infty$, $(n+1)! \to \infty$. Therefore,
$$
\lim_{n\to\infty} \frac{1}{(n+1)!} = 0,
$$
and
$$
\lim_{n\to\infty} \frac{e^{-1}}{(n+1)!} = e^{-1} \cdot 0 = 0.
$$
By the Squeeze Theorem, since $J_n$ is bounded between two sequences that converge to 0, we must have:
$$
\lim_{n\to\infty} J_n = 0.
$$
Now we use the relation $K_n = 1 - J_n$. Taking the limit as $n\to\infty$:
$$
\lim_{n\to\infty} K_n = \lim_{n\to\infty} (1 - J_n) = 1 - \lim_{n\to\infty} J_n = 1 - 0 = 1.
$$
Finally, we can find the limit of the original integral $I_n = e K_n$:
$$
\lim_{n\to\infty} I_n = \lim_{n\to\infty} (e K_n) = e \lim_{n\to\infty} K_n = e \cdot 1 = e.
$$

Final Answer: The final answer is $\boxed{e}$