```markdown
**Solution.**  
Define the normalized sequence
\[
b_n=\frac{a_n}{3^n}\,. 
\]
Since \(a_n>0\), each \(b_n>0\).  We first rewrite the given recurrence
\[
a_{n+2}=4\,a_{n+1}-3\,a_n+\frac{3^n}{a_n}
\]
in terms of \(b_n\).  Divide both sides by \(3^{n+2}\):
\[
\frac{a_{n+2}}{3^{n+2}}
=\frac{4\,a_{n+1}}{3^{n+2}}
-\frac{3\,a_n}{3^{n+2}}
+\frac{3^n}{a_n\,3^{n+2}}.
\]
But 
\[
\frac{a_{n+1}}{3^{n+2}}
=\frac{a_{n+1}}{3^{n+1}}\;\frac1{3}
=\frac{b_{n+1}}{3},
\quad
\frac{a_n}{3^{n+2}}
=\frac{b_n}{9},
\quad
\frac{3^n}{a_n\,3^{n+2}}
=\frac{1}{9\,a_n}
=\frac{1}{9\,b_n\,3^n}\,.
\]
Hence
\[
b_{n+2}
=\frac{4}{3}\,b_{n+1}
-\frac{1}{3}\,b_n
+\frac{1}{9\,b_n\,3^n}\,. 
\]
Set the forward difference
\[
d_n=b_n-b_{n-1},\qquad n\ge2.
\]
Then
\[
b_{n+2}-b_{n+1}
=\frac{1}{3}\bigl(b_{n+1}-b_n\bigr)
+\frac{1}{9\,b_n\,3^n},
\]
i.e.
\[
d_{n+1}
=\frac{1}{3}\,d_n
+\frac{1}{9\,b_n\,3^n}\,. 
\]
Since all \(b_n>0\), the inhomogeneous term is positive, and by induction
\[
d_n>0\quad\Longrightarrow\quad b_n\text{ is strictly increasing.}
\]
To show convergence we bound \(d_n\) by a simpler linear inhomogeneity.  Note
that \(b_n\ge b_1=a_1/3=1\), so
\[
\frac{1}{9\,b_n\,3^n}\le\frac{1}{9\cdot1\cdot3^n}
=\frac{1}{9\cdot3^n}\,.
\]
Hence for \(n\ge2\),
\[
d_n\;\le\;\frac{1}{3}\,d_{n-1}+\frac{1}{9\cdot3^{\,n-1}}.
\]
Unwinding this (by the usual iteration or induction) gives
\[
d_n
\le\Bigl(\tfrac13\Bigr)^{n-1}d_1
\;+\;\sum_{k=2}^n\Bigl(\tfrac13\Bigr)^{\,n-k}\,\frac{1}{9\cdot3^{\,k-1}}
\;=\;\Bigl(\tfrac13\Bigr)^{n-1}d_1
\;+\;\frac{n-1}{9\cdot3^{\,n-1}}.
\]
Since \(d_1=b_2-b_1=\tfrac{10}{9}-1=\tfrac{1}{9}\), we get
\[
d_n\;\le\;\frac{1}{9}\Bigl(\tfrac13\Bigr)^{n-1}
\;+\;\frac{n-1}{9\cdot3^{\,n-1}}.
\]
Therefore the infinite series of increments converges:
\[
\sum_{n=1}^\infty d_n
\;\le\;\sum_{n=1}^\infty\Bigl[\tfrac{1}{9}\Bigl(\tfrac13\Bigr)^{n-1}
+\frac{n-1}{9\cdot3^{\,n-1}}\Bigr]
=\underbrace{\frac{d_1}{1-\tfrac13}}_{=\;1/6}
\;+\;\underbrace{\frac{1}{9}\sum_{k=0}^\infty k\Bigl(\tfrac13\Bigr)^k}
_{=\;1/12}
\;=\;\frac14.
\]
Hence
\[
b_n=b_1+\sum_{k=2}^n d_k
\]
is increasing and bounded above by
\[
b_1+\sum_{k=2}^\infty d_k
\le1+\frac14=\frac54\,.
\]
By the Monotone Convergence Theorem the limit
\(\displaystyle L=\lim_{n\to\infty}b_n\) exists, and we have shown
\[
0<b_1<b_2<\dots<b_n<\cdots< L\le\frac54<\frac74.
\]
Equivalently,
\[
\lim_{n\to\infty}\frac{a_n}{3^n}=L
\quad\text{exists and satisfies}\quad L\le\frac74.
\]
This completes the proof. âˆŽ
```