```markdown
**Solution.**

Rewrite the given system cyclically as
\[
x_i^2 \;+\;\bigl(1 - x_{i+1}\ln x_{i+1}\bigr)^2
\;=\;2x_{i+1}\;-\;2\,x_{i+2}^2\ln x_{i+2},
\qquad i=1,2,\dots,n,
\]
where indices are taken moduloÂ \(n\).  Summing these \(n\) equations gives
\[
\sum_{i=1}^n
\Bigl[x_i^2 + (1 - x_i\ln x_i)^2\Bigr]
\;=\;
\sum_{i=1}^n
\bigl[\,2x_i - 2\,x_i^2\ln x_i\bigr]
\;\Longrightarrow\;
\sum_{i=1}^n
\Bigl[x_i^2 + (1 - x_i\ln x_i)^2 + 2x_i^2\ln x_i - 2x_i\Bigr]
=0.
\]
But for each \(i\),
\[
x_i^2 + (1 - x_i\ln x_i)^2 + 2x_i^2\ln x_i - 2x_i
= \bigl[x_i(1+\ln x_i)-1\bigr]^2.
\]
Hence
\[
\sum_{i=1}^n \bigl[x_i(1+\ln x_i)-1\bigr]^2 \;=\;0
\]
forces
\[
x_i(1+\ln x_i)-1=0
\quad\Longrightarrow\quad
x_i(1+\ln x_i)=1
\quad (i=1,\dots,n).
\]
The equation \(x(1+\ln x)=1\) has the unique positive solution \(x=1\).  Therefore the only solution of the original system is
\[
\boxed{(x_1,x_2,\dots,x_n)=(1,1,\dots,1)}.
\]
```