Let $g(x) = f(x) - f(0)$. Since $f$ has a continuous derivative, $g(x)$ also has a continuous derivative, given by $g'(x) = f'(x)$. The given inequality $|f'(x)| \leq |f(x) - f(0)|$ can be written as $|g'(x)| \leq |g(x)|$ for all $x \in \mathbb{R}$.
Note that $g(0) = f(0) - f(0) = 0$.

We want to show that $f$ is a constant function. This is equivalent to showing that $g(x) = 0$ for all $x \in \mathbb{R}$.

Let's consider the function $h(x) = g(x)^2$. Since $g(x)$ is differentiable and $g'(x)$ is continuous, $h(x)$ is differentiable and $h'(x)$ is continuous.
$h'(x) = 2g(x)g'(x)$.

From the inequality $|g'(x)| \leq |g(x)|$, we have $g'(x)^2 \leq g(x)^2$. Also, we have $-|g(x)| \leq g'(x) \leq |g(x)|$.
Multiplying the inequalities by $g(x)$, we consider two cases:
If $g(x) > 0$, we multiply by $g(x)$ (positive): $-g(x)^2 \leq g(x)g'(x) \leq g(x)^2$.
If $g(x) < 0$, we multiply by $g(x)$ (negative): $g(x)|g(x)| \leq g(x)g'(x) \leq -g(x)|g(x)|$. This becomes $g(x)(-g(x)) \leq g(x)g'(x) \leq -g(x)(g(x))$, which simplifies to $-g(x)^2 \leq g(x)g'(x) \leq g(x)^2$.
If $g(x) = 0$, then $|g'(x)| \leq 0$, which implies $g'(x) = 0$. In this case, $h'(x) = 2(0)(0) = 0$, and $-g(x)^2 \leq g(x)g'(x) \leq g(x)^2$ becomes $0 \leq 0 \leq 0$, which is true.

So, for all $x \in \mathbb{R}$, we have $-g(x)^2 \leq g(x)g'(x) \leq g(x)^2$.
Multiplying by 2, we get $-2g(x)^2 \leq 2g(x)g'(x) \leq 2g(x)^2$.
Since $h(x) = g(x)^2$ and $h'(x) = 2g(x)g'(x)$, this inequality is equivalent to:
$-2h(x) \leq h'(x) \leq 2h(x)$ for all $x \in \mathbb{R}$.

We want to show that $h(x) = 0$ for all $x \in \mathbb{R}$. Since $h(x) = g(x)^2$, $h(x) \geq 0$. Also, $h(0) = g(0)^2 = 0^2 = 0$.

Consider $x > 0$. Define the function $\phi(x) = e^{-2x}h(x)$ for $x \geq 0$.
$\phi(x)$ is differentiable on $(0, \infty)$ and continuous on $[0, \infty)$.
$\phi'(x) = -2e^{-2x}h(x) + e^{-2x}h'(x) = e^{-2x}(h'(x) - 2h(x))$.
From the inequality $h'(x) \leq 2h(x)$, we have $h'(x) - 2h(x) \leq 0$.
Since $e^{-2x} > 0$, we have $\phi'(x) \leq 0$ for $x > 0$.
Thus, $\phi(x)$ is a non-increasing function on $[0, \infty)$.
For any $x > 0$, we have $\phi(x) \leq \phi(0)$.
$\phi(0) = e^{-2(0)}h(0) = e^0 \cdot 0 = 1 \cdot 0 = 0$.
So, for $x > 0$, $\phi(x) \leq 0$.
$e^{-2x}h(x) \leq 0$.
Since $e^{-2x} > 0$, we must have $h(x) \leq 0$.
As $h(x) = g(x)^2 \geq 0$ by definition, the only possibility is $h(x) = 0$ for all $x > 0$.

Consider $x < 0$. Define the function $\psi(x) = e^{2x}h(x)$ for $x \leq 0$.
$\psi(x)$ is differentiable on $(-\infty, 0)$ and continuous on $(-\infty, 0]$.
$\psi'(x) = 2e^{2x}h(x) + e^{2x}h'(x) = e^{2x}(h'(x) + 2h(x))$.
From the inequality $h'(x) \geq -2h(x)$, we have $h'(x) + 2h(x) \geq 0$.
Since $e^{2x} > 0$, we have $\psi'(x) \geq 0$ for $x < 0$.
Thus, $\psi(x)$ is a non-decreasing function on $(-\infty, 0]$.
For any $x < 0$, we have $\psi(x) \leq \psi(0)$.
$\psi(0) = e^{2(0)}h(0) = e^0 \cdot 0 = 1 \cdot 0 = 0$.
So, for $x < 0$, $\psi(x) \leq 0$.
$e^{2x}h(x) \leq 0$.
Since $e^{2x} > 0$, we must have $h(x) \leq 0$.
As $h(x) = g(x)^2 \geq 0$ by definition, the only possibility is $h(x) = 0$ for all $x < 0$.

We have shown that $h(x) = 0$ for all $x > 0$ and for all $x < 0$. Since $h(0) = 0$, we conclude that $h(x) = 0$ for all $x \in \mathbb{R}$.
$h(x) = g(x)^2 = 0$ for all $x \in \mathbb{R}$.
This implies $g(x) = 0$ for all $x \in \mathbb{R}$.
Since $g(x) = f(x) - f(0)$, we have $f(x) - f(0) = 0$ for all $x \in \mathbb{R}$.
$f(x) = f(0)$ for all $x \in \mathbb{R}$.
This shows that $f$ is a constant function.

The final answer is $\boxed{f \text{ is constant}}$.