Of course. Here is a detailed, step-by-step solution to the problem.

### The Problem

Assume that $f,g : (0,\infty) \rightarrow \mathbb{R}$ are differentiable and $g(x) \to \infty$ as $x \to \infty$. Show that if
$$
\lim_{x\to\infty} \left( f(x) + \frac{f'(x)}{g'(x)} \right) = 0,
$$
then
$$
\lim_{x\to\infty} f(x) = 0.
$$

---

### Solution

Our goal is to prove that $\lim_{x\to\infty} f(x) = 0$ given the conditions on $f$ and $g$. The structure of the given limit expression, $f(x) + \frac{f'(x)}{g'(x)}$, is the key to the solution. It suggests a connection to the derivative of a product or quotient involving $e^{g(x)}$. We will use L'Hôpital's Rule to establish the result.

**Step 1: Reformulate the function $f(x)$**

To use L'Hôpital's Rule, we need a limit of a quotient. Let's express $f(x)$ as a fraction in a way that relates to the given expression. A clever way to do this is to multiply and divide by $e^{g(x)}$:
$$
f(x) = \frac{f(x) e^{g(x)}}{e^{g(x)}}
$$
We want to find the limit of this expression as $x \to \infty$. Let's define the numerator and denominator as separate functions:
*   Let $N(x) = f(x) e^{g(x)}$
*   Let $D(x) = e^{g(x)}$

So, we want to evaluate $\lim_{x\to\infty} f(x) = \lim_{x\to\infty} \frac{N(x)}{D(x)}$.

**Step 2: Check the conditions for L'Hôpital's Rule**

L'Hôpital's Rule can be applied to a limit of the form $\lim_{x\to\infty} \frac{N(x)}{D(x)}$ if it results in an indeterminate form $\frac{\infty}{\infty}$ or $\frac{0}{0}$.

Let's examine the denominator, $D(x)$, as $x \to \infty$:
We are given that $\lim_{x\to\infty} g(x) = \infty$.
Therefore, $\lim_{x\to\infty} D(x) = \lim_{x\to\infty} e^{g(x)} = \infty$.

Since the denominator tends to infinity, we have an indeterminate form of the type $\frac{?}{\infty}$. This allows us to investigate the applicability of L'Hôpital's Rule. For the rule to apply, we need to compute the limit of the ratio of the derivatives, $\lim_{x\to\infty} \frac{N'(x)}{D'(x)}$, and show that it exists.

A technical point: The expression $\frac{f'(x)}{g'(x)}$ must be well-defined for the initial limit to exist. This implies that for some $M > 0$, $g'(x) \neq 0$ for all $x > M$. This is a necessary condition for L'Hôpital's Rule to be applied for $x \to \infty$.

**Step 3: Differentiate the numerator and the denominator**

Now we calculate the derivatives $N'(x)$ and $D'(x)$.

*   **Derivative of the denominator, $D(x)$:**
    Using the chain rule:
    $$D'(x) = \frac{d}{dx} \left( e^{g(x)} \right) = e^{g(x)} \cdot g'(x)$$

*   **Derivative of the numerator, $N(x)$:**
    Using the product rule and the chain rule:
    $$N'(x) = \frac{d}{dx} \left( f(x) e^{g(x)} \right) = f'(x) e^{g(x)} + f(x) \frac{d}{dx}\left(e^{g(x)}\right)$$
    $$N'(x) = f'(x) e^{g(x)} + f(x) \left(e^{g(x)} g'(x)\right)$$

**Step 4: Form the ratio of the derivatives and simplify**

Now we form the quotient $\frac{N'(x)}{D'(x)}$:
$$
\frac{N'(x)}{D'(x)} = \frac{f'(x) e^{g(x)} + f(x) e^{g(x)} g'(x)}{e^{g(x)} g'(x)}
$$
We can factor out $e^{g(x)}$ from the numerator:
$$
\frac{N'(x)}{D'(x)} = \frac{e^{g(x)} \left( f'(x) + f(x) g'(x) \right)}{e^{g(x)} g'(x)}
$$
Since $e^{g(x)} > 0$ for all $x$, we can cancel this term:
$$
\frac{N'(x)}{D'(x)} = \frac{f'(x) + f(x) g'(x)}{g'(x)}
$$
Now, we can split the fraction into two parts:
$$
\frac{N'(x)}{D'(x)} = \frac{f'(x)}{g'(x)} + \frac{f(x) g'(x)}{g'(x)}
$$
As established in Step 2, we can assume $g'(x) \neq 0$ for sufficiently large $x$, so we can cancel $g'(x)$ in the second term:
$$
\frac{N'(x)}{D'(x)} = \frac{f'(x)}{g'(x)} + f(x)
$$

**Step 5: Apply the given limit**

We are now ready to find the limit of the ratio of the derivatives as $x \to \infty$:
$$
\lim_{x\to\infty} \frac{N'(x)}{D'(x)} = \lim_{x\to\infty} \left( f(x) + \frac{f'(x)}{g'(x)} \right)
$$
The problem statement gives us the value of this limit:
$$
\lim_{x\to\infty} \left( f(x) + \frac{f'(x)}{g'(x)} \right) = 0
$$
So, we have shown that:
$$
\lim_{x\to\infty} \frac{N'(x)}{D'(x)} = 0
$$

**Step 6: State the final conclusion using L'Hôpital's Rule**

We have successfully verified the conditions for L'Hôpital's Rule:
1.  We are evaluating $\lim_{x\to\infty} \frac{N(x)}{D(x)}$.
2.  $\lim_{x\to\infty} D(x) = \infty$.
3.  The limit of the ratio of the derivatives, $\lim_{x\to\infty} \frac{N'(x)}{D'(x)}$, exists and is equal to 0.

By L'Hôpital's Rule, the limit of the original function ratio is equal to the limit of the derivative ratio:
$$
\lim_{x\to\infty} \frac{N(x)}{D(x)} = \lim_{x\to\infty} \frac{N'(x)}{D'(x)}
$$
Substituting back the expressions for $f(x)$, $N(x)$, and $D(x)$:
$$
\lim_{x\to\infty} f(x) = \lim_{x\to\infty} \frac{f(x) e^{g(x)}}{e^{g(x)}} = 0
$$

Thus, we have proven that $\lim_{x\to\infty} f(x) = 0$.

---
### Summary of the Proof

1.  **Rewrite $f(x)$:** Express $f(x)$ as the quotient $\frac{f(x)e^{g(x)}}{e^{g(x)}}$. Let $N(x) = f(x)e^{g(x)}$ and $D(x) = e^{g(x)}$.
2.  **Check L'Hôpital's Conditions:** Since $g(x) \to \infty$, the denominator $D(x) = e^{g(x)} \to \infty$. This sets up the indeterminate form $\frac{?}{\infty}$.
3.  **Compute Derivatives:**
    *   $N'(x) = e^{g(x)}(f'(x) + f(x)g'(x))$
    *   $D'(x) = e^{g(x)}g'(x)$
4.  **Simplify the Ratio of Derivatives:**
    *   $\frac{N'(x)}{D'(x)} = \frac{e^{g(x)}(f'(x) + f(x)g'(x))}{e^{g(x)}g'(x)} = \frac{f'(x)}{g'(x)} + f(x)$.
5.  **Use the Given Limit:**
    *   $\lim_{x\to\infty} \frac{N'(x)}{D'(x)} = \lim_{x\to\infty} \left(f(x) + \frac{f'(x)}{g'(x)}\right) = 0$.
6.  **Conclude with L'Hôpital's Rule:** Since the limit of the ratio of derivatives exists, L'Hôpital's Rule applies, and
    *   $\lim_{x\to\infty} f(x) = \lim_{x\to\infty} \frac{N(x)}{D(x)} = \lim_{x\to\infty} \frac{N'(x)}{D'(x)} = 0$.