Here is a detailed, step-by-step solution to the problem.

### **Understanding the Problem**

We are given a finite ring $R$ with two specific properties. Our goal is to prove that for any two elements $a, b \in R$, the expression $aba + bab$ can be written as the cube of some element in $R$.

Let's denote the set of all cubes in $R$ as $C = \{x^3 \mid x \in R\}$. The problem can be rephrased as:
1.  **Property 1:** For any $y_1, y_2 \in C$, their sum $y_1+y_2$ is in $C$. (The set of cubes is closed under addition).
2.  **Property 2:** For any $a,b \in R$ with $a \neq b$, we have $a^2b = -ba^2$, which is equivalent to $a^2b + ba^2 = 0$.
3.  **To Prove:** For any $a,b \in R$, the element $aba+bab$ is in $C$.

The proof will proceed in two main steps. First, we will establish a crucial property of the set of cubes $C$. Second, we will use this property to handle the proof, which we split into two cases: $a=b$ and $a \neq b$.

---

### **Step 1: The Set of Cubes is a Subgroup**

Let's analyze the set $C = \{x^3 \mid x \in R\}$. We are given that $R$ is a finite ring. This implies that the additive group $(R, +)$ is a finite abelian group. We will show that $C$ is a subgroup of $(R,+)$.

**Lemma:** The set $C = \{x^3 \mid x \in R\}$ is a subgroup of the additive group $(R, +)$.

**Proof of Lemma:**
A non-empty subset of a finite group is a subgroup if and only if it is closed under the group operation.

1.  **C is non-empty:** Since $R$ is a ring, it must contain at least the zero element, $0$. Thus $0^3 = 0 \in C$, so $C$ is non-empty.

2.  **C is a subset of R:** By definition of $C$, every element of $C$ is an element of $R$.

3.  **C is closed under addition:** This is given directly by Property 1. For any $a, b \in R$, we have $a^3 \in C$ and $b^3 \in C$. Property 1 states that $a^3 + b^3 = c^3$ for some $c \in R$. This means the sum of any two elements from $C$ is another element in $C$.

Since $(R, +)$ is a finite group and $C$ is a non-empty subset of $R$ that is closed under the group operation (+), it follows that $C$ is a subgroup of $(R, +)$.

**Consequences of C being a subgroup:**
*   $C$ is closed under addition (given).
*   The identity element $0$ is in $C$.
*   For every element $y \in C$, its additive inverse $-y$ is also in $C$. This means that if $y=x^3$ for some $x$, then there exists some $z \in R$ such that $-y = -(x^3) = z^3$.

Now we are equipped to prove the main statement.

---

### **Step 2: Proving $aba+bab$ is a Cube**

We will consider two cases for the elements $a,b \in R$.

**Case 1: $a=b$**

In this case, the expression we need to analyze is:
$$ aba + bab = aaa + aaa = a^3 + a^3 = 2a^3 $$
We need to prove that $2a^3$ is a cube for any $a \in R$.
Let $y = a^3$. By definition, $y$ is an element of the set of cubes, $C$.
From our lemma, we know that $C$ is a subgroup of $(R,+)$. Since subgroups are closed under the group operation, if $y \in C$, then $y+y$ must also be in $C$.
Therefore, $2a^3 = a^3 + a^3 = y+y \in C$.
By the definition of $C$, if an element is in $C$, it is the cube of some element in $R$. Thus, there exists an element $d \in R$ such that $2a^3 = d^3$.
This completes the proof for the case $a=b$.

**Case 2: $a \neq b$**

For this case, we will use the second property of the ring. Let's expand the expression $(a+b)^3$ using the distributive property of the ring:
$$ (a+b)^3 = (a+b)(a+b)(a+b) = (a^2+ab+ba+b^2)(a+b) $$
$$ = a^3 + a^2b + aba + ab^2 + ba^2 + bab + b^2a + b^3 $$
Let's rearrange the terms to group related expressions:
$$ (a+b)^3 = (a^3+b^3) + (a^2b+ba^2) + (ab^2+b^2a) + (aba+bab) $$
Now, we use Property 2. Since we are in the case $a \neq b$, we have:
$$ a^2b + ba^2 = 0 $$
The condition $b \neq a$ is the same as $a \neq b$, so we can also apply Property 2 with the roles of $a$ and $b$ interchanged:
$$ b^2a + ab^2 = 0 $$
Substituting these results into the expansion of $(a+b)^3$:
$$ (a+b)^3 = (a^3+b^3) + (0) + (0) + (aba+bab) $$
This simplifies to:
$$ (a+b)^3 = a^3+b^3 + aba+bab $$
We want to show that $aba+bab$ is a cube. Let's isolate this expression:
$$ aba+bab = (a+b)^3 - (a^3+b^3) $$
Now let's analyze the terms on the right-hand side:
*   The term $(a+b)^3$ is the cube of the element $(a+b) \in R$. By definition, $(a+b)^3 \in C$.
*   The term $a^3+b^3$ is a sum of two cubes. By Property 1, there exists $c \in R$ such that $a^3+b^3=c^3$. So, $a^3+b^3$ is also an element of $C$.

Let $y_1 = (a+b)^3$ and $y_2 = a^3+b^3$. We have shown that both $y_1 \in C$ and $y_2 \in C$. The expression we are interested in is $y_1 - y_2$.
As we proved in our lemma, $C$ is a subgroup of $(R,+)$. This means that if $y_1, y_2 \in C$, then their difference $y_1 - y_2 = y_1 + (-y_2)$ must also be in $C$.
Therefore, $aba+bab = (a+b)^3 - (a^3+b^3)$ is an element of $C$.
By the definition of $C$, this means there exists an element $d \in R$ such that $aba+bab = d^3$.
This completes the proof for the case $a \neq b$.

---

### **Conclusion**

We have examined all possible cases.
*   If $a=b$, we showed that $aba+bab = 2a^3$, which is an element of the subgroup $C$ and therefore is a cube.
*   If $a \neq b$, we showed that $aba+bab = (a+b)^3 - (a^3+b^3)$, which is the difference of two elements in the subgroup $C$ and therefore is itself an element of $C$, meaning it is a cube.

In both cases, we have proven that for any $a,b \in R$, there exists a $d \in R$ such that $aba+bab=d^3$. This concludes the proof.