Of course. Here is a detailed, step-by-step solution to the problem.

### **Understanding the Problem**

We are given a polynomial $P(x) = a_n x^n + \dots + a_1 x + a_0$ with the following properties:
1.  All coefficients $a_i$ are integers ($a_i \in \mathbb{Z}$).
2.  The leading coefficient, $a_n$, is a power of 5. So, $a_n = 5^k$ for some non-negative integer $k$. Since it's the leading coefficient, $a_n \neq 0$, so $k \ge 0$.
3.  The constant term, $a_0$, is a power of 3. So, $a_0 = 3^m$ for some non-negative integer $m$. Since $a_0$ could be the only term (if n=0), $m \ge 0$.
4.  The value of the polynomial at $x=-1$, which is $P(-1)$, is an odd integer.

Our goal is to prove that $P(x)$ has no rational roots.

### **Strategy: Proof by Contradiction**

We will use the method of proof by contradiction. We will assume that $P(x)$ *does* have a rational root and then show that this assumption leads to a logical contradiction with the given information. If our assumption leads to a contradiction, it must be false, which will prove the original statement.

### **Step-by-Step Solution**

**Step 1: Assume a rational root exists.**

Let's assume that $P(x)$ has a rational root, which we will call $x_0$. A rational root can be expressed as a fraction $p/q$, where:
*   $p$ and $q$ are integers.
*   $q \neq 0$.
*   $p$ and $q$ are coprime, meaning their greatest common divisor is 1 ($\gcd(p,q) = 1$).

So, let $x_0 = p/q$ be a rational root of $P(x)$.

**Step 2: Apply the Rational Root Theorem.**

The Rational Root Theorem states that if a polynomial with integer coefficients has a rational root $p/q$ (in simplest form), then:
*   $p$ must be a divisor of the constant term, $a_0$.
*   $q$ must be a divisor of the leading coefficient, $a_n$.

Let's apply this to our polynomial $P(x)$:
*   $p$ must divide $a_0 = 3^m$. The only divisors of $3^m$ are of the form $\pm 3^j$ for $0 \le j \le m$.
*   $q$ must divide $a_n = 5^k$. The only divisors of $5^k$ are of the form $\pm 5^l$ for $0 \le l \le k$.

So, any rational root $p/q$ of $P(x)$ must be of the form $\frac{\pm 3^j}{\pm 5^l}$.

**Step 3: Analyze the parity of p and q.**

From Step 2, we know the structure of $p$ and $q$.
*   $p$ must be of the form $\pm 3^j$. Since 3 is an odd number, any integer power of 3 ($3^0=1, 3^1=3, 3^2=9, \dots$) is also odd. Therefore, $p$ must be an **odd** integer.
*   $q$ must be of the form $\pm 5^l$. Since 5 is an odd number, any integer power of 5 ($5^0=1, 5^1=5, 5^2=25, \dots$) is also odd. Therefore, $q$ must be an **odd** integer.

This is a crucial observation: if a rational root $p/q$ exists, both its numerator $p$ and its denominator $q$ must be odd integers.

**Step 4: Use the fact that p/q is a root.**

Since $x_0 = p/q$ is a root of $P(x)$, it must satisfy the polynomial equation $P(x_0)=0$.
$P(p/q) = a_n(p/q)^n + a_{n-1}(p/q)^{n-1} + \dots + a_1(p/q) + a_0 = 0$

To eliminate the denominators, we multiply the entire equation by $q^n$:
$q^n \cdot \left[ a_n\frac{p^n}{q^n} + a_{n-1}\frac{p^{n-1}}{q^{n-1}} + \dots + a_1\frac{p}{q} + a_0 \right] = q^n \cdot 0$

This simplifies to:
$a_n p^n + a_{n-1} p^{n-1}q + a_{n-2}p^{n-2}q^2 + \dots + a_1 p q^{n-1} + a_0 q^n = 0$

**Step 5: Analyze the equation using modular arithmetic (parity).**

We will now examine the parity (whether it's even or odd) of each term in the equation above. This is equivalent to analyzing the equation modulo 2.

We know from Step 3 that both $p$ and $q$ are odd. In modular arithmetic:
*   $p \equiv 1 \pmod{2}$
*   $q \equiv 1 \pmod{2}$

Any power of an odd number is also odd. So, for any positive integer $k$:
*   $p^k \equiv 1^k \equiv 1 \pmod{2}$
*   $q^k \equiv 1^k \equiv 1 \pmod{2}$

Now, let's substitute these into our equation from Step 4, modulo 2:
$a_n p^n + a_{n-1} p^{n-1}q + \dots + a_0 q^n \equiv 0 \pmod{2}$
$a_n(1) + a_{n-1}(1)(1) + \dots + a_1(1)(1) + a_0(1) \equiv 0 \pmod{2}$

This simplifies to:
$a_n + a_{n-1} + a_{n-2} + \dots + a_1 + a_0 \equiv 0 \pmod{2}$

This means that the sum of all coefficients of $P(x)$ must be an **even** number. The sum of the coefficients is simply the value of the polynomial at $x=1$, i.e., $P(1)$.
So, our assumption that a rational root exists implies that **$P(1)$ must be even**.

**Step 6: Connect to the given condition about P(-1).**

We are given that $P(-1)$ is an **odd** integer. Let's compare the parity of $P(1)$ and $P(-1)$.

$P(1) = a_n + a_{n-1} + a_{n-2} + \dots + a_1 + a_0$
$P(-1) = a_n(-1)^n + a_{n-1}(-1)^{n-1} + a_{n-2}(-1)^{n-2} + \dots - a_1 + a_0$

Consider their difference, $P(1) - P(-1)$:
$P(1) - P(-1) = \sum_{i=0}^n a_i - \sum_{i=0}^n a_i(-1)^i = \sum_{i=0}^n a_i(1 - (-1)^i)$

Let's look at the term $(1 - (-1)^i)$:
*   If $i$ is **even**, $1 - (-1)^i = 1 - 1 = 0$.
*   If $i$ is **odd**, $1 - (-1)^i = 1 - (-1) = 2$.

So, all the terms in the sum where $i$ is even become zero. We are left with only the terms where $i$ is odd:
$P(1) - P(-1) = (a_1(1 - (-1)^1)) + (a_3(1 - (-1)^3)) + \dots$
$P(1) - P(-1) = 2a_1 + 2a_3 + 2a_5 + \dots = 2(a_1 + a_3 + a_5 + \dots)$

Since all the coefficients $a_i$ are integers, the sum $(a_1 + a_3 + a_5 + \dots)$ is also an integer. Therefore, $P(1) - P(-1)$ is 2 times an integer, which means it is an **even** number.

If the difference between two integers is even, they must have the same parity.
$P(1) - P(-1) \equiv 0 \pmod{2} \implies P(1) \equiv P(-1) \pmod{2}$

**Step 7: The Contradiction.**

Let's summarize our findings:
1.  From our assumption that a rational root exists, we deduced that **$P(1)$ must be even** (Step 5).
2.  From the problem statement, we are given that **$P(-1)$ is odd**.
3.  From analyzing the structure of the polynomial, we proved that **$P(1)$ and $P(-1)$ must have the same parity** (Step 6).

This is a contradiction. If $P(-1)$ is odd, then $P(1)$ must also be odd. But our assumption of a rational root requires $P(1)$ to be even. An integer cannot be both odd and even.

Therefore, our initial assumption—that $P(x)$ has a rational root—must be false.

### **Conclusion**

The assumption of a rational root leads to a logical contradiction with the given properties of the polynomial. Thus, the polynomial $P(x)$ has no rational roots.