Of course. Here is a detailed, step-by-step solution to the problem.

### **Objective**
We want to show that
$$ \int_0^{\pi/2} e^{\sin x}\ dx = \frac{\pi}{2}\left(1+\sum_{k=1}^{\infty}\frac{(2k-1)!!}{(2k)!(2k)!!}\right)+\sum_{k=0}^{\infty}\frac{(2k)!!}{(2k+1)!(2k+1)!!} $$

### **Step 1: Taylor Series Expansion of the Integrand**

The core of the strategy is to express the integrand, $e^{\sin x}$, as a power series and then integrate term by term. We use the Maclaurin series for the exponential function, $e^y = \sum_{n=0}^{\infty} \frac{y^n}{n!}$.
Substituting $y = \sin x$, we get:
$$ e^{\sin x} = \sum_{n=0}^{\infty} \frac{(\sin x)^n}{n!} $$
Now, we integrate this series from $0$ to $\pi/2$:
$$ \int_0^{\pi/2} e^{\sin x}\ dx = \int_0^{\pi/2} \left( \sum_{n=0}^{\infty} \frac{\sin^n x}{n!} \right) dx $$
Since the series for $e^y$ converges uniformly on any bounded interval, and $|\sin x| \le 1$ for $x \in [0, \pi/2]$, the series for $e^{\sin x}$ converges uniformly on $[0, \pi/2]$. Therefore, we can interchange the order of integration and summation:
$$ \int_0^{\pi/2} e^{\sin x}\ dx = \sum_{n=0}^{\infty} \frac{1}{n!} \int_0^{\pi/2} \sin^n x\ dx $$

### **Step 2: Wallis's Integrals**

The problem is now reduced to evaluating the integrals of powers of sine, which are known as Wallis's integrals. Let $W_n = \int_0^{\pi/2} \sin^n x\ dx$. The value of this integral depends on whether $n$ is even or odd.

The standard formulas for Wallis's integrals are:
1.  If $n = 2k$ is even (for $k \ge 1$):
    $$ W_{2k} = \int_0^{\pi/2} \sin^{2k} x\ dx = \frac{(2k-1)!!}{(2k)!!} \frac{\pi}{2} $$
2.  If $n = 2k+1$ is odd (for $k \ge 0$):
    $$ W_{2k+1} = \int_0^{\pi/2} \sin^{2k+1} x\ dx = \frac{(2k)!!}{(2k+1)!!} $$

Let's also check the base cases:
- For $n=0$: $W_0 = \int_0^{\pi/2} \sin^0 x\ dx = \int_0^{\pi/2} 1\ dx = \frac{\pi}{2}$.
- For $n=1$: $W_1 = \int_0^{\pi/2} \sin x\ dx = [-\cos x]_0^{\pi/2} = 0 - (-1) = 1$. The formula for odd $n$ with $k=0$ gives $\frac{0!!}{1!!} = \frac{1}{1} = 1$, so it holds.

### **Step 3: Splitting the Sum into Even and Odd Terms**

We can split the sum from Step 1 into two parts: one for even values of $n$ and one for odd values of $n$.
Let $n = 2k$ for the even terms ($k=0, 1, 2, \dots$) and $n = 2k+1$ for the odd terms ($k=0, 1, 2, \dots$).

$$ \sum_{n=0}^{\infty} \frac{W_n}{n!} = \sum_{k=0}^{\infty} \frac{W_{2k}}{(2k)!} + \sum_{k=0}^{\infty} \frac{W_{2k+1}}{(2k+1)!} $$

Now we will analyze each of these sums separately.

### **Step 4: Evaluating the Sum of Even Terms**

The sum for the even terms is:
$$ \sum_{k=0}^{\infty} \frac{W_{2k}}{(2k)!} = \frac{W_0}{0!} + \sum_{k=1}^{\infty} \frac{W_{2k}}{(2k)!} $$
We have separated the $k=0$ term because the standard formula for $W_{2k}$ is typically stated for $k \ge 1$.

-   For the $k=0$ term:
    We use $W_0 = \pi/2$ and $0!=1$.
    $$ \frac{W_0}{0!} = \frac{\pi/2}{1} = \frac{\pi}{2} $$
-   For the sum over $k \ge 1$:
    We use the formula $W_{2k} = \frac{(2k-1)!!}{(2k)!!} \frac{\pi}{2}$.
    $$ \sum_{k=1}^{\infty} \frac{W_{2k}}{(2k)!} = \sum_{k=1}^{\infty} \frac{1}{(2k)!} \left( \frac{(2k-1)!!}{(2k)!!} \frac{\pi}{2} \right) $$
    We can factor out the constant $\frac{\pi}{2}$:
    $$ = \frac{\pi}{2} \sum_{k=1}^{\infty} \frac{(2k-1)!!}{(2k)!(2k)!!} $$

Combining the $k=0$ term and the sum for $k \ge 1$, the total contribution from the even terms is:
$$ \sum_{k=0}^{\infty} \frac{W_{2k}}{(2k)!} = \frac{\pi}{2} + \frac{\pi}{2} \sum_{k=1}^{\infty} \frac{(2k-1)!!}{(2k)!(2k)!!} = \frac{\pi}{2} \left( 1 + \sum_{k=1}^{\infty} \frac{(2k-1)!!}{(2k)!(2k)!!} \right) $$
This matches the first part of the desired expression.

### **Step 5: Evaluating the Sum of Odd Terms**

The sum for the odd terms is:
$$ \sum_{k=0}^{\infty} \frac{W_{2k+1}}{(2k+1)!} $$
For these terms, we use the formula $W_{2k+1} = \frac{(2k)!!}{(2k+1)!!}$, which is valid for all $k \ge 0$.
Substituting this into the sum:
$$ \sum_{k=0}^{\infty} \frac{1}{(2k+1)!} \left( \frac{(2k)!!}{(2k+1)!!} \right) $$
This can be written as:
$$ \sum_{k=0}^{\infty} \frac{(2k)!!}{(2k+1)!(2k+1)!!} $$
This expression exactly matches the second part of the desired expression.

### **Step 6: Combining the Results**

Now, we combine the results from the even and odd terms to find the value of the original integral:
$$ \int_0^{\pi/2} e^{\sin x}\ dx = \left( \text{Sum of even terms} \right) + \left( \text{Sum of odd terms} \right) $$
$$ \int_0^{\pi/2} e^{\sin x}\ dx = \frac{\pi}{2} \left( 1 + \sum_{k=1}^{\infty} \frac{(2k-1)!!}{(2k)!(2k)!!} \right) + \sum_{k=0}^{\infty} \frac{(2k)!!}{(2k+1)!(2k+1)!!} $$

This is precisely the identity we were asked to show.

### **Conclusion**

By expanding the integrand $e^{\sin x}$ into its Maclaurin series, integrating term by term using Wallis's formulas for integrals of powers of sine, and then carefully separating the resulting series into its even and odd components, we have successfully derived the target expression. The proof is complete.