Solution:
Let $f:\mathbb{R}\to\mathbb{R}$ be a real function with a continuous derivative $f'$. We are given the inequality $|f'(x)| \leq |f(x) - f(0)|$ for all $x \in \mathbb{R}$. We want to show that $f$ is a constant function, i.e., $f(x) = f(0)$ for all $x \in \mathbb{R}$.

Let $g(x) = f(x) - f(0)$. Then $g(0) = f(0) - f(0) = 0$.
Since $f$ has a continuous derivative $f'$, the function $g$ also has a continuous derivative $g'(x) = f'(x)$.
The given inequality can be rewritten in terms of $g(x)$ as:
$$|g'(x)| \leq |g(x)|$$

Consider the function $h(x) = [g(x)]^2$. Since $g(x)$ is continuously differentiable, $h(x)$ is also continuously differentiable.
Moreover, $h(x) = [g(x)]^2 \geq 0$ for all $x \in \mathbb{R}$.
Also, $h(0) = [g(0)]^2 = 0^2 = 0$.

Let's compute the derivative of $h(x)$:
$$h'(x) = 2 g(x) g'(x)$$
Now, let's bound the absolute value of $h'(x)$:
$$|h'(x)| = |2 g(x) g'(x)| = 2 |g(x)| |g'(x)|$$
Using the inequality $|g'(x)| \leq |g(x)|$, we get:
$$|h'(x)| \leq 2 |g(x)| |g(x)| = 2 |g(x)|^2 = 2 h(x)$$
So, we have the inequality $|h'(x)| \leq 2h(x)$. This implies two inequalities:
1. $h'(x) \leq 2h(x)$
2. $h'(x) \geq -2h(x)$

We will analyze the implications of these inequalities for $x \geq 0$ and $x \leq 0$.

Case 1: $x \geq 0$.
We use the inequality $h'(x) \leq 2h(x)$. This can be written as $h'(x) - 2h(x) \leq 0$.
Consider the auxiliary function $k(x) = e^{-2x} h(x)$. Since $h(x)$ is continuously differentiable, $k(x)$ is also continuously differentiable.
Let's compute the derivative of $k(x)$:
$$k'(x) = \frac{d}{dx} (e^{-2x} h(x)) = -2e^{-2x} h(x) + e^{-2x} h'(x) = e^{-2x} (h'(x) - 2h(x))$$
Since $h'(x) - 2h(x) \leq 0$ and $e^{-2x} > 0$ for all $x$, we have $k'(x) \leq 0$ for all $x$.
A function with a non-positive derivative on an interval is non-increasing on that interval. Thus, $k(x)$ is a non-increasing function on $\mathbb{R}$.
In particular, for any $x \geq 0$, we must have $k(x) \leq k(0)$.
Substituting the definition of $k(x)$, we get:
$$e^{-2x} h(x) \leq e^{-2 \cdot 0} h(0)$$
Since $h(0) = 0$, this becomes:
$$e^{-2x} h(x) \leq 0$$
We know that $h(x) = [g(x)]^2 \geq 0$ and $e^{-2x} > 0$. Therefore, the product $e^{-2x} h(x) \geq 0$.
The only way for $e^{-2x} h(x) \leq 0$ and $e^{-2x} h(x) \geq 0$ to both hold is if $e^{-2x} h(x) = 0$.
Since $e^{-2x} > 0$, this implies $h(x) = 0$.
This holds for all $x \geq 0$.

Case 2: $x \leq 0$.
We use the inequality $h'(x) \geq -2h(x)$. This can be written as $h'(x) + 2h(x) \geq 0$.
Consider the auxiliary function $m(x) = e^{2x} h(x)$. Since $h(x)$ is continuously differentiable, $m(x)$ is also continuously differentiable.
Let's compute the derivative of $m(x)$:
$$m'(x) = \frac{d}{dx} (e^{2x} h(x)) = 2e^{2x} h(x) + e^{2x} h'(x) = e^{2x} (2h(x) + h'(x))$$
Since $h'(x) + 2h(x) \geq 0$ and $e^{2x} > 0$ for all $x$, we have $m'(x) \geq 0$ for all $x$.
A function with a non-negative derivative on an interval is non-decreasing on that interval. Thus, $m(x)$ is a non-decreasing function on $\mathbb{R}$.
In particular, for any $x \leq 0$, we must have $m(x) \leq m(0)$.
Substituting the definition of $m(x)$, we get:
$$e^{2x} h(x) \leq e^{2 \cdot 0} h(0)$$
Since $h(0) = 0$, this becomes:
$$e^{2x} h(x) \leq 0$$
We know that $h(x) = [g(x)]^2 \geq 0$ and $e^{2x} > 0$. Therefore, the product $e^{2x} h(x) \geq 0$.
The only way for $e^{2x} h(x) \leq 0$ and $e^{2x} h(x) \geq 0$ to both hold is if $e^{2x} h(x) = 0$.
Since $e^{2x} > 0$, this implies $h(x) = 0$.
This holds for all $x \leq 0$.

Combining the results from Case 1 and Case 2, we have $h(x) = 0$ for all $x \in \mathbb{R}$.
Since $h(x) = [g(x)]^2$, this means $[g(x)]^2 = 0$ for all $x \in \mathbb{R}$, which implies $g(x) = 0$ for all $x \in \mathbb{R}$.
Recalling the definition $g(x) = f(x) - f(0)$, we have $f(x) - f(0) = 0$ for all $x \in \mathbb{R}$.
This shows that $f(x) = f(0)$ for all $x \in \mathbb{R}$.
Therefore, $f$ is a constant function.

Final Answer: The final answer is $\boxed{f \text{ is constant}}$