Let $N$ be an integer. $N$ is a base $b$ palindrome with 4 digits if its base $b$ representation is of the form $(x y y x)_b$ for some integers $x, y$ such that $1 \le x < b$ and $0 \le y < b$.
The value of $N$ is given by $N = x b^3 + y b^2 + y b + x$.
This expression can be rewritten as $N = x(b^3+1) + y(b^2+b) = x(b^3+1) + yb(b+1)$.
The condition that $N$ has exactly 4 digits in base $b$ means $b^3 \le N < b^4$. Since $x \ge 1$, $N = x b^3 + y b^2 + y b + x \ge 1 \cdot b^3 + 0 \cdot b^2 + 0 \cdot b + 1 = b^3+1$. So $N \ge b^3$ is satisfied.
Since $x < b$ and $y < b$, $N = x b^3 + y b^2 + y b + x \le (b-1)b^3 + (b-1)b^2 + (b-1)b + (b-1) = (b-1)(b^3+b^2+b+1) = (b-1)\frac{b^4-1}{b-1} = b^4-1$. So $N < b^4$ is always satisfied for a 4-digit number.
So the condition is $b^3+1 \le N$. This is automatically included in the condition $b^3 \le N < b^4$ unless $N=b^3$. But $N=b^3 = (1000)_b$ is not a palindrome of the form $(xyyx)_b$. So we only need $b^3 \le N < b^4$.

We can rewrite $N$ as $N = (b+1)(x(b^2-b+1) + yb)$.
This implies that $N$ must be divisible by $b+1$. Let $Q = N/(b+1)$.
$Q = x(b^2-b+1) + yb = x b^2 + (y-x) b + x$.
From this expression, we see that $Q \equiv x \pmod b$. Since $1 \le x < b$, $x$ is the remainder of $Q$ when divided by $b$. We must have $x \ne 0$, which means $Q \not\equiv 0 \pmod b$.
Let $x = Q \pmod b$.
Also, $Q - x = b(x(b-1)+y)$. So $y = \frac{Q-x}{b} - x(b-1)$.
Since $x$ and $Q$ are integers, $Q-x$ must be divisible by $b$. This is guaranteed by $x = Q \pmod b$. So $y$ is an integer.
We must ensure that $0 \le y < b$.
$0 \le \frac{Q-x}{b} - x(b-1)$. This leads to $Q \ge x + bx(b-1) = x(b^2-b+1)$.
$\frac{Q-x}{b} - x(b-1) < b$. This leads to $Q < x(b^2-b+1) + b^2$.
Combining these inequalities with $N = Q(b+1)$:
$x(b+1)(b^2-b+1) \le N < x(b+1)(b^2-b+1) + b^2(b+1)$.
$x(b^3+1) \le N < x(b^3+1) + b^2(b+1)$.
This is the condition for $y$ to be in the required range $[0, b-1)$.

We want to show that for any natural number $n$, there exists an integer $N$ which satisfies these conditions for at least $n$ different values of $b$.
Let $n$ be a given natural number. Choose an integer $m = 3n$.
Let $N = 2^{3(m+n)} = 2^{3(3n+n)} = 2^{12n}$.
Consider the $n$ integers $b_i = 2^{m+i}-1$ for $i=1, 2, \dots, n$.
Since $m=3n$, $b_i = 2^{3n+i}-1$. As $i$ ranges from $1$ to $n$, these $b_i$ are distinct integers.
Also, $b_i \ge b_1 = 2^{3n+1}-1 \ge 2^{3(1)+1}-1 = 2^4-1=15$. So $b_i \ge 15$ for all $i$.

We check if $N$ is a 4-digit palindrome for each base $b_i$.
1.  **Range condition:** We must check $b_i^3 \le N < b_i^4$.
    $b_i^3 = (2^{m+i}-1)^3 < (2^{m+i})^3 = 2^{3(m+i)}$. Since $i \le n$, $m+i \le m+n$. So $3(m+i) \le 3(m+n)$.
    $N=2^{3(m+n)}$, so $b_i^3 < N$.
    We need $N < b_i^4$. $N=2^{3(m+n)}$. $b_i^4 = (2^{m+i}-1)^4$.
    Is $2^{3(m+n)} < (2^{m+i}-1)^4$?
    The inequality is approximately $2^{3(m+n)} < 2^{4(m+i)}$. This means $3(m+n) < 4(m+i)$.
    Substituting $m=3n$, we need $3(3n+n) < 4(3n+i)$, which is $12n < 12n+4i$. This is $0 < 4i$, which is true for $i=1, \dots, n$.
    Let's check more rigorously. $(2^{m+i}-1)^4 = 2^{4(m+i)} - 4 \cdot 2^{3(m+i)} + \dots$.
    We need $2^{3(m+n)} < 2^{4(m+i)} - 4 \cdot 2^{3(m+i)} + \dots$.
    Since $3(m+n) < 4(m+i)$, $2^{3(m+n)}$ is significantly smaller than $2^{4(m+i)}$. As $m=3n$ and $i \ge 1$, $4(m+i) - 3(m+n) = 4(3n+i) - 3(3n+n) = 12n+4i - 12n = 4i \ge 4$. The ratio $b_i^4/N > 2^{4i}/(1-4\cdot 2^{-(m+i)}+\dots) > 2^{4i}/1 \ge 16$. So $N < b_i^4$.
    Thus, $N$ has 4 digits in base $b_i$.

2.  **Divisibility and digits calculation:**
    $N$ must be divisible by $b_i+1$. $b_i+1 = (2^{m+i}-1)+1 = 2^{m+i}$.
    $N = 2^{3(m+n)}$. Since $m+i \le m+n = 4n$, and $3(m+n) = 12n$, we have $m+i \le 4n \le 12n$. So $b_i+1 = 2^{m+i}$ divides $N=2^{12n}$.
    Let $Q_i = N/(b_i+1) = 2^{3(m+n)} / 2^{m+i} = 2^{3m+3n - (m+i)} = 2^{2m+3n-i}$.
    Let $x_i = Q_i \pmod{b_i} = 2^{2m+3n-i} \pmod{2^{m+i}-1}$.
    Since $2^{m+i} \equiv 1 \pmod{2^{m+i}-1}$, we find the remainder of the exponent $2m+3n-i$ modulo $m+i$.
    $2m+3n-i = 2(m+i) + 3n-3i$.
    The remainder is $r = 3n-3i$. We must check $0 \le r < m+i$.
    Since $1 \le i \le n$, $0 \le 3n-3i \le 3n-3$.
    We need $3n-3i < m+i = 3n+i$. This holds because $i \ge 1$. So $3n-3i < 3n+i$.
    So $x_i = 2^{3n-3i}$.
    We must have $1 \le x_i < b_i$.
    $x_i = 2^{3n-3i} \ge 2^{3n-3n} = 2^0 = 1$.
    We need $x_i < b_i$. $2^{3n-3i} < 2^{m+i}-1 = 2^{3n+i}-1$. This holds since $3n-3i < 3n+i$ for $i \ge 1$.

3.  **Range condition for $y_i$:**
    We need $0 \le y_i < b_i$, which is equivalent to $x_i(b_i^3+1) \le N < x_i(b_i^3+1) + b_i^2(b_i+1)$.
    $x_i(b_i^3+1) = 2^{3n-3i}((2^{m+i}-1)^3+1) = 2^{3n-3i}(2^{3(m+i)} - 3 \cdot 2^{2(m+i)} + 3 \cdot 2^{m+i})$.
    $= 2^{3m+3n} - 3 \cdot 2^{2m+3n-i} + 3 \cdot 2^{m+3n-2i}$.
    Since $N=2^{3m+3n}$, we need to check $2^{3m+3n} - 3 \cdot 2^{2m+3n-i} + 3 \cdot 2^{m+3n-2i} \le 2^{3m+3n}$.
    This holds if $3 \cdot 2^{m+3n-2i} \le 3 \cdot 2^{2m+3n-i}$, which is equivalent to $m+3n-2i \le 2m+3n-i$. This simplifies to $m+i \ge 0$, which is true.
    Now check the upper bound: $N < x_i(b_i^3+1) + b_i^2(b_i+1)$.
    $2^{3m+3n} < (2^{3m+3n} - 3 \cdot 2^{2m+3n-i} + 3 \cdot 2^{m+3n-2i}) + (2^{m+i}-1)^2 (2^{m+i})$.
    This inequality is equivalent to $0 < - 3 \cdot 2^{2m+3n-i} + 3 \cdot 2^{m+3n-2i} + (2^{m+i}-1)^2 2^{m+i}$.
    $(2^{m+i}-1)^2 2^{m+i} = (2^{2(m+i)} - 2 \cdot 2^{m+i} + 1) 2^{m+i} = 2^{3(m+i)} - 2 \cdot 2^{2(m+i)} + 2^{m+i}$.
    We need $0 < - 3 \cdot 2^{2m+3n-i} + 3 \cdot 2^{m+3n-2i} + 2^{3m+3i} - 2 \cdot 2^{2m+2i} + 2^{m+i}$.
    The term with the largest exponent is $2^{3m+3i}$ because $m=3n$ and $i \ge 1$. Exponent is $9n+3i$. The next largest exponent is $2m+3n-i = 6n+3n-i = 9n-i$. Since $i \ge 1$, $9n+3i > 9n-i$.
    Since the term with the largest exponent $2^{3m+3i}$ is positive, the sum is positive for sufficiently large $n$. Let's verify this statement for all $n \ge 1$.
    The inequality holds if $2^{3m+3i} > 3 \cdot 2^{2m+3n-i} + 2 \cdot 2^{2m+2i}$.
    Divide by $2^{2m+2i}$: $2^{m+i} > 3 \cdot 2^{3n-3i} + 2$.
    $2^{3n+i} > 3 \cdot 2^{3n-3i} + 2$.
    $2^{3n+i} - 3 \cdot 2^{3n-3i} = 2^{3n-3i}(2^{4i}-3)$.
    We need $2^{3n-3i}(2^{4i}-3) > 2$.
    For $i=1$, $2^{3n-3}(2^4-3) = 13 \cdot 2^{3n-3}$. Since $n \ge 1$, $3n-3 \ge 0$. If $n=1$, $13 \cdot 2^0 = 13 > 2$. If $n > 1$, $13 \cdot 2^{3n-3}$ is even larger.
    For $i>1$, $4i \ge 8$. $2^{4i}-3$ is large and positive. $3n-3i$ can be negative.
    If $i=n$, $2^0(2^{4n}-3) = 2^{4n}-3$. We need $2^{4n}-3 > 2$. $2^{4n} > 5$. This holds for $n \ge 1$.
    The condition $0 \le y_i < b_i$ is satisfied.

We have constructed an integer $N=2^{12n}$ and found $n$ distinct bases $b_i=2^{3n+i}-1$ for $i=1, \dots, n$, such that $N$ is a 4-digit palindrome in each base $b_i$.
The digits are $x_i = 2^{3n-3i}$ and $y_i = (Q_i-x_i)/b_i - x_i(b_i-1)$, which we showed is in $[0, b_i-1)$. For instance, $y_i = (2^{2m+3n-i}-2^{3n-3i})/(2^{m+i}-1) - 2^{3n-3i}(2^{m+i}-2)$.
The calculation in the example showed $y_1=24$ for $n=2$. This is $8(3)=24$. And $y_2=3$ for $n=2$. This is $1(3)=3$. It seems $y_i = x_i \times 3$. Let's test this.
$y_i = (Q_i-x_i)/b_i - x_i(b_i-1)$. $Q_i = x_i b_i + \text{remains}$. No, $Q_i = k b_i + x_i$. $y = k - x_i(b_i-1)$.
$k = (Q_i-x_i)/b_i$.
$Q_i = 2^{2m+3n-i}$. $x_i = 2^{3n-3i}$. $b_i = 2^{m+i}-1$.
$Q_i - x_i = 2^{2m+3n-i} - 2^{3n-3i} = 2^{3n-3i}(2^{2m+2i}-1)$.
$k = \frac{2^{3n-3i}(2^{2m+2i}-1)}{2^{m+i}-1} = \frac{2^{3n-3i}(2^{m+i}-1)(2^{m+i}+1)}{2^{m+i}-1} = 2^{3n-3i}(2^{m+i}+1)$.
$y_i = 2^{3n-3i}(2^{m+i}+1) - 2^{3n-3i}(2^{m+i}-1-1) = 2^{3n-3i}(2^{m+i}+1) - 2^{3n-3i}(b_i-1)$.
$y_i = 2^{3n-3i}(2^{m+i}+1 - (2^{m+i}-2)) = 2^{3n-3i}(3) = 3x_i$.
We need $y_i < b_i$. $3x_i < b_i$. $3 \cdot 2^{3n-3i} < 2^{m+i}-1 = 2^{3n+i}-1$.
$3 \cdot 2^{3n-3i} < 2^{3n+i}-1$. $2^{3n-3i}(2^{4i}-3) > -1$? No, $3 \cdot 2^{3n-3i} + 1 < 2^{3n+i}$.
$2^{3n-3i}(2^{4i}) > 3 \cdot 2^{3n-3i}+1$. $2^{3n+i}$.
For $i=1$, $3 \cdot 2^{3n-3} < 2^{3n+1}-1$. $3/8 \cdot 2^{3n} < 2 \cdot 2^{3n}-1$. This is true for $n \ge 1$.
For $i=n$, $3 \cdot 2^0 = 3 < 2^{4n}-1$. True for $n \ge 1$.
In general, $2^{3n+i} - 3 \cdot 2^{3n-3i} = 2^{3n-3i}(2^{4i}-3) > 1$. This must hold.
$2^{4i}-3 \ge 2^4-3 = 13$. $2^{3n-3i}(13) \ge 13 \cdot 2^0 = 13 > 1$. Holds.

Final Answer: The final answer is $\boxed{N=2^{12n} \text{ is a 4-digit palindrome for the } n \text{ bases } b_i=2^{3n+i}-1 \text{ for } i=1, \dots, n}$