Of course. Here is a detailed, step-by-step solution to the problem.

### **Problem Statement**

Let $x(t)$ be a solution of the system
 \begin{equation}
 \left\{
 \begin{array}{l}
 \dot{x}(t)=A(t)x(t) , \\
 x(0)\neq 0,
 \end{array}
 \right.
 \end{equation}
 where
 \begin{equation*}
 A(t)=\begin{pmatrix}
 1+\sin^2 t & -1 & -1 \\
 1 & 1/(1+\sin^2 t) & -1 \\
 1 & 1 & 1+\cos^2 t
 \end{pmatrix}.
 \end{equation*}
 Show that the function $\mathbb{R}\ni t \mapsto \|x(t)\|\in \mathbb{R}$ is increasing, where $\|\cdot\|$ denotes the Euclidean norm.

---

### **Solution**

**1. Define the Function to Analyze**

We want to show that the function $f(t) = \|x(t)\|$ is increasing. A function is increasing if its derivative is non-negative. To simplify the differentiation process, it is often easier to work with the square of the norm.

Let $g(t) = \|x(t)\|^2$. The Euclidean norm squared is the dot product of the vector with itself, which can be written in matrix notation as $x(t)^T x(t)$.
So, we have:
$$ g(t) = \|x(t)\|^2 = x(t) \cdot x(t) = x_1(t)^2 + x_2(t)^2 + x_3(t)^2 = x(t)^T x(t) $$
where $x(t) = \begin{pmatrix} x_1(t) \\ x_2(t) \\ x_3(t) \end{pmatrix}$.

The relationship between the derivatives of $f(t)$ and $g(t)$ is:
$$ f(t) = \sqrt{g(t)} $$
$$ f'(t) = \frac{d}{dt}\|x(t)\| = \frac{1}{2\sqrt{g(t)}} g'(t) = \frac{g'(t)}{2\|x(t)\|} $$
Since $x(0) \neq 0$, and the system is a linear homogeneous ODE, the solution $x(t)$ is non-zero for all $t \in \mathbb{R}$. This means $\|x(t)\| > 0$ for all $t$. Therefore, the sign of $f'(t)$ is the same as the sign of $g'(t)$. To prove that $f(t)$ is increasing, we need to show that $g'(t) \ge 0$.

**2. Differentiate the Squared Norm**

We compute the derivative of $g(t) = x(t)^T x(t)$ with respect to $t$ using the product rule for matrix multiplication:
$$ g'(t) = \frac{d}{dt} \left( x(t)^T x(t) \right) = \left(\frac{d}{dt} x(t)^T\right) x(t) + x(t)^T \left(\frac{d}{dt} x(t)\right) $$
We know that $\frac{d}{dt} x(t) = \dot{x}(t)$ and $\frac{d}{dt} x(t)^T = (\dot{x}(t))^T$. So,
$$ g'(t) = \dot{x}(t)^T x(t) + x(t)^T \dot{x}(t) $$

**3. Substitute the System's Equation**

Now, we use the given differential equation, $\dot{x}(t) = A(t)x(t)$, to substitute for $\dot{x}(t)$:
$$ g'(t) = (A(t)x(t))^T x(t) + x(t)^T (A(t)x(t)) $$
Using the property of transposes $(AB)^T = B^T A^T$, we get:
$$ g'(t) = x(t)^T A(t)^T x(t) + x(t)^T A(t) x(t) $$
We can factor this expression:
$$ g'(t) = x(t)^T (A(t)^T + A(t)) x(t) $$

**4. Compute the Matrix $A(t)^T + A(t)$**

Let's find the symmetric part of the matrix $A(t)$, which is the sum $A(t) + A(t)^T$.
First, we write down $A(t)$ and its transpose $A(t)^T$:
$$ A(t) = \begin{pmatrix} 1+\sin^2 t & -1 & -1 \\ 1 & 1/(1+\sin^2 t) & -1 \\ 1 & 1 & 1+\cos^2 t \end{pmatrix} $$
$$ A(t)^T = \begin{pmatrix} 1+\sin^2 t & 1 & 1 \\ -1 & 1/(1+\sin^2 t) & 1 \\ -1 & -1 & 1+\cos^2 t \end{pmatrix} $$
Now, we add them together:
$$ A(t) + A(t)^T = \begin{pmatrix} 1+\sin^2 t & -1 & -1 \\ 1 & 1/(1+\sin^2 t) & -1 \\ 1 & 1 & 1+\cos^2 t \end{pmatrix} + \begin{pmatrix} 1+\sin^2 t & 1 & 1 \\ -1 & 1/(1+\sin^2 t) & 1 \\ -1 & -1 & 1+\cos^2 t \end{pmatrix} $$
$$ A(t) + A(t)^T = \begin{pmatrix} 2(1+\sin^2 t) & -1+1 & -1+1 \\ 1-1 & 2/(1+\sin^2 t) & -1+1 \\ 1-1 & 1-1 & 2(1+\cos^2 t) \end{pmatrix} $$
This simplifies to a diagonal matrix:
$$ A(t) + A(t)^T = \begin{pmatrix} 2(1+\sin^2 t) & 0 & 0 \\ 0 & \frac{2}{1+\sin^2 t} & 0 \\ 0 & 0 & 2(1+\cos^2 t) \end{pmatrix} $$

**5. Analyze the Sign of $g'(t)$**

Now we substitute this back into the expression for $g'(t)$:
$$ g'(t) = x(t)^T \begin{pmatrix} 2(1+\sin^2 t) & 0 & 0 \\ 0 & \frac{2}{1+\sin^2 t} & 0 \\ 0 & 0 & 2(1+\cos^2 t) \end{pmatrix} x(t) $$
Let $x(t) = \begin{pmatrix} x_1 \\ x_2 \\ x_3 \end{pmatrix}$. The quadratic form is:
$$ g'(t) = 2(1+\sin^2 t)x_1^2 + \frac{2}{1+\sin^2 t}x_2^2 + 2(1+\cos^2 t)x_3^2 $$
To determine the sign of $g'(t)$, we need to analyze the coefficients of $x_1^2$, $x_2^2$, and $x_3^2$. These are the diagonal entries of the matrix $A(t)+A(t)^T$.

*   For the first coefficient: $0 \le \sin^2 t \le 1$, so $1 \le 1+\sin^2 t \le 2$. Thus, the coefficient $2(1+\sin^2 t)$ is always in the range $[2, 4]$. It is strictly positive.
*   For the second coefficient: Since $1 \le 1+\sin^2 t \le 2$, its reciprocal is $1/2 \le 1/(1+\sin^2 t) \le 1$. Thus, the coefficient $2/(1+\sin^2 t)$ is always in the range $[1, 2]$. It is strictly positive.
*   For the third coefficient: $0 \le \cos^2 t \le 1$, so $1 \le 1+\cos^2 t \le 2$. Thus, the coefficient $2(1+\cos^2 t)$ is always in the range $[2, 4]$. It is strictly positive.

All three coefficients are strictly positive for all $t \in \mathbb{R}$. The terms $x_1^2, x_2^2, x_3^2$ are always non-negative.
Therefore, $g'(t)$ is a sum of non-negative terms:
$$ g'(t) = \underbrace{2(1+\sin^2 t)}_{>0} \underbrace{x_1^2}_{\ge 0} + \underbrace{\frac{2}{1+\sin^2 t}}_{>0} \underbrace{x_2^2}_{\ge 0} + \underbrace{2(1+\cos^2 t)}_{>0} \underbrace{x_3^2}_{\ge 0} \ge 0 $$
Since $x(t) \neq 0$, at least one of its components ($x_1, x_2, x_3$) must be non-zero. This means at least one of $x_1^2, x_2^2, x_3^2$ is strictly positive. As all the coefficients are strictly positive, their sum $g'(t)$ must be strictly positive.
$$ g'(t) > 0 \quad \text{for all } t \in \mathbb{R} $$

**6. Conclusion**

We have established that $g'(t) = \frac{d}{dt}\|x(t)\|^2 > 0$ for all $t$.
Now let's return to the derivative of $f(t) = \|x(t)\|$:
$$ \frac{d}{dt}\|x(t)\| = \frac{g'(t)}{2\|x(t)\|} $$
Since $x(t) \neq 0$, we have $\|x(t)\| > 0$. And we have shown $g'(t) > 0$. Therefore,
$$ \frac{d}{dt}\|x(t)\| > 0 \quad \text{for all } t \in \mathbb{R} $$
A function with a strictly positive derivative is strictly increasing. Since the problem asks to show the function is "increasing" (which can mean non-decreasing), our stronger result of "strictly increasing" is sufficient.

Thus, the function $\mathbb{R}\ni t \mapsto \|x(t)\|\in \mathbb{R}$ is increasing.