We prove that if for any $n\ge 2$ we have $a_n = 33$ and $b_n = 0$, then $a_{n-1} = 33$ and $b_{n-1} = 0$. Indeed, from the conditions we have $a_{n-1}b_{n-1} = 0$, hence one of $a_{n-1}$, $b_{n-1}$ has to be 0. If $a_{n-1} = 0$, this means $a_{n-2} + b_{n-2} = 0$ and $a_{n-2}b_{n-2} = b_{n-1} = 33$, as $a_{n-1} + b_{n-1} = a_n = 33$. But this means $33 = -a_{n-2}^2$, which is impossible. Therefore we have $b_{n-1} = 0$, and hence $a_{n-1} = 33$. 


Going backwards, we now get to $a_1 = 33$, $b_1 = 0$. Hence $a_1^2 + b_1^2 = 33^2 = 1089$.