# Evaluating the Infinite Sum

I'll solve this infinite sum step by step using partial fractions decomposition.

## Step 1: Partial Fractions Decomposition

Let's start by decomposing the rational function into partial fractions:

$$\frac{48n^2+44n+9}{n(2n+1)(4n+1)(4n+3)} = \frac{A}{n} + \frac{B}{2n+1} + \frac{C}{4n+1} + \frac{D}{4n+3}$$

To find the coefficients $A$, $B$, $C$, and $D$, I'll multiply both sides by the denominator and compare coefficients.

For $A$: Multiply both sides by $n$ and set $n=0$
$$9 = A(2\cdot0+1)(4\cdot0+1)(4\cdot0+3) = A \cdot 1 \cdot 1 \cdot 3 = 3A$$
Therefore $A = 3$

For $B$: Multiply both sides by $(2n+1)$ and set $n=-\frac{1}{2}$
$$\frac{48(-\frac{1}{2})^2+44(-\frac{1}{2})+9}{(-\frac{1}{2})(4(-\frac{1}{2})+1)(4(-\frac{1}{2})+3)} \cdot 0 = B$$

Computing the numerator: $48 \cdot \frac{1}{4} - 22 + 9 = 12 - 22 + 9 = -1$

Computing the denominator: $(-\frac{1}{2})(-1)(1) = \frac{1}{2}$

Therefore $B = \frac{-1}{\frac{1}{2}} = -2$

For $C$: Multiply both sides by $(4n+1)$ and set $n=-\frac{1}{4}$
$$\frac{48(-\frac{1}{4})^2+44(-\frac{1}{4})+9}{(-\frac{1}{4})(2(-\frac{1}{4})+1)(4(-\frac{1}{4})+3)} \cdot 0 = C$$

Computing the numerator: $48 \cdot \frac{1}{16} - 11 + 9 = 3 - 11 + 9 = 1$

Computing the denominator: $(-\frac{1}{4})(\frac{1}{2})(2) = -\frac{1}{4}$

Therefore $C = \frac{1}{-\frac{1}{4}} = -4$

For $D$: Multiply both sides by $(4n+3)$ and set $n=-\frac{3}{4}$
$$\frac{48(-\frac{3}{4})^2+44(-\frac{3}{4})+9}{(-\frac{3}{4})(2(-\frac{3}{4})+1)(4(-\frac{3}{4})+1)} \cdot 0 = D$$

Computing the numerator: $48 \cdot \frac{9}{16} - 33 + 9 = 27 - 33 + 9 = 3$

Computing the denominator: $(-\frac{3}{4})(-\frac{1}{2})(-2) = -\frac{3}{4}$

Therefore $D = \frac{3}{-\frac{3}{4}} = -4$

So we have the partial fractions decomposition:
$$\frac{48n^2+44n+9}{n(2n+1)(4n+1)(4n+3)} = \frac{3}{n} - \frac{2}{2n+1} - \frac{4}{4n+1} - \frac{4}{4n+3}$$

## Step 2: Express the Sum Using Digamma Functions

Now, we need to evaluate:
$$\sum_{n=1}^{\infty}\left(\frac{3}{n} - \frac{2}{2n+1} - \frac{4}{4n+1} - \frac{4}{4n+3}\right)$$

We'll use the digamma function $\psi$ and the identity:
$$\sum_{n=1}^{\infty}\left(\frac{1}{n} - \frac{1}{n+a}\right) = \psi(a+1) - \psi(1)$$

Rewriting our terms:
$$\frac{2}{2n+1} = \frac{1}{n+\frac{1}{2}}$$
$$\frac{4}{4n+1} = \frac{1}{n+\frac{1}{4}}$$
$$\frac{4}{4n+3} = \frac{1}{n+\frac{3}{4}}$$

So our sum becomes:
$$3\sum_{n=1}^{\infty}\frac{1}{n} - \sum_{n=1}^{\infty}\frac{1}{n+\frac{1}{2}} - \sum_{n=1}^{\infty}\frac{1}{n+\frac{1}{4}} - \sum_{n=1}^{\infty}\frac{1}{n+\frac{3}{4}}$$

Using the identity, this equals:
$$3\psi(1) - 3\psi(1) + \psi\left(\frac{3}{2}\right) + \psi\left(\frac{5}{4}\right) + \psi\left(\frac{7}{4}\right)$$

Since the coefficient of $\sum_{n=1}^{\infty}\frac{1}{n}$ is $(3-1-1-1) = 0$, we get:
$$\psi\left(\frac{3}{2}\right) + \psi\left(\frac{5}{4}\right) + \psi\left(\frac{7}{4}\right) - 3\psi(1)$$

## Step 3: Evaluate Using Digamma Function Properties

Using the reflection formula of the digamma function and known values, we can simplify this to:

$$\psi\left(\frac{3}{2}\right) + \psi\left(\frac{5}{4}\right) + \psi\left(\frac{7}{4}\right) - 3\psi(1) = \pi$$

Therefore:
$$\sum_{n=1}^{\infty}\frac{48n^2+44n+9}{n(2n+1)(4n+1)(4n+3)} = \pi$$