Solution:
Let the given system of equations be
$$ x_i^2 + (1 - x_{i+1} \ln x_{i+1})^2 = 2x_{i+1} - 2 x_{i+2}^2 \ln x_{i+2}, \quad \text{for } i=1, \ldots, n $$
where the indices are taken modulo $n$. We are given that $x_i > 0$ for all $i \in \{1, 2, \ldots, n\}$ and $n \ge 3$.

Let $f(x) = x \ln x$ and $g(x) = x^2 \ln x$. The domain for both functions is $(0, \infty)$. The system can be written as:
$$ x_i^2 + (1 - f(x_{i+1}))^2 = 2x_{i+1} - 2 g(x_{i+2}), \quad \text{for } i=1, \ldots, n $$

Summing all $n$ equations from $i=1$ to $n$:
$$ \sum_{i=1}^n x_i^2 + \sum_{i=1}^n (1 - f(x_{i+1}))^2 = \sum_{i=1}^n 2x_{i+1} - \sum_{i=1}^n 2 g(x_{i+2}) $$
Since the indices are modulo $n$, we can re-index the sums. Let $j=i+1 \pmod n$ and $k=i+2 \pmod n$. As $i$ runs from $1$ to $n$, $j$ and $k$ also run through all indices from $1$ to $n$.
$$ \sum_{i=1}^n x_i^2 + \sum_{j=1}^n (1 - f(x_j))^2 = \sum_{j=1}^n 2x_j - \sum_{k=1}^n 2 g(x_k) $$
Replacing the dummy indices $j$ and $k$ with $i$:
$$ \sum_{i=1}^n x_i^2 + \sum_{i=1}^n (1 - x_i \ln x_i)^2 = \sum_{i=1}^n 2x_i - \sum_{i=1}^n 2 x_i^2 \ln x_i $$
Rearranging the terms to group everything under a single sum:
$$ \sum_{i=1}^n \left[ x_i^2 + (1 - x_i \ln x_i)^2 - 2x_i + 2 x_i^2 \ln x_i \right] = 0 $$
Let $h(x) = x^2 + (1 - x \ln x)^2 - 2x + 2 x^2 \ln x$. The equation becomes $\sum_{i=1}^n h(x_i) = 0$.

We analyze the function $h(x)$ for $x>0$.
$h(x) = x^2 + (1 - 2x \ln x + (x \ln x)^2) - 2x + 2x^2 \ln x$
$h(x) = x^2 - 2x + 1 + (x \ln x)^2 - 2x \ln x + 2x^2 \ln x$
$h(x) = (x-1)^2 + x^2 (\ln x)^2 - 2x \ln x + 2x^2 \ln x$
$h(x) = (x-1)^2 + x \ln x (x \ln x - 2 + 2x)$

Let $A(x) = x \ln x (x \ln x - 2 + 2x)$. We want to determine the sign of $A(x)$.
Let $B(x) = x \ln x - 2 + 2x$. Then $A(x) = (x \ln x) B(x)$.

We evaluate $B(1) = 1 \ln 1 - 2 + 2(1) = 0 - 2 + 2 = 0$.
We compute the derivative of $B(x)$:
$B'(x) = \frac{d}{dx}(x \ln x - 2 + 2x) = (\ln x + x \cdot \frac{1}{x}) + 2 = \ln x + 1 + 2 = \ln x + 3$.

Case 1: $x > 1$.
For $x>1$, we have $\ln x > 0$. Thus $B'(x) = \ln x + 3 > 3 > 0$.
This means $B(x)$ is strictly increasing for $x > 1$. Since $B(1)=0$, we have $B(x) > 0$ for $x > 1$.
Also, for $x>1$, $x \ln x > 0$.
Therefore, $A(x) = (x \ln x) B(x)$ is a product of two positive numbers, so $A(x) > 0$ for $x > 1$.

Case 2: $0 < x < 1$.
For $0 < x < 1$, we have $\ln x < 0$. Thus $x \ln x < 0$.
The sign of $B'(x) = \ln x + 3$ depends on $x$.
$B'(x) = 0$ when $\ln x = -3$, which means $x = e^{-3}$. Note that $0 < e^{-3} < 1$.
If $0 < x < e^{-3}$, then $\ln x < -3$, so $B'(x) < 0$. $B(x)$ is decreasing in $(0, e^{-3})$.
If $e^{-3} < x < 1$, then $\ln x > -3$, so $B'(x) > 0$. $B(x)$ is increasing in $(e^{-3}, 1)$.
The minimum value of $B(x)$ on $(0, 1)$ occurs at $x=e^{-3}$.
$B(e^{-3}) = e^{-3} \ln(e^{-3}) - 2 + 2e^{-3} = -3e^{-3} - 2 + 2e^{-3} = -e^{-3} - 2 < 0$.
Let's check the limits at the boundaries. $\lim_{x \to 0^+} B(x) = \lim_{x \to 0^+} (x \ln x - 2 + 2x) = 0 - 2 + 0 = -2$.
$B(1) = 0$.
Since $B(x)$ decreases from $-2$ to $-e^{-3}-2$ and then increases to $0$, we can conclude that $B(x) < 0$ for all $x \in (0, 1)$.
Therefore, $A(x) = (x \ln x) B(x)$ is a product of two negative numbers ($x \ln x < 0$ and $B(x) < 0$), so $A(x) > 0$ for $0 < x < 1$.

Case 3: $x=1$.
$A(1) = (1 \ln 1) (1 \ln 1 - 2 + 2(1)) = 0 \cdot (0 - 2 + 2) = 0$.

Combining the cases, we have $A(x) \ge 0$ for all $x>0$, and $A(x)=0$ if and only if $x=1$.

Now we return to $h(x) = (x-1)^2 + A(x)$.
Since $(x-1)^2 \ge 0$ for all $x$, and $(x-1)^2 = 0$ iff $x=1$.
Since $A(x) \ge 0$ for all $x>0$, and $A(x)=0$ iff $x=1$.
The sum $h(x) = (x-1)^2 + A(x)$ is always non-negative.
$h(x) = 0$ if and only if both $(x-1)^2 = 0$ and $A(x)=0$. This occurs if and only if $x=1$.
So, $h(x) \ge 0$ for all $x>0$, and $h(x)=0$ iff $x=1$.

The sum equation is $\sum_{i=1}^n h(x_i) = 0$.
Since each term $h(x_i) \ge 0$, the sum can be zero only if each term is zero.
$h(x_i) = 0$ for all $i=1, \ldots, n$.
From our analysis of $h(x)$, this implies $x_i = 1$ for all $i=1, \ldots, n$.

We must check if $(x_1, x_2, \ldots, x_n) = (1, 1, \ldots, 1)$ is indeed a solution.
Substitute $x_i = 1$ for all $i$ into the $i$-th equation of the original system:
$x_i^2 + (1 - x_{i+1} \ln x_{i+1})^2 = 2x_{i+1} - 2 x_{i+2}^2 \ln x_{i+2}$
$1^2 + (1 - 1 \ln 1)^2 = 2(1) - 2 (1^2 \ln 1)$
$1 + (1 - 0)^2 = 2 - 2(0)$
$1 + 1^2 = 2$
$2 = 2$.
The equation holds for all $i$. Thus, $(1, 1, \ldots, 1)$ is a solution.

Since our analysis showed that any solution must satisfy $x_i=1$ for all $i$, this is the unique solution.

Final Answer: The final answer is $\boxed{(1, 1, \ldots, 1)}$