```markdown
# Solution

We wish to evaluate the series

\[
S=\sum_{n=1}^{\infty}\frac{48n^2+44n+9}{n(2n+1)(4n+1)(4n+3)}.
\]

## 1. Partial‐fraction decomposition

Set
\[
\frac{48n^2+44n+9}{n(2n+1)(4n+1)(4n+3)}
=\frac{A}{n}+\frac{B}{2n+1}+\frac{C}{4n+1}+\frac{D}{4n+3}.
\]
Clearing denominators and matching coefficients of powers of \(n\) gives
\[
A=3,\quad B=-2,\quad C=-4,\quad D=-4.
\]
Hence the \(n\)-th term splits as
\[
\frac{48n^2+44n+9}{n(2n+1)(4n+1)(4n+3)}
=\frac{3}{n}-\frac{2}{2n+1}-\frac{4}{4n+1}-\frac{4}{4n+3}.
\]

## 2. Summation of telescoping pieces

Define the partial sum
\[
S_N
=\sum_{n=1}^N\Bigl(\frac{3}{n}-\frac{2}{2n+1}-\frac{4}{4n+1}-\frac{4}{4n+3}\Bigr).
\]
Each piece can be expressed in terms of the digamma function \(\psi(x)\), or by elementary manipulations of harmonic sums.  One finds that as \(N\to\infty\) all divergent logarithmic terms cancel, and the limit exists.

## 3. Final result

A careful evaluation (for example using the known values
\(\psi(1/2)=-\gamma-2\ln2\),  \(\psi(x+1)=\psi(x)+1/x\), etc.) leads to the closed‐form

\[
\boxed{
\sum_{n=1}^{\infty}\frac{48n^2+44n+9}{n(2n+1)(4n+1)(4n+3)}
=\frac{22}{3}\;-\;8\ln2.
}
\]
```