Of course. Here is a detailed, step-by-step solution to the problem.

### **Understanding the Process**

Let the sequence at step $m$ be denoted by $S_m = (x_1^{(m)}, x_2^{(m)}, \ldots, x_{n-m}^{(m)})$.
The initial sequence is $S_0 = (x_1^{(0)}, x_2^{(0)}, \ldots, x_n^{(0)})$.
The transformation rule is $x_k^{(m+1)} = \sqrt{x_k^{(m)} x_{k+1}^{(m)}}$. This is the geometric mean of two consecutive terms.
The process continues for $n-1$ steps, at which point the sequence contains only one number, $x_1^{(n-1)}$. This is the *result*.

In our specific problem, the initial sequence is $x_k^{(0)} = k$ for $k=1, 2, \ldots, n$.

### **Step 1: Find a General Formula for the Result**

The operation involves repeated multiplication and square roots. This suggests that working with logarithms will simplify the process, transforming geometric means into arithmetic means.

Let $y_k^{(m)} = \ln(x_k^{(m)})$. The transformation rule becomes:
$y_k^{(m+1)} = \ln(\sqrt{x_k^{(m)} x_{k+1}^{(m)}}) = \frac{1}{2} \ln(x_k^{(m)} x_{k+1}^{(m)}) = \frac{1}{2} (\ln(x_k^{(m)}) + \ln(x_{k+1}^{(m)})) = \frac{1}{2} (y_k^{(m)} + y_{k+1}^{(m)})$.

This is a much simpler linear recurrence. Let's find an explicit formula for $y_k^{(m)}$ in terms of the initial values $y_1^{(0)}, y_2^{(0)}, \ldots, y_n^{(0)}$.

Let's compute the first few terms:
- $y_k^{(1)} = \frac{1}{2}y_k^{(0)} + \frac{1}{2}y_{k+1}^{(0)}$
- $y_k^{(2)} = \frac{1}{2}(y_k^{(1)} + y_{k+1}^{(1)}) = \frac{1}{2}\left( (\frac{1}{2}y_k^{(0)} + \frac{1}{2}y_{k+1}^{(0)}) + (\frac{1}{2}y_{k+1}^{(0)} + \frac{1}{2}y_{k+2}^{(0)}) \right) = \frac{1}{4}y_k^{(0)} + \frac{2}{4}y_{k+1}^{(0)} + \frac{1}{4}y_{k+2}^{(0)}$
- $y_k^{(3)} = \frac{1}{2}(y_k^{(2)} + y_{k+1}^{(2)}) = \frac{1}{2}\left( (\frac{1}{4}y_k^{(0)} + \frac{2}{4}y_{k+1}^{(0)} + \frac{1}{4}y_{k+2}^{(0)}) + (\frac{1}{4}y_{k+1}^{(0)} + \frac{2}{4}y_{k+2}^{(0)} + \frac{1}{4}y_{k+3}^{(0)}) \right) = \frac{1}{8}y_k^{(0)} + \frac{3}{8}y_{k+1}^{(0)} + \frac{3}{8}y_{k+2}^{(0)} + \frac{1}{8}y_{k+3}^{(0)}$

The coefficients are binomial coefficients divided by a power of 2. We can see a pattern emerging:
$y_k^{(m)} = \frac{1}{2^m} \sum_{j=0}^{m} \binom{m}{j} y_{k+j}^{(0)}$.

Let's prove this by induction on $m$.
**Base Case (m=1):** $y_k^{(1)} = \frac{1}{2^1} \left( \binom{1}{0}y_k^{(0)} + \binom{1}{1}y_{k+1}^{(0)} \right) = \frac{1}{2}(y_k^{(0)} + y_{k+1}^{(0)})$. This is correct.

**Inductive Step:** Assume the formula is true for $m$. Let's prove it for $m+1$.
$y_k^{(m+1)} = \frac{1}{2}(y_k^{(m)} + y_{k+1}^{(m)})$
Using the inductive hypothesis:
$y_k^{(m+1)} = \frac{1}{2} \left( \frac{1}{2^m} \sum_{j=0}^{m} \binom{m}{j} y_{k+j}^{(0)} + \frac{1}{2^m} \sum_{j=0}^{m} \binom{m}{j} y_{k+1+j}^{(0)} \right)$
$y_k^{(m+1)} = \frac{1}{2^{m+1}} \left( \sum_{j=0}^{m} \binom{m}{j} y_{k+j}^{(0)} + \sum_{j=0}^{m} \binom{m}{j} y_{k+j+1}^{(0)} \right)$

Let's re-index the second sum. Let $l=j+1$. When $j=0, l=1$. When $j=m, l=m+1$.
$y_k^{(m+1)} = \frac{1}{2^{m+1}} \left( \sum_{j=0}^{m} \binom{m}{j} y_{k+j}^{(0)} + \sum_{l=1}^{m+1} \binom{m}{l-1} y_{k+l}^{(0)} \right)$
Let's combine the sums.
$y_k^{(m+1)} = \frac{1}{2^{m+1}} \left( \binom{m}{0}y_k^{(0)} + \sum_{j=1}^{m} \left(\binom{m}{j} + \binom{m}{j-1}\right) y_{k+j}^{(0)} + \binom{m}{m}y_{k+m+1}^{(0)} \right)$

Using Pascal's Identity, $\binom{m}{j} + \binom{m}{j-1} = \binom{m+1}{j}$.
Also, $\binom{m}{0} = 1 = \binom{m+1}{0}$ and $\binom{m}{m} = 1 = \binom{m+1}{m+1}$.
So, we have:
$y_k^{(m+1)} = \frac{1}{2^{m+1}} \left( \binom{m+1}{0}y_k^{(0)} + \sum_{j=1}^{m} \binom{m+1}{j} y_{k+j}^{(0)} + \binom{m+1}{m+1}y_{k+m+1}^{(0)} \right)$
$y_k^{(m+1)} = \frac{1}{2^{m+1}} \sum_{j=0}^{m+1} \binom{m+1}{j} y_{k+j}^{(0)}$.
This completes the induction.

The final result is the single number $x_1^{(n-1)}$, which corresponds to $y_1^{(n-1)}$. Using the formula with $m=n-1$ and $k=1$:
$y_1^{(n-1)} = \frac{1}{2^{n-1}} \sum_{j=0}^{n-1} \binom{n-1}{j} y_{1+j}^{(0)}$.
Let's change the index to $i=j+1$.
$y_1^{(n-1)} = \frac{1}{2^{n-1}} \sum_{i=1}^{n} \binom{n-1}{i-1} y_i^{(0)}$.

Let $R$ be the result. Then $\ln R = y_1^{(n-1)}$.
$\ln R = \sum_{i=1}^{n} \frac{\binom{n-1}{i-1}}{2^{n-1}} y_i^{(0)} = \sum_{i=1}^{n} \frac{\binom{n-1}{i-1}}{2^{n-1}} \ln(x_i^{(0)})$.

This shows that $\ln R$ is a weighted average of the logarithms of the initial numbers. Exponentiating both sides, we get:
$R = \exp\left(\sum_{i=1}^{n} w_i \ln(x_i^{(0)})\right) = \prod_{i=1}^{n} \exp(\ln(x_i^{(0)})^{w_i}) = \prod_{i=1}^{n} (x_i^{(0)})^{w_i}$
where the weights are $w_i = \frac{\binom{n-1}{i-1}}{2^{n-1}}$.
Note that the weights sum to 1: $\sum_{i=1}^{n} w_i = \frac{1}{2^{n-1}} \sum_{i=1}^{n} \binom{n-1}{i-1} = \frac{1}{2^{n-1}} \sum_{j=0}^{n-1} \binom{n-1}{j} = \frac{1}{2^{n-1}} \cdot 2^{n-1} = 1$.
So, the result $R$ is the weighted geometric mean of the initial numbers.

### **Step 2: Apply Jensen's Inequality**

For our specific problem, $x_i^{(0)} = i$. So the result $R$ has a logarithm of:
$\ln R = \sum_{i=1}^{n} \frac{\binom{n-1}{i-1}}{2^{n-1}} \ln(i)$.

We want to prove $R \le \frac{n+1}{2}$. This is equivalent to proving $\ln R \le \ln\left(\frac{n+1}{2}\right)$.
The function $f(x) = \ln x$ is a concave function for $x>0$.
Jensen's inequality for a concave function states that for any set of points $\{x_1, \ldots, x_n\}$ and positive weights $\{w_1, \ldots, w_n\}$ with $\sum w_i = 1$:
$\sum_{i=1}^{n} w_i f(x_i) \le f\left(\sum_{i=1}^{n} w_i x_i\right)$.

Applying this to our problem with $f(x)=\ln x$, points $x_i=i$, and weights $w_i = \frac{\binom{n-1}{i-1}}{2^{n-1}}$:
$\ln R = \sum_{i=1}^{n} \frac{\binom{n-1}{i-1}}{2^{n-1}} \ln(i) \le \ln\left(\sum_{i=1}^{n} \frac{\binom{n-1}{i-1}}{2^{n-1}} i\right)$.

### **Step 3: Calculate the Weighted Arithmetic Mean**

Now we need to compute the argument of the logarithm on the right side. This is the weighted arithmetic mean of the numbers $(1, 2, \ldots, n)$.
Let $A = \sum_{i=1}^{n} \frac{\binom{n-1}{i-1}}{2^{n-1}} i = \frac{1}{2^{n-1}} \sum_{i=1}^{n} i \binom{n-1}{i-1}$.

Let's evaluate the sum $S = \sum_{i=1}^{n} i \binom{n-1}{i-1}$. Let $j = i-1$.
$S = \sum_{j=0}^{n-1} (j+1) \binom{n-1}{j} = \sum_{j=0}^{n-1} j \binom{n-1}{j} + \sum_{j=0}^{n-1} \binom{n-1}{j}$.

The second part of the sum is the sum of all binomial coefficients for $n-1$:
$\sum_{j=0}^{n-1} \binom{n-1}{j} = 2^{n-1}$.

For the first part, we use the identity $j\binom{m}{j} = m\binom{m-1}{j-1}$. With $m=n-1$:
$\sum_{j=0}^{n-1} j \binom{n-1}{j} = \sum_{j=1}^{n-1} j \frac{(n-1)!}{j!(n-1-j)!} = \sum_{j=1}^{n-1} \frac{(n-1)!}{(j-1)!(n-1-j)!}$
$= \sum_{j=1}^{n-1} (n-1) \frac{(n-2)!}{(j-1)!(n-2-(j-1))!} = (n-1) \sum_{j=1}^{n-1} \binom{n-2}{j-1}$.

Let $k=j-1$. The sum becomes:
$(n-1) \sum_{k=0}^{n-2} \binom{n-2}{k} = (n-1) 2^{n-2}$.

Combining the two parts of the sum $S$:
$S = (n-1) 2^{n-2} + 2^{n-1} = (n-1) 2^{n-2} + 2 \cdot 2^{n-2} = (n-1+2) 2^{n-2} = (n+1) 2^{n-2}$.

Now we can calculate the weighted arithmetic mean $A$:
$A = \frac{S}{2^{n-1}} = \frac{(n+1) 2^{n-2}}{2^{n-1}} = \frac{n+1}{2}$.

### **Step 4: Final Conclusion**

From Step 2, we had the inequality:
$\ln R \le \ln(A)$.

From Step 3, we found that $A = \frac{n+1}{2}$.
Therefore, $\ln R \le \ln\left(\frac{n+1}{2}\right)$.

Since the logarithmic function $y=\ln x$ is strictly increasing, we can conclude that:
$R \le \frac{n+1}{2}$.

This completes the proof.

**A note on equality:** For Jensen's inequality with a strictly concave function like $\ln x$, equality holds if and only if all the points $x_i$ are equal. In our case, the points are $(1, 2, \ldots, n)$. These are all equal only if $n=1$.
- If $n=1$, the sequence is (1), the result is 1. $\frac{1+1}{2}=1$. So $R=\frac{n+1}{2}$.
- If $n>1$, the points are not all equal, so the inequality is strict: $R < \frac{n+1}{2}$.
The problem asks to prove that the result is not greater than $\frac{n+1}{2}$, which is what we have shown.

---
**Summary of the proof:**
1.  We simplified the operation by taking logarithms, which turns the geometric mean operation into an arithmetic mean operation.
2.  We derived a general formula for the logarithm of the final result, showing it is a weighted average of the logarithms of the initial numbers, with weights given by normalized binomial coefficients.
3.  We applied Jensen's inequality for the concave function $f(x)=\ln x$. This bounded the logarithm of the result by the logarithm of the weighted arithmetic mean of the initial numbers $(1, 2, \ldots, n)$.
4.  We computed this weighted arithmetic mean by evaluating a sum involving binomial coefficients, and found it to be exactly $\frac{n+1}{2}$.
5.  This leads to the final inequality $R \le \frac{n+1}{2}$.