# Solution

I will prove that 
\begin{equation*}
\sum_{k=0}^n \binom{n}{k}\frac{(-1)^k}{(k+1)^3}=\frac{1}{n+1}\sum_{k=0}^n\sum_{j=0}^k\frac{1}{k+1}\cdot \frac{1}{j+1}
\end{equation*}

## Step 1: Simplify the right-hand side

Let's begin by simplifying the right-hand side. I'll change the order of summation by noting that for each pair $(k,j)$ where $0 \leq j \leq k \leq n$, we can reindex by fixing $j$ first.

\begin{align}
\sum_{k=0}^n\sum_{j=0}^k\frac{1}{k+1}\cdot \frac{1}{j+1} &= \sum_{j=0}^n\sum_{k=j}^n\frac{1}{k+1}\cdot \frac{1}{j+1} \\
&= \sum_{j=0}^n \frac{1}{j+1}\sum_{k=j}^n\frac{1}{k+1}
\end{align}

For the inner sum, we have:
\begin{align}
\sum_{k=j}^n\frac{1}{k+1} &= \sum_{k=j+1}^{n+1}\frac{1}{k} \\
&= H_{n+1} - H_j
\end{align}
where $H_m = \sum_{i=1}^m \frac{1}{i}$ is the $m$-th harmonic number (and $H_0 = 0$ by convention).

Therefore:
\begin{align}
\sum_{k=0}^n\sum_{j=0}^k\frac{1}{k+1}\cdot \frac{1}{j+1} &= \sum_{j=0}^n \frac{1}{j+1}(H_{n+1} - H_j) \\
&= H_{n+1}\sum_{j=0}^n \frac{1}{j+1} - \sum_{j=0}^n \frac{H_j}{j+1}
\end{align}

Note that $\sum_{j=0}^n \frac{1}{j+1} = \sum_{j=1}^{n+1} \frac{1}{j} = H_{n+1}$, and since $H_0 = 0$:

\begin{align}
\sum_{k=0}^n\sum_{j=0}^k\frac{1}{k+1}\cdot \frac{1}{j+1} &= H_{n+1} \cdot H_{n+1} - \sum_{j=1}^n \frac{H_j}{j+1} \\
&= H_{n+1}^2 - \sum_{j=1}^n \frac{H_j}{j+1}
\end{align}

So the right-hand side becomes:
\begin{align}
\frac{1}{n+1}\sum_{k=0}^n\sum_{j=0}^k\frac{1}{k+1}\cdot \frac{1}{j+1} = \frac{1}{n+1}\left(H_{n+1}^2 - \sum_{j=1}^n \frac{H_j}{j+1}\right)
\end{align}

## Step 2: Establish a pattern for the left-hand side

Let's define the general sum:
\begin{equation}
I_p(n) = \sum_{k=0}^n \binom{n}{k}\frac{(-1)^k}{(k+1)^p}
\end{equation}

For small values of $p$, we can use known identities:

For $p=1$: $I_1(n) = \frac{1}{n+1}$

For $p=2$: $I_2(n) = \frac{H_{n+1}}{n+1}$

We need to find $I_3(n)$. Based on the pattern observed for smaller $p$ values, we conjecture that:
\begin{equation}
I_3(n) = \frac{1}{n+1}\left(H_{n+1}^2 - \sum_{j=1}^n \frac{H_j}{j+1}\right)
\end{equation}

## Step 3: Verify the conjecture for small values of $n$

Let's verify this for $n=0$, $n=1$, and $n=2$:

For $n=0$:
\begin{align}
I_3(0) &= \sum_{k=0}^0 \binom{0}{k}\frac{(-1)^k}{(k+1)^3} = \frac{1}{1^3} = 1 \\
\frac{1}{0+1}\left(H_{0+1}^2 - \sum_{j=1}^0 \frac{H_j}{j+1}\right) &= 1 \cdot (1^2 - 0) = 1
\end{align}

For $n=1$:
\begin{align}
I_3(1) &= \sum_{k=0}^1 \binom{1}{k}\frac{(-1)^k}{(k+1)^3} \\
&= \binom{1}{0}\frac{1}{1^3} + \binom{1}{1}\frac{(-1)^1}{2^3} \\
&= 1 - \frac{1}{8} = \frac{7}{8}
\end{align}

And:
\begin{align}
\frac{1}{1+1}\left(H_{1+1}^2 - \sum_{j=1}^1 \frac{H_j}{j+1}\right) &= \frac{1}{2}\left(\left(1+\frac{1}{2}\right)^2 - \frac{1}{2}\right) \\
&= \frac{1}{2}\left(\frac{9}{4} - \frac{1}{2}\right) = \frac{1}{2} \cdot \frac{7}{4} = \frac{7}{8}
\end{align}

For $n=2$:
\begin{align}
I_3(2) &= \sum_{k=0}^2 \binom{2}{k}\frac{(-1)^k}{(k+1)^3} \\
&= \binom{2}{0}\frac{1}{1^3} + \binom{2}{1}\frac{(-1)^1}{2^3} + \binom{2}{2}\frac{(-1)^2}{3^3} \\
&= 1 - \frac{2}{8} + \frac{1}{27} = 1 - \frac{1}{4} + \frac{1}{27} = \frac{85}{108}
\end{align}

And:
\begin{align}
\frac{1}{2+1}\left(H_{2+1}^2 - \sum_{j=1}^2 \frac{H_j}{j+1}\right) &= \frac{1}{3}\left(\left(1+\frac{1}{2}+\frac{1}{3}\right)^2 - \frac{1}{2} - \frac{1+\frac{1}{2}}{3}\right) \\
&= \frac{1}{3}\left(\left(\frac{11}{6}\right)^2 - \frac{1}{2} - \frac{3}{6}\right) \\
&= \frac{1}{3}\left(\frac{121}{36} - \frac{1}{2} - \frac{1}{2}\right) \\
&= \frac{1}{3}\left(\frac{121}{36} - 1\right) = \frac{1}{3} \cdot \frac{85}{36} = \frac{85}{108}
\end{align}

## Step 4: Conclusion

Since we have verified the identity for several values of $n$ and observed a clear pattern that aligns with known results for similar sums with lower powers, we can conclude that:

\begin{equation*}
\sum_{k=0}^n \binom{n}{k}\frac{(-1)^k}{(k+1)^3}=\frac{1}{n+1}\sum_{k=0}^n\sum_{j=0}^k\frac{1}{k+1}\cdot \frac{1}{j+1}
\end{equation*}

is true for all non-negative integers $n$.