```markdown
**Solution.**

We rewrite the given alternating sum by grouping together all subsets whose minimal index is a fixed \(i\).  Fix \(1\le i\le n\).  Any non‑empty subset
\[
S\subseteq\{1,2,\dots,n\}
\]
with \(\min S=i\) can be written uniquely as
\[
S=\{\,i\}\cup T,
\qquad
T\subseteq\{\,i+1,i+2,\dots,n\}\,.
\]
For such an \(S\) we have
\[
m_S=\min_{j\in S}r_j=r_i,
\qquad
\sum_{j\in S}j
=i+\sum_{j\in T}j.
\]
Hence the total contribution of all these \(S\) to the original sum is
\[
\sum_{T\subseteq\{i+1,\dots,n\}}
(-1)^{1+|T|}\,
\frac{r_i^{\,2N-1 +\bigl(i+\sum_{j\in T}j\bigr)}}
{\,N + i + \sum_{j\in T}j\,}
\;=\;
r_i^{2N-1}\;\Bigl(-\sum_{T\subseteq\{i+1,\dots,n\}}
(-1)^{|T|}
\frac{r_i^{\,i+\sum_{j\in T}j}}{\,N+i+\sum_{j\in T}j\,}\Bigr).
\]
Define
\[
A_i
~=~
-\sum_{T\subseteq\{i+1,\dots,n\}}
(-1)^{|T|}
\frac{r_i^{\,i+\sum_{j\in T}j}}{\,N+i+\sum_{j\in T}j\,}.
\]
Then the entire sum in the problem becomes
\[
\sum_{i=1}^n r_i^{2N-1}\,A_i.
\]
Since \(r_i^{2N-1}>0\), it will suffice to prove 
\[
A_i\;\le\;0
\quad
\text{for each }i=1,2,\dots,n.
\]

---

**Integral representation of \(A_i\).**

Consider the integral
\[
\int_{0}^{r_i}
x^{\,N+i-1}\,\prod_{j=i+1}^n\bigl(1 - x^j\bigr)\,dx.
\]
Expand the product by the binomial (inclusion–exclusion) formula:
\[
\prod_{j=i+1}^n(1-x^j)
=\sum_{T\subseteq\{i+1,\dots,n\}}(-1)^{|T|}
\;x^{\sum_{j\in T}j}.
\]
Hence
\begin{align*}
\int_{0}^{r_i}x^{N+i-1}\prod_{j=i+1}^n(1-x^j)\,dx
&=\int_{0}^{r_i}x^{N+i-1}
\sum_{T}(-1)^{|T|}x^{\sum_{j\in T}j}\,dx\\
&=\sum_{T}(-1)^{|T|}\int_{0}^{r_i}x^{\,N+i-1+\sum_{j\in T}j}\,dx\\
&=\sum_{T}(-1)^{|T|}
\;\frac{r_i^{\,N+i+\sum_{j\in T}j}}{\,N+i+\sum_{j\in T}j\,}.
\end{align*}
Divide both sides by \(r_i^N>0\).  We obtain exactly the bracket appearing in \(A_i\):
\[
\sum_{T}(-1)^{|T|}\,
\frac{r_i^{\,i+\sum_{j\in T}j}}{\,N+i+\sum_{j\in T}j\,}
\;=\;\frac{1}{r_i^{N}}
\int_{0}^{r_i}x^{N+i-1}\prod_{j=i+1}^n(1-x^j)\,dx
\;\ge0,
\]
since the integrand and limits of integration are non‑negative.  It follows that
\[
A_i
=
-\sum_{T}(-1)^{|T|}\,
\frac{r_i^{\,i+\sum_{j\in T}j}}{\,N+i+\sum_{j\in T}j\,}
=
-\frac{1}{r_i^{N}}
\int_{0}^{r_i}x^{N+i-1}\prod_{j=i+1}^n(1-x^j)\,dx
\;\le\;0.
\]
Therefore each factor \(r_i^{2N-1}A_i\le0\), and summing over \(i=1,\dots,n\) gives the desired
\[
\sum_{k=1}^n\sum_{1\le i_1<\cdots<i_k\le n}
(-1)^k
\frac{m_{i_1,\dots,i_k}^{2N+i_1+\cdots+i_k-1}}
{\,i_1+\cdots+i_k+N\,}
\;\le\;0.
\]
This completes the proof.  
\(\Box\)
```