Of course. Here is a detailed, step-by-step solution to the problem.

Let $P(z_1, z_2)$ be the assertion $f(f(z_1)+z_2)=z_1+f(z_2)$.

### Step 1: Initial deductions from the equation

We begin by substituting specific values for $z_1$ and $z_2$ to uncover the basic properties of the function $f$.

1.  **Set $z_1 = 0$:**
    $P(0, z_2) \implies f(f(0)+z_2) = 0 + f(z_2)$.
    Let $c = f(0)$. Then we have:
    $f(c + z_2) = f(z_2)$ for all $z_2 \in V$.
    This shows that $f$ is a periodic function with period $c$.

2.  **Set $z_2 = 0$:**
    $P(z_1, 0) \implies f(f(z_1)+0) = z_1 + f(0)$.
    Using $c=f(0)$ again, we get:
    $f(f(z_1)) = z_1 + c$ for all $z_1 \in V$.
    This tells us how the double application of $f$ behaves.

3.  **Combine the properties to find $c$:**
    Let's apply the function $f$ to both sides of the equation $f(f(z)) = z+c$:
    $f(f(f(z))) = f(z+c)$.

    From property (1), we know $f(z+c) = f(z)$. So the right side is $f(z)$.
    $f(f(f(z))) = f(z)$.

    Now let's analyze the left side, $f(f(f(z)))$, using property (2). Let $w = f(z)$. Then $f(f(w)) = w+c$.
    Substituting $w=f(z)$ back, we get:
    $f(f(f(z))) = f(z) + c$.

    Comparing our two derived expressions for $f(f(f(z)))$:
    $f(z) = f(z) + c$.
    Subtracting $f(z)$ from both sides gives $c = 0$.

4.  **Update properties with $c=0$:**
    Since $c=f(0)=0$, our two main properties simplify significantly:
    -   From $c=0$, we have $f(0)=0$.
    -   From $f(f(z)) = z+c$, we have $f(f(z)) = z$ for all $z \in V$.
    This means $f$ is an **involution**. An immediate consequence is that $f$ is its own inverse, $f^{-1}=f$, which implies $f$ must be a bijection (both injective and surjective).

### Step 2: Proving $f$ is a linear transformation

Now we use the fact that $f(f(z))=z$ to simplify the original equation and prove linearity.

1.  **Simplify the original equation:**
    The original equation is $f(f(z_1)+z_2) = z_1+f(z_2)$.
    Apply $f$ to both sides:
    $f(f(f(z_1)+z_2)) = f(z_1+f(z_2))$.

    Since $f(f(w))=w$ for any $w$, the left side becomes:
    $f(z_1)+z_2 = f(z_1+f(z_2))$.

2.  **Prove additivity:**
    The equation we just derived is $f(z_1)+z_2 = f(z_1+f(z_2))$.
    Since $f$ is surjective, for any vector $y \in V$, there exists some $x \in V$ such that $f(x)=y$.
    Let's substitute $z_2 = f(y)$ for an arbitrary $y \in V$ into this equation.
    $f(z_1) + f(y) = f(z_1 + f(f(y)))$.

    Since $f(f(y))=y$, this simplifies to:
    $f(z_1) + f(y) = f(z_1 + y)$.

    This is the Cauchy functional equation for vectors. It shows that $f$ is **additive**.

3.  **Prove homogeneity over $Q$:**
    Since $f$ is additive and the vector space $V$ is over the field of rational numbers $Q$, $f$ must be a $Q$-linear transformation. Let's show this explicitly.
    -   For any integer $n \in \mathbb{N}$, $f(nz) = f(z+\dots+z) = f(z)+\dots+f(z) = n f(z)$.
    -   We know $f(0)=0$. Also, $f(z) + f(-z) = f(z-z)=f(0)=0$, so $f(-z) = -f(z)$.
    -   For any integer $n \in \mathbb{Z}$, $f(nz) = n f(z)$.
    -   For any rational number $q \in Q$, let $q = p/r$ with $p \in \mathbb{Z}$ and $r \in \mathbb{N}, r \neq 0$.
    Let $z \in V$. We have $f(r(q z)) = f(p z)$.
    Using the integer homogeneity, $r f(q z) = p f(z)$.
    Since $V$ is a vector space over $Q$ and $r \neq 0$, we can multiply by $1/r$:
    $f(q z) = (p/r) f(z) = q f(z)$.

    Thus, $f$ satisfies both additivity and homogeneity over $Q$, which means $f$ is a **$Q$-linear transformation**.

### Step 3: Characterizing the solutions

We have reduced the problem to finding all $Q$-linear transformations $f: V \to V$ that also satisfy the condition $f(f(z)) = z$ for all $z \in V$. In operator notation, this is $f^2 = I$, where $I$ is the identity operator. Such operators are called **involutory linear transformations**.

Let's characterize these transformations. The equation $f^2 - I = 0$ implies that the minimal polynomial of $f$ must divide $x^2-1 = (x-1)(x+1)$. This means the only possible eigenvalues of $f$ are $\lambda=1$ and $\lambda=-1$.

Let's define two subspaces of $V$:
-   $V_1 = \ker(f - I) = \{v \in V \mid f(v) = v\}$. This is the eigenspace corresponding to the eigenvalue $\lambda=1$.
-   $V_{-1} = \ker(f + I) = \{v \in V \mid f(v) = -v\}$. This is the eigenspace corresponding to the eigenvalue $\lambda=-1$.

For any vector $v \in V$, we can write it as a sum of two vectors, one in $V_1$ and one in $V_{-1}$. Consider the following construction:
-   Let $v_1 = \frac{1}{2}(v + f(v))$.
-   Let $v_{-1} = \frac{1}{2}(v - f(v))$.

(Note: This is possible because $V$ is a vector space over $Q$, so division by 2 is well-defined as multiplication by the scalar $1/2 \in Q$.)

Let's check which subspace these vectors belong to:
-   $f(v_1) = f(\frac{1}{2}(v + f(v))) = \frac{1}{2}(f(v) + f(f(v))) = \frac{1}{2}(f(v) + v) = v_1$.
    So, $v_1 \in V_1$.
-   $f(v_{-1}) = f(\frac{1}{2}(v - f(v))) = \frac{1}{2}(f(v) - f(f(v))) = \frac{1}{2}(f(v) - v) = -\frac{1}{2}(v - f(v)) = -v_{-1}$.
    So, $v_{-1} \in V_{-1}$.

Adding these two vectors gives:
$v_1 + v_{-1} = \frac{1}{2}(v + f(v)) + \frac{1}{2}(v - f(v)) = \frac{1}{2}(2v) = v$.
This shows that any vector $v \in V$ can be uniquely written as a sum of a vector from $V_1$ and a vector from $V_{-1}$, which means $V$ is the direct sum of these subspaces:
$V = V_1 \oplus V_{-1}$.

This means that any solution $f$ determines a direct sum decomposition of $V$. Conversely, any such decomposition defines a valid function $f$.

### Step 4: Final Solution

Let's formulate the complete set of solutions.
A function $f: V \to V$ is a solution to the given functional equation if and only if it is constructed as follows:

1.  Choose two subspaces of $V$, let's call them $W_1$ and $W_2$, such that $V$ is their direct sum: $V = W_1 \oplus W_2$. This means that for any vector $v \in V$, there is a unique pair of vectors $w_1 \in W_1$ and $w_2 \in W_2$ such that $v = w_1 + w_2$.

2.  Define the function $f$ based on this decomposition as:
    $f(v) = f(w_1 + w_2) = w_1 - w_2$.

This function corresponds to a reflection across the subspace $W_1$ along the subspace $W_2$.

**Verification:**
Let's check that any function of this form satisfies the original equation.
First, we show it is a linear map satisfying $f(f(v))=v$.
-   **Linearity:** Let $v = w_1+w_2$ and $u=u_1+u_2$. For $a, b \in Q$,
    $a v + b u = a(w_1+w_2) + b(u_1+u_2) = (aw_1+bu_1) + (aw_2+bu_2)$.
    The first part is in $W_1$ and the second is in $W_2$.
    $f(av+bu) = (aw_1+bu_1) - (aw_2+bu_2) = a(w_1-w_2) + b(u_1-u_2) = a f(v) + b f(u)$.
    So $f$ is linear.
-   **Involution property:**
    $f(v) = w_1 - w_2$. The $W_1$ component is $w_1$ and the $W_2$ component is $-w_2$.
    $f(f(v)) = f(w_1 + (-w_2)) = w_1 - (-w_2) = w_1 + w_2 = v$.
    So $f(f(v))=v$.

Since $f$ is linear and $f(f(v))=v$, our derivation in Step 2 shows it must satisfy the original equation. For completeness:
$f(f(z_1)+z_2) = z_1+f(z_2)$.
Let $z_1 = w_1+w_2$ and $z_2 = u_1+u_2$.
LHS = $f(f(w_1+w_2) + (u_1+u_2)) = f((w_1-w_2) + (u_1+u_2)) = f((w_1+u_1) + (u_2-w_2))$.
The term $(w_1+u_1) \in W_1$ and $(u_2-w_2) \in W_2$. So,
LHS = $(w_1+u_1) - (u_2-w_2) = w_1+u_1-u_2+w_2$.

RHS = $z_1 + f(z_2) = (w_1+w_2) + (u_1-u_2) = w_1+w_2+u_1-u_2$.

LHS = RHS, so the verification is complete.

**Examples:**
-   If we choose $W_1=V$ and $W_2=\{0\}$, then any $v \in V$ is just $v \in W_1$. So $f(v) = v$. This is the identity function.
-   If we choose $W_1=\{0\}$ and $W_2=V$, then any $v \in V$ is just $v \in W_2$. So $f(v) = 0 - v = -v$. This is the negation function.

---
### Summary of the Solution

The set of all functions $f: V \to V$ satisfying the given equation is the set of all involutory linear transformations on $V$.
A function $f$ is a solution if and only if there exist subspaces $W_1, W_2 \subseteq V$ such that $V=W_1 \oplus W_2$, and $f$ is defined for any $v=w_1+w_2$ (with $w_1 \in W_1, w_2 \in W_2$) by:
$$f(v) = w_1 - w_2$$