```markdown
**Solution.**  
Denote
\[
A=(2n)!\,,\quad B=(2m)!\,,\quad C=(2k)!\,,\quad
D=(n+m)!\,,\quad E=(n+k)!\,,\quad F=(m+k)!.
\]
The inequality to prove is
\[
xA+yB+zC\;\ge\;(x-y+z)\,E+(-x+y+z)\,F+(x+y-z)\,D.
\]
Rearranging gives
\[
x\,(A+E-D-F)+y\,(B+F-D-E)+z\,(C+D-E-F)\;\ge\;0
\]
which is an affine (in fact linear) function of \((x,y,z)\).  Hence on the box
\[
1\le x,y,z\le4
\]
its minimum occurs at one of the \(2^3=8\) vertices \((x,y,z)\in\{1,4\}^3\).  
By the obvious cyclic symmetry in \((x,n),(y,m),(z,k)\), there are only three essentially different vertices to check:
\[
(1,1,1),\quad(1,1,4),\quad(1,4,4),
\]
the others following by symmetry or by multiplying by~4.

---

### 1. The case \((x,y,z)=(1,1,1)\)

We must show
\[
A+B+C\;\ge\;D+E+F.
\]
But for any two non‐negative integers \(u,v\) one has the *two‐term* estimate
\[
(2u)!+(2v)!\;\ge\;2\,(u+v)!,
\]
because \(\log(n!)\) is convex in \(n\).  Applying it to the three pairs \((n,m)\), \((m,k)\), \((k,n)\) and summing,
\[
\begin{aligned}
(2n)!+(2m)!&\ge2\,(n+m)!,\\
(2m)!+(2k)!&\ge2\,(m+k)!,\\
(2k)!+(2n)!&\ge2\,(n+k)!,
\end{aligned}
\]
we get
\[
2\,(A+B+C)\;\ge\;2\,(D+E+F),
\]
i.e. \(A+B+C\ge D+E+F\).  This settles \((1,1,1)\).  Multiplying by 4 gives the case \((4,4,4)\).

---

### 2. The case \((x,y,z)=(1,1,4)\)

Here the inequality reads
\[
A+B+4\,C\;\ge\;4\,E+4\,F-2\,D,
\]
or equivalently
\[
A+B+4C\;+\;2D\;\ge\;4E+4F.
\]
We split this into three applications of the two‐term estimate:
1.  \((2n)!+(2m)!\ge2\,(n+m)!=2D\),  
2.  \((2k)!+D\ge E+F\),  applied **four** times.  

Summing one copy of (1) and four copies of (2) gives
\[
\bigl(A+B+2D\bigr)\;+\;4\bigl(C+D\bigr)\;\ge\;2D\;+\;4\,(E+F)
\]
i.e.
\[
A+B+4C+6D\;\ge\;4E+4F+2D,
\]
hence
\[
A+B+4C+2D\;\ge\;4E+4F,
\]
as required.

---

### 3. The case \((x,y,z)=(1,4,4)\)

Now one must show
\[
A+4B+4C\;\ge\;E+7F+D.
\]
Rewritten,
\[
A+4B+4C\;-\;D\;-\;E\;-\;7F\;\ge0.
\]
We build it from these two‐term facts:
  •  \((2m)!+(2k)!\ge2\,(m+k)!=2F\), applied **three** times,  
  •  \((2n)!+B\ge2\,(n+m)!=2D\),  
  •  \((2n)!+C\ge2\,(n+k)!=2E\).  

Summing three copies of the first and one copy each of the last two, we get
\[
3\,(B+C)+\bigl(A+B\bigr)+\bigl(A+C\bigr)
\;\ge\;6F+2D+2E,
\]
i.e.
\[
A+4B+4C+2A
\;\ge\;6F+2D+2E
\quad\Longrightarrow\quad
A+4B+4C\;\ge\;E+D+7F.
\]
This is exactly the desired form.

---

Since the only extreme points give true inequalities, by linearity in \((x,y,z)\) the original inequality holds for _all_ real \(1\le x,y,z\le4\).  This completes the proof.  
∎
```