Below is one complete solution in markdown with LaTeX. One may show that the only continuous function
\[
f:\mathbb{R}^+ \to \mathbb{R}^+
\]
satisfying
\[
\frac{f(x)+f(y)}{f(xy)}=\frac{1}{f(x+y)}-2xy,\quad \forall x,y>0,
\]
is
\[
f(x)=\frac{1}{x^2}\,.
\]

In what follows we describe one way to arrive at that answer.

---

### Step 1. Rewrite the Equation

We wish to find all continuous functions \( f:\mathbb{R}^+\to\mathbb{R}^+ \) such that
\[
\frac{f(x)+f(y)}{f(xy)}=\frac{1}{f(x+y)}-2xy.
\]
A natural idea is to “invert” the function. Define
\[
g(x)=\frac{1}{f(x)},\quad x>0.
\]
Then the given equation becomes (writing \( f(x)=1/g(x) \)):

\[
\frac{\displaystyle \frac{1}{g(x)}+\frac{1}{g(y)}}{\frac{1}{g(xy)}}=
\frac{g(x)+g(y)}{g(x)g(y)}\,g(xy)
=\frac{1}{f(x+y)}-2xy = g(x+y)-2xy.
\]
That is, in terms of \( g \) the equation is
\[
\frac{(g(x)+g(y))\,g(xy)}{g(x)g(y)} = g(x+y) - 2xy,\quad\forall x,y>0.
\]

---

### Step 2. A “Quadratic‐Ansatz”

The appearance of the term \(2xy\) on the right–hand side suggests that a quadratic function might work. In other words, one is led to try an ansatz of the form
\[
g(x)=Ax^2+B,\quad A,B\in\mathbb{R},
\]
which in turn means
\[
f(x)=\frac{1}{Ax^2+B}\,.
\]
Since \( f(x)>0 \) for \( x>0 \) we must have \(Ax^2+B>0\) for all \(x>0\).

Let us substitute
\[
g(x)=Ax^2+B,\quad g(y)=Ay^2+B,\quad g(xy)=A(xy)^2+B,\quad g(x+y)=A(x+y)^2+B
\]
into
\[
\frac{(g(x)+g(y))\,g(xy)}{g(x)g(y)} = g(x+y) - 2xy.
\]

First note that
\[
g(x)+g(y)=A(x^2+y^2)+2B,
\]
and
\[
g(x)g(y)=(Ax^2+B)(Ay^2+B)=A^2x^2y^2+AB(x^2+y^2)+B^2.
\]
Also,
\[
g(xy)=Ax^2y^2+B,\quad\text{and}\quad g(x+y)=A(x+y)^2+B=A(x^2+2xy+y^2)+B.
\]

A good idea is to see what happens when we take the special case \(x=y\). Setting \( x=y \) gives
\[
g(x)=Ax^2+B,\quad g(x^2)=Ax^4+B,\quad g(2x)=A(2x)^2+B=4Ax^2+B.
\]
Then the equation becomes
\[
\frac{\bigl(2Ax^2+2B\bigr)(Ax^4+B)}{(Ax^2+B)^2} = 4Ax^2+B - 2x^2.
\]
Since
\[
\frac{2Ax^4+2B x^0}{(Ax^2+B)^2} = 2\,\frac{Ax^4+B}{Ax^2+B}\,,
\]
we obtain
\[
2\,\frac{Ax^4+B}{Ax^2+B} = (4A-2)x^2+B.
\]
Multiplying both sides by \(Ax^2+B\) gives
\[
2(Ax^4+B)=\Bigl[(4A-2)x^2+B\Bigr](Ax^2+B).
\]
Expanding the right–hand side yields
\[
2Ax^4+2B = (4A-2)Ax^4 + \Bigl[(4A-2)B+AB\Bigr]x^2 + B^2.
\]
Because this is to hold for all \(x>0\) the coefficients must match. Equate the coefficient of \(x^4\):
\[
2A = (4A-2)A.
\]
Since \(A\neq 0\) (or else \(g\) would be constant) one may cancel \(A\) to obtain
\[
2=4A-2\quad\Longrightarrow\quad 4A=4\quad\Longrightarrow\quad A=1.
\]
Next, equate the coefficient of \(x^2\). (Notice that on the left–hand side there is no \(x^2\) term.)
\[
0= (4A-2)B + AB = B(4A-2+A)=B(5A-2).
\]
With \(A=1\) this gives
\[
B(5-2)=3B=0\quad \Longrightarrow\quad B=0.
\]
Finally, equate the constant term:
\[
2B=B^2.
\]
This is automatically satisfied by \(B=0\).

Thus our ansatz forces
\[
g(x)=x^2,
\]
which means
\[
f(x)=\frac{1}{g(x)}=\frac{1}{x^2}\,.
\]

---

### Step 3. Verification

It is always a good idea to check the candidate solution in the original equation. Assume
\[
f(x)=\frac{1}{x^2}.
\]
Then for any \(x,y>0\) we compute
\[
\frac{f(x)+f(y)}{f(xy)}=\frac{\frac{1}{x^2}+\frac{1}{y^2}}{\frac{1}{(xy)^2}}
=\Bigl(\frac{1}{x^2}+\frac{1}{y^2}\Bigr)(x^2y^2)
=x^2+y^2.
\]
On the other hand,
\[
\frac{1}{f(x+y)}-2xy=\,(x+y)^2-2xy=x^2+2xy+y^2-2xy=x^2+y^2.
\]
Thus the two sides agree, and \(f(x)=1/x^2\) does indeed satisfy
\[
\frac{f(x)+f(y)}{f(xy)}=\frac{1}{f(x+y)}-2xy,\quad\forall x,y>0.
\]

---

### Conclusion

We have shown that the only continuous function \(f:\mathbb{R}^+\to\mathbb{R}^+\) satisfying
\[
\frac{f(x)+f(y)}{f(xy)}=\frac{1}{f(x+y)}-2xy
\]
is
\[
\boxed{f(x)=\frac{1}{x^2}\,.}
\]

Below is the complete markdown code with LaTeX.

---

```markdown
# Solution

We wish to find all continuous functions 
\[
f:\mathbb{R}^+\to\mathbb{R}^+
\]
satisfying
\[
\frac{f(x)+f(y)}{f(xy)}=\frac{1}{f(x+y)}-2xy,\quad\forall x,y>0.
\]

## Step 1. Passing to the Reciprocal

Define
\[
g(x)=\frac{1}{f(x)}.
\]
Then, since \( f(x)=\frac{1}{g(x)} \), the equation becomes
\[
\frac{\frac{1}{g(x)}+\frac{1}{g(y)}}{\frac{1}{g(xy)}}
=\frac{g(x)+g(y)}{g(x)g(y)}\,g(xy)
=g(x+y)-2xy.
\]
Thus, the equation in terms of \(g\) is
\[
\frac{(g(x)+g(y))\,g(xy)}{g(x)g(y)} = g(x+y)-2xy.
\]

## Step 2. A Quadratic Ansatz

The presence of a \(2xy\) term suggests trying a quadratic function. Suppose that
\[
g(x)=Ax^2+B,\quad A,B\in\mathbb{R}.
\]
Then
\[
f(x)=\frac{1}{Ax^2+B}.
\]
We have
\[
\begin{aligned}
g(x)+g(y)&=A(x^2+y^2)+2B,\\[1mm]
g(x)g(y)&=(Ax^2+B)(Ay^2+B)=A^2x^2y^2+AB(x^2+y^2)+B^2,\\[1mm]
g(xy)&=A(xy)^2+B \quad \text{and} \quad
g(x+y)=A(x+y)^2+B=A(x^2+2xy+y^2)+B.
\end{aligned}
\]
It is convenient to set \(x=y\). Then:

- \(g(x)=Ax^2+B\),
- \(g(x^2)=Ax^4+B\),
- \(g(2x)=4Ax^2+B\).

For \(x=y\) the equation becomes
\[
\frac{(2Ax^2+2B)(Ax^4+B)}{(Ax^2+B)^2}
=4Ax^2+B-2x^2.
\]
A short calculation shows that the left–hand side simplifies to
\[
2\,\frac{Ax^4+B}{Ax^2+B}.
\]
Thus, we must have
\[
2\,\frac{Ax^4+B}{Ax^2+B}=(4A-2)x^2+B,\quad\forall x>0.
\]
Multiplying by \(Ax^2+B\) yields
\[
2(Ax^4+B) = \Bigl[(4A-2)x^2+B\Bigr](Ax^2+B).
\]
Expanding the right–hand side and equating coefficients yields:

1. For \(x^4\): 
\[
2A = (4A-2)A.
\]
Since \(A\neq0\), it follows that
\[
2=4A-2\quad\Longrightarrow\quad A=1.
\]

2. For \(x^2\): The coefficient must vanish:
\[
0=B(5A-2)=B(5-2)=3B,\quad\Longrightarrow\quad B=0.
\]

3. The constant term automatically gives \(2B=B^2\) which holds when \(B=0\).

Thus, \(g(x)=x^2\) and so
\[
f(x)=\frac{1}{g(x)}=\frac{1}{x^2}.
\]

## Step 3. Verification

Let us check that 
\[
f(x)=\frac{1}{x^2}
\]
satisfies the equation. For every \(x,y>0\),
\[
\begin{aligned}
\frac{f(x)+f(y)}{f(xy)}
&=\frac{\frac{1}{x^2}+\frac{1}{y^2}}{\frac{1}{(xy)^2}}
=\Bigl(\frac{1}{x^2}+\frac{1}{y^2}\Bigr)(x^2y^2)\\[1mm]
&= y^2 + x^2,
\end{aligned}
\]
and
\[
\frac{1}{f(x+y)}-2xy = (x+y)^2-2xy = x^2+2xy+y^2-2xy=x^2+y^2.
\]
Since the two sides are equal, \(f(x)=\frac{1}{x^2}\) is indeed a solution.

## Conclusion

The only continuous function \( f:\mathbb{R}^+\to\mathbb{R}^+ \) satisfying
\[
\frac{f(x)+f(y)}{f(xy)}=\frac{1}{f(x+y)}-2xy
\]
is
\[
\boxed{f(x)=\frac{1}{x^2}\,.}
\]
```

---

### Final Answer

\[
\boxed{f(x)=\frac{1}{x^2}}
\]

Any function other than \( f(x)=\frac{1}{x^2} \) can be ruled out (for example, assuming a solution of the form \( f(x)=\frac{c}{x^2} \) forces \( c=1 \) by a short calculation). Hence, the unique solution is
\[
f(x)=\frac{1}{x^2}\,.
\]