```markdown
We start by defining
\[
a = \sqrt{5}+2 \quad \text{and} \quad b = \sqrt{5}-2.
\]
Notice that
\[
a \cdot b = (\sqrt{5}+2)(\sqrt{5}-2) = (\sqrt{5})^2 - (2)^2 = 5-4 = 1,
\]
so
\[
b = \frac{1}{a}.
\]

Now, consider the expression \((\sqrt{5}+2)^{2n}=a^{2n}\). Because \(b=\sqrt{5}-2\) satisfies \(0<b<1\) (since \(\sqrt{5} \approx 2.236\), so \(b \approx 0.236\)), raising \(b\) to any positive power yields
\[
0 < b^{2n} < 1.
\]

Next, look at the sum
\[
a^{2n} + b^{2n} = (\sqrt{5}+2)^{2n}+(\sqrt{5}-2)^{2n}.
\]
It turns out that this sum is an integer. (This can be verified using the Binomial Theorem or by noting that the sequence
\[
x_n = (\sqrt{5}+2)^n+(\sqrt{5}-2)^n
\]
satisfies a linear recurrence with integer coefficients.)

Since \(0 < b^{2n} < 1\), we have
\[
a^{2n} < a^{2n} + b^{2n} < a^{2n} + 1.
\]
Thus, the integer
\[
I = (\sqrt{5}+2)^{2n}+(\sqrt{5}-2)^{2n}
\]
satisfies
\[
I-1 < (\sqrt{5}+2)^{2n} < I.
\]
This shows that \(I\) is the smallest integer greater than \((\sqrt{5}+2)^{2n}\).

Therefore, the answer is
\[
\boxed{(\sqrt{5}+2)^{2n}+(\sqrt{5}-2)^{2n}}.
\]
```