Let $S_0 = (x_1, x_2, \ldots, x_n)$ be the initial sequence. In this problem, $x_k = k$ for $k=1, 2, \ldots, n$.
Let $S_m = (x_{m,1}, x_{m,2}, \ldots, x_{m, n-m})$ denote the sequence after $m$ actions.
The transformation rule is given by $x_{m,i} = \sqrt{x_{m-1,i} x_{m-1,i+1}}$ for $m \ge 1$ and $1 \le i \le n-m$.
The process continues for $n-1$ actions, after which only one number remains. This final number is the result, denoted by $R$. The final number is $x_{n-1, 1}$.

Let's express the elements of the sequences in terms of the initial sequence $S_0 = (x_{0,1}, \ldots, x_{0,n})$.
$x_{1,i} = (x_{0,i} x_{0,i+1})^{1/2}$
$x_{2,i} = \sqrt{x_{1,i} x_{1,i+1}} = ((x_{0,i} x_{0,i+1})^{1/2} (x_{0,i+1} x_{0,i+2})^{1/2})^{1/2} = (x_{0,i}^{1/2} x_{0,i+1} x_{0,i+2}^{1/2})^{1/2} = x_{0,i}^{1/4} x_{0,i+1}^{1/2} x_{0,i+2}^{1/4}$
Let's claim that the general form is given by:
$x_{m,i} = \prod_{j=0}^m x_{0, i+j}^{c_{m,j}}$, where $c_{m,j} = \frac{\binom{m}{j}}{2^m}$.

We prove this by induction on $m$.
Base case $m=1$: $x_{1,i} = x_{0,i}^{1/2} x_{0,i+1}^{1/2}$. The formula gives $c_{1,0} = \binom{1}{0}/2^1 = 1/2$ and $c_{1,1} = \binom{1}{1}/2^1 = 1/2$. This matches.
Assume the formula holds for $m-1$. So $x_{m-1,i} = \prod_{j=0}^{m-1} x_{0, i+j}^{\binom{m-1}{j} / 2^{m-1}}$.
Then $x_{m,i} = \sqrt{x_{m-1,i} x_{m-1,i+1}}$.
$x_{m,i} = \left( \left( \prod_{j=0}^{m-1} x_{0, i+j}^{\binom{m-1}{j} / 2^{m-1}} \right) \left( \prod_{j=0}^{m-1} x_{0, i+1+j}^{\binom{m-1}{j} / 2^{m-1}} \right) \right)^{1/2}$
Let $k=j+1$ in the second product.
$x_{m,i} = \left( \left( \prod_{j=0}^{m-1} x_{0, i+j}^{\binom{m-1}{j} / 2^{m-1}} \right) \left( \prod_{k=1}^{m} x_{0, i+k}^{\binom{m-1}{k-1} / 2^{m-1}} \right) \right)^{1/2}$
$x_{m,i} = \left( x_{0,i}^{\binom{m-1}{0}/2^{m-1}} \left( \prod_{j=1}^{m-1} x_{0, i+j}^{\binom{m-1}{j} / 2^{m-1}} \right) \left( \prod_{k=1}^{m-1} x_{0, i+k}^{\binom{m-1}{k-1} / 2^{m-1}} \right) x_{0, i+m}^{\binom{m-1}{m-1}/2^{m-1}} \right)^{1/2}$
Combining terms with the same base $x_{0,i+j}$ (for $j=k$):
$x_{m,i} = \left( x_{0,i}^{\binom{m-1}{0}/2^{m-1}} \left( \prod_{j=1}^{m-1} x_{0, i+j}^{(\binom{m-1}{j} + \binom{m-1}{j-1}) / 2^{m-1}} \right) x_{0, i+m}^{\binom{m-1}{m-1}/2^{m-1}} \right)^{1/2}$
Using Pascal's identity $\binom{n}{k} + \binom{n}{k-1} = \binom{n+1}{k}$, we have $\binom{m-1}{j} + \binom{m-1}{j-1} = \binom{m}{j}$.
Also $\binom{m-1}{0} = 1 = \binom{m}{0}$ and $\binom{m-1}{m-1} = 1 = \binom{m}{m}$.
$x_{m,i} = \left( x_{0,i}^{\binom{m}{0}/2^{m-1}} \left( \prod_{j=1}^{m-1} x_{0, i+j}^{\binom{m}{j} / 2^{m-1}} \right) x_{0, i+m}^{\binom{m}{m}/2^{m-1}} \right)^{1/2}$
$x_{m,i} = \left( \prod_{j=0}^{m} x_{0, i+j}^{\binom{m}{j} / 2^{m-1}} \right)^{1/2} = \prod_{j=0}^{m} x_{0, i+j}^{\binom{m}{j} / 2^m}$.
This completes the induction step.

The final result $R$ is $x_{n-1, 1}$. We set $m=n-1$ and $i=1$.
$R = \prod_{j=0}^{n-1} x_{0, 1+j}^{\binom{n-1}{j} / 2^{n-1}}$.
The initial sequence is $x_{0,k} = k$. So $x_{0, 1+j} = 1+j$.
$R = \prod_{j=0}^{n-1} (1+j)^{\binom{n-1}{j} / 2^{n-1}}$.
Let $k = j+1$. As $j$ goes from $0$ to $n-1$, $k$ goes from $1$ to $n$.
$R = \prod_{k=1}^{n} k^{\binom{n-1}{k-1} / 2^{n-1}}$.

This expression is a weighted geometric mean of the numbers $1, 2, \ldots, n$.
Let the weights be $w_k = \frac{\binom{n-1}{k-1}}{2^{n-1}}$ for $k=1, \ldots, n$.
The weights are positive since $\binom{n-1}{k-1} \ge 1$ for $0 \le k-1 \le n-1$.
The sum of the weights is:
$\sum_{k=1}^{n} w_k = \sum_{k=1}^{n} \frac{\binom{n-1}{k-1}}{2^{n-1}} = \frac{1}{2^{n-1}} \sum_{j=0}^{n-1} \binom{n-1}{j}$ (substituting $j=k-1$).
By the binomial theorem, $\sum_{j=0}^{n-1} \binom{n-1}{j} = (1+1)^{n-1} = 2^{n-1}$.
So $\sum_{k=1}^{n} w_k = \frac{1}{2^{n-1}} \times 2^{n-1} = 1$.

The weighted Arithmetic Mean - Geometric Mean (AM-GM) inequality states that for any set of positive numbers $x_1, \ldots, x_n$ and non-negative weights $w_1, \ldots, w_n$ such that $\sum_{k=1}^n w_k = 1$, we have:
$\prod_{k=1}^n x_k^{w_k} \le \sum_{k=1}^n w_k x_k$.
Equality holds if and only if $x_1 = x_2 = \ldots = x_n$.

In our case, $x_k = k$. The weighted geometric mean is $R = \prod_{k=1}^{n} k^{w_k}$.
The weighted arithmetic mean is $A = \sum_{k=1}^{n} w_k k = \sum_{k=1}^{n} \frac{\binom{n-1}{k-1}}{2^{n-1}} k$.
Let's calculate the sum $A$.
$A = \frac{1}{2^{n-1}} \sum_{k=1}^{n} k \binom{n-1}{k-1}$.
Using the identity $k \binom{n-1}{k-1} = (k-1+1) \binom{n-1}{k-1} = (k-1)\binom{n-1}{k-1} + \binom{n-1}{k-1}$.
Let $j=k-1$.
$A = \frac{1}{2^{n-1}} \sum_{j=0}^{n-1} (j+1) \binom{n-1}{j} = \frac{1}{2^{n-1}} \left( \sum_{j=0}^{n-1} j \binom{n-1}{j} + \sum_{j=0}^{n-1} \binom{n-1}{j} \right)$.
The second sum is $2^{n-1}$.
For the first sum, we use the identity $j \binom{n-1}{j} = (n-1) \binom{n-2}{j-1}$ for $j \ge 1$. The term for $j=0$ is $0$.
$\sum_{j=1}^{n-1} j \binom{n-1}{j} = \sum_{j=1}^{n-1} (n-1) \binom{n-2}{j-1}$.
This identity requires $n-1 \ge 1$, so $n \ge 2$. Let's assume $n \ge 2$.
Let $l = j-1$. As $j$ goes from $1$ to $n-1$, $l$ goes from $0$ to $n-2$.
$\sum_{l=0}^{n-2} (n-1) \binom{n-2}{l} = (n-1) \sum_{l=0}^{n-2} \binom{n-2}{l} = (n-1) 2^{n-2}$. This holds for $n-2 \ge 0$, i.e. $n \ge 2$.
So, for $n \ge 2$:
$A = \frac{1}{2^{n-1}} \left( (n-1) 2^{n-2} + 2^{n-1} \right) = \frac{(n-1) 2^{n-2}}{2^{n-1}} + \frac{2^{n-1}}{2^{n-1}} = \frac{n-1}{2} + 1 = \frac{n+1}{2}$.

Applying the weighted AM-GM inequality: $R \le A$.
$R \le \frac{n+1}{2}$.
The equality holds if and only if all the numbers $k$ are equal, i.e., $1 = 2 = \ldots = n$. This condition holds only for $n=1$.
If $n=1$, the initial sequence is (1). There are $n-1=0$ actions. The result is $R=1$. And $\frac{n+1}{2} = \frac{1+1}{2} = 1$. So $R = \frac{n+1}{2}$ for $n=1$.
However, the problem statement implies $n \ge 2$. It mentions transforming the sequence into a "shorter sequence", which requires the initial length $n$ to be at least 2. Also, it says $(n-1)$ actions are performed. If $n=1$, $0$ actions are performed.
Assuming $n \ge 2$, the numbers $1, 2, \ldots, n$ are not all equal.
Therefore, the inequality in the weighted AM-GM must be strict for $n \ge 2$.
$R < A = \frac{n+1}{2}$.

Thus, for the sequence $(1, 2, \ldots, n)$ with $n \ge 2$, the result $R$ is strictly smaller than $\frac{n+1}{2}$.

Final conclusion:
The result of the process is $R = \prod_{k=1}^{n} k^{\binom{n-1}{k-1} / 2^{n-1}}$.
By the weighted AM-GM inequality, $R \le \sum_{k=1}^{n} \frac{\binom{n-1}{k-1}}{2^{n-1}} k$.
We calculated the weighted sum to be $\frac{n+1}{2}$.
So, $R \le \frac{n+1}{2}$.
Equality holds if and only if $1=2=\ldots=n$, which means $n=1$.
Since the problem description implies $n \ge 2$, the numbers $1, 2, \ldots, n$ are not all equal, and the inequality is strict.
Therefore, $R < \frac{n+1}{2}$.

```markdown
Let the initial sequence be $S_0 = (x_{0,1}, x_{0,2}, \ldots, x_{0,n})$. According to the problem statement, $x_{0,k} = k$ for $k=1, 2, \ldots, n$.
The sequence is transformed iteratively. Let $S_m = (x_{m,1}, x_{m,2}, \ldots, x_{m, n-m})$ be the sequence after $m$ actions. The transformation rule is given by $x_{m,i} = \sqrt{x_{m-1,i} x_{m-1,i+1}}$ for $m \ge 1$ and $1 \le i \le n-m$.
The process continues for $n-1$ actions, resulting in a single number $R = x_{n-1, 1}$.

We can express the elements of the sequence $S_m$ in terms of the initial sequence $S_0$. It can be shown by induction that
$$x_{m,i} = \prod_{j=0}^m x_{0, i+j}^{\binom{m}{j} / 2^m}$$
The final result $R$ is obtained by setting $m=n-1$ and $i=1$:
$$R = x_{n-1, 1} = \prod_{j=0}^{n-1} x_{0, 1+j}^{\binom{n-1}{j} / 2^{n-1}}$$
Since $x_{0,k} = k$, we have $x_{0, 1+j} = 1+j$. Let $k = j+1$. As $j$ ranges from $0$ to $n-1$, $k$ ranges from $1$ to $n$.
$$R = \prod_{k=1}^{n} k^{\binom{n-1}{k-1} / 2^{n-1}}$$
This expression is a weighted geometric mean of the numbers $(1, 2, \ldots, n)$. Let the weights be $w_k = \frac{\binom{n-1}{k-1}}{2^{n-1}}$ for $k=1, \ldots, n$.
The weights are positive and sum to 1:
$$ \sum_{k=1}^{n} w_k = \sum_{k=1}^{n} \frac{\binom{n-1}{k-1}}{2^{n-1}} = \frac{1}{2^{n-1}} \sum_{j=0}^{n-1} \binom{n-1}{j} = \frac{1}{2^{n-1}} 2^{n-1} = 1 $$
Here we substituted $j=k-1$.

By the weighted Arithmetic Mean - Geometric Mean (AM-GM) inequality, for positive numbers $x_1, \ldots, x_n$ and non-negative weights $w_1, \ldots, w_n$ summing to 1, we have:
$$ \prod_{k=1}^n x_k^{w_k} \le \sum_{k=1}^n w_k x_k $$
Equality holds if and only if $x_1 = x_2 = \ldots = x_n$.

In our case, $x_k = k$. The weighted geometric mean is $R$. The weighted arithmetic mean is $A = \sum_{k=1}^{n} w_k k$.
$$ A = \sum_{k=1}^{n} \frac{\binom{n-1}{k-1}}{2^{n-1}} k $$
Let's compute this sum. Substitute $j=k-1$:
$$ A = \frac{1}{2^{n-1}} \sum_{j=0}^{n-1} \binom{n-1}{j} (j+1) = \frac{1}{2^{n-1}} \left( \sum_{j=0}^{n-1} j \binom{n-1}{j} + \sum_{j=0}^{n-1} \binom{n-1}{j} \right) $$
The second sum is $2^{n-1}$. For the first sum, we use the identity $j \binom{n-1}{j} = (n-1) \binom{n-2}{j-1}$ for $j \ge 1$ (and the term is 0 for $j=0$). This identity assumes $n-1 \ge 1$, so $n \ge 2$.
$$ \sum_{j=1}^{n-1} j \binom{n-1}{j} = \sum_{j=1}^{n-1} (n-1) \binom{n-2}{j-1} = (n-1) \sum_{l=0}^{n-2} \binom{n-2}{l} = (n-1) 2^{n-2} $$
where we substituted $l=j-1$. This calculation is valid for $n \ge 2$.
So, for $n \ge 2$:
$$ A = \frac{1}{2^{n-1}} \left( (n-1) 2^{n-2} + 2^{n-1} \right) = \frac{(n-1)2^{n-2}}{2^{n-1}} + \frac{2^{n-1}}{2^{n-1}} = \frac{n-1}{2} + 1 = \frac{n+1}{2} $$
By the weighted AM-GM inequality, $R \le A$, so $R \le \frac{n+1}{2}$.
The equality case holds if and only if $1 = 2 = \ldots = n$, which is true only for $n=1$.
The problem statement implies $n \ge 2$, as it refers to transforming the sequence into a "shorter sequence" and performing $n-1$ actions. For $n=1$, the sequence length is 1, and $n-1=0$ actions are performed.
Thus, we can assume $n \ge 2$. In this case, the numbers $1, 2, \ldots, n$ are not all equal.
Therefore, the inequality is strict:
$$ R < \frac{n+1}{2} $$

This completes the proof.
```