

To solve the problem, we utilize the given properties of the finite ring \( R \).

**Step 1:** Expand \( (a + b)^3 \) for \( a, b \in R \):
\[
(a + b)^3 = a^3 + a^2b + aba + ab^2 + ba^2 + bab + b^2a + b^3.
\]

**Step 2:** Apply the second property when \( a \neq b \):
- For \( a \neq b \), \( a^2b = -ba^2 \) and \( ab^2 = -b^2a \), leading to cancellations:
\[
a^2b + ba^2 = 0 \quad \text{and} \quad ab^2 + b^2a = 0.
\]
Thus, the expansion simplifies to:
\[
(a + b)^3 = a^3 + b^3 + aba + bab.
\]

**Step 3:** By the first property, there exists \( c \in R \) such that \( a^3 + b^3 = c^3 \). Substitute:
\[
(a + b)^3 = c^3 + aba + bab \implies aba + bab = (a + b)^3 - c^3.
\]

**Step 4:** Express \( (a + b)^3 - c^3 \) as a sum of cubes:
- \( (a + b)^3 \) is the cube of \( a + b \).
- \( -c^3 = (-c)^3 \), so the difference is a sum of two cubes:
\[
(a + b)^3 + (-c)^3.
\]

**Step 5:** By the first property again, there exists \( d \in R \) such that:
\[
(a + b)^3 + (-c)^3 = d^3 \implies aba + bab = d^3.
\]

**Case \( a = b \):** Directly apply the first property:
\[
aba + bab = 2a^3 = a^3 + a^3 = d^3 \quad \text{for some } d \in R.
\]

Thus, for all \( a, b \in R \), there exists \( d \in R \) with \( aba + bab = d^3 \).

```markdown
**Final Answer**
\boxed{aba + bab = d^3 \text{ for some } d \in R}
```