# Solution

Given a square matrix $M$ of dimension 3 with eigenvalue $1$ whose algebraic multiplicity is $3$, we need to find coefficients $a_m$, $b_m$, and $c_m$ such that
$$M^m = a_m M^2 + b_m M + c_m I_3$$
for $m \geq 3$.

Since the eigenvalue $1$ has algebraic multiplicity $3$, the characteristic polynomial of $M$ is $(x-1)^3$. By the Cayley-Hamilton theorem, $M$ satisfies its own characteristic polynomial, meaning:
$$(M-I_3)^3 = 0$$

Expanding this:
$$M^3 - 3M^2 + 3M - I_3 = 0$$

Which gives us:
$$M^3 = 3M^2 - 3M + I_3$$

To find a general formula for $M^m$, I'll use the fact that if we define $N = M - I_3$, then $N^3 = 0$. Since $M = N + I_3$, we can use the binomial theorem:

$$M^m = (N + I_3)^m = \sum_{k=0}^m \binom{m}{k} N^k$$

Since $N^3 = 0$, only terms with $k = 0, 1, 2$ survive:

$$M^m = \binom{m}{0}N^0 + \binom{m}{1}N^1 + \binom{m}{2}N^2 = I_3 + mN + \binom{m}{2}N^2$$

Now, we need to express this in terms of $M$ and $I_3$. Using $N = M - I_3$:
$$N^2 = (M - I_3)^2 = M^2 - 2M + I_3$$

Substituting:
\begin{align}
M^m &= I_3 + m(M - I_3) + \binom{m}{2}(M^2 - 2M + I_3) \\
&= I_3 + mM - mI_3 + \binom{m}{2}M^2 - 2\binom{m}{2}M + \binom{m}{2}I_3 \\
&= \binom{m}{2}M^2 + (m - 2\binom{m}{2})M + (1 - m + \binom{m}{2})I_3
\end{align}

Therefore:
\begin{align}
a_m &= \binom{m}{2} = \frac{m(m-1)}{2} \\
b_m &= m - 2\binom{m}{2} = m - m(m-1) = 2m - m^2 = -m(m-2) \\
c_m &= 1 - m + \binom{m}{2} = 1 - m + \frac{m(m-1)}{2} = \frac{(m-1)(m-2)}{2}
\end{align}

## Answer
For $m \geq 3$:
$$a_m = \frac{m(m-1)}{2}$$
$$b_m = -m(m-2)$$
$$c_m = \frac{(m-1)(m-2)}{2}$$