This is a detailed step-by-step solution to the problem.

### Step 1: Parameterization and Tangent Lines

Let the points $P$ and $Q$ on the hyperbola $\mathcal{H}$ be parameterized by their x-coordinates, $p$ and $q$. Since they are on the positive branch, we have $p, q > 0$. The condition $P \neq Q$ implies $p \neq q$.
The coordinates of the points are:
$$ P = \left(p, \frac{1}{p}\right), \quad Q = \left(q, \frac{1}{q}\right) $$
The function defining the hyperbola is $f(x) = 1/x$. Its derivative is $f'(x) = -1/x^2$.

The tangent line $k$ at point $P$ has a slope $m_k = f'(p) = -1/p^2$. The equation of line $k$ is given by the point-slope form $y - y_0 = m(x - x_0)$:
$$ y - \frac{1}{p} = -\frac{1}{p^2}(x - p) $$
Multiplying by $p^2$, we get:
$$ p^2y - p = -x + p \implies x + p^2y = 2p $$
Similarly, the equation for the tangent line $l$ at point $Q$ is:
$$ x + q^2y = 2q $$

### Step 2: Finding the Intersection Point R

The point $R(x_R, y_R)$ is the intersection of lines $k$ and $l$. We solve the system of linear equations:
1.  $x_R + p^2y_R = 2p$
2.  $x_R + q^2y_R = 2q$

Subtracting the second equation from the first gives:
$$ (p^2 - q^2)y_R = 2(p - q) $$
Since $P \neq Q$, we have $p \neq q$, so $p-q \neq 0$. Also, since $p,q > 0$, $p+q \neq 0$.
$$ (p-q)(p+q)y_R = 2(p-q) \implies y_R = \frac{2}{p+q} $$
Substituting $y_R$ back into the first equation:
$$ x_R = 2p - p^2y_R = 2p - p^2\left(\frac{2}{p+q}\right) = \frac{2p(p+q) - 2p^2}{p+q} = \frac{2p^2 + 2pq - 2p^2}{p+q} = \frac{2pq}{p+q} $$
So, the coordinates of the intersection point $R$ are:
$$ R = \left(\frac{2pq}{p+q}, \frac{2}{p+q}\right) $$

### Step 3: Calculating the Circumradius of Triangle PQR

The radius $r$ of the circumcircle of a triangle can be calculated using the formula $r = \frac{a}{2\sin A}$, where $a$ is one of the side lengths and $A$ is the opposite angle. Let's use the side $PQ$ and the angle $\angle PRQ$.

The square of the distance between $P$ and $Q$ is:
$$ d_{PQ}^2 = (p-q)^2 + \left(\frac{1}{p} - \frac{1}{q}\right)^2 = (p-q)^2 + \left(\frac{q-p}{pq}\right)^2 = (p-q)^2\left(1 + \frac{1}{p^2q^2}\right) = \frac{(p-q)^2(p^2q^2+1)}{p^2q^2} $$
Taking the square root, $d_{PQ} = \frac{|p-q|\sqrt{p^2q^2+1}}{pq}$ (since $p,q > 0$).

The angle $\theta_R = \angle PRQ$ is the angle between the tangent lines $k$ and $l$. The angle $\alpha$ between two lines with slopes $m_k$ and $m_l$ is given by $\tan \alpha = \left|\frac{m_k - m_l}{1+m_k m_l}\right|$.
Here, $m_k = -1/p^2$ and $m_l = -1/q^2$.
$$ \tan(\theta_R) = \left|\frac{-1/p^2 - (-1/q^2)}{1 + (-1/p^2)(-1/q^2)}\right| = \left|\frac{1/q^2 - 1/p^2}{1 + 1/(p^2q^2)}\right| = \left|\frac{(p^2-q^2)/(p^2q^2)}{(p^2q^2+1)/(p^2q^2)}\right| = \frac{|p^2-q^2|}{p^2q^2+1} $$
We need $\sin(\theta_R)$. Using the identity $\sin\alpha = \frac{\tan\alpha}{\sqrt{1+\tan^2\alpha}}$ for $\alpha \in [0, \pi/2)$ (the angle in a triangle is in $(0,\pi)$, but its tan could be negative, however the formula with absolute values gives the smaller angle between lines, so $\tan \theta_R > 0$):
$$ \sin(\theta_R) = \frac{\frac{|p^2-q^2|}{p^2q^2+1}}{\sqrt{1 + \frac{(p^2-q^2)^2}{(p^2q^2+1)^2}}} = \frac{|p^2-q^2|}{\sqrt{(p^2q^2+1)^2 + (p^2-q^2)^2}} $$
The term under the square root in the denominator is:
$$ (p^4q^4 + 2p^2q^2 + 1) + (p^4 - 2p^2q^2 + q^4) = p^4q^4 + p^4 + q^4 + 1 = (p^4+1)(q^4+1) $$
So, $\sin(\theta_R) = \frac{|p^2-q^2|}{\sqrt{(p^4+1)(q^4+1)}} = \frac{|p-q|(p+q)}{\sqrt{(p^4+1)(q^4+1)}}$ since $p,q > 0$.

Now we can compute the circumradius $r(P,Q)$:
$$ r(P,Q) = \frac{d_{PQ}}{2\sin(\theta_R)} = \frac{\frac{|p-q|\sqrt{p^2q^2+1}}{pq}}{2 \frac{|p-q|(p+q)}{\sqrt{(p^4+1)(q^4+1)}}} = \frac{\sqrt{p^2q^2+1}\sqrt{(p^4+1)(q^4+1)}}{2pq(p+q)} $$

### Step 4: Minimizing the Circumradius

The expression for $r(P,Q)$ is complex. To simplify, we perform a change of variables. Let $p=e^x$ and $q=e^y$ for some $x,y \in \mathbb{R}$. The condition $p \neq q$ means $x \neq y$.
Let's express $r^2$ in terms of $x$ and $y$:
$$ r^2(p,q) = \frac{(p^2q^2+1)(p^4+1)(q^4+1)}{4p^2q^2(p+q)^2} $$
Substitute $p=e^x, q=e^y$:
*   $p^2q^2+1 = e^{2(x+y)}+1 = e^{x+y}(e^{x+y}+e^{-(x+y)}) = 2e^{x+y}\cosh(x+y)$
*   $p^4+1 = e^{4x}+1 = e^{2x}(e^{2x}+e^{-2x}) = 2e^{2x}\cosh(2x)$
*   $q^4+1 = e^{4y}+1 = e^{2y}(e^{2y}+e^{-2y}) = 2e^{2y}\cosh(2y)$
*   $4p^2q^2 = 4e^{2(x+y)}$
*   $(p+q)^2 = (e^x+e^y)^2 = \left(e^{\frac{x+y}{2}}(e^{\frac{x-y}{2}}+e^{-\frac{x-y}{2}})\right)^2 = e^{x+y}(2\cosh(\frac{x-y}{2}))^2 = 4e^{x+y}\cosh^2\left(\frac{x-y}{2}\right)$

Substitute these into the expression for $r^2$:
$$ r^2(x,y) = \frac{(2e^{x+y}\cosh(x+y))(2e^{2x}\cosh(2x))(2e^{2y}\cosh(2y))}{(4e^{2(x+y)})(4e^{x+y}\cosh^2(\frac{x-y}{2}))} $$
$$ r^2(x,y) = \frac{8 e^{3x+3y} \cosh(x+y)\cosh(2x)\cosh(2y)}{16 e^{3x+3y} \cosh^2(\frac{x-y}{2})} = \frac{\cosh(x+y)\cosh(2x)\cosh(2y)}{2\cosh^2(\frac{x-y}{2})} $$
To minimize this expression, we use another change of variables: $u = x+y$ and $v = x-y$.
Then $x = (u+v)/2$ and $y = (u-v)/2$. Note that $x \neq y$ implies $v \neq 0$.
$$ r^2(u,v) = \frac{\cosh(u)\cosh(u+v)\cosh(u-v)}{2\cosh^2(v/2)} $$
Using the identity $\cosh(A+B)\cosh(A-B) = \frac{\cosh(2A)+\cosh(2B)}{2}$, we have:
$$ \cosh(u+v)\cosh(u-v) = \frac{\cosh(2u)+\cosh(2v)}{2} $$
So the expression for $r^2$ becomes:
$$ r^2(u,v) = \frac{\cosh(u)(\cosh(2u)+\cosh(2v))}{4\cosh^2(v/2)} $$
Let's fix $v \neq 0$ and minimize with respect to $u$. Let $g(u) = \cosh(u)(\cosh(2u)+\cosh(2v))$.
To find the minimum of $g(u)$, we can analyze its derivative:
$$ g'(u) = \sinh(u)(\cosh(2u)+\cosh(2v)) + \cosh(u)(2\sinh(2u)) $$
Using $\sinh(2u) = 2\sinh(u)\cosh(u)$:
$$ g'(u) = \sinh(u)\cosh(2u) + \sinh(u)\cosh(2v) + 4\sinh(u)\cosh^2(u) $$
$$ g'(u) = \sinh(u)[\cosh(2u) + \cosh(2v) + 4\cosh^2(u)] $$
Since $v \neq 0$, $\cosh(2v)>1$. Also $\cosh(2u) \ge 1$ and $\cosh^2(u) \ge 1$. The term in the square brackets is always positive.
Therefore, the sign of $g'(u)$ is determined by the sign of $\sinh(u)$.
$g'(u) < 0$ for $u < 0$, $g'(u) = 0$ for $u=0$, and $g'(u) > 0$ for $u > 0$.
This shows that $g(u)$ has a unique global minimum at $u=0$.

The minimum value for a fixed $v$ is obtained when $u=0$. This corresponds to $x+y=0$, which means $y=-x$. In terms of $p$ and $q$, this is $\ln q = -\ln p = \ln(1/p)$, so $q=1/p$. This represents a symmetric configuration of points $P,Q$ with respect to the line $y=x$.

Let's evaluate $r^2$ at $u=0$:
$$ r^2(0,v) = \frac{\cosh(0)(\cosh(0)+\cosh(2v))}{4\cosh^2(v/2)} = \frac{1+\cosh(2v)}{4\cosh^2(v/2)} $$
Using the identity $1+\cosh(2A) = 2\cosh^2(A)$:
$$ r^2(0,v) = \frac{2\cosh^2(v)}{4\cosh^2(v/2)} = \frac{\cosh^2(v)}{2\cosh^2(v/2)} $$
Let $w = \cosh(v/2)$. Since $v\neq 0$, we have $v/2 \neq 0$, so $w = \cosh(v/2) > 1$.
Using the identity $\cosh(v) = 2\cosh^2(v/2) - 1 = 2w^2-1$:
$$ r^2 = \frac{(2w^2-1)^2}{2w^2} $$
We want to find the infimum of this expression for $w \in (1, \infty)$. Let $F(w) = \frac{(2w^2-1)^2}{2w^2}$.
$$ F(w) = \frac{4w^4-4w^2+1}{2w^2} = 2w^2 - 2 + \frac{1}{2w^2} $$
To find the minimum, we can check its derivative:
$$ F'(w) = 4w - \frac{1}{w^3} = \frac{4w^4-1}{w^3} $$
For $w>1$, $4w^4-1 > 4-1 = 3 > 0$, so $F'(w)>0$.
The function $F(w)$ is strictly increasing for $w>1$.
The infimum is therefore the limit as $w$ approaches the lower bound of its domain, i.e., $w \to 1^+$.
$$ \inf_{w>1} F(w) = \lim_{w\to 1^+} \frac{(2w^2-1)^2}{2w^2} = \frac{(2(1)^2-1)^2}{2(1)^2} = \frac{1^2}{2} = \frac{1}{2} $$
This is the infimum of $r^2(P,Q)$.
The infimum of the radius $r(P,Q)$ is the square root of this value:
$$ \inf_{P,Q} r(P,Q) = \sqrt{\frac{1}{2}} = \frac{1}{\sqrt{2}} = \frac{\sqrt{2}}{2} $$
This infimum is approached as the two points $P$ and $Q$ approach each other in a symmetric configuration, i.e., $P=(p, 1/p)$ and $Q=(1/p, p)$ with $p \to 1$. Note that for any finite choice of $P,Q$ with $P\neq Q$, the radius $r(P,Q)$ is strictly greater than $1/\sqrt{2}$.