# Solution

I'll work through this problem by finding an explicit formula for $p(x)$ and then evaluating it at $x = k-1$.

## Step 1: Establish a recursive relation for the derivatives.

Let's consider the identity $(x^k+1) \cdot f(x) = 1$, which holds given that $f(x) = \frac{1}{x^k+1}$.

Taking the derivative of both sides using the product rule:
$$(x^k+1) \cdot f'(x) + kx^{k-1} \cdot f(x) = 0$$

Rearranging:
$$f'(x) = -\frac{kx^{k-1} \cdot f(x)}{x^k+1}$$

For higher derivatives, we can generalize this. For any $n \geq 1$:
$$(x^k+1) \cdot f^{(n)}(x) + nkx^{k-1} \cdot f^{(n-1)}(x) = 0$$

This gives us:
$$f^{(n)}(x) = -\frac{nkx^{k-1} \cdot f^{(n-1)}(x)}{x^k+1}$$

## Step 2: Define and find a formula for an auxiliary function.

Let's define $g_n(x) = (x^k+1)^n \cdot f^{(n)}(x)$.

Using our recursive relation:
$$g_n(x) = (x^k+1)^n \cdot f^{(n)}(x) = (x^k+1)^n \cdot \left(-\frac{nkx^{k-1} \cdot f^{(n-1)}(x)}{x^k+1}\right)$$

Simplifying:
$$g_n(x) = -nkx^{k-1} \cdot (x^k+1)^{n-1} \cdot f^{(n-1)}(x) = -nkx^{k-1} \cdot g_{n-1}(x)$$

Starting with $g_0(x) = (x^k+1)^0 \cdot f^{(0)}(x) = f(x) = \frac{1}{x^k+1}$, we can compute:

$g_1(x) = -kx^{k-1} \cdot g_0(x) = -kx^{k-1} \cdot \frac{1}{x^k+1}$

$g_2(x) = -2kx^{k-1} \cdot g_1(x) = -2kx^{k-1} \cdot \left(-kx^{k-1} \cdot \frac{1}{x^k+1}\right) = 2k^2x^{2(k-1)} \cdot \frac{1}{x^k+1}$

Continuing this pattern and proving by induction, we get:
$$g_n(x) = (-1)^n \cdot n! \cdot k^n \cdot x^{n(k-1)} \cdot \frac{1}{x^k+1}$$

## Step 3: Calculate $p(x)$ and evaluate at $x = k-1$.

From the problem statement, we have:
$$p(x) = (x^k+1)^{n+1} \cdot f^{(n)}(x)$$

Using our formula for $g_n(x)$:
$$p(x) = (x^k+1) \cdot g_n(x) = (x^k+1) \cdot \left((-1)^n \cdot n! \cdot k^n \cdot x^{n(k-1)} \cdot \frac{1}{x^k+1}\right)$$

Simplifying:
$$p(x) = (-1)^n \cdot n! \cdot k^n \cdot x^{n(k-1)}$$

Evaluating at $x = k-1$:
$$p(k-1) = (-1)^n \cdot n! \cdot k^n \cdot (k-1)^{n(k-1)}$$

## Step 4: Prove the claims.

1. Is $p(k-1) \in \mathbb{Z}$?  
   Yes, because $p(k-1)$ is the product of integers: $(-1)^n$, $n!$, $k^n$, and $(k-1)^{n(k-1)}$ are all integers.

2. Does $k | p(k-1)$?  
   Yes, because $p(k-1)$ has a factor of $k^n$, and since $n \geq 1$ (given in the problem), there's at least one factor of $k$ in $p(k-1)$.

Therefore, we've shown that $p(k-1) \in \mathbb{Z}$ and $k | p(k-1)$.