Let us look at the first equation. Bringing everything to the left side, we get $(y-x+1)(y-x^2) = 0$. This means that $y=x-1$ or $y=x^2$. Analogously, $z = y-1$ or $z=y^2$ and $x=z-1$ or $x=z^2$. Of course it is not possible that the first equation holds in all three cases. Therefore we have three possibilities: the first one holds in zero cases, one case, or two cases.
 
 For the first one, we have $y = x^2$, $z=y^2$, $x=z^2$. This means that $x^8 = x$. Hence $x = 0$ or $x=1$. This gives two solutions of the system: $(0,0,0)$ and $(1,1,1)$.
 
 Now in the second case, without lose of generality we can assume $y=x^2$, $z=y^2$, $x=z-1$. This means that $x^4-1 = x$. A simple reasoning shows that such equation has two irrational solutions $x_1$ and $x_2$. This then gives solutions $(x_1,x_1^2,x_1^4)$ and $(x_2,x_2^2,x_2^4)$, with cyclic permutations there are 6 of them (they are clearly pairwise distinct).
 
 Now assume the third situation. Without lose of generality we have $y=x-1$,$z=y-1$, $x=z^2$. This means that $x = (x-2)^2$. Equivalently
 $$0 = x^2-5x+4 = (x-4)(x-1).$$
 Hence we have $x=4$ or $x=1$. This gives triples $(4,3,2)$ and $(1,0,-1)$. With cyclic permutations, we get 6 solutions.
 
 Therefore in total we have $14$ solutions.