Solution:

Let $N = a^{2^k} + b^{2^k}$. We are given that $p$ is a prime divisor of $N$ with $p>2$. We are also given that $k, a, b$ are positive integers with $\gcd(a,b)=1$. We want to show that $p$ must be of the form $p=2^{d}m+1$, where $d \geq k+1$ and $m$ is an odd positive integer.

Since $p$ is a prime divisor of $N$, we have $a^{2^k} + b^{2^k} \equiv 0 \pmod{p}$.

First, we show that $p$ does not divide $a$ and $p$ does not divide $b$.
Assume $p|a$. Since $a^{2^k} + b^{2^k} \equiv 0 \pmod{p}$, this implies $0 + b^{2^k} \equiv 0 \pmod{p}$, so $p | b^{2^k}$. Since $p$ is prime, $p|b$. However, $p|a$ and $p|b$ contradicts the given condition $\gcd(a,b)=1$. Thus, $p \nmid a$.
Similarly, assume $p|b$. Then $b^{2^k} \equiv 0 \pmod{p}$. The congruence $a^{2^k} + b^{2^k} \equiv 0 \pmod{p}$ implies $a^{2^k} + 0 \equiv 0 \pmod{p}$, so $p | a^{2^k}$. Since $p$ is prime, $p|a$. This again contradicts $\gcd(a,b)=1$. Thus, $p \nmid b$.

Since $p \nmid b$, $b$ has a multiplicative inverse modulo $p$. Let $b^{-1}$ denote this inverse, i.e., $b b^{-1} \equiv 1 \pmod{p}$.
Multiply the congruence $a^{2^k} + b^{2^k} \equiv 0 \pmod{p}$ by $(b^{-1})^{2^k}$:
$a^{2^k} (b^{-1})^{2^k} + b^{2^k} (b^{-1})^{2^k} \equiv 0 \pmod{p}$
$(a b^{-1})^{2^k} + (b b^{-1})^{2^k} \equiv 0 \pmod{p}$
$(a b^{-1})^{2^k} + 1^{2^k} \equiv 0 \pmod{p}$
Let $x = a b^{-1} \pmod{p}$. Since $p \nmid a$ and $p \nmid b$, $x$ is well-defined and $x \not\equiv 0 \pmod{p}$. The congruence becomes:
$x^{2^k} + 1 \equiv 0 \pmod{p}$
$x^{2^k} \equiv -1 \pmod{p}$

Now, let's determine the order of $x$ modulo $p$. Let $h = \text{ord}_p(x)$ be the smallest positive integer such that $x^h \equiv 1 \pmod{p}$.
From $x^{2^k} \equiv -1 \pmod{p}$, we know that $x^{2^k} \not\equiv 1 \pmod{p}$ because $p>2$, so $-1 \not\equiv 1 \pmod{p}$.
This implies that the order $h$ cannot divide $2^k$.

Squaring both sides of $x^{2^k} \equiv -1 \pmod{p}$:
$(x^{2^k})^2 \equiv (-1)^2 \pmod{p}$
$x^{2^k \cdot 2} \equiv 1 \pmod{p}$
$x^{2^{k+1}} \equiv 1 \pmod{p}$
This implies that the order $h$ must divide $2^{k+1}$.

So, $h$ must be a divisor of $2^{k+1}$, and $h$ must not be a divisor of $2^k$.
The divisors of $2^{k+1}$ are $1, 2, 2^2, \dots, 2^k, 2^{k+1}$.
The divisors of $2^k$ are $1, 2, 2^2, \dots, 2^k$.
The only divisor of $2^{k+1}$ that is not a divisor of $2^k$ is $2^{k+1}$.
Therefore, the order of $x$ modulo $p$ must be $h = 2^{k+1}$.

By Lagrange's theorem, the order of any element in a finite group divides the order of the group. Here, $x$ is an element of the multiplicative group $(\mathbb{Z}/p\mathbb{Z})^\times$, which has order $\phi(p) = p-1$.
Thus, the order of $x$, which is $2^{k+1}$, must divide $p-1$.
So, $p-1$ is a multiple of $2^{k+1}$. We can write this as:
$p-1 = c \cdot 2^{k+1}$ for some positive integer $c$.
This means $p = c \cdot 2^{k+1} + 1$.

We need to express $p$ in the form $p=2^d m + 1$ where $d \geq k+1$ and $m$ is an odd positive integer.
Any positive integer $c$ can be uniquely written as $c = 2^j m$, where $m$ is an odd positive integer and $j \geq 0$ is an integer.
Substituting this into the expression for $p$:
$p = (2^j m) \cdot 2^{k+1} + 1$
$p = 2^{k+1+j} m + 1$

Let $d = k+1+j$.
Since $j \geq 0$, we have $d = k+1+j \geq k+1$.
The integer $m$ is an odd positive integer.
Thus, $p$ is of the form $p = 2^d m + 1$, where $d \geq k+1$ and $m$ is an odd positive integer.

This completes the proof.

Final Answer: The final answer is $\boxed{p=2^{d}m+1, \text{ where } d\geq k+1 \text{ and } m \text{ is an odd positive integer}}$