Here is a detailed, step-by-step solution to the problem.

### 1. Understanding the System of Equations

The given system of equations is:
$$
 \left\{
 \begin{array}{lll}
 x_1^2 &+ (1 - x_2 \ln x_2)^2 &= 2x_2 -2 x_3^2 \ln x_3, \\
 x_2^2 &+ (1 - x_3 \ln x_3)^2 &= 2x_3 -2 x_4^2 \ln x_4, \\
 & &\vdots \\
 x_{n-1}^2 &+ (1 - x_{n} \ln x_{n})^2 &= 2x_n -2 x_1^2 \ln x_1, \\
 x_{n}^2 &+ (1 - x_{1} \ln x_{1})^2 &= 2x_1 -2 x_2^2 \ln x_2.
 \end{array} 
 \right.
$$
The variables $x_i$ are all positive real numbers ($x_i > 0$), and $n \geq 3$. The system exhibits a cyclic structure. We can write the general $i$-th equation by taking the indices modulo $n$. For $i \in \{1, 2, \ldots, n\}$, the $i$-th equation is:
$$x_i^2 + (1 - x_{i+1} \ln x_{i+1})^2 = 2x_{i+1} - 2x_{i+2}^2 \ln x_{i+2}$$
where $x_{n+k}$ is understood as $x_k$.

### 2. Summing the Equations

A common strategy for systems with cyclic symmetry is to sum all the equations. Let's sum the $n$ equations:
$$ \sum_{i=1}^{n} \left[ x_i^2 + (1 - x_{i+1} \ln x_{i+1})^2 \right] = \sum_{i=1}^{n} \left[ 2x_{i+1} - 2x_{i+2}^2 \ln x_{i+2} \right] $$
Due to the cyclic nature of the indices, the sum of a function of $x_{i+1}$ or $x_{i+2}$ over $i=1, \ldots, n$ is the same as the sum of that function of $x_i$.
For example, $\sum_{i=1}^{n} f(x_{i+1}) = f(x_2) + f(x_3) + \ldots + f(x_n) + f(x_1) = \sum_{i=1}^{n} f(x_i)$.
Applying this, we can re-index the summations to be over $x_i$:
$$ \sum_{i=1}^{n} x_i^2 + \sum_{i=1}^{n} (1 - x_i \ln x_i)^2 = \sum_{i=1}^{n} 2x_i - \sum_{i=1}^{n} 2x_i^2 \ln x_i $$

### 3. Rearranging the Sum to find a Condition on each $x_i$

Now, let's expand the terms and move everything to one side of the equation.
$$ \sum_{i=1}^{n} x_i^2 + \sum_{i=1}^{n} \left[1 - 2x_i \ln x_i + (x_i \ln x_i)^2\right] = \sum_{i=1}^{n} 2x_i - \sum_{i=1}^{n} 2x_i^2 \ln x_i $$
Combining these into a single summation:
$$ \sum_{i=1}^{n} \left[ x_i^2 + 1 - 2x_i \ln x_i + x_i^2(\ln x_i)^2 - 2x_i + 2x_i^2 \ln x_i \right] = 0 $$
Let's focus on the expression inside the summation for a single variable $x$:
$$ E(x) = x^2 - 2x + 1 - 2x \ln x + x^2(\ln x)^2 + 2x^2 \ln x $$
Our goal is to simplify this expression. Let's try to group the terms to form a perfect square.
$$ E(x) = (x^2 + 2x^2 \ln x + x^2(\ln x)^2) - (2x + 2x \ln x) + 1 $$
The first group of terms looks related to $(x + x \ln x)^2$. Let's check:
$$ (x + x \ln x)^2 = x^2 (1 + \ln x)^2 = x^2(1 + 2\ln x + (\ln x)^2) = x^2 + 2x^2 \ln x + x^2(\ln x)^2 $$
This matches the first parenthesis perfectly.
The second group is $-2x(1 + \ln x)$.
So, the expression becomes:
$$ E(x) = x^2(1 + \ln x)^2 - 2x(1 + \ln x) + 1 $$
This is a perfect square of the form $A^2 - 2A + 1 = (A-1)^2$, where $A = x(1 + \ln x)$.
$$ E(x) = [x(1 + \ln x) - 1]^2 = [x + x \ln x - 1]^2 $$
Substituting this back into our sum equation:
$$ \sum_{i=1}^{n} [x_i(1 + \ln x_i) - 1]^2 = 0 $$

### 4. Solving for $x_i$

The expression $[x_i(1 + \ln x_i) - 1]^2$ is a square of a real number, so it is always non-negative. The sum of non-negative terms is zero if and only if each term is zero.
Therefore, for each $i \in \{1, 2, \ldots, n\}$, we must have:
$$ [x_i(1 + \ln x_i) - 1]^2 = 0 $$
$$ x_i(1 + \ln x_i) - 1 = 0 $$
This means that all $x_i$ must be solutions to the equation $g(x) = 0$, where $g(x) = x(1 + \ln x) - 1$.

Let's analyze the function $g(x) = x + x \ln x - 1$ for $x > 0$.
To find the solutions, we can use calculus. Let's find the derivative of $g(x)$:
$$ g'(x) = \frac{d}{dx}(x + x \ln x - 1) = 1 + \left(1 \cdot \ln x + x \cdot \frac{1}{x}\right) - 0 = 1 + \ln x + 1 = 2 + \ln x $$
Set the derivative to zero to find critical points:
$g'(x) = 0 \implies 2 + \ln x = 0 \implies \ln x = -2 \implies x = e^{-2}$.

To determine if this is a minimum or maximum, we check the second derivative:
$g''(x) = \frac{d}{dx}(2 + \ln x) = \frac{1}{x}$.
Since $x > 0$, $g''(x) > 0$. This means that $g(x)$ is a strictly convex function, and the critical point $x=e^{-2}$ is a global minimum.

The minimum value of $g(x)$ is:
$$ g(e^{-2}) = e^{-2}(1 + \ln e^{-2}) - 1 = e^{-2}(1 - 2) - 1 = -e^{-2} - 1 < 0 $$
Let's check the behavior of $g(x)$ at the boundaries of its domain $(0, \infty)$:
*   As $x \to 0^+$, using the fact that $\lim_{x\to 0^+} x\ln x = 0$, we have:
    $\lim_{x\to 0^+} g(x) = \lim_{x\to 0^+} (x + x \ln x - 1) = 0 + 0 - 1 = -1$.
*   As $x \to \infty$:
    $\lim_{x\to \infty} g(x) = \lim_{x\to \infty} (x(1 + \ln x) - 1) = \infty$.

The function $g(x)$ decreases from $-1$ to its minimum value $-e^{-2}-1$ on the interval $(0, e^{-2}]$ and increases from $-e^{-2}-1$ to $\infty$ on $[e^{-2}, \infty)$.
Since $g(e^{-2}) < 0$ and $\lim_{x\to \infty} g(x) = \infty$, by the Intermediate Value Theorem, there must be exactly one root for $x > e^{-2}$.
Let's test an integer value, for instance $x=1$:
$$ g(1) = 1(1 + \ln 1) - 1 = 1(1+0)-1 = 1-1=0 $$
So, $x=1$ is a solution to $g(x)=0$. Since we established that there is only one root in $(0, \infty)$, $x=1$ must be the unique solution.

Thus, for all $i \in \{1, 2, \ldots, n\}$, we must have $x_i=1$.

### 5. Verification of the Solution

The only possible solution is $(x_1, x_2, \ldots, x_n) = (1, 1, \ldots, 1)$. We must verify that this solution satisfies the original system of equations.
Let's substitute $x_i = 1$ for all $i$ into the general equation:
$$ x_i^2 + (1 - x_{i+1} \ln x_{i+1})^2 = 2x_{i+1} - 2x_{i+2}^2 \ln x_{i+2} $$
Substituting the values:
$$ 1^2 + (1 - 1 \ln 1)^2 = 2(1) - 2(1^2) \ln 1 $$
$$ 1 + (1 - 1 \cdot 0)^2 = 2 - 2(1 \cdot 0) $$
$$ 1 + (1 - 0)^2 = 2 - 0 $$
$$ 1 + 1^2 = 2 $$
$$ 2 = 2 $$
The equation holds. Since this is true for any choice of $i$, the solution $(1, 1, \ldots, 1)$ is valid for the entire system.

### Conclusion

The only solution to the given system of equations for $n \geq 3$ with $x_i > 0$ is
$$ (x_1, x_2, \ldots, x_n) = (1, 1, \ldots, 1) $$