Here is a detailed, step-by-step solution to the problem.

### **1. Understanding the Problem**

We are asked to find the value of the sum
$$ S = \sum_{i=1}^4\frac{2x_i^2+1}{(x_i^2-1)^2} $$
where $x_1, x_2, x_3, x_4$ are the roots of the polynomial equation $P(x) = x^4-2x-1=0$.

### **2. Strategy**

Directly finding the roots $x_i$ of a quartic equation is generally very difficult and not the intended method. Instead, we can use techniques from the theory of polynomials that relate properties of the roots to the coefficients of the polynomial.

The strategy will be as follows:
1.  Verify that the denominator $(x_i^2-1)^2$ is not zero for any of the roots.
2.  Use the logarithmic derivative of $P(x)$ to find sums of simple rational functions of the roots.
3.  Decompose the complex fraction $\frac{2x^2+1}{(x^2-1)^2}$ into simpler fractions using partial fraction decomposition.
4.  Combine the results to calculate the final sum.

### **3. Step-by-Step Solution**

#### **Step 1: Check the Denominator**

The denominator is $(x_i^2-1)^2$. This is zero if and only if $x_i^2-1=0$, which means $x_i = 1$ or $x_i = -1$. Let's check if $x=1$ or $x=-1$ are roots of $P(x)=x^4-2x-1=0$.
-   For $x=1$: $P(1) = 1^4 - 2(1) - 1 = 1 - 2 - 1 = -2 \neq 0$.
-   For $x=-1$: $P(-1) = (-1)^4 - 2(-1) - 1 = 1 + 2 - 1 = 2 \neq 0$.
Since neither $1$ nor $-1$ are roots of the polynomial, the denominator $(x_i^2-1)^2$ is never zero for any root $x_i$. The sum is well-defined.

#### **Step 2: Using the Logarithmic Derivative**

Let $P(x) = x^4-2x-1 = (x-x_1)(x-x_2)(x-x_3)(x-x_4)$.
The logarithmic derivative of $P(x)$ is given by $\frac{P'(x)}{P(x)}$.
$$ \frac{P'(x)}{P(x)} = \frac{d}{dx} \ln|P(x)| = \frac{d}{dx} \sum_{i=1}^4 \ln|x-x_i| = \sum_{i=1}^4 \frac{1}{x-x_i} $$
This formula allows us to compute sums of the form $\sum \frac{1}{c-x_i}$ by evaluating $\frac{P'(c)}{P(c)}$.

Let's compute the derivatives of $P(x)$:
-   $P(x) = x^4 - 2x - 1$
-   $P'(x) = 4x^3 - 2$
-   $P''(x) = 12x^2$

We will evaluate these at $x=1$ and $x=-1$ to get sums involving $(1-x_i)$ and $(1+x_i)$, which are the factors of $(1-x_i^2)$.

**Evaluation at x=1:**
-   $P(1) = -2$
-   $P'(1) = 4(1)^3 - 2 = 2$
-   $P''(1) = 12(1)^2 = 12$

Using the formula for the logarithmic derivative at $x=1$:
$$ \sum_{i=1}^4 \frac{1}{1-x_i} = \frac{P'(1)}{P(1)} = \frac{2}{-2} = -1 \quad (*)$$

**Evaluation at x=-1:**
-   $P(-1) = 2$
-   $P'(-1) = 4(-1)^3 - 2 = -4 - 2 = -6$
-   $P''(-1) = 12(-1)^2 = 12$

Using the formula at $x=-1$:
$$ \sum_{i=1}^4 \frac{1}{-1-x_i} = \frac{P'(-1)}{P(-1)} = \frac{-6}{2} = -3 $$
$$ -\sum_{i=1}^4 \frac{1}{1+x_i} = -3 \implies \sum_{i=1}^4 \frac{1}{1+x_i} = 3 \quad (**) $$

To find sums involving squared denominators, we differentiate $\frac{P'(x)}{P(x)}$:
$$ \frac{d}{dx}\left(\frac{P'(x)}{P(x)}\right) = \sum_{i=1}^4 \frac{-1}{(x-x_i)^2} $$
The derivative of the quotient is $\frac{P''(x)P(x) - (P'(x))^2}{P(x)^2}$.

**Evaluation of the derivative at x=1:**
$$ \sum_{i=1}^4 \frac{-1}{(1-x_i)^2} = \frac{P''(1)P(1) - (P'(1))^2}{P(1)^2} = \frac{(12)(-2) - (2)^2}{(-2)^2} = \frac{-24-4}{4} = \frac{-28}{4} = -7 $$
$$ \implies \sum_{i=1}^4 \frac{1}{(1-x_i)^2} = 7 \quad (***) $$

**Evaluation of the derivative at x=-1:**
$$ \sum_{i=1}^4 \frac{-1}{(-1-x_i)^2} = \sum_{i=1}^4 \frac{-1}{(1+x_i)^2} = \frac{P''(-1)P(-1) - (P'(-1))^2}{P(-1)^2} = \frac{(12)(2) - (-6)^2}{(2)^2} = \frac{24-36}{4} = \frac{-12}{4} = -3 $$
$$ \implies \sum_{i=1}^4 \frac{1}{(1+x_i)^2} = 3 \quad (****) $$

#### **Step 3: Partial Fraction Decomposition**

We need to express the term $\frac{2x^2+1}{(x^2-1)^2}$ as a sum of the simpler fractions for which we have calculated the sums. Notice that $(x^2-1)^2 = (1-x^2)^2$. Let $u=x_i$. We decompose the expression $\frac{2u^2+1}{(1-u^2)^2} = \frac{2u^2+1}{(1-u)^2(1+u)^2}$.

The general form of the decomposition is:
$$ \frac{2u^2+1}{(1-u)^2(1+u)^2} = \frac{A}{1-u} + \frac{B}{(1-u)^2} + \frac{C}{1+u} + \frac{D}{(1+u)^2} $$
We can find the coefficients $A, B, C, D$ using the Heaviside cover-up method.

-   To find $B$: Multiply by $(1-u)^2$ and set $u=1$.
    $B = \left. \frac{2u^2+1}{(1+u)^2} \right|_{u=1} = \frac{2(1)^2+1}{(1+1)^2} = \frac{3}{4}$.

-   To find $D$: Multiply by $(1+u)^2$ and set $u=-1$.
    $D = \left. \frac{2u^2+1}{(1-u)^2} \right|_{u=-1} = \frac{2(-1)^2+1}{(1-(-1))^2} = \frac{3}{4}$.

-   To find $A$: Multiply by $(1-u)^2$, differentiate with respect to $u$, and then set $u=1$.
    $\frac{d}{du}\left(\frac{2u^2+1}{(1+u)^2}\right) = -A$.
    $\frac{4u(1+u)^2 - (2u^2+1)2(1+u)}{(1+u)^4} = \frac{4u(1+u) - 2(2u^2+1)}{(1+u)^3}$.
    At $u=1$: $\frac{4(1)(2) - 2(2(1)^2+1)}{(1+1)^3} = \frac{8-6}{8} = \frac{2}{8} = \frac{1}{4}$.
    So, $-A = \frac{1}{4} \implies A = -\frac{1}{4}$.

-   To find $C$: Multiply by $(1+u)^2$, differentiate with respect to $u$, and then set $u=-1$.
    $\frac{d}{du}\left(\frac{2u^2+1}{(1-u)^2}\right) = C$.
    $\frac{4u(1-u)^2 - (2u^2+1)2(1-u)(-1)}{(1-u)^4} = \frac{4u(1-u) + 2(2u^2+1)}{(1-u)^3}$.
    At $u=-1$: $\frac{4(-1)(1-(-1)) + 2(2(-1)^2+1)}{(1-(-1))^3} = \frac{4(-1)(2) + 2(3)}{2^3} = \frac{-8+6}{8} = \frac{-2}{8} = -\frac{1}{4}$.
    So, $C = -\frac{1}{4}$.

The decomposition is:
$$ \frac{2x_i^2+1}{(x_i^2-1)^2} = \frac{-1/4}{1-x_i} + \frac{3/4}{(1-x_i)^2} - \frac{1/4}{1+x_i} + \frac{3/4}{(1+x_i)^2} $$

#### **Step 4: Calculate the Final Sum**

Now we can compute the sum $S$ by summing the decomposition over all roots $x_i$:
$$ S = \sum_{i=1}^4 \left( -\frac{1}{4}\frac{1}{1-x_i} + \frac{3}{4}\frac{1}{(1-x_i)^2} - \frac{1}{4}\frac{1}{1+x_i} + \frac{3}{4}\frac{1}{(1+x_i)^2} \right) $$
Using the linearity of summation, we can regroup the terms:
$$ S = -\frac{1}{4}\sum_{i=1}^4\frac{1}{1-x_i} + \frac{3}{4}\sum_{i=1}^4\frac{1}{(1-x_i)^2} - \frac{1}{4}\sum_{i=1}^4\frac{1}{1+x_i} + \frac{3}{4}\sum_{i=1}^4\frac{1}{(1+x_i)^2} $$
Now, substitute the values from equations $(*), (**), (***), (****)$:
-   $\sum \frac{1}{1-x_i} = -1$
-   $\sum \frac{1}{1+x_i} = 3$
-   $\sum \frac{1}{(1-x_i)^2} = 7$
-   $\sum \frac{1}{(1+x_i)^2} = 3$

$$ S = -\frac{1}{4}(-1) + \frac{3}{4}(7) - \frac{1}{4}(3) + \frac{3}{4}(3) $$
$$ S = \frac{1}{4} + \frac{21}{4} - \frac{3}{4} + \frac{9}{4} $$
$$ S = \frac{1+21-3+9}{4} = \frac{28}{4} = 7 $$

Alternatively, we can group the terms as follows:
$$ S = -\frac{1}{4}\left(\sum\frac{1}{1-x_i} + \sum\frac{1}{1+x_i}\right) + \frac{3}{4}\left(\sum\frac{1}{(1-x_i)^2} + \sum\frac{1}{(1+x_i)^2}\right) $$
$$ S = -\frac{1}{4}(-1 + 3) + \frac{3}{4}(7 + 3) $$
$$ S = -\frac{1}{4}(2) + \frac{3}{4}(10) $$
$$ S = -\frac{2}{4} + \frac{30}{4} = \frac{28}{4} = 7 $$

### **Conclusion**

The sum is
$$ \sum_{i=1}^4\frac{2x_i^2+1}{(x_i^2-1)^2} = 7. $$