Of course. Here is a detailed, step-by-step solution to the problem.

### **Problem Statement**
Let $A$ and $B$ be $n\times n$ invertible matrices such that $A+B=I$ and $A^4+B^4=I$, where $I$ is the identity matrix. Compute $\det(AB)$.

### **Solution**

**Step 1: Establish that A and B commute.**

We are given the equation $A+B=I$. From this, we can express $B$ in terms of $A$ (and vice versa):
$B = I - A$.

Now, let's check if $A$ and $B$ commute, i.e., if $AB = BA$.
$AB = A(I-A) = A \cdot I - A \cdot A = A - A^2$.
$BA = (I-A)A = I \cdot A - A \cdot A = A - A^2$.

Since both products are equal to $A - A^2$, we have $AB = BA$. This is a crucial property, as it allows us to manipulate expressions involving $A$ and $B$ as if they were scalar variables (with respect to multiplication).

**Step 2: Use the given equations to find a relationship for the product AB.**

We are given two fundamental equations:
1.  $A+B=I$
2.  $A^4+B^4=I$

Let's take the first equation and raise it to the fourth power. Since $A$ and $B$ commute, we can use the binomial expansion:
$(A+B)^4 = A^4 + 4A^3B + 6A^2B^2 + 4AB^3 + B^4$.

From $A+B=I$, we have $(A+B)^4 = I^4 = I$.
Substituting this into the expansion, we get:
$I = A^4 + 4A^3B + 6A^2B^2 + 4AB^3 + B^4$.

We can group the $A^4$ and $B^4$ terms:
$I = (A^4 + B^4) + 4A^3B + 6A^2B^2 + 4AB^3$.

Now, we use the second given equation, $A^4+B^4=I$, and substitute it into the equation above:
$I = (I) + 4A^3B + 6A^2B^2 + 4AB^3$.

Subtracting $I$ from both sides gives us the zero matrix, $O$:
$O = 4A^3B + 6A^2B^2 + 4AB^3$.

**Step 3: Simplify the resulting matrix equation.**

We can factor the right-hand side of the equation. Let's factor out the common term $2AB$:
$O = 2AB(2A^2 + 3AB + 2B^2)$.

We are given that matrices $A$ and $B$ are invertible. This means $\det(A) \neq 0$ and $\det(B) \neq 0$.
The determinant of the product $2AB$ is $\det(2AB) = \det(2I \cdot A \cdot B) = \det(2I)\det(A)\det(B) = 2^n \det(A)\det(B)$.
Since $2^n \neq 0$, $\det(A) \neq 0$, and $\det(B) \neq 0$, their product is non-zero.
Therefore, $\det(2AB) \neq 0$, which implies that the matrix $2AB$ is invertible.

Now, we have an equation of the form $C \cdot D = O$, where $C = 2AB$ is invertible. We can multiply by the inverse of $C$ from the left:
$C^{-1}(CD) = C^{-1}O$
$(C^{-1}C)D = O$
$ID = O$
$D = O$.

Applying this to our equation, we must have:
$2A^2 + 3AB + 2B^2 = O$.

**Step 4: Express the equation in terms of AB and I.**

Let's try to simplify the expression $2A^2 + 3AB + 2B^2$. We can rewrite it as:
$2(A^2 + B^2) + 3AB = O$.

To proceed, we need to find an expression for $A^2+B^2$. We can obtain this by squaring the initial equation $A+B=I$:
$(A+B)^2 = I^2$
$A^2 + 2AB + B^2 = I$.

From this, we can isolate $A^2+B^2$:
$A^2+B^2 = I - 2AB$.

Now, substitute this expression for $A^2+B^2$ back into our equation from Step 3:
$2(I - 2AB) + 3AB = O$.

Distribute the 2:
$2I - 4AB + 3AB = O$.

Combine the terms involving $AB$:
$2I - AB = O$.

This gives us a simple expression for the matrix product $AB$:
$AB = 2I$.

**Step 5: Compute the determinant of AB.**

Our goal is to find $\det(AB)$. Using the result from the previous step:
$\det(AB) = \det(2I)$.

The matrix $2I$ is an $n \times n$ diagonal matrix with all its diagonal entries equal to 2:
$2I = \begin{pmatrix}
2 & 0 & \cdots & 0 \\
0 & 2 & \cdots & 0 \\
\vdots & \vdots & \ddots & \vdots \\
0 & 0 & \cdots & 2
\end{pmatrix}$

The determinant of a diagonal matrix is the product of its diagonal entries. In this case, we multiply 2 by itself $n$ times.
$\det(2I) = 2 \times 2 \times \cdots \times 2 \quad (n \text{ times}) = 2^n$.

Therefore, $\det(AB) = 2^n$.

### **Final Answer**

The value of $\det(AB)$ is $\boldsymbol{2^n}$.