```markdown
We are given a set of \( n \) biased coins where the \( m \)-th coin (for \( m=1,2,\ldots,n \)) has a probability 
\[
p_m = \frac{1}{2m+1}
\]
of landing heads, and all tosses are independent. We wish to find the probability that the total number of heads is even.

A well-known result for independent coin tosses is that the probability of getting an even number of heads is given by:
\[
P_{\text{even}} = \frac{1}{2}\left(1 + \prod_{m=1}^{n}(1-2p_m)\right).
\]

Substitute \( p_m = \frac{1}{2m+1} \) into the product:
\[
1 - 2p_m = 1 - \frac{2}{2m+1} = \frac{2m+1-2}{2m+1} = \frac{2m-1}{2m+1}.
\]
Thus, the product becomes:
\[
\prod_{m=1}^{n} \frac{2m-1}{2m+1} = \frac{1}{3} \times \frac{3}{5} \times \frac{5}{7} \times \cdots \times \frac{2n-1}{2n+1}.
\]

Notice that this is a telescoping product. All the intermediate terms cancel, leaving:
\[
\prod_{m=1}^{n} \frac{2m-1}{2m+1} = \frac{1}{2n+1}.
\]

Now, substitute this back into the expression for \( P_{\text{even}} \):
\[
P_{\text{even}} = \frac{1}{2}\left(1 + \frac{1}{2n+1}\right).
\]

Thus, the probability of getting an even number of heads is:
\[
\boxed{\frac{1}{2}\left(1 + \frac{1}{2n+1}\right)}.
\]
```