# Solution

Let's analyze the given equation:
$$(n-(m-1))^2 + \ldots + (n-1)^2 + n^2 = (n+1)^2 + (n+2)^2 + \ldots + (n+k)^2.$$

## Part 1: Showing $m \geq k$

The left side has $m$ terms, starting from $(n-(m-1))^2$ and ending at $n^2$. The right side has $k$ terms, starting from $(n+1)^2$ and ending at $(n+k)^2$.

Note that every term on the right side is greater than every term on the left side. Specifically, the smallest term on the right, $(n+1)^2$, is greater than the largest term on the left, $n^2$ (since $(n+1)^2 = n^2 + 2n + 1 > n^2$ for $n > 0$).

Since the sums are equal and each term on the right is larger than any term on the left, the left side must have at least as many terms as the right to achieve equality. Therefore, $m \geq k$.

## Part 2: Showing $m \leq 7k$

Using the formula for the sum of consecutive squares:
$$\sum_{i=a}^{b} i^2 = \frac{b(b+1)(2b+1) - (a-1)a(2a-1)}{6}$$

We can express the left side of our equation as:
$$\sum_{i=n-m+1}^{n} i^2 = \frac{n(n+1)(2n+1) - (n-m)(n-m+1)(2(n-m)+1)}{6}$$

Similarly, for the right side:
$$\sum_{i=n+1}^{n+k} i^2 = \frac{(n+k)(n+k+1)(2(n+k)+1) - n(n+1)(2n+1)}{6}$$

Given our equation, these expressions are equal. After canceling $\frac{n(n+1)(2n+1)}{6}$ from both sides, we get:
$$-(n-m)(n-m+1)(2(n-m)+1) = (n+k)(n+k+1)(2(n+k)+1) - n(n+1)(2n+1)$$

For simplicity, let's define $f(x) = x(x+1)(2x+1) = 2x^3 + 3x^2 + x$. Our equation becomes:
$$-f(n-m) = f(n+k) - f(n)$$

Rearranging:
$$f(n) - f(n-m) = f(n+k) - f(n)$$

To show that $m \leq 7k$, we'll prove that if $m > 7k$, a contradiction arises.

If $m > 7k$, then $n-m < n-7k$. Since $f$ is an increasing function for positive $x$, we have $f(n-m) < f(n-7k)$. This implies:
$$f(n) - f(n-m) > f(n) - f(n-7k)$$

For our equation to hold, we need:
$$f(n) - f(n-7k) \leq f(n+k) - f(n)$$

This is equivalent to:
$$f(n-7k) + f(n+k) \leq 2f(n)$$

Let's define $g(n) = f(n-7k) + f(n+k) - 2f(n)$ and check if $g(n) \leq 0$ for $n \geq 7k$ and $k \geq 1$.

Substituting and expanding:
$$g(n) = -36n^2k + 256nk + 297k^2 - 684k^3$$

For $n = 7k$ (the smallest possible value for $n$ under our constraints):
$$g(7k) = -36(7k)^2k + 256(7k)k + 297k^2 - 684k^3$$
$$g(7k) = -1764k^3 + 1792k^2 + 297k^2 - 684k^3$$
$$g(7k) = -2448k^3 + 2089k^2 = k^2(-2448k + 2089)$$

For $k \geq 1$, we have $-2448k + 2089 < 0$, so $g(7k) < 0$. This contradiction implies that we must have $m \leq 7k$.

## Part 3: Showing $7k \leq 7n$

From Part 1, we established $m \geq k$. Given the constraint $n \geq m$, we have $n \geq m \geq k$, which implies $n \geq k$ or $7k \leq 7n$.

Combining our results, we've shown $m \leq 7k \leq 7n$.