```markdown
We wish to evaluate
\[
S=\sum_{n=1}^{\infty}\frac{48n^2+44n+9}{n(2n+1)(4n+1)(4n+3)}.
\]
A good way to attack the problem is to decompose the summand into partial fractions. We want to find constants \(A\), \(B\), \(C\), and \(D\) such that
\[
\frac{48n^2+44n+9}{n(2n+1)(4n+1)(4n+3)}=\frac{A}{n}+\frac{B}{2n+1}+\frac{C}{4n+1}+\frac{D}{4n+3}\,.
\]
Multiplying both sides by the common denominator \(n(2n+1)(4n+1)(4n+3)\) gives
\[
48n^2+44n+9 = A\,(2n+1)(4n+1)(4n+3) + B\,n(4n+1)(4n+3) + C\,n(2n+1)(4n+3) + D\,n(2n+1)(4n+1)~.
\]

### Step 1. Find the Constants

1. **Set \(n=0\):**  
   The left‐hand side becomes
   \[
   48\cdot0^2+44\cdot0+9=9.
   \]
   On the right, only the first term survives:
   \[
   A\,(2\cdot0+1)(4\cdot0+1)(4\cdot0+3)=A\cdot(1)(1)(3)=3A.
   \]
   Hence,
   \[
   3A=9\quad\Longrightarrow\quad A=3\,.
   \]

2. **Set \(2n+1=0\) (i.e. \(n=-\tfrac12\)):**  
   Substituting \(n=-\frac{1}{2}\) we have
   \[
   48\left(-\tfrac12\right)^2+44\left(-\tfrac12\right)+9
   =48\cdot\frac{1}{4}-22+9
   =12-22+9=-1\,.
   \]
   On the right, note that \(2n+1=0\) annihilates the terms with factors \((2n+1)\) so only the \(B\)–term contributes:
   \[
   B\,n(4n+1)(4n+3)\quad\text{with}\quad n=-\frac{1}{2}\,.
   \]
   Compute:
   \[
   4n+1=4\Bigl(-\frac{1}{2}\Bigr)+1=-2+1=-1,\quad 4n+3=-2+3=1\,.
   \]
   Thus the contribution is
   \[
   B\left(-\frac{1}{2}\right)(-1)(1)= \frac{B}{2}\,.
   \]
   Equate:
   \[
   \frac{B}{2}=-1\quad\Longrightarrow\quad B=-2\,.
   \]

3. **Set \(4n+1=0\) (i.e. \(n=-\tfrac{1}{4}\)):**  
   Substituting \(n=-\frac{1}{4}\) we get 
   \[
   48\left(-\frac{1}{4}\right)^2+44\left(-\frac{1}{4}\right)+9
   =48\cdot\frac{1}{16}-11+9
   =3-11+9=1\,.
   \]
   Now, the terms with a factor \((4n+1)\) vanish. Only the \(C\)–term survives:
   \[
   C\,n(2n+1)(4n+3) \quad \text{with } n=-\frac{1}{4}\,.
   \]
   Evaluate:
   \[
   2n+1=2\Bigl(-\frac{1}{4}\Bigr)+1=-\frac{1}{2}+1=\frac{1}{2}\,,\quad
   4n+3=4\Bigl(-\frac{1}{4}\Bigr)+3=-1+3=2\,,
   \]
   and \(n=-\frac{1}{4}\). Hence the term equals:
   \[
   C\left(-\frac{1}{4}\right)\left(\frac{1}{2}\right)(2)
   =-\frac{C}{4}\,.
   \]
   So,
   \[
   -\frac{C}{4}=1\quad\Longrightarrow\quad C=-4\,.
   \]

4. **Set \(4n+3=0\) (i.e. \(n=-\tfrac{3}{4}\)):**  
   For \(n=-\frac{3}{4}\):
   \[
   48\left(-\frac{3}{4}\right)^2+44\left(-\frac{3}{4}\right)+9
   =48\cdot\frac{9}{16}-33+9
   =27-33+9=3\,.
   \]
   Here only the \(D\)–term survives (since it contains the factor \((4n+3)\) that now vanishes in the other terms):
   \[
   D\,n(2n+1)(4n+1)\,.
   \]
   Compute:
   \[
   n=-\frac{3}{4},\quad
   2n+1=2\Bigl(-\frac{3}{4}\Bigr)+1=-\frac{3}{2}+1=-\frac{1}{2},\quad
   4n+1=4\Bigl(-\frac{3}{4}\Bigr)+1=-3+1=-2\,.
   \]
   So we have:
   \[
   D\left(-\frac{3}{4}\right)\left(-\frac{1}{2}\right)(-2)
   =D\left(-\frac{3}{4}\cdot \frac{1}{2}\cdot (-2) \right)
   =D\left(-\frac{3}{4}\right)
   \,.
   \]
   Hence,
   \[
   -\frac{3}{4}D=3\quad\Longrightarrow\quad D=-4\,.
   \]

Thus, the constants are:
\[
A=3,\quad B=-2,\quad C=-4,\quad D=-4\,.
\]

### Step 2. Expressing the Sum

With the partial fractions in hand, we write
\[
\frac{48n^2+44n+9}{n(2n+1)(4n+1)(4n+3)}
=\frac{3}{n}-\frac{2}{2n+1}-\frac{4}{4n+1}-\frac{4}{4n+3}\,.
\]
Therefore,
\[
S=\sum_{n=1}^{\infty}\left(\frac{3}{n}-\frac{2}{2n+1}-\frac{4}{4n+1}-\frac{4}{4n+3}\right)\,.
\]

Although each individual series is divergent, when taken together the divergent parts cancel. (A quick check at \(n=1\) verifies the decomposition:
\[
\frac{48+44+9}{1\cdot3\cdot5\cdot7}=\frac{101}{105}\approx 0.9619
\]
and
\[
\frac{3}{1}-\frac{2}{3}-\frac{4}{5}-\frac{4}{7}\approx3-0.6667-0.8-0.5714\approx0.9619\,.)
\]

A standard technique is to sum these terms using properties of the digamma function \(\psi(z)\). One may write the partial sums in the form
\[
S_N=3\sum_{n=1}^{N}\frac{1}{n}-2\sum_{n=1}^{N}\frac{1}{2n+1}-4\sum_{n=1}^{N}\frac{1}{4n+1}-4\sum_{n=1}^{N}\frac{1}{4n+3}\,.
\]
Expressing these sums in terms of the digamma function (recalling that \(\sum_{n=1}^{N}\frac{1}{n}=\psi(N+1)+\gamma\) where \(\gamma\) is Euler’s constant) and using the relation
\[
\sum_{n=1}^{N}\frac{1}{n+a}=\psi(N+1+a)-\psi(1+a)\,,
\]
one finds after some rearrangement that the divergent pieces cancel in the \(N\to\infty\) limit and one is left with
\[
S=3\gamma+\psi\Bigl(\frac{3}{2}\Bigr)+\psi\Bigl(\frac{5}{4}\Bigr)+\psi\Bigl(\frac{7}{4}\Bigr)\,.
\]

Using the known values
\[
\psi\Bigl(\frac{1}{2}\Bigr)=-\gamma-2\ln2,\qquad \psi\Bigl(\frac{3}{2}\Bigr)=\psi\Bigl(\frac{1}{2}\Bigr)+2=2-\gamma-2\ln2\,,
\]
and the relations
\[
\psi\Bigl(1+z\Bigr)=\psi(z)+\frac{1}{z}\,,
\]
one obtains
\[
\psi\Bigl(\frac{5}{4}\Bigr)=\psi\Bigl(\frac{1}{4}\Bigr)+4,\quad
\psi\Bigl(\frac{7}{4}\Bigr)=\psi\Bigl(\frac{3}{4}\Bigr)+\frac{4}{3}\,.
\]
Moreover, using the reflection formula
\[
\psi(1-z)-\psi(z)=\pi\cot(\pi z)
\]
it can be shown that the constants combine so that
\[
S=\frac{22}{3}-8\ln2\,.
\]

### Final Answer

Thus, we conclude that
\[
\boxed{\sum_{n=1}^{\infty}\frac{48n^2+44n+9}{n(2n+1)(4n+1)(4n+3)}=\frac{22}{3}-8\ln2\,.}
\]
```