Let the given integrals be $I_1$ and $I_2$.
$$I_1 = \int_0^{\infty}\frac{e^{-2x}}{1+x^2}dx$$
$$I_2 = \int_0^{\infty}\frac{\cos x}{2+x}dx$$
We want to show that $I_1 = I_2$.

Let's analyze $I_1$. We can represent $\frac{1}{1+x^2}$ using an integral. One representation is $\frac{1}{1+x^2} = \int_0^\infty e^{-k} \cos(kx) dk$.
Substitute this into $I_1$:
$$I_1 = \int_0^{\infty} e^{-2x} \left( \int_0^{\infty} e^{-k} \cos(kx) dk \right) dx$$
Assuming we can swap the order of integration (justified below), we have:
$$I_1 = \int_0^{\infty} e^{-k} \left( \int_0^{\infty} e^{-2x} \cos(kx) dx \right) dk$$
The inner integral is the Laplace transform of $\cos(kx)$ with respect to $x$, evaluated at $s=2$.
$$\int_0^{\infty} e^{-2x} \cos(kx) dx = \text{Re} \int_0^{\infty} e^{-2x} e^{ikx} dx = \text{Re} \int_0^{\infty} e^{-(2-ik)x} dx$$
$$= \text{Re} \left[ \frac{e^{-(2-ik)x}}{-(2-ik)} \right]_0^{\infty} = \text{Re} \left( 0 - \frac{1}{-(2-ik)} \right) = \text{Re} \left( \frac{1}{2-ik} \right)$$
$$= \text{Re} \left( \frac{2+ik}{4+k^2} \right) = \frac{2}{4+k^2}$$
Substituting this back into the expression for $I_1$:
$$I_1 = \int_0^{\infty} e^{-k} \frac{2}{4+k^2} dk$$
Let $S(a) = \int_0^{\infty} \frac{a e^{-k}}{a^2+k^2} dk$. Then $I_1 = S(2)$.

Let's analyze $I_2$. We can represent $\frac{1}{2+x}$ using an integral: $\frac{1}{2+x} = \int_0^\infty e^{-(2+x)t} dt$.
$$I_2 = \int_0^{\infty} \cos x \left( \int_0^{\infty} e^{-2t} e^{-xt} dt \right) dx$$
Assuming we can swap the order of integration:
$$I_2 = \int_0^{\infty} e^{-2t} \left( \int_0^{\infty} e^{-xt} \cos x dx \right) dt$$
The inner integral is $\int_0^{\infty} e^{-xt} \cos x dx$. From the previous calculation (with $k=1$ and $2$ replaced by $t$), this evaluates to $\frac{t}{t^2+1}$.
$$I_2 = \int_0^{\infty} e^{-2t} \frac{t}{t^2+1} dt$$
Let $C(a) = \int_0^{\infty} \frac{t e^{-at}}{1+t^2} dt$. Then $I_2 = C(2)$.

To show $I_1=I_2$, we must show $S(2)=C(2)$.
Let's transform $S(2)$ with the substitution $k=2u$, $dk=2du$.
$$I_1 = S(2) = \int_0^{\infty} \frac{2 e^{-k}}{4+k^2} dk = \int_0^{\infty} \frac{2 e^{-2u}}{4+(2u)^2} (2du) = \int_0^{\infty} \frac{4 e^{-2u}}{4+4u^2} du = \int_0^{\infty} \frac{e^{-2u}}{1+u^2} du$$
Let's rename the integration variable $u$ to $t$.
$$I_1 = \int_0^{\infty} \frac{e^{-2t}}{1+t^2} dt$$
So we need to show:
$$\int_0^{\infty} \frac{e^{-2t}}{1+t^2} dt = \int_0^{\infty} \frac{t e^{-2t}}{1+t^2} dt$$
This is equivalent to showing that the difference is zero:
$$\int_0^{\infty} \frac{(1-t)e^{-2t}}{1+t^2} dt = 0$$
Let $K(a) = \int_0^\infty \frac{(1-t)e^{-at}}{1+t^2} dt$. We need to show $K(2)=0$.
We can express $K(a)$ in terms of the auxiliary sine and cosine integrals.
$K(a) = \int_0^\infty \frac{e^{-at}}{1+t^2} dt - \int_0^\infty \frac{t e^{-at}}{1+t^2} dt = S(a) - C(a)$.
Using the standard definitions $\text{Ci}(a) = -\int_a^\infty \frac{\cos t}{t} dt$ and $\text{si}(a) = -\int_a^\infty \frac{\sin t}{t} dt$, we have the known identities for $a>0$:
$S(a) = \int_0^\infty \frac{e^{-at}}{1+t^2} dt = \sin a \text{Ci}(a) - \cos a \text{si}(a)$.
$C(a) = \int_0^\infty \frac{t e^{-at}}{1+t^2} dt = -\cos a \text{Ci}(a) - \sin a \text{si}(a)$.
So $K(a) = S(a) - C(a) = (\sin a + \cos a)\text{Ci}(a) - (\cos a - \sin a)\text{si}(a)$.
We need $K(2)=0$, which means
$$(\sin 2 + \cos 2)\text{Ci}(2) = (\cos 2 - \sin 2)\text{si}(2)$$
Let's check this condition numerically.
Using $\sin 2 \approx 0.9093$, $\cos 2 \approx -0.4161$, $\text{Ci}(2) \approx -0.4230$, $\text{si}(2) \approx -0.6978$.
LHS $\approx (0.9093 - 0.4161)(-0.4230) = (0.4932)(-0.4230) \approx -0.2086$.
RHS $\approx (-0.4161 - 0.9093)(-0.6978) = (-1.3254)(-0.6978) \approx 0.9249$.
Since LHS $\ne$ RHS, the condition $K(2)=0$ is false. This means $I_1 \ne I_2$.

Conclusion: The statement of the problem appears to be incorrect. The identity $\int_0^{\infty}\frac{e^{-ax}}{1+x^2}dx=\int_0^{\infty}\frac{\sin x}{a+x}dx$ is a known identity. If the second integral in the problem were $I_4 = \int_0^{\infty}\frac{\sin x}{2+x}dx$, then we would have $I_1 = S(2)$ and $I_4 = S(2)$, which implies $I_1 = I_4$.

Assuming the problem statement *is* correct, then the proof requires demonstrating that $\int_0^\infty \frac{(1-t)e^{-2t}}{1+t^2} dt = 0$. Based on the analysis using standard special functions Si and Ci, this identity is false. Therefore, based on current mathematical knowledge and standard function definitions, the equality stated in the problem cannot be shown. There might be a non-standard definition context or a typo in the problem statement.

However, if we are forced to provide a "proof" assuming the statement is true, it would rely on accepting the identity $\int_0^\infty \frac{(1-t)e^{-2t}}{1+t^2} dt = 0$ as given or proven through some non-standard analysis. If this identity holds, then $I_1 = \int_0^\infty \frac{e^{-2t}}{1+t^2} dt$ and $I_2 = \int_0^\infty \frac{t e^{-2t}}{1+t^2} dt$ would indeed be equal.

Final conclusion based on rigorous analysis: The statement is incorrect as stated. A likely correction is that the second integral should feature $\sin x$ instead of $\cos x$.


Let's check the justification for swapping the order of integration.
For $I_1 = \int_0^{\infty} e^{-k} \left( \int_0^{\infty} e^{-2x} \cos(kx) dx \right) dk$. The integrand is $f(x,k) = e^{-2x} e^{-k} \cos(kx)$.
$\int_0^\infty \int_0^\infty |f(x,k)| dx dk = \int_0^\infty e^{-k} (\int_0^\infty e^{-2x} |\cos(kx)| dx) dk$.
$\int_0^\infty e^{-2x} |\cos(kx)| dx \le \int_0^\infty e^{-2x} dx = 1/2$.
So $\int_0^\infty \int_0^\infty |f(x,k)| dx dk \le \int_0^\infty e^{-k} (1/2) dk = 1/2$.
Since the integral of the absolute value is finite, Fubini-Tonelli theorem permits the swap of integration order.
For $I_2 = \int_0^{\infty} e^{-2t} \left( \int_0^{\infty} e^{-xt} \cos x dx \right) dt$. The integrand is $g(x,t) = e^{-2t} e^{-xt} \cos x$.
$\int_0^\infty \int_0^\infty |g(x,t)| dt dx = \int_0^\infty (\int_0^\infty e^{-(2+x)t} dt) |\cos x| dx$.
$\int_0^\infty \frac{1}{2+x} |\cos x| dx$. This integral diverges. For large $x$, $\frac{|\cos x|}{2+x} \sim \frac{|\cos x|}{x}$. $\int^\infty \frac{|\cos x|}{x} dx$ diverges.
So Fubini-Tonelli does not apply directly. However, the iterated integrals exist, and the calculation formally carried out showed $I_2 = C(2)$. This swap requires separate justification (e.g., dominated convergence on finite intervals), which is standard for Laplace transform manipulations.


Final Answer: The final answer is $\boxed{I_1 = \int_0^\infty \frac{e^{-2t}}{1+t^2} dt \text{ and } I_2 = \int_0^\infty \frac{t e^{-2t}}{1+t^2} dt \text{; the identity } I_1=I_2 \text{ is likely incorrect as stated.}}$