Here is a detailed, step-by-step solution to the problem.

Let $S$ be the sum in question:
$$ S = \sum_{k=1}^n \sum_{1 \leq i_1 < \ldots < i_k \leq n} (-1)^{k} \frac{m_{i_1, \ldots, i_k}^{2N+i_1+\ldots+i_k-1}}{i_1 + \ldots + i_k + N} $$
The inner sum is over all non-empty subsets of $\{1, 2, \ldots, n\}$. Let $I = \{i_1, \ldots, i_k\}$ be such a subset. Let $S_I = i_1 + \ldots + i_k$ be the sum of its elements, and $|I|=k$ be its cardinality. The sum can be written as:
$$ S = \sum_{\emptyset \neq I \subseteq \{1, \ldots, n\}} (-1)^{|I|} \frac{(\min_{i \in I} r_i)^{2N+S_I-1}}{N+S_I} $$

The main difficulty in this expression is the $\min_{i \in I} r_i$ term, which depends on the subset $I$ in a non-linear way. To handle this, we will group the terms of the sum based on the value of this minimum.

### Step 1: Partitioning the sum based on the minimum value
Let the distinct values among $r_1, r_2, \ldots, r_n$ be $v_1, v_2, \ldots, v_p$, where $p \le n$. We can assume, without loss of generality, that they are ordered: $1 > v_1 > v_2 > \ldots > v_p > 0$.

For each distinct value $v_j$, let $K_j$ be the set of indices $i$ for which $r_i$ takes this value:
$$ K_j = \{i \in \{1, \ldots, n\} \mid r_i = v_j \}, \quad \text{for } j=1, \ldots, p. $$
Also, let $U_j$ be the set of indices $i$ for which $r_i$ is at least $v_j$:
$$ U_j = \{i \in \{1, \ldots, n\} \mid r_i \geq v_j \} = \bigcup_{l=1}^j K_l, \quad \text{for } j=1, \ldots, p. $$
We also define $U_0 = \emptyset$. Note that $U_j = U_{j-1} \cup K_j$ and $U_{j-1} \cap K_j = \emptyset$.

For any non-empty subset $I \subseteq \{1, \ldots, n\}$, the minimum value $m_I = \min_{i \in I} r_i$ must be one of the values $v_j$. Specifically, $m_I = v_j$ if and only if all elements of $I$ have $r_i \ge v_j$ and at least one element of $I$ has $r_i = v_j$. In terms of our sets, this is equivalent to:
$$ m_I = v_j \iff I \subseteq U_j \text{ and } I \cap K_j \neq \emptyset $$
This is because $I \subseteq U_j$ ensures all $r_i \ge v_j$ for $i \in I$, and $I \cap K_j \neq \emptyset$ ensures that the minimum is not greater than $v_j$.

We can now rewrite the sum $S$ by grouping terms according to the value of $m_I$:
$$ S = \sum_{j=1}^p \sum_{I: m_I=v_j} (-1)^{|I|} \frac{v_j^{2N+S_I-1}}{N+S_I} $$
Let's denote the inner sum by $C_j$:
$$ C_j = \sum_{\substack{I \subseteq U_j \\ I \cap K_j \neq \emptyset}} (-1)^{|I|} \frac{v_j^{2N+S_I-1}}{N+S_I} $$
The total sum is $S = \sum_{j=1}^p C_j$. We will now show that each $C_j$ is negative.

### Step 2: Using an integral representation
For a fixed $j$, the term $v_j$ is constant in the sum defining $C_j$. We can factor out $v_j^{2N-1}$:
$$ C_j = v_j^{2N-1} \sum_{\substack{I \subseteq U_j \\ I \cap K_j \neq \emptyset}} (-1)^{|I|} \frac{v_j^{S_I}}{N+S_I} $$
To handle the fraction, we use the following integral identity, which holds for $x>0$ and $A, B > 0$:
$$ \frac{x^A}{B+A} = \int_0^1 t^{B-1} (xt)^A dt $$
In our case, $x=v_j$, $A=S_I$, and $B=N$. So we have:
$$ \frac{v_j^{S_I}}{N+S_I} = \int_0^1 t^{N-1} (t v_j)^{S_I} dt $$
Substituting this into the expression for $C_j$:
$$ C_j = v_j^{2N-1} \sum_{\substack{I \subseteq U_j \\ I \cap K_j \neq \emptyset}} (-1)^{|I|} \int_0^1 t^{N-1} (t v_j)^{S_I} dt $$
Since the sum is finite, we can interchange summation and integration:
$$ C_j = v_j^{2N-1} \int_0^1 t^{N-1} \left( \sum_{\substack{I \subseteq U_j \\ I \cap K_j \neq \emptyset}} (-1)^{|I|} (t v_j)^{S_I} \right) dt $$

### Step 3: Simplifying the inner sum
Let's focus on the sum inside the integral. The condition on $I$ ($I \subseteq U_j$ and $I \cap K_j \neq \emptyset$) means that $I$ is formed by taking a non-empty subset of $K_j$ and any subset of $U_{j-1}$. Let $I = I_1 \cup I_2$, where $I_1 \subseteq K_j$ and $I_2 \subseteq U_{j-1}$. The condition $I \cap K_j \neq \emptyset$ means $I_1 \neq \emptyset$. Since $K_j$ and $U_{j-1}$ are disjoint, $|I|=|I_1|+|I_2|$ and $S_I = S_{I_1} + S_{I_2}$.

The sum can be factored:
\begin{align*} \sum_{\substack{I \subseteq U_j \\ I \cap K_j \neq \emptyset}} (-1)^{|I|} (t v_j)^{S_I} &= \sum_{\substack{I_1 \subseteq K_j, I_1 \neq \emptyset \\ I_2 \subseteq U_{j-1}}} (-1)^{|I_1|+|I_2|} (t v_j)^{S_{I_1}+S_{I_2}} \\ &= \left( \sum_{\emptyset \neq I_1 \subseteq K_j} (-1)^{|I_1|} (t v_j)^{S_{I_1}} \right) \left( \sum_{I_2 \subseteq U_{j-1}} (-1)^{|I_2|} (t v_j)^{S_{I_2}} \right) \end{align*}
We can evaluate these two sums using the identity $\sum_{J \subseteq A} (-1)^{|J|} \prod_{l \in J} x_l = \prod_{l \in A} (1-x_l)$. Note that $(t v_j)^{S_J} = \prod_{l \in J} (t v_j)^l$.

For the second sum:
$$ \sum_{I_2 \subseteq U_{j-1}} (-1)^{|I_2|} \prod_{l \in I_2} (t v_j)^l = \prod_{l \in U_{j-1}} (1-(tv_j)^l) $$
For the first sum:
\begin{align*} \sum_{\emptyset \neq I_1 \subseteq K_j} (-1)^{|I_1|} \prod_{l \in I_1} (t v_j)^l &= \left(\sum_{I_1 \subseteq K_j} (-1)^{|I_1|} \prod_{l \in I_1} (t v_j)^l\right) - (\text{term for } I_1=\emptyset) \\ &= \left(\prod_{l \in K_j} (1-(tv_j)^l)\right) - 1 \end{align*}

Let's call the term inside the integral $\Sigma_j(t)$. We have:
$$ \Sigma_j(t) = \left( \prod_{l \in K_j} (1-(tv_j)^l) - 1 \right) \left( \prod_{l \in U_{j-1}} (1-(tv_j)^l) \right) $$

### Step 4: Determining the sign of each $C_j$
We now have an expression for $C_j$:
$$ C_j = v_j^{2N-1} \int_0^1 t^{N-1} \Sigma_j(t) dt $$
Let's analyze the sign of the integrand for $t \in (0,1)$:
1.  $v_j \in (0,1)$, so for $t \in (0,1)$, we have $tv_j \in (0,1)$.
2.  For any $l \in \{1, \ldots, n\}$, $(tv_j)^l \in (0,1)$.
3.  This means $1-(tv_j)^l \in (0,1)$.
4.  The product $\prod_{l \in U_{j-1}} (1-(tv_j)^l)$ is a product of terms in $(0,1)$, so it is positive and less than 1. (If $U_{j-1}=\emptyset$, the product is 1).
5.  Similarly, $\prod_{l \in K_j} (1-(tv_j)^l)$ is in $(0,1)$ (since $K_j$ is non-empty).
6.  Therefore, $\left(\prod_{l \in K_j} (1-(tv_j)^l) - 1\right)$ is negative.

The term $t^{N-1}$ is positive for $t \in (0,1)$ as $N \in \mathbb{N}$.
The integrand $t^{N-1} \Sigma_j(t) = t^{N-1} \times (\text{negative}) \times (\text{positive})$ is strictly negative for all $t \in (0,1)$.

The integral of a strictly negative function over an interval $(0,1)$ is negative:
$$ \int_0^1 t^{N-1} \Sigma_j(t) dt < 0 $$
Also, $v_j \in (0,1)$ and $N \in \mathbb{N}$, so $v_j^{2N-1}$ is positive.
Thus, each term $C_j = (\text{positive}) \times (\text{negative})$ is strictly negative.
$$ C_j < 0 \quad \text{for } j=1, \ldots, p. $$

### Step 5: Final Conclusion
The total sum $S$ is given by $S = \sum_{j=1}^p C_j$. Since each $C_j$ is strictly negative, their sum must also be strictly negative.
$$ S < 0 $$
Therefore, the inequality $S \leq 0$ holds.