Let the given inequality be
 \[
 \left(\prod_{i=1}^n a_i\right)^\frac 1n+\left(\prod_{i=1}^n b_i\right)^\frac 1n+\left(\prod_{i=1}^n c_i\right)^\frac 1n\leq \left(\prod_{i=1}^n (a_i+b_i+c_i)\right)^\frac 1n.
 \]
The numbers $a_i, b_i, c_i$ are non-negative real numbers.

Case 1: For some index $k \in \{1, \ldots, n\}$, $a_k+b_k+c_k=0$.
Since $a_k, b_k, c_k$ are non-negative, $a_k+b_k+c_k=0$ implies $a_k=0$, $b_k=0$, and $c_k=0$.
In this case, the term $(a_k+b_k+c_k)$ in the product $\prod_{i=1}^n (a_i+b_i+c_i)$ is 0, so the product is 0. The right-hand side (RHS) of the inequality is $(0)^{1/n} = 0$.
For the left-hand side (LHS), since $a_k=0$, the product $\prod_{i=1}^n a_i$ is 0, so $(\prod_{i=1}^n a_i)^{1/n}=0$. Similarly, since $b_k=0$, $(\prod_{i=1}^n b_i)^{1/n}=0$, and since $c_k=0$, $(\prod_{i=1}^n c_i)^{1/n}=0$.
Thus, the LHS is $0+0+0=0$.
The inequality becomes $0 \leq 0$, which is true.
So the inequality holds if $a_i+b_i+c_i=0$ for some $i$.

Case 2: $a_i+b_i+c_i > 0$ for all $i \in \{1, \ldots, n\}$.
Let $S_i = a_i+b_i+c_i$. Since $S_i > 0$ for all $i$, the product $\prod_{i=1}^n S_i > 0$. We can divide the inequality by $(\prod_{i=1}^n S_i)^{1/n}$.
The inequality becomes
\[
 \frac{\left(\prod a_i\right)^\frac 1n}{\left(\prod S_i\right)^\frac 1n}+\frac{\left(\prod b_i\right)^\frac 1n}{\left(\prod S_i\right)^\frac 1n}+\frac{\left(\prod c_i\right)^\frac 1n}{\left(\prod S_i\right)^\frac 1n}\leq 1.
\]
Using the property $(\prod x_i / \prod y_i)^{1/n} = (\prod (x_i/y_i))^{1/n}$, this is equivalent to
\[
 \left(\prod_{i=1}^n \frac{a_i}{S_i}\right)^\frac 1n+\left(\prod_{i=1}^n \frac{b_i}{S_i}\right)^\frac 1n+\left(\prod_{i=1}^n \frac{c_i}{S_i}\right)^\frac 1n\leq 1.
\]
Let $x_i = \frac{a_i}{S_i}$, $y_i = \frac{b_i}{S_i}$, and $z_i = \frac{c_i}{S_i}$ for $i=1, \ldots, n$.
Since $a_i, b_i, c_i \ge 0$ and $S_i > 0$, we have $x_i, y_i, z_i \ge 0$ for all $i$.
Also, for each $i$, $x_i+y_i+z_i = \frac{a_i}{S_i}+\frac{b_i}{S_i}+\frac{c_i}{S_i} = \frac{a_i+b_i+c_i}{S_i} = \frac{S_i}{S_i} = 1$.
The inequality we need to prove is
\[
 \left(\prod_{i=1}^n x_i\right)^\frac 1n+\left(\prod_{i=1}^n y_i\right)^\frac 1n+\left(\prod_{i=1}^n z_i\right)^\frac 1n\leq 1.
\]
We apply the AM-GM inequality to the non-negative numbers $x_1, \ldots, x_n$:
\[
 \left(\prod_{i=1}^n x_i\right)^\frac 1n \leq \frac{1}{n}\sum_{i=1}^n x_i.
\]
Similarly, applying the AM-GM inequality to $y_1, \ldots, y_n$ and $z_1, \ldots, z_n$:
\[
 \left(\prod_{i=1}^n y_i\right)^\frac 1n \leq \frac{1}{n}\sum_{i=1}^n y_i,
\]
\[
 \left(\prod_{i=1}^n z_i\right)^\frac 1n \leq \frac{1}{n}\sum_{i=1}^n z_i.
\]
Summing these three inequalities, we get:
\[
 \left(\prod_{i=1}^n x_i\right)^\frac 1n+\left(\prod_{i=1}^n y_i\right)^\frac 1n+\left(\prod_{i=1}^n z_i\right)^\frac 1n \leq \frac{1}{n}\sum_{i=1}^n x_i + \frac{1}{n}\sum_{i=1}^n y_i + \frac{1}{n}\sum_{i=1}^n z_i.
\]
The right-hand side can be written as:
\[
 \frac{1}{n}\sum_{i=1}^n (x_i+y_i+z_i).
\]
Since $x_i+y_i+z_i=1$ for each $i$, the sum $\sum_{i=1}^n (x_i+y_i+z_i) = \sum_{i=1}^n 1 = n$.
Therefore, the RHS is $\frac{1}{n}(n) = 1$.
So we have
\[
 \left(\prod_{i=1}^n x_i\right)^\frac 1n+\left(\prod_{i=1}^n y_i\right)^\frac 1n+\left(\prod_{i=1}^n z_i\right)^\frac 1n \leq 1.
\]
Substituting back $x_i = \frac{a_i}{a_i+b_i+c_i}$, $y_i = \frac{b_i}{a_i+b_i+c_i}$, and $z_i = \frac{c_i}{a_i+b_i+c_i}$, we get
\[
 \left(\prod_{i=1}^n \frac{a_i}{a_i+b_i+c_i}\right)^\frac 1n+\left(\prod_{i=1}^n \frac{b_i}{a_i+b_i+c_i}\right)^\frac 1n+\left(\prod_{i=1}^n \frac{c_i}{a_i+b_i+c_i}\right)^\frac 1n\leq 1.
\]
\[
 \frac{\left(\prod a_i\right)^\frac 1n}{\left(\prod (a_i+b_i+c_i)\right)^\frac 1n}+\frac{\left(\prod b_i\right)^\frac 1n}{\left(\prod (a_i+b_i+c_i)\right)^\frac 1n}+\frac{\left(\prod c_i\right)^\frac 1n}{\left(\prod (a_i+b_i+c_i)\right)^\frac 1n}\leq 1.
\]
\[
 \frac{\left(\prod a_i\right)^\frac 1n+\left(\prod b_i\right)^\frac 1n+\left(\prod c_i\right)^\frac 1n}{\left(\prod (a_i+b_i+c_i)\right)^\frac 1n}\leq 1.
\]
Multiplying by the denominator $\left(\prod (a_i+b_i+c_i)\right)^\frac 1n$ (which is positive in this case), we obtain the desired inequality:
\[
 \left(\prod_{i=1}^n a_i\right)^\frac 1n+\left(\prod_{i=1}^n b_i\right)^\frac 1n+\left(\prod_{i=1}^n c_i\right)^\frac 1n\leq \left(\prod_{i=1}^n (a_i+b_i+c_i)\right)^\frac 1n.
\]

The equality holds if and only if the equality holds in all three applications of the AM-GM inequality and in the summation step. Equality in AM-GM holds if and only if the terms are equal. So we need $x_1=\dots=x_n$, $y_1=\dots=y_n$, and $z_1=\dots=z_n$. Let these common values be $x, y, z$ respectively. Then $x_i=x, y_i=y, z_i=z$ for all $i$.
Since $x_i+y_i+z_i=1$, we have $x+y+z=1$.
This means $\frac{a_i}{a_i+b_i+c_i}=x$, $\frac{b_i}{a_i+b_i+c_i}=y$, $\frac{c_i}{a_i+b_i+c_i}=z$ for all $i$.
This is equivalent to $(a_i, b_i, c_i)$ being proportional to $(x, y, z)$ for all $i$, i.e., $(a_i, b_i, c_i) = k_i (x, y, z)$ for some scalar $k_i = a_i+b_i+c_i > 0$ and constants $x, y, z \ge 0$ with $x+y+z=1$. This condition means that the vectors $(a_i, b_i, c_i)$ are all parallel.

The final answer is $\boxed{\left(\prod_{i=1}^n a_i\right)^\frac 1n+\left(\prod_{i=1}^n b_i\right)^\frac 1n+\left(\prod_{i=1}^n c_i\right)^\frac 1n\leq \left(\prod_{i=1}^n (a_i+b_i+c_i)\right)^\frac 1n}$.