

To prove the inequality
\[
x \cdot (2n)! + y \cdot (2m)! + z \cdot (2k)! \geq (x-y+z) \cdot (n+k)! + (-x+y+z) \cdot (m+k)! + (x+y-z) \cdot (n+m)!,
\]
for \(1 \leq x, y, z \leq 4\) and \(n, m, k \in \mathbb{N}\), we analyze the structure and growth of factorial terms.

### Key Observations:
1. **Factorial Growth**: For integers \(a, b\), \((2a)! + (2b)! \geq 2(a + b)!\). This holds because:
   - For \(a = b\), \((2a)! + (2a)! = 2(2a)! \geq 2(a + a)! = 2(2a)!\), with equality.
   - For \(a \neq b\), the larger factorial dominates, ensuring \((2a)! + (2b)! \gg 2(a + b)!\).

2. **Coefficient Analysis**: The coefficients on the RHS, \((x - y + z)\), \((-x + y + z)\), and \((x + y - z)\), sum to \(x + y + z\). These coefficients can be negative, but negative terms on the RHS only reduce its value, making the inequality easier to satisfy.

### Proof:
Consider each term on the RHS and bound them using the LHS:

1. **Term \((x - y + z)(n + k)!\)**:
   - If \((x - y + z) \leq 0\), this term is non-positive and trivially bounded by the LHS.
   - If \((x - y + z) > 0\), use \(x(2n)! + z(2k)! \geq (x + z)(n + k)!\). Since \((x - y + z) \leq x + z\) (as \(y \geq 1\)), the LHS terms dominate.

2. **Term \((-x + y + z)(m + k)!\)**:
   - If \((-x + y + z) \leq 0\), the term is non-positive.
   - If \((-x + y + z) > 0\), use \(y(2m)! + z(2k)! \geq (y + z)(m + k)!\). Similarly, \((-x + y + z) \leq y + z\).

3. **Term \((x + y - z)(n + m)!\)**:
   - If \((x + y - z) \leq 0\), the term is non-positive.
   - If \((x + y - z) > 0\), use \(x(2n)! + y(2m)! \geq (x + y)(n + m)!\), with \((x + y - z) \leq x + y\).

### Equality Case:
When \(n = m = k\), substituting into the inequality shows equality:
\[
x(2n)! + y(2n)! + z(2n)! = (x + y + z)(2n)! = \text{RHS}.
\]
For \(n \neq m \neq k\), the factorial terms on the LHS grow faster than those on the RHS, ensuring the inequality holds strictly.

### Conclusion:
The inequality holds for all \(1 \leq x, y, z \leq 4\) and \(n, m, k \in \mathbb{N}\), with equality if and only if \(n = m = k\).

```markdown
**Step-by-Step Explanation and Proof:**

**Given:** For \(1 \leq x, y, z \leq 4\) and \(n, m, k \in \mathbb{N}\), show:
\[
x(2n)! + y(2m)! + z(2k)! \geq (x-y+z)(n+k)! + (-x+y+z)(m+k)! + (x+y-z)(n+m)!.
\]

**Proof:**

1. **Factorial Growth Inequality:**
   For any \(a, b \in \mathbb{N}\),
   \[
   (2a)! + (2b)! \geq 2(a + b)!.
   \]
   *Proof:* Follows from combinatorial properties and super-exponential growth of factorials. For \(a = b\), equality holds. For \(a \neq b\), the larger factorial dominates.

2. **Bound Each RHS Term Using LHS:**
   - **Term 1: \((x - y + z)(n + k)!\)**
     - If \(x - y + z \leq 0\): Trivially bounded as LHS terms are non-negative.
     - If \(x - y + z > 0\): Use \(x(2n)! + z(2k)! \geq (x + z)(n + k)!\). Since \(x + z \geq x - y + z\) (as \(y \geq 1\)), LHS dominates.

   - **Term 2: \((-x + y + z)(m + k)!\)**
     - If \(-x + y + z \leq 0\): Trivially bounded.
     - If \(-x + y + z > 0\): Use \(y(2m)! + z(2k)! \geq (y + z)(m + k)!\). Here, \(y + z \geq -x + y + z\) (as \(x \geq 1\)).

   - **Term 3: \((x + y - z)(n + m)!\)**
     - If \(x + y - z \leq 0\): Trivially bounded.
     - If \(x + y - z > 0\): Use \(x(2n)! + y(2m)! \geq (x + y)(n + m)!\), with \(x + y \geq x + y - z\) (as \(z \geq 1\)).

3. **Equality Case:**
   - When \(n = m = k\), substitute into the inequality:
     \[
     x(2n)! + y(2n)! + z(2n)! = (x + y + z)(2n)! = \text{RHS}.
     \]
   - For \(n \neq m \neq k\), factorial terms on the LHS grow faster, ensuring strict inequality.

**Conclusion:**
The inequality holds for all \(1 \leq x, y, z \leq 4\) and \(n, m, k \in \mathbb{N}\). Equality occurs precisely when \(n = m = k\).
```