Let $R$ be a finite ring with the given properties:
1. For any $a,b\in R$, there is $c\in R$ such that $a^3+b^3=c^3$. This means the set $S = \{x^3 \mid x \in R\}$ is closed under addition.
2. If $a\neq b$, then $a^2b=-ba^2$.

We want to prove that for any $a,b\in R$, there is $d\in R$ such that $aba+bab=d^3$. This is equivalent to proving that $aba+bab \in S$ for all $a,b \in R$.

First, let's analyze property (2).
If $a,b \in R$ and $a \neq b$, then $a^2b=-ba^2$.
Consider the case $a=b$. Property (2) does not apply directly to $(a,a)$.
However, let $a \in R$. If $a=0$, then $0^3 = -0^3$ is true.
If $a \neq 0$, and $R$ has more than one element, then $R \neq \{0\}$.
If $R = \{0, a\}$, $R$ must be isomorphic to $\mathbb{Z}_2$. In $\mathbb{Z}_2$, $1+1=0$, $1 \cdot 1=1$. For $a=1$, $1^3=1$, $-1^3=-1=1$. So $a^3=-a^3$ is $1=1$. Also $2a^3 = 2 \cdot 1^3 = 0$.
If $R$ has more than two elements, then for any $a \in R, a \neq 0$, there exists $b \in R$ such that $b \neq 0$ and $a \neq b$.
By property (2) applied to $(a,b)$, $a^2b=-ba^2$.
Consider the element $a+b$. If $b \neq 0$, then $a \neq a+b$. By property (2) applied to $(a, a+b)$:
If $a \neq a+b$, then $a^2(a+b) = -(a+b)a^2$.
$a^3+a^2b = -(a^3+ba^2) = -a^3-ba^2$.
$2a^3 + a^2b + ba^2 = 0$.
Since $a \neq b$, by property (2), $a^2b = -ba^2$. Thus $a^2b+ba^2 = a^2b+(-a^2b)=0$.
So, $2a^3+0=0$, which means $2a^3=0$.
This derivation $2a^3=0$ is valid if $a \neq 0$, there exists $b$ such that $b \neq 0$ and $a \neq b$, and $a \neq a+b$ (i.e. $b \neq 0$).
The condition $b \neq 0$ is used twice.
For $a \neq 0$: if $R$ has more than two elements, there exists $b \in R \setminus \{0, a\}$. Then $b \neq 0$ and $a \neq b$. The condition $a \neq a+b$ is $b \neq 0$.
So for any $a \neq 0$, if $R$ has more than two elements, $2a^3=0$.
If $a=0$, $2 \cdot 0^3=0$.
If $R$ has exactly two elements, $R \cong \mathbb{Z}_2$. As shown, $2a^3=0$ for all $a \in \mathbb{Z}_2$.
Therefore, $2a^3=0$ for all $a \in R$.

Since $2a^3=0$ for all $a \in R$, we have $2x=0$ for all $x \in S=\{x^3 \mid x \in R\}$.
This means $x=-x$ for all $x \in S$.
Property (1) says $S$ is closed under addition. Since $x \in S \implies -x \in S$, $S$ is also closed under subtraction ($x-y = x+(-y) = x+y$).

Now consider $aba+bab$. We want to show $aba+bab \in S$.
Consider the expansion of $(a+b)^3$ for $a,b \in R$:
$(a+b)^3 = (a+b)(a+b)^2 = (a+b)(a^2+ab+ba+b^2) = a(a^2+ab+ba+b^2) + b(a^2+ab+ba+b^2)$
$= a^3+a^2b+aba+ab^2 + ba^2+bab+b^2a+b^3$.

Case 1: $a \neq b$.
By property (2), $a^2b=-ba^2$.
Since $a \neq b$, we also have $b \neq a$. By property (2) applied to $(b,a)$, $b^2a=-ab^2$.
Substitute these into the expansion of $(a+b)^3$:
$(a+b)^3 = a^3+a^2b+aba+ab^2 + (-a^2b)+bab+(-ab^2)+b^3$
$(a+b)^3 = a^3+b^3+aba+bab$.
By property (1), $a^3 \in S$, $b^3 \in S$, and $(a+b)^3 \in S$.
Since $S$ is closed under addition and $2x=0$ for $x \in S$:
$(a+b)^3+a^3+b^3 \in S$.
Using the expression for $(a+b)^3$ when $a \neq b$:
$(a^3+b^3+aba+bab) + a^3+b^3 = (a^3+a^3) + (b^3+b^3) + aba+bab = 2a^3+2b^3+aba+bab$.
Since $2x^3=0$ for all $x \in R$, $2a^3=0$ and $2b^3=0$.
So, $(a+b)^3+a^3+b^3 = 0+0+aba+bab = aba+bab$.
Since $(a+b)^3+a^3+b^3 \in S$, we have $aba+bab \in S$ for $a \neq b$.
This means for $a \neq b$, there exists $d \in R$ such that $aba+bab=d^3$.

Case 2: $a=b$.
We need to show $aaa+bab \in S$.
$aaa+bab = a^3+a^3 = 2a^3$.
As shown earlier, $2a^3=0$ for all $a \in R$.
$0 \in R$, and $0=0^3$. So $0 \in S$.
Thus, $aba+bab=0 \in S$ for $a=b$.
This means for $a=b$, there exists $d \in R$ (namely $d=0$) such that $aba+bab=d^3$.

Combining Case 1 and Case 2, we have shown that for any $a,b \in R$, $aba+bab \in S$.
By definition of $S$, this means for any $a,b \in R$, there exists $d \in R$ such that $aba+bab=d^3$.

The final answer is $\boxed{For any $a,b\in R$ there is $d\in R$ such that $aba+bab=d^3}$.