Of course. Here is a detailed, step-by-step solution to the problem.

### **1. Understanding the Problem and Using the Eigenvalue Information**

The problem states that $M$ is a $3 \times 3$ matrix and that $\lambda=1$ is an eigenvalue with an algebraic multiplicity of 3.

The **characteristic polynomial** of a $3 \times 3$ matrix $M$, denoted by $p(\lambda) = \det(M - \lambda I_3)$, is a polynomial of degree 3 in $\lambda$. The roots of the characteristic polynomial are the eigenvalues of the matrix.

Since $\lambda=1$ is an eigenvalue with algebraic multiplicity 3, it means that $(\lambda-1)$ is a factor of the characteristic polynomial three times. Therefore, the characteristic polynomial must be of the form:
$p(\lambda) = C(\lambda-1)^3$
for some constant $C$.

The characteristic polynomial is defined as $\det(M - \lambda I_3)$. The term with the highest power of $\lambda$ comes from the product of the diagonal entries, $(m_{11}-\lambda)(m_{22}-\lambda)(m_{33}-\lambda)$, which gives a leading term of $-\lambda^3$. Thus, the coefficient of $\lambda^3$ in $p(\lambda)$ is $-1$.
In our form $p(\lambda) = C(\lambda-1)^3 = C(\lambda^3 - 3\lambda^2 + 3\lambda - 1)$, the coefficient of $\lambda^3$ is $C$. Therefore, we must have $C = -1$.

So, the characteristic polynomial of $M$ is:
$p(\lambda) = -(\lambda-1)^3 = (1-\lambda)^3$.

### **2. Applying the Cayley-Hamilton Theorem**

The **Cayley-Hamilton Theorem** states that every square matrix satisfies its own characteristic equation. In our case, this means $p(M) = O_3$, where $O_3$ is the $3 \times 3$ zero matrix.

Substituting $M$ into its characteristic polynomial:
$p(M) = (I_3 - M)^3 = O_3$.

Let's expand this expression:
$(I_3 - M)^3 = I_3^3 - 3I_3^2M + 3I_3M^2 - M^3 = O_3$
$I_3 - 3M + 3M^2 - M^3 = O_3$.

Rearranging this equation gives us a fundamental relationship between the powers of $M$:
\begin{equation}
M^3 = 3M^2 - 3M + I_3 \quad (*).
\end{equation}
This equation shows that any power of $M$ greater than or equal to 3 can be expressed as a linear combination of $M^2$, $M$, and $I_3$. This confirms the form given in the problem statement. For $m=3$, we can see immediately that $a_3=3, b_3=-3, c_3=1$.

### **3. A Method Using Polynomial Division (The Remainder Theorem)**

We are looking for coefficients $a_m, b_m, c_m$ such that $M^m = a_m M^2 + b_m M + c_m I_3$.
Let's consider the polynomial $f(x) = x^m$. We want to find the polynomial $r(x) = a_m x^2 + b_m x + c_m$ such that $f(M) = r(M)$.

From the Cayley-Hamilton theorem, we know that any polynomial in $M$ can be reduced modulo the polynomial $P(x) = (x-1)^3$. Let $P(x)=(x-1)^3$. The fact that $P(M)=(M-I_3)^3=O_3$ allows us to find the coefficients.

By the polynomial remainder theorem, we can write $x^m$ as:
\begin{equation*}
x^m = q(x)(x-1)^3 + r(x),
\end{equation*}
where $q(x)$ is the quotient and $r(x) = a_m x^2 + b_m x + c_m$ is the remainder.
If we substitute the matrix $M$ for $x$, we get:
$M^m = q(M)(M-I_3)^3 + r(M)$.
Since $(M-I_3)^3 = O_3$, this simplifies to:
$M^m = r(M) = a_m M^2 + b_m M + c_m I_3$.

Our task is to find the coefficients of the remainder polynomial $r(x)$. We can find these coefficients by evaluating the equation $x^m = q(x)(x-1)^3 + r(x)$ and its derivatives at the root of the divisor, $x=1$.

Let $f(x) = x^m$ and $r(x) = a_m x^2 + b_m x + c_m$. The equation is $f(x) = q(x)(x-1)^3 + r(x)$.

**Step 3.1: Evaluate at x=1**
At $x=1$, the term $q(x)(x-1)^3$ becomes zero.
$f(1) = r(1)$
$1^m = a_m(1)^2 + b_m(1) + c_m$
\begin{equation}
1 = a_m + b_m + c_m \quad (1)
\end{equation}

**Step 3.2: Differentiate and evaluate at x=1**
First, we differentiate the equation with respect to $x$:
$f'(x) = q'(x)(x-1)^3 + 3q(x)(x-1)^2 + r'(x)$.
At $x=1$, all terms containing $(x-1)$ become zero.
$f'(1) = r'(1)$.

We have:
$f'(x) = mx^{m-1} \implies f'(1) = m(1)^{m-1} = m$.
$r'(x) = 2a_m x + b_m \implies r'(1) = 2a_m + b_m$.
Therefore,
\begin{equation}
m = 2a_m + b_m \quad (2)
\end{equation}

**Step 3.3: Differentiate a second time and evaluate at x=1**
We differentiate $f'(x)$ and $r'(x)$:
$f''(x) = [\text{terms containing }(x-1)] + r''(x)$.
Evaluating at $x=1$:
$f''(1) = r''(1)$.

We have:
$f''(x) = m(m-1)x^{m-2} \implies f''(1) = m(m-1)$.
$r''(x) = 2a_m \implies r''(1) = 2a_m$.
Therefore,
\begin{equation}
m(m-1) = 2a_m \quad (3)
\end{equation}

### **4. Solving for the Coefficients**

We now have a system of three linear equations for $a_m, b_m, c_m$:
1.  $a_m + b_m + c_m = 1$
2.  $2a_m + b_m = m$
3.  $2a_m = m(m-1)$

We can solve this system easily.
From equation (3):
$a_m = \frac{m(m-1)}{2}$.

Substitute this result into equation (2) to find $b_m$:
$m(m-1) + b_m = m$
$b_m = m - m(m-1) = m - m^2 + m = 2m - m^2 = -m(m-2)$.

Finally, substitute $a_m$ and $b_m$ into equation (1) to find $c_m$:
$c_m = 1 - a_m - b_m$
$c_m = 1 - \frac{m(m-1)}{2} - (-m(m-2))$
$c_m = 1 - \frac{m^2-m}{2} + m^2-2m$
To combine these terms, we use a common denominator of 2:
$c_m = \frac{2 - (m^2-m) + 2(m^2-2m)}{2}$
$c_m = \frac{2 - m^2 + m + 2m^2 - 4m}{2}$
$c_m = \frac{m^2 - 3m + 2}{2}$
Factoring the numerator gives:
$c_m = \frac{(m-1)(m-2)}{2}$.

The coefficients can also be expressed using binomial coefficients:
$a_m = \binom{m}{2}$
$c_m = \binom{m-1}{2}$

### **Conclusion**

For any natural number $m \geq 3$, the coefficients $a_m, b_m, c_m$ that satisfy the equation $M^m=a_mM^2+b_mM+c_mI_3$ are:

\begin{align*}
a_m &= \frac{m(m-1)}{2} = \binom{m}{2} \\
b_m &= -m(m-2) \\
c_m &= \frac{(m-1)(m-2)}{2} = \binom{m-1}{2}
\end{align*}

It is important to note that this result holds for any matrix $M$ satisfying the given conditions. The existence of a matrix $M$ whose minimal polynomial is $(x-1)^3$ (e.g., a single Jordan block of size 3) ensures that the set of matrices $\{I_3, M, M^2\}$ is linearly independent, which guarantees that these coefficients $a_m, b_m, c_m$ are unique.